@prefix freebase: <http://rdf.freebase.com/ns/> .
@prefix dcterms: <http://purl.org/dc/terms/> .
@prefix foaf: <http://xmlns.com/foaf/0.1/> .
@prefix owl: <http://www.w3.org/2002/07/owl#> .
@prefix dc: <http://purl.org/dc/elements/1.1/> .
@prefix rdfs: <http://www.w3.org/2000/01/rdf-schema#> .
@prefix skos: <http://www.w3.org/2004/02/skos/core#> .
@prefix dbpedia: <http://dbpedia.org/resource/> .
@prefix csw: <http://semantic-web.at/ontologies/csw.owl#> .
@prefix rdf: <http://www.w3.org/1999/02/22-rdf-syntax-ns#> .
@prefix cycAnnot: <http://sw.cyc.com/CycAnnotations_v1#> .
@prefix tags: <http://www.holygoat.co.uk/owl/redwood/0.1/tags/> .
@prefix opencyc: <http://sw.opencyc.org/concept/> .
@prefix cyc: <http://sw.cyc.com/concept/> .
@prefix ctag: <http://commontag.org/ns#> .
@prefix xsd: <http://www.w3.org/2001/XMLSchema#> .

<http://schema.semantic-web.at/ppt/3.2/quality/scenario/dialog.qualitysettings.scenario.restricted> <http://schema.semantic-web.at/ppt/3.2/quality/activeScenario> true .

<http://vocabulary.semantic-web.at/cocktails/021c85c0-a60a-4414-8fd8-bd3383b794f1> dcterms:contributor <http://localhost/user/blumauera> ;
	dcterms:created "2015-05-01T08:09:10Z"^^xsd:dateTime ;
	dcterms:creator <http://localhost/user/blumauera> ;
	dcterms:modified "2015-05-07T07:01:04Z"^^xsd:dateTime ;
	<http://schema.semantic-web.at/ppt/inScheme> <http://vocabulary.semantic-web.at/cocktails/eff672ac-6601-42c6-a3e9-0adda3b45df8> ;
	<http://schema.semantic-web.at/ppt/inSubtree> <http://vocabulary.semantic-web.at/cocktails/4f20d6bb-710d-4870-bde4-b6e835d7d13f> ;
	<http://vocabulary.semantic-web.at/cocktail-ontology/is-part-of> <http://vocabulary.semantic-web.at/cocktails/bca7bc6d-6709-48b8-ae52-fe194c212398> ;
	<http://vocabulary.semantic-web.at/cocktail-ontology/is-used-by_2> <http://vocabulary.semantic-web.at/cocktails/12f4790a-560f-4e1c-b57a-53b8171ae39a> , <http://vocabulary.semantic-web.at/cocktails/2c032fe6-a518-44be-851a-dbf1c253be63> , <http://vocabulary.semantic-web.at/cocktails/4f85cadd-4fd4-4ffc-a78d-cddb0763fa4b> , <http://vocabulary.semantic-web.at/cocktails/60d3a991-48d3-4e73-9d62-5961893fd311> , <http://vocabulary.semantic-web.at/cocktails/7e4a73d5-f73d-4890-972c-f3dfd6952fd8> , <http://vocabulary.semantic-web.at/cocktails/a47e8f08-057a-45f2-8398-9be51ed351fc> , <http://vocabulary.semantic-web.at/cocktails/bab016bd-2fd5-4809-bfe7-3225d25f116d> , <http://vocabulary.semantic-web.at/cocktails/bed073f2-de84-4322-a490-4f34ec54c6d1> , <http://vocabulary.semantic-web.at/cocktails/f01f6a10-01a5-4810-860f-d3a52fd36b1b> ;
	a <http://vocabulary.semantic-web.at/cocktail-ontology/Garnish> , <http://vocabulary.semantic-web.at/cocktail-ontology/Ingredients> , skos:Concept ;
	skos:altLabel "Bonji Water"@en , "Bonji water"@en , "Citrus Limonum"@en , "Citrus limonum"@en , "Lime (Citrus aurantifolia)"@en , "Lime (botany)"@en , "Lime Oil"@en , "Lime fruit"@en ;
	skos:broader <http://vocabulary.semantic-web.at/cocktails/4f20d6bb-710d-4870-bde4-b6e835d7d13f> ;
	skos:definition "Lime is a term referring to a citrus fruit which is typically round, green to yellow in colour, 3–6 cm in diameter, and containing sour and acidic pulp. Limes are a good source of vitamin C, and are often used to accent the flavours of foods and beverages. They are grown all year round and are usually smaller and less sour than lemons."@en ;
	skos:exactMatch <http://dbpedia.org/resource/Lime_(fruit)> ;
	skos:prefLabel "Lime"@en .

<http://vocabulary.semantic-web.at/cocktails/0381bd47-ad07-428a-b5c4-ee2608f2ebd3> dcterms:contributor <http://localhost/user/nagyhel> ;
	dcterms:created "2015-05-02T18:43:53Z"^^xsd:dateTime ;
	dcterms:creator <http://localhost/user/blumauera> ;
	dcterms:modified "2015-07-02T15:05:26Z"^^xsd:dateTime ;
	<http://schema.semantic-web.at/ppt/inScheme> <http://vocabulary.semantic-web.at/cocktails/f09732a9-a0e6-494a-8ce9-299ef036aaaf> ;
	<http://vocabulary.semantic-web.at/cocktail-ontology/is-used-by> <http://vocabulary.semantic-web.at/cocktails/2c032fe6-a518-44be-851a-dbf1c253be63> , <http://vocabulary.semantic-web.at/cocktails/ea946e07-e812-4492-a0ed-124d73bfbba7> ;
	a <http://vocabulary.semantic-web.at/cocktail-ontology/Drinkware> , skos:Concept ;
	skos:broader <http://vocabulary.semantic-web.at/cocktails/d6c5f29f-bef7-41c5-9d39-535d83e9f750> ;
	skos:prefLabel "Copper mug"@en .

<http://vocabulary.semantic-web.at/cocktails/038615ab-5b6e-4293-a8ca-53cf0fb92340> dcterms:contributor <http://localhost/user/blumauera> ;
	dcterms:created "2015-05-01T08:29:29Z"^^xsd:dateTime ;
	dcterms:creator <http://localhost/user/blumauera> ;
	dcterms:modified "2015-05-07T06:49:15Z"^^xsd:dateTime ;
	<http://schema.semantic-web.at/ppt/inScheme> <http://vocabulary.semantic-web.at/cocktails/591cf89a-57af-49b8-9042-3fc77408c93e> ;
	<http://schema.semantic-web.at/ppt/inSubtree> <http://vocabulary.semantic-web.at/cocktails/e86c1671-4a67-494b-ae5d-bcb750865acc> ;
	<http://vocabulary.semantic-web.at/cocktail-ontology/is-part-of> <http://vocabulary.semantic-web.at/cocktails/117bd4d2-6da3-4d69-8c79-bc1d873b5010> , <http://vocabulary.semantic-web.at/cocktails/13b85b5c-7f69-4871-bb08-3cd5281f6039> , <http://vocabulary.semantic-web.at/cocktails/c151ee28-45d2-4128-8587-1f1b69060d9d> , <http://vocabulary.semantic-web.at/cocktails/c3b197cc-8583-4e2f-8e45-3a7fed1309c1> ;
	a <http://vocabulary.semantic-web.at/cocktail-ontology/Beverages> , <http://vocabulary.semantic-web.at/cocktail-ontology/Ingredients> , <http://vocabulary.semantic-web.at/cocktail-ontology/Non-alcoholic-Beverages> , skos:Concept ;
	skos:altLabel "Cream (food)"@en , "Creams"@en , "Creme"@en , "Crème"@en , "Double cream"@en , "Half cream"@en , "Heavy cream"@en , "Heavy whipping cream"@en , "Kaffeeober"@en , "Kaffeeobers"@en , "Kreme"@en , "Light whipping cream"@en , "Milk Cream"@en , "Single cream"@en , "Sweet cream"@en , "Vrhnje"@en ;
	skos:broader <http://vocabulary.semantic-web.at/cocktails/b6ce7a37-ceda-4e8c-86a0-fe7bc5fd0908> ;
	skos:definition "Cream is a dairy product that is composed of the higher-butterfat layer skimmed from the top of milk before homogenization. In un-homogenized milk, the fat, which is less dense, will eventually rise to the top. In the industrial production of cream this process is accelerated by using centrifuges called \"separators\". In many countries, cream is sold in several grades depending on the total butterfat content. Cream can be dried to a powder for shipment to distant markets."@en ;
	skos:exactMatch dbpedia:Cream ;
	skos:prefLabel "Cream"@en .

<http://vocabulary.semantic-web.at/cocktails/05206233-09be-41ac-9f2e-91263873a20e> dcterms:created "2015-05-02T08:15:21Z"^^xsd:dateTime ;
	dcterms:creator <http://localhost/user/blumauera> ;
	<http://schema.semantic-web.at/ppt/inScheme> <http://vocabulary.semantic-web.at/cocktails/591cf89a-57af-49b8-9042-3fc77408c93e> ;
	<http://schema.semantic-web.at/ppt/inSubtree> <http://vocabulary.semantic-web.at/cocktails/403d1249-f37f-4f43-bebf-8dde9677d886> ;
	a <http://vocabulary.semantic-web.at/cocktail-ontology/Alcoholic-Beverages> , <http://vocabulary.semantic-web.at/cocktail-ontology/Beverages> , <http://vocabulary.semantic-web.at/cocktail-ontology/Ingredients> , skos:Concept ;
	skos:broader <http://vocabulary.semantic-web.at/cocktails/2944baef-5338-421b-a5f5-0e51f75244c2> ;
	skos:narrower <http://vocabulary.semantic-web.at/cocktails/2d108ce2-7bf0-4a5d-8f88-636419eba9a3> ;
	skos:prefLabel "Lemon-flavored liqueur"@en .

<http://vocabulary.semantic-web.at/cocktails/05a0d86b-79fc-4d75-91e4-dc77e8167db9> dcterms:contributor <http://localhost/user/blumauera> ;
	dcterms:created "2015-05-02T19:41:29Z"^^xsd:dateTime ;
	dcterms:creator <http://localhost/user/blumauera> ;
	dcterms:modified "2015-05-05T07:56:29Z"^^xsd:dateTime ;
	<http://schema.semantic-web.at/ppt/inScheme> <http://vocabulary.semantic-web.at/cocktails/591cf89a-57af-49b8-9042-3fc77408c93e> ;
	<http://schema.semantic-web.at/ppt/inSubtree> <http://vocabulary.semantic-web.at/cocktails/403d1249-f37f-4f43-bebf-8dde9677d886> ;
	<http://vocabulary.semantic-web.at/cocktail-ontology/is-part-of> <http://vocabulary.semantic-web.at/cocktails/2c682ed8-e2ba-473e-8cb7-979598080e18> ;
	a <http://vocabulary.semantic-web.at/cocktail-ontology/Alcoholic-Beverages> , <http://vocabulary.semantic-web.at/cocktail-ontology/Beverages> , <http://vocabulary.semantic-web.at/cocktail-ontology/Ingredients> , skos:Concept ;
	skos:broader <http://vocabulary.semantic-web.at/cocktails/917d78d0-0938-4fe0-80c4-cfd2eb16e6a4> ;
	skos:definition "Aperol is an Italian aperitif originally produced by the Barbieri company, based in Padua. Aperol is now produced by the Campari company. While Aperol was originally created in 1919, it did not become successful until after World War II. Its ingredients are, among others, bitter orange, gentian, rhubarb, and cinchona. Although it looks, tastes, and smells much like Campari, Aperol has an alcohol content of 11%—less than half of Campari. Aperol and Campari have the same sugar content."@en ;
	skos:exactMatch dbpedia:Aperol ;
	skos:prefLabel "Aperol"@en .

<http://vocabulary.semantic-web.at/cocktails/074c3acb-bc4d-4c6e-ad8a-e553d5ec7eff> dcterms:contributor <http://localhost/user/blumauera> ;
	dcterms:created "2015-05-03T18:50:01Z"^^xsd:dateTime ;
	dcterms:creator <http://localhost/user/blumauera> ;
	dcterms:modified "2015-05-07T07:07:28Z"^^xsd:dateTime ;
	<http://schema.semantic-web.at/ppt/inScheme> <http://vocabulary.semantic-web.at/cocktails/591cf89a-57af-49b8-9042-3fc77408c93e> ;
	<http://schema.semantic-web.at/ppt/inSubtree> <http://vocabulary.semantic-web.at/cocktails/403d1249-f37f-4f43-bebf-8dde9677d886> ;
	<http://vocabulary.semantic-web.at/cocktail-ontology/is-part-of> <http://vocabulary.semantic-web.at/cocktails/11d68913-3a30-4591-bc41-25fea3f38520> , <http://vocabulary.semantic-web.at/cocktails/1d5b39cc-fcab-48b2-bb24-9840b7e34d64> , <http://vocabulary.semantic-web.at/cocktails/b8075344-1e6d-4348-bdee-83948203a974> ;
	a <http://vocabulary.semantic-web.at/cocktail-ontology/Alcoholic-Beverages> , <http://vocabulary.semantic-web.at/cocktail-ontology/Beverages> , <http://vocabulary.semantic-web.at/cocktail-ontology/Ingredients> , skos:Concept ;
	skos:broader <http://vocabulary.semantic-web.at/cocktails/8cfd00fe-9f5a-414e-be27-858a8bc43c7c> ;
	skos:narrower <http://vocabulary.semantic-web.at/cocktails/5d0fdad6-6256-4042-a1a0-709f332cf373> , <http://vocabulary.semantic-web.at/cocktails/96c173d1-f047-4811-8950-45b071588fdc> ;
	skos:prefLabel "Dry vermouth"@en .

<http://vocabulary.semantic-web.at/cocktails/099726a2-ec4b-4b0f-b4e4-e6f25cdfd685> dcterms:contributor <http://localhost/user/blumauera> ;
	dcterms:created "2015-05-01T15:19:40Z"^^xsd:dateTime ;
	dcterms:creator <http://localhost/user/blumauera> ;
	dcterms:modified "2015-05-05T06:16:35Z"^^xsd:dateTime ;
	<http://schema.semantic-web.at/ppt/inScheme> <http://vocabulary.semantic-web.at/cocktails/8d052dfc-44bf-4985-8ce3-4564570a161b> ;
	<http://vocabulary.semantic-web.at/cocktail-ontology/consists-of> <http://vocabulary.semantic-web.at/cocktails/e406119b-7637-43f9-9a62-5a8ea500ebc4> , <http://vocabulary.semantic-web.at/cocktails/fd76c5ab-be62-4c4b-a2c6-7fa9bc359f47> ;
	<http://vocabulary.semantic-web.at/cocktail-ontology/iba> <http://www.iba-world.com/index.php?option=com_content&id=210&Itemid=532> ;
	<http://vocabulary.semantic-web.at/cocktail-ontology/image> <http://www.iba-world.com/images/cocktail_drinks/stinger.jpg> ;
	<http://vocabulary.semantic-web.at/cocktail-ontology/preparation> "Pour in a mixing glass with ice, stir and strain into a cocktail glass. May also be served on rocks in a rocks glass."@en ;
	<http://vocabulary.semantic-web.at/cocktail-ontology/served> "Straight up; without ice"@en ;
	<http://vocabulary.semantic-web.at/cocktail-ontology/uses> <http://vocabulary.semantic-web.at/cocktails/19dee0d8-fd30-469f-9ecd-91c902ff717c> ;
	a <http://vocabulary.semantic-web.at/cocktail-ontology/Cocktail> , skos:Concept ;
	skos:broader <http://vocabulary.semantic-web.at/cocktails/87cf1079-05d6-44da-acbe-c94b3ba52bd7> , <http://vocabulary.semantic-web.at/cocktails/caae2ea0-7e60-400b-a2bb-14ef79720668> ;
	skos:definition "A stinger is a Duo cocktail made by adding crème de menthe to a spirit. The classic recipe is based on brandy and white crème de menthe, shaken and served in a cocktail glass. The origins of this drink are unclear, but it is mentioned in bartender's recipe books as far back as Tom Bullock's Ideal Bartender, published in 1917. Mixing brandy with green crème de menthe, in place of white, yields a Green Hornet."@en ;
	skos:exactMatch <http://dbpedia.org/resource/Stinger_(cocktail)> ;
	skos:prefLabel "Stinger"@en .

<http://vocabulary.semantic-web.at/cocktails/0a9e12b8-afa5-425a-b08b-941374b3bdc4> dcterms:contributor <http://localhost/user/blumauera> ;
	dcterms:created "2015-05-05T06:17:25Z"^^xsd:dateTime ;
	dcterms:creator <http://localhost/user/blumauera> ;
	dcterms:modified "2015-05-05T06:18:27Z"^^xsd:dateTime ;
	<http://schema.semantic-web.at/ppt/inScheme> <http://vocabulary.semantic-web.at/cocktails/591cf89a-57af-49b8-9042-3fc77408c93e> ;
	<http://schema.semantic-web.at/ppt/inSubtree> <http://vocabulary.semantic-web.at/cocktails/403d1249-f37f-4f43-bebf-8dde9677d886> ;
	<http://vocabulary.semantic-web.at/cocktail-ontology/is-part-of> <http://vocabulary.semantic-web.at/cocktails/1d5b39cc-fcab-48b2-bb24-9840b7e34d64> ;
	a <http://vocabulary.semantic-web.at/cocktail-ontology/Alcoholic-Beverages> , <http://vocabulary.semantic-web.at/cocktail-ontology/Beverages> , <http://vocabulary.semantic-web.at/cocktail-ontology/Ingredients> , skos:Concept ;
	skos:altLabel "Tom gin"@en ;
	skos:broader <http://vocabulary.semantic-web.at/cocktails/5d96c50c-ee48-4c40-bb4c-4b9a42d11de6> ;
	skos:definition "Old Tom Gin (or Tom Gin or Old Tom) is a gin recipe popular in 18th-century England that now is rarely available. It is slightly sweeter than London Dry, but slightly drier than Dutch/Holland Gin/Jenever, thus is sometimes called The Missing Link. The name Old Tom Gin purportedly came from wooden plaques shaped like a black cat (an \"Old Tom\") mounted on the outside wall of some pubs above a public walkway in 18th century England."@en ;
	skos:exactMatch dbpedia:Old_Tom_Gin ;
	skos:prefLabel "Old Tom Gin"@en .

<http://vocabulary.semantic-web.at/cocktails/0bbdca98-077b-48d1-99d6-47eca59c442c> dcterms:contributor <http://localhost/user/turdeant> ;
	dcterms:created "2015-05-01T08:44:44Z"^^xsd:dateTime ;
	dcterms:creator <http://localhost/user/blumauera> ;
	dcterms:modified "2015-08-13T16:33:08Z"^^xsd:dateTime ;
	<http://schema.semantic-web.at/ppt/inScheme> <http://vocabulary.semantic-web.at/cocktails/8d052dfc-44bf-4985-8ce3-4564570a161b> ;
	<http://vocabulary.semantic-web.at/cocktail-ontology/consists-of> <http://vocabulary.semantic-web.at/cocktails/224b4628-2f46-44a1-9d2f-8b5ef0b31e79> , <http://vocabulary.semantic-web.at/cocktails/2d7c2c72-a6a1-43ef-9175-02885fcf4518> , <http://vocabulary.semantic-web.at/cocktails/5d96c50c-ee48-4c40-bb4c-4b9a42d11de6> , <http://vocabulary.semantic-web.at/cocktails/9c2ce399-c6ae-4f4d-bf37-7fd8ffe2a19d> ;
	<http://vocabulary.semantic-web.at/cocktail-ontology/iba> <http://www.iba-world.com/index.php?option=com_content&id=188&Itemid=532> ;
	<http://vocabulary.semantic-web.at/cocktail-ontology/image> <https://upload.wikimedia.org/wikipedia/commons/4/4f/Aviation_Cocktail.jpg> ;
	<http://vocabulary.semantic-web.at/cocktail-ontology/is-variant-of> <http://vocabulary.semantic-web.at/cocktails/b33091cd-8c57-45e3-a89b-9de91ffce1e8> ;
	<http://vocabulary.semantic-web.at/cocktail-ontology/preparation> "Add all ingredients into cocktail shaker filled with ice. Shake well and strain into cocktail glass. Garnish with a cherry."@en ;
	<http://vocabulary.semantic-web.at/cocktail-ontology/served> "Straight up; without ice"@en ;
	<http://vocabulary.semantic-web.at/cocktail-ontology/uses> <http://vocabulary.semantic-web.at/cocktails/19dee0d8-fd30-469f-9ecd-91c902ff717c> ;
	<http://vocabulary.semantic-web.at/cocktail-ontology/uses_2> <http://vocabulary.semantic-web.at/cocktails/62fbc16f-3f84-4cc7-8c6f-5afebfc1510a> ;
	a <http://vocabulary.semantic-web.at/cocktail-ontology/Cocktail> , skos:Concept ;
	skos:altLabel "Aviation cocktail"@en ;
	skos:broader <http://vocabulary.semantic-web.at/cocktails/caae2ea0-7e60-400b-a2bb-14ef79720668> ;
	skos:definition "The Aviation is a classic cocktail made with gin, maraschino liqueur, crème de violette, and lemon juice. Some recipes omit the crème de violette. It is served straight up, in a cocktail glass."@en ;
	skos:exactMatch <http://dbpedia.org/resource/Aviation_(cocktail)> ;
	skos:prefLabel "Aviation"@en .

<http://vocabulary.semantic-web.at/cocktails/0e385475-f369-4832-b8e3-20f35028988d> dcterms:contributor <http://localhost/user/blumauera> ;
	dcterms:created "2015-05-01T14:10:42Z"^^xsd:dateTime ;
	dcterms:creator <http://localhost/user/blumauera> ;
	dcterms:modified "2015-05-05T07:55:49Z"^^xsd:dateTime ;
	<http://schema.semantic-web.at/ppt/inScheme> <http://vocabulary.semantic-web.at/cocktails/87384ce8-f20a-4201-b06d-3e0b8d832e5d> ;
	a <http://vocabulary.semantic-web.at/cocktail-ontology/Ingredients> , skos:Concept ;
	skos:altLabel "Liquid sugar"@en , "Sirup"@en , "Syrups"@en , "Syrupy"@en ;
	skos:definition "In cooking, a syrup or sirup is a thick, viscous liquid consisting primarily of a solution of sugar in water, containing a large amount of dissolved sugars but showing little tendency to deposit crystals. The viscosity arises from the multiple hydrogen bonds between the dissolved sugar, which has many hydroxyl (OH) groups, and the water. Syrups can be made by dissolving sugar in water or by reducing naturally sweet juices such as cane juice, sorghum juice, or maple sap."@en ;
	skos:exactMatch dbpedia:Syrup ;
	skos:narrower <http://vocabulary.semantic-web.at/cocktails/371797a7-e9a8-453b-8744-2e89f2fd30d2> , <http://vocabulary.semantic-web.at/cocktails/3bc44d8c-4e94-4f84-9354-8770018e8a8d> , <http://vocabulary.semantic-web.at/cocktails/457aff50-b86b-4879-8e17-41ca59cf03a7> , <http://vocabulary.semantic-web.at/cocktails/70bf85cb-53bb-4ebd-8bcb-e5efe304e5e2> , <http://vocabulary.semantic-web.at/cocktails/71210bd1-3071-4533-8da4-fe0f7d7694a0> , <http://vocabulary.semantic-web.at/cocktails/72cf9c86-734f-4954-b4c2-f02ee89373e8> , <http://vocabulary.semantic-web.at/cocktails/ced2e755-fe48-4d7b-86ab-6b39fe359a32> ;
	skos:prefLabel "Syrup"@en ;
	skos:topConceptOf <http://vocabulary.semantic-web.at/cocktails/87384ce8-f20a-4201-b06d-3e0b8d832e5d> .

<http://vocabulary.semantic-web.at/cocktails/0f11bcdf-a69e-451f-b824-48b1743c5916> dcterms:contributor <http://localhost/user/blumauera> ;
	dcterms:created "2015-05-02T08:18:07Z"^^xsd:dateTime ;
	dcterms:creator <http://localhost/user/blumauera> ;
	dcterms:modified "2015-07-02T14:56:19Z"^^xsd:dateTime ;
	<http://schema.semantic-web.at/ppt/inScheme> <http://vocabulary.semantic-web.at/cocktails/591cf89a-57af-49b8-9042-3fc77408c93e> ;
	<http://schema.semantic-web.at/ppt/inSubtree> <http://vocabulary.semantic-web.at/cocktails/e86c1671-4a67-494b-ae5d-bcb750865acc> ;
	<http://vocabulary.semantic-web.at/cocktail-ontology/is-part-of> <http://vocabulary.semantic-web.at/cocktails/ce8f4591-ccd4-4d90-a761-244115d64061> , <http://vocabulary.semantic-web.at/cocktails/f01f6a10-01a5-4810-860f-d3a52fd36b1b> ;
	a <http://vocabulary.semantic-web.at/cocktail-ontology/Beverages> , <http://vocabulary.semantic-web.at/cocktail-ontology/Ingredients> , <http://vocabulary.semantic-web.at/cocktail-ontology/Non-alcoholic-Beverages> , skos:Concept ;
	skos:altLabel "Clear cola"@en , "Coke (cola)"@en , "Cola drinks"@en , "Diet cola"@en ;
	skos:broader <http://vocabulary.semantic-web.at/cocktails/a2b8e0e7-0dd0-40e2-a9a4-6178c7728cd0> ;
	skos:definition "Cola is a carbonated beverage that originally contained caffeine from the kola nut and cocaine from coca leaves and was flovoured with vanilla and other ingredients. Most colas now use other flavoring (and caffeinating) ingredients with a similar taste and no longer contain cocaine. It became popular worldwide after druggist John Pemberton invented Coca-Cola in 1886. His non-alcoholic recipe was inspired by the Coca wine of pharmacist Angelo Mariani, created in 1863; it still contained cocaine."@en ;
	skos:exactMatch dbpedia:Cola ;
	skos:prefLabel "Cola"@en .

<http://vocabulary.semantic-web.at/cocktails/0f6d360f-af24-4d66-8f70-760c927ed0a7> dcterms:created "2015-05-02T17:29:41Z"^^xsd:dateTime ;
	dcterms:creator <http://localhost/user/blumauera> ;
	<http://schema.semantic-web.at/ppt/inScheme> <http://vocabulary.semantic-web.at/cocktails/591cf89a-57af-49b8-9042-3fc77408c93e> ;
	<http://schema.semantic-web.at/ppt/inSubtree> <http://vocabulary.semantic-web.at/cocktails/403d1249-f37f-4f43-bebf-8dde9677d886> ;
	a <http://vocabulary.semantic-web.at/cocktail-ontology/Alcoholic-Beverages> , <http://vocabulary.semantic-web.at/cocktail-ontology/Beverages> , <http://vocabulary.semantic-web.at/cocktail-ontology/Ingredients> , skos:Concept ;
	skos:broader <http://vocabulary.semantic-web.at/cocktails/2944baef-5338-421b-a5f5-0e51f75244c2> ;
	skos:narrower <http://vocabulary.semantic-web.at/cocktails/687a5d86-1f4e-4a6b-b5ca-3b5d74aeafcc> , <http://vocabulary.semantic-web.at/cocktails/ee61817b-0d10-4862-b44b-740c990e676e> ;
	skos:prefLabel "Berry liqueurs"@en .

<http://vocabulary.semantic-web.at/cocktails/0f8cc862-9056-49be-b636-cd22f8d7282d> dcterms:contributor <http://localhost/user/blumauera> ;
	dcterms:created "2015-05-02T17:16:18Z"^^xsd:dateTime ;
	dcterms:creator <http://localhost/user/blumauera> ;
	dcterms:modified "2015-05-07T06:42:33Z"^^xsd:dateTime ;
	<http://schema.semantic-web.at/ppt/inScheme> <http://vocabulary.semantic-web.at/cocktails/8d052dfc-44bf-4985-8ce3-4564570a161b> ;
	<http://vocabulary.semantic-web.at/cocktail-ontology/consists-of> <http://vocabulary.semantic-web.at/cocktails/22df810d-e509-4da8-979c-0758e94de3e6> , <http://vocabulary.semantic-web.at/cocktails/2ce50273-13b2-4ba1-9ff2-8cfbd835c1f2> , <http://vocabulary.semantic-web.at/cocktails/4be1257b-f797-4ab9-a2b3-af09b958173e> ;
	<http://vocabulary.semantic-web.at/cocktail-ontology/iba> <http://www.iba-world.com/index.php?option=com_content&id=263&Itemid=532> ;
	<http://vocabulary.semantic-web.at/cocktail-ontology/image> <http://upload.wikimedia.org/wikipedia/commons/4/44/Harvey_Wallbanger.jpg> ;
	<http://vocabulary.semantic-web.at/cocktail-ontology/preparation> "Stir the vodka and orange juice with ice in the glass, then float the Galliano on top. Garnish and serve."@en ;
	<http://vocabulary.semantic-web.at/cocktail-ontology/served> "On the rocks; poured over ice"@en ;
	<http://vocabulary.semantic-web.at/cocktail-ontology/uses> <http://vocabulary.semantic-web.at/cocktails/a54d2096-6214-4006-beaf-afcc77824710> ;
	<http://vocabulary.semantic-web.at/cocktail-ontology/uses_2> <http://vocabulary.semantic-web.at/cocktails/62fbc16f-3f84-4cc7-8c6f-5afebfc1510a> , <http://vocabulary.semantic-web.at/cocktails/99171f20-c59f-40c4-998a-a9c8f1909168> ;
	a <http://vocabulary.semantic-web.at/cocktail-ontology/Cocktail> , skos:Concept ;
	skos:broader <http://vocabulary.semantic-web.at/cocktails/b9bf3799-a4e4-47f7-9aea-7697cc998a34> ;
	skos:definition "The Harvey Wallbanger is a cocktail made with vodka, Galliano, and orange juice."@en ;
	skos:exactMatch dbpedia:Harvey_Wallbanger ;
	skos:prefLabel "Harvey Wallbanger"@en .

<http://vocabulary.semantic-web.at/cocktails/105184cf-c7fa-4e7c-b668-b4db7a689ab7> dcterms:contributor <http://localhost/user/huberf> ;
	dcterms:created "2015-05-02T08:23:44Z"^^xsd:dateTime ;
	dcterms:creator <http://localhost/user/blumauera> ;
	dcterms:modified "2016-10-05T09:34:43Z"^^xsd:dateTime ;
	<http://schema.semantic-web.at/ppt/inScheme> <http://vocabulary.semantic-web.at/cocktails/6fe33361-f993-416d-bc13-cb36c326736b> ;
	a <http://vocabulary.semantic-web.at/cocktail-ontology/Ingredients> , skos:Concept ;
	skos:altLabel "Chile sauce"@en , "Chili Sauce"@en , "Chili sauce"@en , "Chilli sauce"@en , "Pepper extract"@en , "Pepper sauce"@en ;
	skos:definition "Hot sauce, chili sauce or pepper sauce refers to any spicy sauce condiment made from chili peppers and other ingredients."@en ;
	skos:exactMatch dbpedia:Hot_sauce ;
	skos:narrower <http://vocabulary.semantic-web.at/cocktails/94cca1b4-3603-472b-9c78-6d6a43b6b4ca> ;
	skos:prefLabel "Hot sauce"@en ;
	skos:topConceptOf <http://vocabulary.semantic-web.at/cocktails/6fe33361-f993-416d-bc13-cb36c326736b> .

<http://vocabulary.semantic-web.at/cocktails/108f19eb-a64b-47ce-b25f-c15049a0f4be> dcterms:contributor <http://localhost/user/blumauera> ;
	dcterms:created "2015-05-02T19:49:53Z"^^xsd:dateTime ;
	dcterms:creator <http://localhost/user/blumauera> ;
	dcterms:modified "2015-05-05T13:07:25Z"^^xsd:dateTime ;
	<http://schema.semantic-web.at/ppt/inScheme> <http://vocabulary.semantic-web.at/cocktails/591cf89a-57af-49b8-9042-3fc77408c93e> ;
	<http://schema.semantic-web.at/ppt/inSubtree> <http://vocabulary.semantic-web.at/cocktails/d5286375-41b3-468b-9602-8fcf698e3e83> ;
	<http://vocabulary.semantic-web.at/cocktail-ontology/is-part-of> <http://vocabulary.semantic-web.at/cocktails/b00a123f-a2b5-49d2-8325-a81d1d26ddc6> ;
	a <http://vocabulary.semantic-web.at/cocktail-ontology/Alcoholic-Beverages> , <http://vocabulary.semantic-web.at/cocktail-ontology/Beverages> , <http://vocabulary.semantic-web.at/cocktail-ontology/Ingredients> , skos:Concept ;
	skos:altLabel "Kina Lillet"@en , "Kina lillet"@en ;
	skos:broader <http://vocabulary.semantic-web.at/cocktails/70c69ab8-78ab-41b8-a93c-314cdeda1da4> ;
	skos:definition "Lillet (French pronunciation) is a brand of French aperitif wine. It is a blend of 85% Bordeaux wines (Sauvignon Blanc, Semillon and Muscadelle for the Blanc; Merlot and Cabernet Sauvignon for the Rouge) and 15% macerated liqueurs, mostly citrus liqueurs from the peels of sweet oranges from Spain and Morocco and the peels of bitter green oranges from Haiti."@en ;
	skos:exactMatch dbpedia:Lillet ;
	skos:prefLabel "Lillet"@en .

<http://vocabulary.semantic-web.at/cocktails/117bd4d2-6da3-4d69-8c79-bc1d873b5010> dcterms:contributor <http://localhost/user/blumauera> ;
	dcterms:created "2015-05-02T17:14:04Z"^^xsd:dateTime ;
	dcterms:creator <http://localhost/user/blumauera> ;
	dcterms:modified "2016-02-22T16:43:54Z"^^xsd:dateTime ;
	<http://schema.semantic-web.at/ppt/inScheme> <http://vocabulary.semantic-web.at/cocktails/8d052dfc-44bf-4985-8ce3-4564570a161b> ;
	<http://vocabulary.semantic-web.at/cocktail-ontology/consists-of> <http://vocabulary.semantic-web.at/cocktails/038615ab-5b6e-4293-a8ca-53cf0fb92340> , <http://vocabulary.semantic-web.at/cocktails/8352ad8c-0355-4ca4-9ff7-c3dff28931c5> , <http://vocabulary.semantic-web.at/cocktails/e406119b-7637-43f9-9a62-5a8ea500ebc4> ;
	<http://vocabulary.semantic-web.at/cocktail-ontology/iba> <http://www.iba-world.com/index.php?option=com_content&id=220&Itemid=532> ;
	<http://vocabulary.semantic-web.at/cocktail-ontology/image> <http://upload.wikimedia.org/wikipedia/commons/thumb/7/7b/Grasshopper_cocktail.jpg/440px-Grasshopper_cocktail.jpg> ;
	<http://vocabulary.semantic-web.at/cocktail-ontology/preparation> "Pour ingredients into a cocktail shaker with ice. Shake briskly and then strain into a chilled cocktail glass."@en ;
	<http://vocabulary.semantic-web.at/cocktail-ontology/served> "Straight up; without ice"@en ;
	<http://vocabulary.semantic-web.at/cocktail-ontology/uses> <http://vocabulary.semantic-web.at/cocktails/19dee0d8-fd30-469f-9ecd-91c902ff717c> ;
	a <http://vocabulary.semantic-web.at/cocktail-ontology/Cocktail> , skos:Concept ;
	skos:altLabel "Grasshopper (beverage)"@en , "Grasshopper (drink)"@en , "Grasshopper cocktail"@en ;
	skos:broader <http://vocabulary.semantic-web.at/cocktails/b9bf3799-a4e4-47f7-9aea-7697cc998a34> ;
	skos:definition "A grasshopper is a sweet, mint-flavored, after-dinner drink. The name of the drink is derived from its green color, which is provided by the crème de menthe. The drink reputedly originated at Tujague's, a landmark bar in the French Quarter of New Orleans, Louisiana, and gained popularity during the 1950s and 1960s throughout the American South."@en ;
	skos:exactMatch <http://dbpedia.org/resource/Grasshopper_(cocktail)> ;
	skos:prefLabel "Grasshopper"@en .

<http://vocabulary.semantic-web.at/cocktails/11d68913-3a30-4591-bc41-25fea3f38520> dcterms:contributor <http://localhost/user/nagyhel> ;
	dcterms:created "2015-05-02T19:20:26Z"^^xsd:dateTime ;
	dcterms:creator <http://localhost/user/blumauera> ;
	dcterms:modified "2015-11-03T14:54:18Z"^^xsd:dateTime ;
	<http://schema.semantic-web.at/ppt/inScheme> <http://vocabulary.semantic-web.at/cocktails/8d052dfc-44bf-4985-8ce3-4564570a161b> ;
	<http://vocabulary.semantic-web.at/cocktail-ontology/consists-of> <http://vocabulary.semantic-web.at/cocktails/074c3acb-bc4d-4c6e-ad8a-e553d5ec7eff> , <http://vocabulary.semantic-web.at/cocktails/441a0d9e-f4e1-434a-9cb4-503bb840e23a> , <http://vocabulary.semantic-web.at/cocktails/5d96c50c-ee48-4c40-bb4c-4b9a42d11de6> ;
	<http://vocabulary.semantic-web.at/cocktail-ontology/iba> <http://www.iba-world.com/index.php?option=com_content&id=241&Itemid=532> ;
	<http://vocabulary.semantic-web.at/cocktail-ontology/image> <http://www.iba-world.com/images/cocktail_drinks/dirty_martini.jpg> ;
	<http://vocabulary.semantic-web.at/cocktail-ontology/is-variant-of> <http://vocabulary.semantic-web.at/cocktails/a0fba95c-d29e-4954-8800-f5e6de1e6f86> ;
	<http://vocabulary.semantic-web.at/cocktail-ontology/preparation> "Pour all ingredients into mixing glass with ice cubes. Stir well. Strain in chilled martini glass. Garnish with green olive."@en ;
	<http://vocabulary.semantic-web.at/cocktail-ontology/uses> <http://vocabulary.semantic-web.at/cocktails/19dee0d8-fd30-469f-9ecd-91c902ff717c> ;
	<http://vocabulary.semantic-web.at/cocktail-ontology/uses_2> <http://vocabulary.semantic-web.at/cocktails/cec5e96c-41c6-4b82-ab3a-0a057a54f70a> ;
	a <http://vocabulary.semantic-web.at/cocktail-ontology/Cocktail> , skos:Concept ;
	skos:broader <http://vocabulary.semantic-web.at/cocktails/ccee1079-43df-4ff1-bef0-d15d3dc8fa6f> ;
	skos:prefLabel "Dirty Martini"@en .

<http://vocabulary.semantic-web.at/cocktails/12da816f-8ad3-487d-b8f9-2190e4b3e1b8> dcterms:contributor <http://localhost/user/blumauera> ;
	dcterms:created "2015-05-01T14:56:52Z"^^xsd:dateTime ;
	dcterms:creator <http://localhost/user/blumauera> ;
	dcterms:modified "2015-05-07T07:13:48Z"^^xsd:dateTime ;
	<http://schema.semantic-web.at/ppt/inScheme> <http://vocabulary.semantic-web.at/cocktails/591cf89a-57af-49b8-9042-3fc77408c93e> ;
	<http://schema.semantic-web.at/ppt/inSubtree> <http://vocabulary.semantic-web.at/cocktails/e86c1671-4a67-494b-ae5d-bcb750865acc> ;
	<http://vocabulary.semantic-web.at/cocktail-ontology/is-part-of> <http://vocabulary.semantic-web.at/cocktails/43111fc3-3b59-420c-a588-024cd2d33896> , <http://vocabulary.semantic-web.at/cocktails/4792b0b8-0046-47ca-8c2a-f3ad58922182> , <http://vocabulary.semantic-web.at/cocktails/4d15a643-f7c7-4ee5-8f56-4ebd2bcf74b5> , <http://vocabulary.semantic-web.at/cocktails/680c7429-30a7-4044-b32f-e28c99dcb9f4> , <http://vocabulary.semantic-web.at/cocktails/785b30fd-1eb4-445b-8247-7e1e57b35b0f> , <http://vocabulary.semantic-web.at/cocktails/9c287d15-c699-4f56-bd65-bf8cc75a2cca> ;
	a <http://vocabulary.semantic-web.at/cocktail-ontology/Beverages> , <http://vocabulary.semantic-web.at/cocktail-ontology/Ingredients> , <http://vocabulary.semantic-web.at/cocktail-ontology/Non-alcoholic-Beverages> , skos:Concept ;
	skos:broader <http://vocabulary.semantic-web.at/cocktails/6c0607a9-410d-4b65-87a1-b189a8e36352> ;
	skos:prefLabel "Pineapple juice"@en .

<http://vocabulary.semantic-web.at/cocktails/12f4790a-560f-4e1c-b57a-53b8171ae39a> dcterms:contributor <http://localhost/user/blumauera> ;
	dcterms:created "2015-05-01T07:35:58Z"^^xsd:dateTime ;
	dcterms:creator <http://localhost/user/blumauera> ;
	dcterms:modified "2015-05-03T10:08:50Z"^^xsd:dateTime ;
	<http://schema.semantic-web.at/ppt/inScheme> <http://vocabulary.semantic-web.at/cocktails/8d052dfc-44bf-4985-8ce3-4564570a161b> ;
	<http://vocabulary.semantic-web.at/cocktail-ontology/consists-of> <http://vocabulary.semantic-web.at/cocktails/22df810d-e509-4da8-979c-0758e94de3e6> , <http://vocabulary.semantic-web.at/cocktails/45234a8f-9357-49d2-931b-638c48e3772e> , <http://vocabulary.semantic-web.at/cocktails/abe8b872-3a29-49a3-9a8e-1b71db770a3f> ;
	<http://vocabulary.semantic-web.at/cocktail-ontology/iba> <http://www.iba-world.com/index.php?option=com_content&id=234> ;
	<http://vocabulary.semantic-web.at/cocktail-ontology/image> <http://upload.wikimedia.org/wikipedia/commons/b/b1/Cocktail_with_vodka.jpg> ;
	<http://vocabulary.semantic-web.at/cocktail-ontology/preparation> "Build all ingredients in a highball glass filled with ice. Garnish with lime wedge."@en ;
	<http://vocabulary.semantic-web.at/cocktail-ontology/served> "On the rocks; poured over ice"@en ;
	<http://vocabulary.semantic-web.at/cocktail-ontology/uses> <http://vocabulary.semantic-web.at/cocktails/a54d2096-6214-4006-beaf-afcc77824710> ;
	<http://vocabulary.semantic-web.at/cocktail-ontology/uses_2> <http://vocabulary.semantic-web.at/cocktails/021c85c0-a60a-4414-8fd8-bd3383b794f1> ;
	a <http://vocabulary.semantic-web.at/cocktail-ontology/Cocktail> , skos:Concept ;
	skos:broader <http://vocabulary.semantic-web.at/cocktails/54702498-ad42-4af6-b28a-2276215450da> , <http://vocabulary.semantic-web.at/cocktails/b9bf3799-a4e4-47f7-9aea-7697cc998a34> ;
	skos:definition "A Sea Breeze is a cocktail containing vodka with cranberry juice and grapefruit juice. The cocktail is usually consumed during summer months. The drink may be shaken in order to create a foamy surface. It is considered an IBA Official Cocktail. The drink follows the classic cocktail principle of balancing strong with weak and sweet and sour. A Bay Breeze, or a Hawaiian Sea Breeze, is similar to a Sea Breeze except for the substitution of pineapple juice for grapefruit juice."@en ;
	skos:exactMatch <http://dbpedia.org/resource/Sea_Breeze_(cocktail)> ;
	skos:prefLabel "Sea Breeze"@en .

<http://vocabulary.semantic-web.at/cocktails/13b85b5c-7f69-4871-bb08-3cd5281f6039> dcterms:contributor <http://localhost/user/blumauera> ;
	dcterms:created "2015-05-02T17:12:48Z"^^xsd:dateTime ;
	dcterms:creator <http://localhost/user/blumauera> ;
	dcterms:modified "2015-05-06T13:00:12Z"^^xsd:dateTime ;
	<http://schema.semantic-web.at/ppt/inScheme> <http://vocabulary.semantic-web.at/cocktails/8d052dfc-44bf-4985-8ce3-4564570a161b> ;
	<http://vocabulary.semantic-web.at/cocktail-ontology/consists-of> <http://vocabulary.semantic-web.at/cocktails/038615ab-5b6e-4293-a8ca-53cf0fb92340> , <http://vocabulary.semantic-web.at/cocktails/2ce50273-13b2-4ba1-9ff2-8cfbd835c1f2> , <http://vocabulary.semantic-web.at/cocktails/397d0ec3-98e2-47d9-a8c2-eca9702ff94d> , <http://vocabulary.semantic-web.at/cocktails/4be1257b-f797-4ab9-a2b3-af09b958173e> ;
	<http://vocabulary.semantic-web.at/cocktail-ontology/iba> <http://www.iba-world.com/index.php?option=com_content&id=219&Itemid=532> ;
	<http://vocabulary.semantic-web.at/cocktail-ontology/image> <http://upload.wikimedia.org/wikipedia/commons/1/15/Godlen-Dream_Mixed_Drink_Cocktail_%282360538105%29.jpg> ;
	<http://vocabulary.semantic-web.at/cocktail-ontology/uses> <http://vocabulary.semantic-web.at/cocktails/19dee0d8-fd30-469f-9ecd-91c902ff717c> ;
	a <http://vocabulary.semantic-web.at/cocktail-ontology/Cocktail> , skos:Concept ;
	skos:broader <http://vocabulary.semantic-web.at/cocktails/b9bf3799-a4e4-47f7-9aea-7697cc998a34> ;
	skos:definition "The Golden Dream is an IBA official cocktail made with the uncommon Liquore Galliano and Cointreau. It is classed as an \"after dinner\" drink."@en ;
	skos:exactMatch <http://dbpedia.org/resource/Golden_dream_(cocktail)> ;
	skos:prefLabel "Golden dream"@en .

<http://vocabulary.semantic-web.at/cocktails/1439e6c3-a155-4c80-8a5d-723453b4d17e> dcterms:contributor <http://localhost/user/blumauera> ;
	dcterms:created "2015-05-01T08:36:35Z"^^xsd:dateTime ;
	dcterms:creator <http://localhost/user/blumauera> ;
	dcterms:modified "2015-05-07T07:13:17Z"^^xsd:dateTime ;
	<http://schema.semantic-web.at/ppt/inScheme> <http://vocabulary.semantic-web.at/cocktails/591cf89a-57af-49b8-9042-3fc77408c93e> ;
	<http://schema.semantic-web.at/ppt/inSubtree> <http://vocabulary.semantic-web.at/cocktails/403d1249-f37f-4f43-bebf-8dde9677d886> ;
	<http://vocabulary.semantic-web.at/cocktail-ontology/is-part-of> <http://vocabulary.semantic-web.at/cocktails/2d85fb1b-96cb-4c48-8df5-707032f34e71> , <http://vocabulary.semantic-web.at/cocktails/43111fc3-3b59-420c-a588-024cd2d33896> ;
	a <http://vocabulary.semantic-web.at/cocktail-ontology/Alcoholic-Beverages> , <http://vocabulary.semantic-web.at/cocktail-ontology/Beverages> , <http://vocabulary.semantic-web.at/cocktail-ontology/Ingredients> , skos:Concept ;
	skos:altLabel "Cuantro"@en ;
	skos:broader <http://vocabulary.semantic-web.at/cocktails/397d0ec3-98e2-47d9-a8c2-eca9702ff94d> ;
	skos:definition "Cointreau is a brand of triple sec (an orange-flavoured liqueur) produced in Saint-Barthélemy-d'Anjou, France. It is drunk as an apéritif and digestif, and is a component of several well-known cocktails. It was originally called \"Curaçao Blanco Triple Sec\"."@en ;
	skos:exactMatch dbpedia:Cointreau ;
	skos:prefLabel "Cointreau"@en .

<http://vocabulary.semantic-web.at/cocktails/1529fd23-9c55-45d7-b8c6-b0fc229a3871> dcterms:contributor <http://localhost/user/blumauera> ;
	dcterms:created "2015-05-02T18:34:58Z"^^xsd:dateTime ;
	dcterms:creator <http://localhost/user/blumauera> ;
	dcterms:modified "2015-05-07T06:57:02Z"^^xsd:dateTime ;
	<http://schema.semantic-web.at/ppt/inScheme> <http://vocabulary.semantic-web.at/cocktails/8d052dfc-44bf-4985-8ce3-4564570a161b> ;
	<http://vocabulary.semantic-web.at/cocktail-ontology/consists-of> <http://vocabulary.semantic-web.at/cocktails/3e2d26b8-928b-462d-99ee-59eac11b241f> , <http://vocabulary.semantic-web.at/cocktails/84c72e0e-7830-46ef-ac35-44cad56d27ec> , <http://vocabulary.semantic-web.at/cocktails/91b112c0-2fcc-4495-b68c-b1f09fa0a698> , <http://vocabulary.semantic-web.at/cocktails/cd4b845c-d8db-4f73-9a0c-b60743c58019> ;
	<http://vocabulary.semantic-web.at/cocktail-ontology/iba> <http://www.iba-world.com/index.php?option=com_content&id=231&Itemid=532> ;
	<http://vocabulary.semantic-web.at/cocktail-ontology/image> <http://upload.wikimedia.org/wikipedia/commons/thumb/5/55/Mint_Julep_im_Silberbecher.jpg/440px-Mint_Julep_im_Silberbecher.jpg> ;
	<http://vocabulary.semantic-web.at/cocktail-ontology/preparation> "In a highball glass gently muddle the mint, sugar and water. Fill the glass with cracked ice, add Bourbon and stir well until the glass is frost. Garnish with a mint spring."@en ;
	<http://vocabulary.semantic-web.at/cocktail-ontology/served> "On the rocks; poured over ice"@en ;
	<http://vocabulary.semantic-web.at/cocktail-ontology/uses> <http://vocabulary.semantic-web.at/cocktails/a54d2096-6214-4006-beaf-afcc77824710> ;
	<http://vocabulary.semantic-web.at/cocktail-ontology/uses_2> <http://vocabulary.semantic-web.at/cocktails/91b112c0-2fcc-4495-b68c-b1f09fa0a698> ;
	a <http://vocabulary.semantic-web.at/cocktail-ontology/Cocktail> , skos:Concept ;
	skos:altLabel "Julep"@en , "Mint julip"@en ;
	skos:broader <http://vocabulary.semantic-web.at/cocktails/b9bf3799-a4e4-47f7-9aea-7697cc998a34> ;
	skos:definition "The mint julep is a mixed alcoholic drink, or cocktail, associated with the cuisine of the Southern United States."@en ;
	skos:exactMatch dbpedia:Mint_julep ;
	skos:prefLabel "Mint julep"@en .

<http://vocabulary.semantic-web.at/cocktails/1576f08f-5936-4071-b85e-d4e85f31c303> dcterms:contributor <http://localhost/user/blumauera> ;
	dcterms:created "2015-05-01T15:13:28Z"^^xsd:dateTime ;
	dcterms:creator <http://localhost/user/blumauera> ;
	dcterms:modified "2015-05-04T11:39:23Z"^^xsd:dateTime ;
	<http://schema.semantic-web.at/ppt/inScheme> <http://vocabulary.semantic-web.at/cocktails/8d052dfc-44bf-4985-8ce3-4564570a161b> ;
	<http://vocabulary.semantic-web.at/cocktail-ontology/consists-of> <http://vocabulary.semantic-web.at/cocktails/3c94f5fc-4664-4177-a880-88643c0be9c1> , <http://vocabulary.semantic-web.at/cocktails/c96d576c-9640-4c21-af92-d6da3560c9d0> , <http://vocabulary.semantic-web.at/cocktails/fbfae34b-60d5-47e6-83dc-31507a8d4f78> , <http://vocabulary.semantic-web.at/cocktails/fd76c5ab-be62-4c4b-a2c6-7fa9bc359f47> ;
	<http://vocabulary.semantic-web.at/cocktail-ontology/iba> <http://www.iba-world.com/index.php?option=com_content&id=208&Itemid=532> ;
	<http://vocabulary.semantic-web.at/cocktail-ontology/image> <http://upload.wikimedia.org/wikipedia/commons/thumb/d/dd/SazeracRooseveltNOLA1July2009.JPG/440px-SazeracRooseveltNOLA1July2009.JPG> ;
	<http://vocabulary.semantic-web.at/cocktail-ontology/preparation> "Rinse a chilled old-fashioned glass with the absinthe, add crushed ice and set it aside. Stir the remaining ingredients over ice and set it aside. Discard the ice and any excess absinthe from the prepared glass, and strain the drink into the glass. Add the Lemon peel for garnish."@en ;
	<http://vocabulary.semantic-web.at/cocktail-ontology/served> "Straight up; without ice"@en ;
	<http://vocabulary.semantic-web.at/cocktail-ontology/uses> <http://vocabulary.semantic-web.at/cocktails/2dce3576-2603-41f9-8dce-ab21f639c2a7> ;
	<http://vocabulary.semantic-web.at/cocktail-ontology/uses_2> <http://vocabulary.semantic-web.at/cocktails/33df103a-03ac-4177-b620-7953fe094236> ;
	a <http://vocabulary.semantic-web.at/cocktail-ontology/Cocktail> , skos:Concept ;
	skos:altLabel "Sazarac"@en , "Sazerac (cocktail)"@en ;
	skos:broader <http://vocabulary.semantic-web.at/cocktails/caae2ea0-7e60-400b-a2bb-14ef79720668> ;
	skos:definition "The Sazerac is a local New Orleans variation of a Cognac or whiskey cocktail, named for the Sazerac de Forge et Fils brand of Cognac brandy that served as its original main ingredient."@en ;
	skos:exactMatch dbpedia:Sazerac ;
	skos:prefLabel "Sazerac"@en .

<http://vocabulary.semantic-web.at/cocktails/16b625c5-3930-4cf8-a75b-b25e72f2bfb6> dcterms:contributor <http://localhost/user/blumauera> ;
	dcterms:created "2015-05-01T08:38:17Z"^^xsd:dateTime ;
	dcterms:creator <http://localhost/user/blumauera> ;
	dcterms:modified "2015-05-03T10:11:03Z"^^xsd:dateTime ;
	<http://schema.semantic-web.at/ppt/inScheme> <http://vocabulary.semantic-web.at/cocktails/591cf89a-57af-49b8-9042-3fc77408c93e> ;
	<http://schema.semantic-web.at/ppt/inSubtree> <http://vocabulary.semantic-web.at/cocktails/403d1249-f37f-4f43-bebf-8dde9677d886> ;
	<http://vocabulary.semantic-web.at/cocktail-ontology/is-part-of> <http://vocabulary.semantic-web.at/cocktails/b3834414-af63-4e6f-9c3c-6c353e9600ee> ;
	a <http://vocabulary.semantic-web.at/cocktail-ontology/Alcoholic-Beverages> , <http://vocabulary.semantic-web.at/cocktail-ontology/Beverages> , <http://vocabulary.semantic-web.at/cocktail-ontology/Ingredients> , skos:Concept ;
	skos:altLabel "Calvados (beverage)"@en , "Calvados (spirit)"@en , "Calvados (spirits)"@en , "Trou Normand"@en ;
	skos:broader <http://vocabulary.semantic-web.at/cocktails/8f09ee6f-d5b9-4b8a-aa17-b0665fae4e83> ;
	skos:definition "Calvados is an apple brandy from the French region of Lower Normandy (Basse-Normandie). It is sometimes abbreviated to Calva."@en ;
	skos:exactMatch <http://dbpedia.org/resource/Calvados_(brandy)> ;
	skos:prefLabel "Calvados"@en .

<http://vocabulary.semantic-web.at/cocktails/19316511-1d42-4516-9504-873c3fd8fb85> dcterms:contributor <http://localhost/user/blumauera> ;
	dcterms:created "2015-05-01T08:27:04Z"^^xsd:dateTime ;
	dcterms:creator <http://localhost/user/blumauera> ;
	dcterms:modified "2015-05-03T11:35:46Z"^^xsd:dateTime ;
	<http://schema.semantic-web.at/ppt/inScheme> <http://vocabulary.semantic-web.at/cocktails/591cf89a-57af-49b8-9042-3fc77408c93e> ;
	<http://schema.semantic-web.at/ppt/inSubtree> <http://vocabulary.semantic-web.at/cocktails/403d1249-f37f-4f43-bebf-8dde9677d886> ;
	a <http://vocabulary.semantic-web.at/cocktail-ontology/Alcoholic-Beverages> , <http://vocabulary.semantic-web.at/cocktail-ontology/Beverages> , <http://vocabulary.semantic-web.at/cocktail-ontology/Ingredients> , skos:Concept ;
	skos:altLabel "Chocolate liquer"@en , "Ratafia de cacao"@en , "Ratafia de chocolat"@en ;
	skos:broader <http://vocabulary.semantic-web.at/cocktails/2944baef-5338-421b-a5f5-0e51f75244c2> ;
	skos:definition "Chocolate liqueur is a liqueur with a principal flavor of chocolate."@en ;
	skos:exactMatch dbpedia:Chocolate_liqueur ;
	skos:narrower <http://vocabulary.semantic-web.at/cocktails/8352ad8c-0355-4ca4-9ff7-c3dff28931c5> ;
	skos:prefLabel "Chocolate liqueur"@en .

<http://vocabulary.semantic-web.at/cocktails/19dee0d8-fd30-469f-9ecd-91c902ff717c> dcterms:contributor <http://localhost/user/blumauera> ;
	dcterms:created "2015-05-01T08:39:06Z"^^xsd:dateTime ;
	dcterms:creator <http://localhost/user/blumauera> ;
	dcterms:modified "2015-11-17T08:00:27Z"^^xsd:dateTime ;
	<http://schema.semantic-web.at/ppt/inScheme> <http://vocabulary.semantic-web.at/cocktails/f09732a9-a0e6-494a-8ce9-299ef036aaaf> ;
	<http://vocabulary.semantic-web.at/cocktail-ontology/image_2> <http://upload.wikimedia.org/wikipedia/commons/thumb/1/19/Coctail_glass.svg/32px-Coctail_glass.svg.png> ;
	<http://vocabulary.semantic-web.at/cocktail-ontology/is-used-by> <http://vocabulary.semantic-web.at/cocktails/099726a2-ec4b-4b0f-b4e4-e6f25cdfd685> , <http://vocabulary.semantic-web.at/cocktails/0bbdca98-077b-48d1-99d6-47eca59c442c> , <http://vocabulary.semantic-web.at/cocktails/117bd4d2-6da3-4d69-8c79-bc1d873b5010> , <http://vocabulary.semantic-web.at/cocktails/11d68913-3a30-4591-bc41-25fea3f38520> , <http://vocabulary.semantic-web.at/cocktails/13b85b5c-7f69-4871-bb08-3cd5281f6039> , <http://vocabulary.semantic-web.at/cocktails/1d5b39cc-fcab-48b2-bb24-9840b7e34d64> , <http://vocabulary.semantic-web.at/cocktails/21b94d69-280e-4546-be1a-fdd1d9aa5d32> , <http://vocabulary.semantic-web.at/cocktails/22f838ea-3c2b-4b63-99d1-fdb6280b5705> , <http://vocabulary.semantic-web.at/cocktails/236b36df-93ca-4408-836c-133ace53798a> , <http://vocabulary.semantic-web.at/cocktails/2c3083d2-8650-4460-b019-cae7aea38f14> , <http://vocabulary.semantic-web.at/cocktails/36671f9c-904a-4629-937a-519d094ecefc> , <http://vocabulary.semantic-web.at/cocktails/44cc99c1-28ac-4c50-a55d-7244b2c5c07b> , <http://vocabulary.semantic-web.at/cocktails/4f85cadd-4fd4-4ffc-a78d-cddb0763fa4b> , <http://vocabulary.semantic-web.at/cocktails/60d3a991-48d3-4e73-9d62-5961893fd311> , <http://vocabulary.semantic-web.at/cocktails/680c7429-30a7-4044-b32f-e28c99dcb9f4> , <http://vocabulary.semantic-web.at/cocktails/785b30fd-1eb4-445b-8247-7e1e57b35b0f> , <http://vocabulary.semantic-web.at/cocktails/7e4a73d5-f73d-4890-972c-f3dfd6952fd8> , <http://vocabulary.semantic-web.at/cocktails/7e5afb63-30ec-42b4-a9f5-f61fc456107d> , <http://vocabulary.semantic-web.at/cocktails/85669fcc-a38a-4ceb-ae23-90ae3fb7e16c> , <http://vocabulary.semantic-web.at/cocktails/926b14fe-1b83-4f46-bbf9-f946be1889aa> , <http://vocabulary.semantic-web.at/cocktails/a0fba95c-d29e-4954-8800-f5e6de1e6f86> , <http://vocabulary.semantic-web.at/cocktails/a47e8f08-057a-45f2-8398-9be51ed351fc> , <http://vocabulary.semantic-web.at/cocktails/b3834414-af63-4e6f-9c3c-6c353e9600ee> , <http://vocabulary.semantic-web.at/cocktails/b8075344-1e6d-4348-bdee-83948203a974> , <http://vocabulary.semantic-web.at/cocktails/b970d408-39ca-49b0-98fc-838f96c94608> , <http://vocabulary.semantic-web.at/cocktails/bab016bd-2fd5-4809-bfe7-3225d25f116d> , <http://vocabulary.semantic-web.at/cocktails/c3ae5830-1bfd-4f37-afc9-3e88849d03cf> , <http://vocabulary.semantic-web.at/cocktails/cfa8539e-ede2-42ec-b563-d084ddb33280> , <http://vocabulary.semantic-web.at/cocktails/e039633b-03c1-47bd-a705-a104a4323e45> , <http://vocabulary.semantic-web.at/cocktails/f632b16d-1490-4587-a637-fb393d7b1e7f> ;
	a <http://vocabulary.semantic-web.at/cocktail-ontology/Drinkware> , skos:Concept ;
	skos:altLabel "Cocktail glass🍸"@en , "Double cocktail glass"@en , "Double martini"@en , "Straight up glass"@en ;
	skos:broader <http://vocabulary.semantic-web.at/cocktails/2ea18d11-7415-4282-9608-7a3f497a0928> ;
	skos:definition "A cocktail glass (also called a martini glass) is a stemmed glass which has a cone-shaped bowl placed upon a stem above a flat base. It is mainly used to serve cocktails. Its form derives from the fact that all cocktails are traditionally served chilled and contain an aromatic element."@en ;
	skos:exactMatch dbpedia:Cocktail_glass ;
	skos:prefLabel "Martini glass"@en .

<http://vocabulary.semantic-web.at/cocktails/1b9d9c87-9a94-465a-b7e9-feee6c77bf03> dcterms:contributor <http://localhost/user/blumauera> ;
	dcterms:created "2015-05-01T14:34:12Z"^^xsd:dateTime ;
	dcterms:creator <http://localhost/user/blumauera> ;
	dcterms:modified "2015-05-01T14:34:12Z"^^xsd:dateTime ;
	<http://schema.semantic-web.at/ppt/inScheme> <http://vocabulary.semantic-web.at/cocktails/591cf89a-57af-49b8-9042-3fc77408c93e> ;
	<http://schema.semantic-web.at/ppt/inSubtree> <http://vocabulary.semantic-web.at/cocktails/403d1249-f37f-4f43-bebf-8dde9677d886> ;
	a <http://vocabulary.semantic-web.at/cocktail-ontology/Alcoholic-Beverages> , <http://vocabulary.semantic-web.at/cocktail-ontology/Beverages> , <http://vocabulary.semantic-web.at/cocktail-ontology/Ingredients> , skos:Concept ;
	skos:altLabel "Chinzano"@en , "Cinzano Bianco"@en , "Cinzano Rosso"@en ;
	skos:broader <http://vocabulary.semantic-web.at/cocktails/8cfd00fe-9f5a-414e-be27-858a8bc43c7c> ;
	skos:definition "Cinzano is an Italian brand of vermouth, a brand owned since 1999 by Gruppo Campari. It comes in four versions: Cinzano Rosso, which is amber-coloured; Cinzano Bianco, which is white and drier than Rosso, yet still considered a sweet vermouth; Cinzano Extra Dry, a dry vermouth; Cinzano Rosé, the newest of the four, rosy-coloured with orange highlights"@en ;
	skos:exactMatch dbpedia:Cinzano ;
	skos:narrower <http://vocabulary.semantic-web.at/cocktails/5d0fdad6-6256-4042-a1a0-709f332cf373> , <http://vocabulary.semantic-web.at/cocktails/7a2ef9c4-4083-4531-9edc-b27e0353349e> ;
	skos:prefLabel "Cinzano"@en .

<http://vocabulary.semantic-web.at/cocktails/1be6ee21-daf9-4b15-847d-6acdb88f9104> dcterms:contributor <http://localhost/user/blumauera> ;
	dcterms:created "2015-05-01T08:46:06Z"^^xsd:dateTime ;
	dcterms:creator <http://localhost/user/blumauera> ;
	dcterms:modified "2015-05-07T07:12:59Z"^^xsd:dateTime ;
	<http://schema.semantic-web.at/ppt/inScheme> <http://vocabulary.semantic-web.at/cocktails/591cf89a-57af-49b8-9042-3fc77408c93e> ;
	<http://schema.semantic-web.at/ppt/inSubtree> <http://vocabulary.semantic-web.at/cocktails/403d1249-f37f-4f43-bebf-8dde9677d886> ;
	<http://vocabulary.semantic-web.at/cocktail-ontology/is-part-of> <http://vocabulary.semantic-web.at/cocktails/43111fc3-3b59-420c-a588-024cd2d33896> ;
	a <http://vocabulary.semantic-web.at/cocktail-ontology/Alcoholic-Beverages> , <http://vocabulary.semantic-web.at/cocktail-ontology/Beverages> , <http://vocabulary.semantic-web.at/cocktail-ontology/Ingredients> , skos:Concept ;
	skos:broader <http://vocabulary.semantic-web.at/cocktails/2944baef-5338-421b-a5f5-0e51f75244c2> ;
	skos:narrower <http://vocabulary.semantic-web.at/cocktails/224b4628-2f46-44a1-9d2f-8b5ef0b31e79> ;
	skos:prefLabel "Cherry-flavored liqueur"@en .

<http://vocabulary.semantic-web.at/cocktails/1c6b25d5-2b8e-49f9-8d26-5d26438cb1aa> dcterms:contributor <http://localhost/user/blumauera> ;
	dcterms:created "2015-05-07T07:09:20Z"^^xsd:dateTime ;
	dcterms:creator <http://localhost/user/blumauera> ;
	dcterms:modified "2015-05-07T07:09:20Z"^^xsd:dateTime ;
	<http://schema.semantic-web.at/ppt/inScheme> <http://vocabulary.semantic-web.at/cocktails/591cf89a-57af-49b8-9042-3fc77408c93e> ;
	<http://schema.semantic-web.at/ppt/inSubtree> <http://vocabulary.semantic-web.at/cocktails/403d1249-f37f-4f43-bebf-8dde9677d886> ;
	a <http://vocabulary.semantic-web.at/cocktail-ontology/Alcoholic-Beverages> , <http://vocabulary.semantic-web.at/cocktail-ontology/Beverages> , <http://vocabulary.semantic-web.at/cocktail-ontology/Ingredients> , skos:Concept ;
	skos:altLabel "Eau-de-vie"@en , "Eaux de vie"@en , "Eaux-de-vie"@en ;
	skos:broader <http://vocabulary.semantic-web.at/cocktails/8f09ee6f-d5b9-4b8a-aa17-b0665fae4e83> ;
	skos:definition "An eau de vie (plural, eaux de vie — also spelled eau-de-vie and eaux-de-vie) is a clear, colorless fruit brandy that is produced by means of fermentation and double distillation. The fruit flavor is typically very light. In English speaking countries, eau de vie refers to a distilled beverage made from fruit other than grapes. Similar terms may be local translations or may specify the fruit used to produce it."@en ;
	skos:exactMatch dbpedia:Eau_de_vie ;
	skos:prefLabel "Eau de vie"@en .

<http://vocabulary.semantic-web.at/cocktails/1ca477d1-98d5-4a16-82e2-a4b07c34fdbe> dcterms:contributor <http://localhost/user/blumauera> ;
	dcterms:created "2015-05-02T07:32:03Z"^^xsd:dateTime ;
	dcterms:creator <http://localhost/user/blumauera> ;
	dcterms:modified "2015-11-12T12:38:57Z"^^xsd:dateTime ;
	<http://schema.semantic-web.at/ppt/inScheme> <http://vocabulary.semantic-web.at/cocktails/eff672ac-6601-42c6-a3e9-0adda3b45df8> ;
	<http://schema.semantic-web.at/ppt/inSubtree> <http://vocabulary.semantic-web.at/cocktails/469959a3-10dc-4539-80ff-08bf9ff2de1c> ;
	<http://vocabulary.semantic-web.at/cocktail-ontology/is-used-by_2> <http://vocabulary.semantic-web.at/cocktails/268fb62f-8ef1-45cd-844f-8c7da85a6a0b> ;
	a <http://vocabulary.semantic-web.at/cocktail-ontology/Garnish> , <http://vocabulary.semantic-web.at/cocktail-ontology/Ingredients> , skos:Concept ;
	skos:altLabel "Apium graveolens"@en , "Celery (vegetable)"@en , "Celery seed"@en , "Chinese celery"@en , "Smallage"@en ;
	skos:broader <http://vocabulary.semantic-web.at/cocktails/469959a3-10dc-4539-80ff-08bf9ff2de1c> ;
	skos:definition "Apium graveolens var. dulce is a plant variety in the family Apiaceae. The plant grows to 1 m tall. The leaves are pinnate to bipinnate leaves with rhombic leaflets 3–6 cm long and 2–4 cm broad. The flowers are creamy-white, 2–3 mm diameter, produced in dense compound umbels. The seeds are broad ovoid to globose, 1.5–2 mm long and wide."@en ;
	skos:exactMatch dbpedia:Celery ;
	skos:prefLabel "Celery"@en .

<http://vocabulary.semantic-web.at/cocktails/1d5b39cc-fcab-48b2-bb24-9840b7e34d64> dcterms:contributor <http://localhost/user/blumauera> ;
	dcterms:created "2015-05-02T07:14:16Z"^^xsd:dateTime ;
	dcterms:creator <http://localhost/user/blumauera> ;
	dcterms:modified "2015-05-05T06:20:03Z"^^xsd:dateTime ;
	<http://schema.semantic-web.at/ppt/inScheme> <http://vocabulary.semantic-web.at/cocktails/8d052dfc-44bf-4985-8ce3-4564570a161b> ;
	<http://vocabulary.semantic-web.at/cocktail-ontology/consists-of> <http://vocabulary.semantic-web.at/cocktails/074c3acb-bc4d-4c6e-ad8a-e553d5ec7eff> , <http://vocabulary.semantic-web.at/cocktails/0a9e12b8-afa5-425a-b08b-941374b3bdc4> , <http://vocabulary.semantic-web.at/cocktails/224b4628-2f46-44a1-9d2f-8b5ef0b31e79> , <http://vocabulary.semantic-web.at/cocktails/809f470a-4be7-47e8-9356-cb71009c31c2> , <http://vocabulary.semantic-web.at/cocktails/c96d576c-9640-4c21-af92-d6da3560c9d0> ;
	<http://vocabulary.semantic-web.at/cocktail-ontology/iba> <http://www.iba-world.com/index.php?option=com_content&id=213&Itemid=532> ;
	<http://vocabulary.semantic-web.at/cocktail-ontology/image> <http://www.iba-world.com/images/cocktail_drinks/tuxedo.jpg> ;
	<http://vocabulary.semantic-web.at/cocktail-ontology/preparation> "Stir all ingredients with ice and strain into cocktail glass. Garnish with a cocktail cherry and a lemon zest twist."@en ;
	<http://vocabulary.semantic-web.at/cocktail-ontology/uses> <http://vocabulary.semantic-web.at/cocktails/19dee0d8-fd30-469f-9ecd-91c902ff717c> ;
	<http://vocabulary.semantic-web.at/cocktail-ontology/uses_2> <http://vocabulary.semantic-web.at/cocktails/33df103a-03ac-4177-b620-7953fe094236> , <http://vocabulary.semantic-web.at/cocktails/62fbc16f-3f84-4cc7-8c6f-5afebfc1510a> ;
	a <http://vocabulary.semantic-web.at/cocktail-ontology/Cocktail> , skos:Concept ;
	skos:broader <http://vocabulary.semantic-web.at/cocktails/caae2ea0-7e60-400b-a2bb-14ef79720668> ;
	skos:prefLabel "Tuxedo"@en .

<http://vocabulary.semantic-web.at/cocktails/1d8d3cdc-91a7-421d-ad66-4814f475eddc> dcterms:contributor <http://localhost/user/blumauera> ;
	dcterms:created "2015-05-03T17:39:33Z"^^xsd:dateTime ;
	dcterms:creator <http://localhost/user/blumauera> ;
	dcterms:modified "2015-05-03T17:40:24Z"^^xsd:dateTime ;
	<http://schema.semantic-web.at/ppt/inScheme> <http://vocabulary.semantic-web.at/cocktails/591cf89a-57af-49b8-9042-3fc77408c93e> ;
	<http://schema.semantic-web.at/ppt/inSubtree> <http://vocabulary.semantic-web.at/cocktails/403d1249-f37f-4f43-bebf-8dde9677d886> ;
	<http://vocabulary.semantic-web.at/cocktail-ontology/is-part-of> <http://vocabulary.semantic-web.at/cocktails/85669fcc-a38a-4ceb-ae23-90ae3fb7e16c> ;
	a <http://vocabulary.semantic-web.at/cocktail-ontology/Alcoholic-Beverages> , <http://vocabulary.semantic-web.at/cocktail-ontology/Beverages> , <http://vocabulary.semantic-web.at/cocktail-ontology/Ingredients> , skos:Concept ;
	skos:broader <http://vocabulary.semantic-web.at/cocktails/d40e2215-bc1b-4bae-8cf8-d10b1ad36d44> ;
	skos:prefLabel "Peach bitters"@en .

<http://vocabulary.semantic-web.at/cocktails/204c40af-075d-4bf6-a54e-33a60c54ac35> dcterms:contributor <http://localhost/user/blumauera> ;
	dcterms:created "2015-05-01T15:04:43Z"^^xsd:dateTime ;
	dcterms:creator <http://localhost/user/blumauera> ;
	dcterms:modified "2015-05-01T15:05:38Z"^^xsd:dateTime ;
	<http://schema.semantic-web.at/ppt/inScheme> <http://vocabulary.semantic-web.at/cocktails/591cf89a-57af-49b8-9042-3fc77408c93e> ;
	<http://schema.semantic-web.at/ppt/inSubtree> <http://vocabulary.semantic-web.at/cocktails/e86c1671-4a67-494b-ae5d-bcb750865acc> ;
	a <http://vocabulary.semantic-web.at/cocktail-ontology/Beverages> , <http://vocabulary.semantic-web.at/cocktail-ontology/Ingredients> , <http://vocabulary.semantic-web.at/cocktail-ontology/Non-alcoholic-Beverages> , skos:Concept ;
	skos:altLabel "Essential water"@en , "Herb distillate"@en , "Herbal distillates"@en , "Hydrolate"@en , "Hydrosol"@en ;
	skos:broader <http://vocabulary.semantic-web.at/cocktails/e86c1671-4a67-494b-ae5d-bcb750865acc> ;
	skos:definition "Herbal distillates are aqueous solutions or colloidal suspensions (hydrosol) of essential oils usually obtained by steam distillation from aromatic plants. These herbal distillates have uses as flavorings, medicine and in skin care. Herbal distillates go by many other names including floral water, hydrosol, hydrolate, herbal water and essential water. Herbal distillates are produced in the same manner as essential oils."@en ;
	skos:exactMatch dbpedia:Herbal_distillate ;
	skos:narrower <http://vocabulary.semantic-web.at/cocktails/47c10a33-a7b2-44f5-9614-2bca65cff2fd> ;
	skos:prefLabel "Herbal distillate"@en .

<http://vocabulary.semantic-web.at/cocktails/204cd4e7-58d7-4417-837a-7f9cc41663c8> dcterms:contributor <http://localhost/user/blumauera> ;
	dcterms:created "2015-05-01T07:40:52Z"^^xsd:dateTime ;
	dcterms:creator <http://localhost/user/blumauera> ;
	dcterms:modified "2015-05-06T12:51:15Z"^^xsd:dateTime ;
	<http://schema.semantic-web.at/ppt/inScheme> <http://vocabulary.semantic-web.at/cocktails/8d052dfc-44bf-4985-8ce3-4564570a161b> ;
	a <http://vocabulary.semantic-web.at/cocktail-ontology/Cocktail> , skos:Concept ;
	skos:altLabel "Cocktails with wine"@en , "List of wine cocktails"@en ;
	skos:definition "A wine cocktail is a mixed drink, similar to a true cocktail. It is made predominantly with wine, into which distilled alcohol or other drink mixer is combined. The distinction between a wine cocktail and a cocktail with wine is the relative amounts of the various alcohols. In a wine cocktail, the wine product is the primary alcohol by volume compared to the distilled alcohol or mixer. <div id=\"list\"/>"@en ;
	skos:exactMatch dbpedia:Wine_cocktail ;
	skos:narrower <http://vocabulary.semantic-web.at/cocktails/2c682ed8-e2ba-473e-8cb7-979598080e18> , <http://vocabulary.semantic-web.at/cocktails/4d15a643-f7c7-4ee5-8f56-4ebd2bcf74b5> , <http://vocabulary.semantic-web.at/cocktails/61a18ebf-fd92-4ef1-8ab1-bfd3c26867b9> , <http://vocabulary.semantic-web.at/cocktails/698723d7-e8b8-410e-91a8-9bdc867b3f8a> , <http://vocabulary.semantic-web.at/cocktails/a73d88e9-0c50-45d2-b364-9dec5abe206d> , <http://vocabulary.semantic-web.at/cocktails/b8075344-1e6d-4348-bdee-83948203a974> , <http://vocabulary.semantic-web.at/cocktails/c2249dc0-0529-4a11-ad82-5d710b5e9c31> , <http://vocabulary.semantic-web.at/cocktails/ea946e07-e812-4492-a0ed-124d73bfbba7> ;
	skos:prefLabel "Wine cocktail"@en ;
	skos:topConceptOf <http://vocabulary.semantic-web.at/cocktails/8d052dfc-44bf-4985-8ce3-4564570a161b> .

<http://vocabulary.semantic-web.at/cocktails/20d288cb-4e38-46f9-9bec-1c79d8397215> dcterms:contributor <http://localhost/user/blumauera> ;
	dcterms:created "2015-05-02T18:37:55Z"^^xsd:dateTime ;
	dcterms:creator <http://localhost/user/blumauera> ;
	dcterms:modified "2015-05-07T07:23:42Z"^^xsd:dateTime ;
	<http://schema.semantic-web.at/ppt/inScheme> <http://vocabulary.semantic-web.at/cocktails/f09732a9-a0e6-494a-8ce9-299ef036aaaf> ;
	<http://vocabulary.semantic-web.at/cocktail-ontology/image_2> <http://upload.wikimedia.org/wikipedia/commons/thumb/e/e4/Collins_glass_silhouette.svg/22px-Collins_glass_silhouette.svg.png> ;
	<http://vocabulary.semantic-web.at/cocktail-ontology/is-used-by> <http://vocabulary.semantic-web.at/cocktails/55c40695-8b41-41ed-8c6a-70fe6930067e> , <http://vocabulary.semantic-web.at/cocktails/bee1e709-b317-4f46-b06f-a22367baefdf> , <http://vocabulary.semantic-web.at/cocktails/c151ee28-45d2-4128-8587-1f1b69060d9d> ;
	a <http://vocabulary.semantic-web.at/cocktail-ontology/Drinkware> , skos:Concept ;
	skos:broader <http://vocabulary.semantic-web.at/cocktails/2e839563-8037-4e59-8dbf-27736605d687> ;
	skos:definition "A collins glass is a glass tumbler which typically will contain 10 to 14 fluid ounces (300 to 410 ml). It is used to serve mixed drinks, especially Tom Collins cocktails. It is cylindrical in shape and narrower than a highball glass."@en ;
	skos:exactMatch dbpedia:Collins_glass ;
	skos:prefLabel "Collins glass"@en .

<http://vocabulary.semantic-web.at/cocktails/21b94d69-280e-4546-be1a-fdd1d9aa5d32> dcterms:contributor <http://localhost/user/blumauera> ;
	dcterms:created "2015-05-01T08:23:57Z"^^xsd:dateTime ;
	dcterms:creator <http://localhost/user/blumauera> ;
	dcterms:modified "2015-05-03T10:08:04Z"^^xsd:dateTime ;
	<http://schema.semantic-web.at/ppt/inScheme> <http://vocabulary.semantic-web.at/cocktails/8d052dfc-44bf-4985-8ce3-4564570a161b> ;
	<http://vocabulary.semantic-web.at/cocktail-ontology/consists-of> <http://vocabulary.semantic-web.at/cocktails/8352ad8c-0355-4ca4-9ff7-c3dff28931c5> , <http://vocabulary.semantic-web.at/cocktails/fd76c5ab-be62-4c4b-a2c6-7fa9bc359f47> ;
	<http://vocabulary.semantic-web.at/cocktail-ontology/iba> <http://www.iba-world.com/index.php?option=com_content&id=89> ;
	<http://vocabulary.semantic-web.at/cocktail-ontology/image> <http://upload.wikimedia.org/wikipedia/commons/a/ac/Gin_Alexander_%284371721753%29.jpg> ;
	<http://vocabulary.semantic-web.at/cocktail-ontology/preparation> "Shake all ingredients with ice and strain contents into a cocktail glass. Sprinkle nutmeg on top and serve"@en ;
	<http://vocabulary.semantic-web.at/cocktail-ontology/served> "Straight up; without ice"@en ;
	<http://vocabulary.semantic-web.at/cocktail-ontology/uses> <http://vocabulary.semantic-web.at/cocktails/19dee0d8-fd30-469f-9ecd-91c902ff717c> ;
	<http://vocabulary.semantic-web.at/cocktail-ontology/uses_2> <http://vocabulary.semantic-web.at/cocktails/cb1bb8c3-5013-4c5f-80e3-5267367fe2fb> ;
	a <http://vocabulary.semantic-web.at/cocktail-ontology/Cocktail> , skos:Concept ;
	skos:broader <http://vocabulary.semantic-web.at/cocktails/caae2ea0-7e60-400b-a2bb-14ef79720668> ;
	skos:definition "The Alexander is a gin cocktail consisting of gin, Chocolate Liqueur, and Cream."@en ;
	skos:exactMatch <http://dbpedia.org/resource/Alexander_(cocktail)> ;
	skos:prefLabel "Alexander"@en .

<http://vocabulary.semantic-web.at/cocktails/224b4628-2f46-44a1-9d2f-8b5ef0b31e79> dcterms:contributor <http://localhost/user/blumauera> ;
	dcterms:created "2015-05-01T08:46:15Z"^^xsd:dateTime ;
	dcterms:creator <http://localhost/user/blumauera> ;
	dcterms:modified "2015-05-07T06:37:03Z"^^xsd:dateTime ;
	<http://schema.semantic-web.at/ppt/inScheme> <http://vocabulary.semantic-web.at/cocktails/591cf89a-57af-49b8-9042-3fc77408c93e> ;
	<http://schema.semantic-web.at/ppt/inSubtree> <http://vocabulary.semantic-web.at/cocktails/403d1249-f37f-4f43-bebf-8dde9677d886> ;
	<http://vocabulary.semantic-web.at/cocktail-ontology/is-part-of> <http://vocabulary.semantic-web.at/cocktails/0bbdca98-077b-48d1-99d6-47eca59c442c> , <http://vocabulary.semantic-web.at/cocktails/1d5b39cc-fcab-48b2-bb24-9840b7e34d64> , <http://vocabulary.semantic-web.at/cocktails/44cc99c1-28ac-4c50-a55d-7244b2c5c07b> , <http://vocabulary.semantic-web.at/cocktails/785b30fd-1eb4-445b-8247-7e1e57b35b0f> , <http://vocabulary.semantic-web.at/cocktails/926b14fe-1b83-4f46-bbf9-f946be1889aa> ;
	a <http://vocabulary.semantic-web.at/cocktail-ontology/Alcoholic-Beverages> , <http://vocabulary.semantic-web.at/cocktail-ontology/Beverages> , <http://vocabulary.semantic-web.at/cocktail-ontology/Ingredients> , skos:Concept ;
	skos:altLabel "Maraschino Liqueur"@en ;
	skos:broader <http://vocabulary.semantic-web.at/cocktails/1be6ee21-daf9-4b15-847d-6acdb88f9104> ;
	skos:definition "Maraschino is a bittersweet, clear liqueur flavored with Marasca cherries, which were originally from Dalmatia but are grown today mostly around the city of Zadar and in Torreglia. The liqueur's distinctive flavor comes from the Marasca cherries and crushed cherry pits, which lend an almond-like flavor. Honey is also part of the ancient recipe. The distillate matures for at least two years in ashwood vats, since this wood does not lend its colour to the liqueur, and is then diluted and sugared."@en ;
	skos:exactMatch dbpedia:Maraschino ;
	skos:prefLabel "Maraschino"@en .

<http://vocabulary.semantic-web.at/cocktails/22c81328-d483-4c62-8338-cb732ee39734> dcterms:contributor <http://localhost/user/huberf> ;
	dcterms:created "2015-05-02T18:46:11Z"^^xsd:dateTime ;
	dcterms:creator <http://localhost/user/blumauera> ;
	dcterms:modified "2016-10-05T09:33:54Z"^^xsd:dateTime ;
	<http://schema.semantic-web.at/ppt/inScheme> <http://vocabulary.semantic-web.at/cocktails/f09732a9-a0e6-494a-8ce9-299ef036aaaf> ;
	<http://vocabulary.semantic-web.at/cocktail-ontology/image_2> <http://upload.wikimedia.org/wikipedia/commons/thumb/3/35/Hurricane_Glass_Silhouette.svg/22px-Hurricane_Glass_Silhouette.svg.png> ;
	<http://vocabulary.semantic-web.at/cocktail-ontology/is-used-by> <http://vocabulary.semantic-web.at/cocktails/4792b0b8-0046-47ca-8c2a-f3ad58922182> ;
	a <http://vocabulary.semantic-web.at/cocktail-ontology/Drinkware> , skos:Concept ;
	skos:broader <http://vocabulary.semantic-web.at/cocktails/2ea18d11-7415-4282-9608-7a3f497a0928> ;
	skos:definition "A Hurricane glass is a glass tumbler which typically will contain 20 fluid ounces (600 ml). It is used to serve mixed drinks, particularly the Hurricane from which it is named originating at Pat O'Brien's Bar in New Orleans. Other drinks served in this glass include June bug, Piña colada and Blue Hawaii. It is shaped similarly to a vase or a hurricane lamp and is typically taller and wider than a highball glass."@en ;
	skos:exactMatch dbpedia:Hurricane_glass ;
	skos:prefLabel "Hurricane glass"@en .

<http://vocabulary.semantic-web.at/cocktails/22df810d-e509-4da8-979c-0758e94de3e6> dcterms:contributor <http://localhost/user/blumauera> ;
	dcterms:created "2015-05-01T07:51:18Z"^^xsd:dateTime ;
	dcterms:creator <http://localhost/user/blumauera> ;
	dcterms:modified "2015-08-07T15:06:52Z"^^xsd:dateTime ;
	<http://schema.semantic-web.at/ppt/inScheme> <http://vocabulary.semantic-web.at/cocktails/591cf89a-57af-49b8-9042-3fc77408c93e> ;
	<http://schema.semantic-web.at/ppt/inSubtree> <http://vocabulary.semantic-web.at/cocktails/403d1249-f37f-4f43-bebf-8dde9677d886> ;
	<http://vocabulary.semantic-web.at/cocktail-ontology/image_3> <http://preview.poolparty.biz/sparqlingCocktails/resources/images/vodka.png> ;
	<http://vocabulary.semantic-web.at/cocktail-ontology/is-part-of> <http://vocabulary.semantic-web.at/cocktails/0f8cc862-9056-49be-b636-cd22f8d7282d> , <http://vocabulary.semantic-web.at/cocktails/12f4790a-560f-4e1c-b57a-53b8171ae39a> , <http://vocabulary.semantic-web.at/cocktails/268fb62f-8ef1-45cd-844f-8c7da85a6a0b> , <http://vocabulary.semantic-web.at/cocktails/2c032fe6-a518-44be-851a-dbf1c253be63> , <http://vocabulary.semantic-web.at/cocktails/33d9a47f-0622-4b0f-ad1b-62eb96fc6799> , <http://vocabulary.semantic-web.at/cocktails/680c7429-30a7-4044-b32f-e28c99dcb9f4> , <http://vocabulary.semantic-web.at/cocktails/72a77af2-bbee-4b75-871f-a96dcd3a452b> , <http://vocabulary.semantic-web.at/cocktails/79d4686d-4f5b-4067-a2ef-99beccc51242> , <http://vocabulary.semantic-web.at/cocktails/7e5afb63-30ec-42b4-a9f5-f61fc456107d> , <http://vocabulary.semantic-web.at/cocktails/a47e8f08-057a-45f2-8398-9be51ed351fc> , <http://vocabulary.semantic-web.at/cocktails/b00a123f-a2b5-49d2-8325-a81d1d26ddc6> , <http://vocabulary.semantic-web.at/cocktails/c8f4f6bd-4ac1-456a-a3aa-595e4b93d979> , <http://vocabulary.semantic-web.at/cocktails/ce8f4591-ccd4-4d90-a761-244115d64061> , <http://vocabulary.semantic-web.at/cocktails/dff0a7f4-ded0-48d5-bd31-881b70fbe36a> ;
	a <http://vocabulary.semantic-web.at/cocktail-ontology/Alcoholic-Beverages> , <http://vocabulary.semantic-web.at/cocktail-ontology/Beverages> , <http://vocabulary.semantic-web.at/cocktail-ontology/Ingredients> , skos:Concept ;
	skos:altLabel "Balkan 176deg"@en , "Balkan 176°"@en , "Blackcurrant vodka"@en , "Filtering vodka"@en , "Russian vodka"@en , "Vodak"@en , "Vodka and Coke"@en , "Vokda"@en , "Wodka"@en , "Водка"@en ;
	skos:broader <http://vocabulary.semantic-web.at/cocktails/403d1249-f37f-4f43-bebf-8dde9677d886> , <http://vocabulary.semantic-web.at/cocktails/f3000285-36b0-4ffe-af90-740c2dd8fff5> ;
	skos:definition "Vodka is a distilled beverage composed primarily of water and ethanol, sometimes with traces of impurities and flavorings. Vodka is made by the distillation of fermented substances such as grains, potatoes, or sometimes fruits or sugar. Vodka is a spirit that was virtually unknown in the United States prior to the 1940s. Traditionally prepared vodkas had an alcoholic content of 40% by volume."@en ;
	skos:exactMatch dbpedia:Vodka ;
	skos:narrower <http://vocabulary.semantic-web.at/cocktails/b6725284-f65d-4802-b79d-029c539a1580> ;
	skos:prefLabel "Vodka"@en .

<http://vocabulary.semantic-web.at/cocktails/22f838ea-3c2b-4b63-99d1-fdb6280b5705> dcterms:contributor <http://localhost/user/blumauera> ;
	dcterms:created "2015-05-01T14:15:13Z"^^xsd:dateTime ;
	dcterms:creator <http://localhost/user/blumauera> ;
	dcterms:modified "2015-05-03T10:36:13Z"^^xsd:dateTime ;
	<http://schema.semantic-web.at/ppt/inScheme> <http://vocabulary.semantic-web.at/cocktails/8d052dfc-44bf-4985-8ce3-4564570a161b> ;
	<http://vocabulary.semantic-web.at/cocktail-ontology/consists-of> <http://vocabulary.semantic-web.at/cocktails/9c2ce399-c6ae-4f4d-bf37-7fd8ffe2a19d> , <http://vocabulary.semantic-web.at/cocktails/d530df52-cc54-4be3-8409-85734e5ec67f> , <http://vocabulary.semantic-web.at/cocktails/f5cd2a2b-2153-4b7e-ae79-678b939765ca> , <http://vocabulary.semantic-web.at/cocktails/fd76c5ab-be62-4c4b-a2c6-7fa9bc359f47> ;
	<http://vocabulary.semantic-web.at/cocktail-ontology/iba> <http://www.iba-world.com/index.php?option=com_content&id=190&Itemid=532> ;
	<http://vocabulary.semantic-web.at/cocktail-ontology/image> <http://www.iba-world.com/images/cocktail_drinks/between_sheets.jpg> ;
	<http://vocabulary.semantic-web.at/cocktail-ontology/preparation> "Pour all ingredients into shaker with ice cubes, shake, strain into chilled cocktail glass."@en ;
	<http://vocabulary.semantic-web.at/cocktail-ontology/served> "Straight up; without ice"@en ;
	<http://vocabulary.semantic-web.at/cocktail-ontology/uses> <http://vocabulary.semantic-web.at/cocktails/19dee0d8-fd30-469f-9ecd-91c902ff717c> ;
	a <http://vocabulary.semantic-web.at/cocktail-ontology/Cocktail> , skos:Concept ;
	skos:altLabel "Maiden's Prayer"@en ;
	skos:broader <http://vocabulary.semantic-web.at/cocktails/caae2ea0-7e60-400b-a2bb-14ef79720668> ;
	skos:definition "The Between the Sheets (also known as the Maiden's Prayer) is a cocktail consisting of white rum, cognac, triple sec, and lemon juice."@en ;
	skos:prefLabel "Between the Sheets"@en ;
	skos:related <http://vocabulary.semantic-web.at/cocktails/e039633b-03c1-47bd-a705-a104a4323e45> .

<http://vocabulary.semantic-web.at/cocktails/236b36df-93ca-4408-836c-133ace53798a> dcterms:contributor <http://localhost/user/blumauera> ;
	dcterms:created "2015-05-02T19:27:58Z"^^xsd:dateTime ;
	dcterms:creator <http://localhost/user/blumauera> ;
	dcterms:modified "2015-05-05T07:48:06Z"^^xsd:dateTime ;
	<http://schema.semantic-web.at/ppt/inScheme> <http://vocabulary.semantic-web.at/cocktails/8d052dfc-44bf-4985-8ce3-4564570a161b> ;
	<http://vocabulary.semantic-web.at/cocktail-ontology/consists-of> <http://vocabulary.semantic-web.at/cocktails/9c2ce399-c6ae-4f4d-bf37-7fd8ffe2a19d> , <http://vocabulary.semantic-web.at/cocktails/b6725284-f65d-4802-b79d-029c539a1580> , <http://vocabulary.semantic-web.at/cocktails/d530df52-cc54-4be3-8409-85734e5ec67f> ;
	<http://vocabulary.semantic-web.at/cocktail-ontology/iba> <http://www.iba-world.com/index.php?option=com_content&id=245&Itemid=532> ;
	<http://vocabulary.semantic-web.at/cocktail-ontology/image> <http://www.iba-world.com/images/cocktail_drinks/lemon_drop.jpg> ;
	<http://vocabulary.semantic-web.at/cocktail-ontology/preparation> "Shake and strain into a chilled cocktail glass rimmed with sugar, garnish with a slice of lemon."@en ;
	<http://vocabulary.semantic-web.at/cocktail-ontology/uses> <http://vocabulary.semantic-web.at/cocktails/19dee0d8-fd30-469f-9ecd-91c902ff717c> ;
	<http://vocabulary.semantic-web.at/cocktail-ontology/uses_2> <http://vocabulary.semantic-web.at/cocktails/33df103a-03ac-4177-b620-7953fe094236> , <http://vocabulary.semantic-web.at/cocktails/3c94f5fc-4664-4177-a880-88643c0be9c1> ;
	a <http://vocabulary.semantic-web.at/cocktail-ontology/Cocktail> , skos:Concept ;
	skos:broader <http://vocabulary.semantic-web.at/cocktails/ccee1079-43df-4ff1-bef0-d15d3dc8fa6f> ;
	skos:prefLabel "Lemon Drop Martini"@en .

<http://vocabulary.semantic-web.at/cocktails/268fb62f-8ef1-45cd-844f-8c7da85a6a0b> dcterms:contributor <http://localhost/user/blumauera> ;
	dcterms:created "2015-05-02T07:30:21Z"^^xsd:dateTime ;
	dcterms:creator <http://localhost/user/blumauera> ;
	dcterms:modified "2015-08-11T08:56:20Z"^^xsd:dateTime ;
	<http://schema.semantic-web.at/ppt/inScheme> <http://vocabulary.semantic-web.at/cocktails/8d052dfc-44bf-4985-8ce3-4564570a161b> ;
	<http://vocabulary.semantic-web.at/cocktail-ontology/consists-of> <http://vocabulary.semantic-web.at/cocktails/22df810d-e509-4da8-979c-0758e94de3e6> , <http://vocabulary.semantic-web.at/cocktails/48499a53-a687-4156-b966-1e16e3e967bd> , <http://vocabulary.semantic-web.at/cocktails/6f6c504d-2272-4561-b46b-35bbccad8355> , <http://vocabulary.semantic-web.at/cocktails/790d1a2d-d20b-4ecd-a3d0-f9a931156e14> , <http://vocabulary.semantic-web.at/cocktails/94cca1b4-3603-472b-9c78-6d6a43b6b4ca> , <http://vocabulary.semantic-web.at/cocktails/9c2ce399-c6ae-4f4d-bf37-7fd8ffe2a19d> ;
	<http://vocabulary.semantic-web.at/cocktail-ontology/iba> <http://www.iba-world.com/index.php?option=com_content&id=216&Itemid=532> ;
	<http://vocabulary.semantic-web.at/cocktail-ontology/image> <http://upload.wikimedia.org/wikipedia/commons/thumb/1/12/Bloody_Mary.jpg/440px-Bloody_Mary.jpg> ;
	<http://vocabulary.semantic-web.at/cocktail-ontology/preparation> "Add dashes of Worcestershire Sauce, Tabasco, salt and pepper into highball glass, then pour all ingredients into highball with ice cubes. Stir gently. Garnish with celery stalk and lemon wedge "@en ;
	<http://vocabulary.semantic-web.at/cocktail-ontology/served> "On the rocks; poured over ice"@en ;
	<http://vocabulary.semantic-web.at/cocktail-ontology/uses> <http://vocabulary.semantic-web.at/cocktails/a54d2096-6214-4006-beaf-afcc77824710> ;
	<http://vocabulary.semantic-web.at/cocktail-ontology/uses_2> <http://vocabulary.semantic-web.at/cocktails/1ca477d1-98d5-4a16-82e2-a4b07c34fdbe> , <http://vocabulary.semantic-web.at/cocktails/33df103a-03ac-4177-b620-7953fe094236> ;
	a <http://vocabulary.semantic-web.at/cocktail-ontology/Cocktail> , skos:Concept ;
	skos:altLabel "Bloody Maria"@en , "Bloody mary mix"@en , "Bloody shame"@en , "Bull Shot"@en , "Queen of drinks"@en , "The queen of drinks"@en , "Virgin Mary"@en ;
	skos:broader <http://vocabulary.semantic-web.at/cocktails/b9bf3799-a4e4-47f7-9aea-7697cc998a34> ;
	skos:definition "A Bloody Mary is a popular cocktail containing vodka, tomato juice, and usually other spices or flavorings such as Worcestershire sauce, Tabasco sauce, piri piri sauce, beef consommé or bouillon, horseradish, celery, olive, salt, black pepper, cayenne pepper, lemon juice, and celery salt. It has been called \"the world's most complex cocktail.\""@en ;
	skos:exactMatch <http://dbpedia.org/resource/Bloody_Mary_(cocktail)> ;
	skos:prefLabel "Bloody Mary"@en .

<http://vocabulary.semantic-web.at/cocktails/26ca4892-5265-4ce6-875c-ef92348ff7a4> dcterms:contributor <http://localhost/user/blumauera> ;
	dcterms:created "2015-05-02T18:50:49Z"^^xsd:dateTime ;
	dcterms:creator <http://localhost/user/blumauera> ;
	dcterms:modified "2015-05-07T07:04:01Z"^^xsd:dateTime ;
	<http://schema.semantic-web.at/ppt/inScheme> <http://vocabulary.semantic-web.at/cocktails/591cf89a-57af-49b8-9042-3fc77408c93e> ;
	<http://schema.semantic-web.at/ppt/inSubtree> <http://vocabulary.semantic-web.at/cocktails/e86c1671-4a67-494b-ae5d-bcb750865acc> ;
	<http://vocabulary.semantic-web.at/cocktail-ontology/is-part-of> <http://vocabulary.semantic-web.at/cocktails/4792b0b8-0046-47ca-8c2a-f3ad58922182> ;
	a <http://vocabulary.semantic-web.at/cocktail-ontology/Beverages> , <http://vocabulary.semantic-web.at/cocktail-ontology/Ingredients> , <http://vocabulary.semantic-web.at/cocktail-ontology/Non-alcoholic-Beverages> , skos:Concept ;
	skos:broader <http://vocabulary.semantic-web.at/cocktails/e86c1671-4a67-494b-ae5d-bcb750865acc> ;
	skos:definition "Coconut milk is the liquid that comes from the grated meat of a coconut. The color and rich taste of the milk can be attributed to the high oil content. Most of the fat is saturated fat. Coconut milk is a very popular food ingredient used in Southeast Asia, especially in Thailand, Malaysia, Indonesia, Singapore, and the Philippines."@en ;
	skos:exactMatch dbpedia:Coconut_milk ;
	skos:prefLabel "Coconut milk"@en .

<http://vocabulary.semantic-web.at/cocktails/27c48d24-bb0b-46a3-9b0c-4b09e38a4b07> dcterms:contributor <http://localhost/user/blumauera> ;
	dcterms:created "2015-05-02T18:58:28Z"^^xsd:dateTime ;
	dcterms:creator <http://localhost/user/blumauera> ;
	dcterms:modified "2015-11-20T19:25:55Z"^^xsd:dateTime ;
	<http://schema.semantic-web.at/ppt/inScheme> <http://vocabulary.semantic-web.at/cocktails/591cf89a-57af-49b8-9042-3fc77408c93e> ;
	<http://schema.semantic-web.at/ppt/inSubtree> <http://vocabulary.semantic-web.at/cocktails/403d1249-f37f-4f43-bebf-8dde9677d886> ;
	<http://vocabulary.semantic-web.at/cocktail-ontology/image_3> <http://preview.poolparty.biz/sparqlingCocktails/resources/images/schnaps.png> ;
	a <http://vocabulary.semantic-web.at/cocktail-ontology/Alcoholic-Beverages> , <http://vocabulary.semantic-web.at/cocktail-ontology/Beverages> , <http://vocabulary.semantic-web.at/cocktail-ontology/Ingredients> , skos:Concept ;
	skos:altLabel "Butterscotch Schnapps"@en , "Butterscotch schnapps"@en , "Obstler"@en , "Schnaps"@en , "Scnapps"@en ;
	skos:broader <http://vocabulary.semantic-web.at/cocktails/403d1249-f37f-4f43-bebf-8dde9677d886> , <http://vocabulary.semantic-web.at/cocktails/f3000285-36b0-4ffe-af90-740c2dd8fff5> ;
	skos:definition "Schnapps is a term that refers to any kind of strong alcoholic beverage. The English word \"schnapps\" is derived from the German Schnaps (plural, Schnäpse). Schnaps is a Low German noun that means \"swallow\"; it has been documented in its High German meaning since before the 18th century."@en ;
	skos:exactMatch dbpedia:Schnapps ;
	skos:narrower <http://vocabulary.semantic-web.at/cocktails/7738a6e2-84c2-4ae3-b605-8bb6420e6e28> , <http://vocabulary.semantic-web.at/cocktails/9cbe0ac7-b97d-431c-8ea6-a1d7ccc44d4f> ;
	skos:prefLabel "Schnapps"@en .

<http://vocabulary.semantic-web.at/cocktails/2944baef-5338-421b-a5f5-0e51f75244c2> dcterms:contributor <http://localhost/user/blumauera> ;
	dcterms:created "2015-05-01T08:26:29Z"^^xsd:dateTime ;
	dcterms:creator <http://localhost/user/blumauera> ;
	dcterms:modified "2015-11-13T14:27:46Z"^^xsd:dateTime ;
	<http://schema.semantic-web.at/ppt/inScheme> <http://vocabulary.semantic-web.at/cocktails/591cf89a-57af-49b8-9042-3fc77408c93e> ;
	<http://schema.semantic-web.at/ppt/inSubtree> <http://vocabulary.semantic-web.at/cocktails/403d1249-f37f-4f43-bebf-8dde9677d886> ;
	<http://vocabulary.semantic-web.at/cocktail-ontology/image_3> <http://preview.poolparty.biz/sparqlingCocktails/resources/images/liqeur.png> ;
	a <http://vocabulary.semantic-web.at/cocktail-ontology/Alcoholic-Beverages> , <http://vocabulary.semantic-web.at/cocktail-ontology/Beverages> , <http://vocabulary.semantic-web.at/cocktail-ontology/Ingredients> , skos:Concept ;
	skos:altLabel "Alcoholic cordial"@en , "Liquer"@en , "Liquour"@en ;
	skos:broader <http://vocabulary.semantic-web.at/cocktails/403d1249-f37f-4f43-bebf-8dde9677d886> , <http://vocabulary.semantic-web.at/cocktails/f3000285-36b0-4ffe-af90-740c2dd8fff5> ;
	skos:definition "A liqueur is an alcoholic beverage made from a distilled spirit that has been flavored with fruit, cream, herbs, spices, flowers or nuts and bottled with added sugar or other sweetener. Liqueurs are typically quite sweet; they are usually not aged for long after the ingredients are mixed, but may have resting periods during their production to allow flavors to marry."@en ;
	skos:exactMatch dbpedia:Liqueur ;
	skos:narrower <http://vocabulary.semantic-web.at/cocktails/05206233-09be-41ac-9f2e-91263873a20e> , <http://vocabulary.semantic-web.at/cocktails/0f6d360f-af24-4d66-8f70-760c927ed0a7> , <http://vocabulary.semantic-web.at/cocktails/19316511-1d42-4516-9504-873c3fd8fb85> , <http://vocabulary.semantic-web.at/cocktails/1be6ee21-daf9-4b15-847d-6acdb88f9104> , <http://vocabulary.semantic-web.at/cocktails/397d0ec3-98e2-47d9-a8c2-eca9702ff94d> , <http://vocabulary.semantic-web.at/cocktails/47635419-edef-4b78-8da1-e58a96d96f61> , <http://vocabulary.semantic-web.at/cocktails/4c6a85a7-de2a-42a9-9664-3279e53bac48> , <http://vocabulary.semantic-web.at/cocktails/917d78d0-0938-4fe0-80c4-cfd2eb16e6a4> , <http://vocabulary.semantic-web.at/cocktails/a12b3836-dba0-49e9-92c6-7725ccf35944> , <http://vocabulary.semantic-web.at/cocktails/a1c1e015-91fd-4f6e-b2a8-5edae9aa0b9d> , <http://vocabulary.semantic-web.at/cocktails/a62bc4d7-b07a-4e32-9254-9facbeb8831d> , <http://vocabulary.semantic-web.at/cocktails/af5df232-948a-4dc9-8dd1-1d7bfbf523f1> , <http://vocabulary.semantic-web.at/cocktails/d40e2215-bc1b-4bae-8cf8-d10b1ad36d44> , <http://vocabulary.semantic-web.at/cocktails/ec2452b9-849d-4750-8190-bc696f2271fa> ;
	skos:prefLabel "Liqueur"@en .

<http://vocabulary.semantic-web.at/cocktails/2c032fe6-a518-44be-851a-dbf1c253be63> dcterms:contributor <http://localhost/user/blumauera> ;
	dcterms:created "2015-05-02T18:39:58Z"^^xsd:dateTime ;
	dcterms:creator <http://localhost/user/blumauera> ;
	dcterms:modified "2015-05-07T07:03:16Z"^^xsd:dateTime ;
	<http://schema.semantic-web.at/ppt/inScheme> <http://vocabulary.semantic-web.at/cocktails/8d052dfc-44bf-4985-8ce3-4564570a161b> ;
	<http://vocabulary.semantic-web.at/cocktail-ontology/consists-of> <http://vocabulary.semantic-web.at/cocktails/22df810d-e509-4da8-979c-0758e94de3e6> , <http://vocabulary.semantic-web.at/cocktails/5b4cd5f6-19e8-4854-8c5e-0b6d58cbb702> , <http://vocabulary.semantic-web.at/cocktails/88f5de3d-3de4-4a2f-9523-50bc7bb06600> ;
	<http://vocabulary.semantic-web.at/cocktail-ontology/iba> <http://www.iba-world.com/index.php?option=com_content&id=230&Itemid=532> ;
	<http://vocabulary.semantic-web.at/cocktail-ontology/image> <http://upload.wikimedia.org/wikipedia/commons/thumb/a/a7/Moscow_Mule.jpg/440px-Moscow_Mule.jpg> ;
	<http://vocabulary.semantic-web.at/cocktail-ontology/preparation> "Combine the vodka and ginger beer. Add lime juice.  Garnish with a lime slice."@en ;
	<http://vocabulary.semantic-web.at/cocktail-ontology/served> "On the rocks; poured over ice"@en ;
	<http://vocabulary.semantic-web.at/cocktail-ontology/uses> <http://vocabulary.semantic-web.at/cocktails/0381bd47-ad07-428a-b5c4-ee2608f2ebd3> , <http://vocabulary.semantic-web.at/cocktails/a54d2096-6214-4006-beaf-afcc77824710> ;
	<http://vocabulary.semantic-web.at/cocktail-ontology/uses_2> <http://vocabulary.semantic-web.at/cocktails/021c85c0-a60a-4414-8fd8-bd3383b794f1> ;
	a <http://vocabulary.semantic-web.at/cocktail-ontology/Cocktail> , skos:Concept ;
	skos:altLabel "Moose can"@en ;
	skos:broader <http://vocabulary.semantic-web.at/cocktails/54702498-ad42-4af6-b28a-2276215450da> , <http://vocabulary.semantic-web.at/cocktails/b9bf3799-a4e4-47f7-9aea-7697cc998a34> ;
	skos:definition "A Moscow Mule is a buck or mule cocktail made with vodka, ginger beer and lime which was popular during the vodka craze in the United States during the 1950s. The name refers to the popular perception of vodka as a Russian product."@en ;
	skos:exactMatch dbpedia:Moscow_mule ;
	skos:prefLabel "Moscow mule"@en .

<http://vocabulary.semantic-web.at/cocktails/2c3083d2-8650-4460-b019-cae7aea38f14> dcterms:contributor <http://localhost/user/blumauera> ;
	dcterms:created "2015-05-01T14:52:57Z"^^xsd:dateTime ;
	dcterms:creator <http://localhost/user/blumauera> ;
	dcterms:modified "2015-05-27T12:47:19Z"^^xsd:dateTime ;
	<http://schema.semantic-web.at/ppt/inScheme> <http://vocabulary.semantic-web.at/cocktails/8d052dfc-44bf-4985-8ce3-4564570a161b> ;
	<http://vocabulary.semantic-web.at/cocktail-ontology/consists-of> <http://vocabulary.semantic-web.at/cocktails/2ce50273-13b2-4ba1-9ff2-8cfbd835c1f2> , <http://vocabulary.semantic-web.at/cocktails/5caedba2-9aef-4fab-b26b-6e20cf014419> , <http://vocabulary.semantic-web.at/cocktails/5d96c50c-ee48-4c40-bb4c-4b9a42d11de6> ;
	<http://vocabulary.semantic-web.at/cocktail-ontology/iba> <http://www.iba-world.com/index.php?option=com_content&id=203&Itemid=532> ;
	<http://vocabulary.semantic-web.at/cocktail-ontology/image> <http://upload.wikimedia.org/wikipedia/commons/thumb/b/b3/Paradise_cocktail.jpg/440px-Paradise_cocktail.jpg> ;
	<http://vocabulary.semantic-web.at/cocktail-ontology/preparation> "Pour all ingredients into cocktail shaker filled with ice. Shake and strain into chilled cocktail glass."@en ;
	<http://vocabulary.semantic-web.at/cocktail-ontology/served> "Straight up; without ice"@en ;
	<http://vocabulary.semantic-web.at/cocktail-ontology/uses> <http://vocabulary.semantic-web.at/cocktails/19dee0d8-fd30-469f-9ecd-91c902ff717c> ;
	a <http://vocabulary.semantic-web.at/cocktail-ontology/Cocktail> , skos:Concept ;
	skos:broader <http://vocabulary.semantic-web.at/cocktails/b523727e-7f49-4e1b-9c09-55002ee3a81e> , <http://vocabulary.semantic-web.at/cocktails/caae2ea0-7e60-400b-a2bb-14ef79720668> ;
	skos:definition "The Paradise is an IBA official cocktail, and is classified as a \"pre-dinner\" drink, an apéritif. The earliest known in-print recipe for the Paradise Cocktail was written by Harry Craddock. This cocktail is prepared using gin, apricot brandy (apricot liqueur), and orange juice in a 2:1:1 ratio, with a splash of lemon juice."@en ;
	skos:exactMatch <http://dbpedia.org/resource/Paradise_(cocktail)> ;
	skos:prefLabel "Paradise"@en .

<http://vocabulary.semantic-web.at/cocktails/2c682ed8-e2ba-473e-8cb7-979598080e18> dcterms:contributor <http://localhost/user/blumauera> ;
	dcterms:created "2015-05-02T19:32:22Z"^^xsd:dateTime ;
	dcterms:creator <http://localhost/user/blumauera> ;
	dcterms:modified "2015-05-05T07:58:39Z"^^xsd:dateTime ;
	<http://schema.semantic-web.at/ppt/inScheme> <http://vocabulary.semantic-web.at/cocktails/8d052dfc-44bf-4985-8ce3-4564570a161b> ;
	<http://vocabulary.semantic-web.at/cocktail-ontology/consists-of> <http://vocabulary.semantic-web.at/cocktails/05a0d86b-79fc-4d75-91e4-dc77e8167db9> , <http://vocabulary.semantic-web.at/cocktails/7448dbed-7603-41f7-a316-99f754c9ae45> , <http://vocabulary.semantic-web.at/cocktails/a293047d-788b-4e8c-96bc-65e62fec4b0b> ;
	<http://vocabulary.semantic-web.at/cocktail-ontology/iba> <http://www.iba-world.com/index.php?option=com_content&id=248&Itemid=532> ;
	<http://vocabulary.semantic-web.at/cocktail-ontology/image> <http://www.iba-world.com/images/cocktail_drinks/spritz_veneziano.jpg> ;
	<http://vocabulary.semantic-web.at/cocktail-ontology/preparation> "Build into an old-fashioned glass filled with ice. Top with a splash of soda water. Garnish with half orange slice."@en ;
	<http://vocabulary.semantic-web.at/cocktail-ontology/uses> <http://vocabulary.semantic-web.at/cocktails/2dce3576-2603-41f9-8dce-ab21f639c2a7> ;
	<http://vocabulary.semantic-web.at/cocktail-ontology/uses_2> <http://vocabulary.semantic-web.at/cocktails/99171f20-c59f-40c4-998a-a9c8f1909168> ;
	a <http://vocabulary.semantic-web.at/cocktail-ontology/Cocktail> , skos:Concept ;
	skos:altLabel "Spritz"@en ;
	skos:broader <http://vocabulary.semantic-web.at/cocktails/204cd4e7-58d7-4417-837a-7f9cc41663c8> , <http://vocabulary.semantic-web.at/cocktails/b523727e-7f49-4e1b-9c09-55002ee3a81e> , <http://vocabulary.semantic-web.at/cocktails/ccee1079-43df-4ff1-bef0-d15d3dc8fa6f> ;
	skos:definition "The Spritz is a wine-based cocktail commonly served as an aperitif in northern Italy, especially in the Veneto region and surrounding areas. The drink is prepared with prosecco wine, a dash of some bitter liqueur such as Aperol, Campari, Select or Cynar. The glass is then topped off with sparkling mineral water. It is usually served over ice in a lowball glass (or sometimes a martini glass or wine glass) and garnished a slice of orange, or sometimes an olive, depending on the liqueur."@en ;
	skos:exactMatch <http://dbpedia.org/resource/Spritz_(alcoholic_beverage)> ;
	skos:prefLabel "Spritz Veneziano"@en .

<http://vocabulary.semantic-web.at/cocktails/2ce50273-13b2-4ba1-9ff2-8cfbd835c1f2> dcterms:contributor <http://localhost/user/blumauera> ;
	dcterms:created "2015-05-01T08:21:37Z"^^xsd:dateTime ;
	dcterms:creator <http://localhost/user/blumauera> ;
	dcterms:modified "2015-05-07T07:15:59Z"^^xsd:dateTime ;
	<http://schema.semantic-web.at/ppt/inScheme> <http://vocabulary.semantic-web.at/cocktails/591cf89a-57af-49b8-9042-3fc77408c93e> ;
	<http://schema.semantic-web.at/ppt/inSubtree> <http://vocabulary.semantic-web.at/cocktails/e86c1671-4a67-494b-ae5d-bcb750865acc> ;
	<http://vocabulary.semantic-web.at/cocktail-ontology/is-part-of> <http://vocabulary.semantic-web.at/cocktails/0f8cc862-9056-49be-b636-cd22f8d7282d> , <http://vocabulary.semantic-web.at/cocktails/13b85b5c-7f69-4871-bb08-3cd5281f6039> , <http://vocabulary.semantic-web.at/cocktails/2c3083d2-8650-4460-b019-cae7aea38f14> , <http://vocabulary.semantic-web.at/cocktails/55c40695-8b41-41ed-8c6a-70fe6930067e> , <http://vocabulary.semantic-web.at/cocktails/79d4686d-4f5b-4067-a2ef-99beccc51242> , <http://vocabulary.semantic-web.at/cocktails/9c287d15-c699-4f56-bd65-bf8cc75a2cca> , <http://vocabulary.semantic-web.at/cocktails/a5db05ca-eda3-41ef-a8ab-ba77b3e4baba> , <http://vocabulary.semantic-web.at/cocktails/c2249dc0-0529-4a11-ad82-5d710b5e9c31> , <http://vocabulary.semantic-web.at/cocktails/dff0a7f4-ded0-48d5-bd31-881b70fbe36a> ;
	a <http://vocabulary.semantic-web.at/cocktail-ontology/Beverages> , <http://vocabulary.semantic-web.at/cocktail-ontology/Ingredients> , <http://vocabulary.semantic-web.at/cocktail-ontology/Non-alcoholic-Beverages> , skos:Concept ;
	skos:altLabel "FCOJ"@en , "Just Juice"@en , "Not From Concentrate"@en , "Virgin Screwdriver"@en ;
	skos:broader <http://vocabulary.semantic-web.at/cocktails/6c0607a9-410d-4b65-87a1-b189a8e36352> ;
	skos:definition "Orange juice refers to the juice of oranges. It is made by extraction from the fresh fruit, by desiccation and subsequent reconstitution of dried juice, or by concentration of the juice and the subsequent addition of water to the concentrate. In American English, the slang term O.J. may also be used to refer to orange juice."@en ;
	skos:exactMatch dbpedia:Orange_juice ;
	skos:prefLabel "Orange juice"@en .

<http://vocabulary.semantic-web.at/cocktails/2d108ce2-7bf0-4a5d-8f88-636419eba9a3> dcterms:contributor <http://localhost/user/blumauera> ;
	dcterms:created "2015-05-02T08:15:29Z"^^xsd:dateTime ;
	dcterms:creator <http://localhost/user/blumauera> ;
	dcterms:modified "2015-05-02T08:15:29Z"^^xsd:dateTime ;
	<http://schema.semantic-web.at/ppt/inScheme> <http://vocabulary.semantic-web.at/cocktails/591cf89a-57af-49b8-9042-3fc77408c93e> ;
	<http://schema.semantic-web.at/ppt/inSubtree> <http://vocabulary.semantic-web.at/cocktails/403d1249-f37f-4f43-bebf-8dde9677d886> ;
	a <http://vocabulary.semantic-web.at/cocktail-ontology/Alcoholic-Beverages> , <http://vocabulary.semantic-web.at/cocktail-ontology/Beverages> , <http://vocabulary.semantic-web.at/cocktail-ontology/Ingredients> , skos:Concept ;
	skos:altLabel "Lemon Cello"@en , "Lemon cellow"@en , "Lemoncello"@en , "Limoncellos"@en , "Limoncelo"@en ;
	skos:broader <http://vocabulary.semantic-web.at/cocktails/05206233-09be-41ac-9f2e-91263873a20e> ;
	skos:definition "Limoncello is an Italian lemon liqueur mainly produced in Southern Italy, especially in the region around the Gulf of Naples, the Sorrentine Peninsula and the coast of Amalfi and islands of Procida, Ischia and Capri. It is also produced in Sicily, Sardinia, Menton in France, and the Maltese island of Gozo. Though there is debate about the exact origin of the drink, it is at least one hundred years old. Traditionally, it is made from the zest of Femminello St."@en ;
	skos:exactMatch dbpedia:Limoncello ;
	skos:prefLabel "Limoncello"@en .

<http://vocabulary.semantic-web.at/cocktails/2d7c2c72-a6a1-43ef-9175-02885fcf4518> dcterms:contributor <http://localhost/user/blumauera> ;
	dcterms:created "2015-05-03T10:18:09Z"^^xsd:dateTime ;
	dcterms:creator <http://localhost/user/blumauera> ;
	dcterms:modified "2015-05-03T10:18:24Z"^^xsd:dateTime ;
	<http://schema.semantic-web.at/ppt/inScheme> <http://vocabulary.semantic-web.at/cocktails/591cf89a-57af-49b8-9042-3fc77408c93e> ;
	<http://schema.semantic-web.at/ppt/inSubtree> <http://vocabulary.semantic-web.at/cocktails/403d1249-f37f-4f43-bebf-8dde9677d886> ;
	<http://vocabulary.semantic-web.at/cocktail-ontology/is-part-of> <http://vocabulary.semantic-web.at/cocktails/0bbdca98-077b-48d1-99d6-47eca59c442c> ;
	a <http://vocabulary.semantic-web.at/cocktail-ontology/Alcoholic-Beverages> , <http://vocabulary.semantic-web.at/cocktail-ontology/Beverages> , <http://vocabulary.semantic-web.at/cocktail-ontology/Ingredients> , skos:Concept ;
	skos:altLabel "Creme violette"@en , "Crème de violette"@en , "Liqueur de violette"@en ;
	skos:broader <http://vocabulary.semantic-web.at/cocktails/47635419-edef-4b78-8da1-e58a96d96f61> ;
	skos:definition "Crème de Violette, also known as liqueur de violette, is a generic term for a liqueur with natural and/or artificial violet flower flavoring and coloring with either a brandy base, a neutral spirit base, or a combination of the two. The taste profile and aroma are distinctly floral and sweet, and to many reminiscent of the violet candies popular in the early to mid 20th century. Its known production dates back to the early 19th century when it was served with dry vermouth or alone as a cordial."@en ;
	skos:exactMatch dbpedia:Creme_de_violette ;
	skos:prefLabel "Creme de violette"@en .

<http://vocabulary.semantic-web.at/cocktails/2d85fb1b-96cb-4c48-8df5-707032f34e71> dcterms:contributor <http://localhost/user/blumauera> ;
	dcterms:created "2015-05-01T08:11:53Z"^^xsd:dateTime ;
	dcterms:creator <http://localhost/user/blumauera> ;
	dcterms:modified "2016-08-04T14:11:16Z"^^xsd:dateTime ;
	<http://schema.semantic-web.at/ppt/inScheme> <http://vocabulary.semantic-web.at/cocktails/8d052dfc-44bf-4985-8ce3-4564570a161b> ;
	<http://vocabulary.semantic-web.at/cocktail-ontology/consists-of> <http://vocabulary.semantic-web.at/cocktails/1439e6c3-a155-4c80-8a5d-723453b4d17e> , <http://vocabulary.semantic-web.at/cocktails/7dede323-e986-4417-b723-c9c7a7fe82ba> , <http://vocabulary.semantic-web.at/cocktails/88f5de3d-3de4-4a2f-9523-50bc7bb06600> ;
	<http://vocabulary.semantic-web.at/cocktail-ontology/iba> <http://www.iba-world.com/index.php?option=com_content&id=259&Itemid=532> ;
	<http://vocabulary.semantic-web.at/cocktail-ontology/image> <http://upload.wikimedia.org/wikipedia/commons/thumb/3/37/MargaritaReal.jpg/440px-MargaritaReal.jpg> ;
	<http://vocabulary.semantic-web.at/cocktail-ontology/preparation> "Pour all ingredients into shaker with ice. Shake well and strain into cocktail glass rimmed with salt "@en ;
	<http://vocabulary.semantic-web.at/cocktail-ontology/served> "On the rocks; poured over ice"@en ;
	<http://vocabulary.semantic-web.at/cocktail-ontology/uses> <http://vocabulary.semantic-web.at/cocktails/e90dfeeb-19f6-4c8f-8b2e-a230850fb35b> ;
	<http://vocabulary.semantic-web.at/cocktail-ontology/uses_2> <http://vocabulary.semantic-web.at/cocktails/e2d63a1c-56e7-47d2-b01b-8cf88cac3d8b> ;
	a <http://vocabulary.semantic-web.at/cocktail-ontology/Cocktail> , skos:Concept ;
	skos:altLabel "Bob and Rita"@en , "Margarita (cocktail)"@en , "Margarita (drink)"@en , "Margerita"@en , "Upside Down Margarita"@en ;
	skos:broader <http://vocabulary.semantic-web.at/cocktails/7516b400-963a-4151-8fdc-f6b23bad1dd5> , <http://vocabulary.semantic-web.at/cocktails/b9bf3799-a4e4-47f7-9aea-7697cc998a34> ;
	skos:definition "The margarita is a Mexican cocktail consisting of tequila mixed with Cointreau or similar orange-flavoured liqueur and lime or lemon juice, often served with salt on the glass rim. It is the most common tequila-based cocktail in the United States. The drink is served shaken with ice (on the rocks), blended with ice (frozen margarita), or without ice (straight up)."@en ;
	skos:exactMatch dbpedia:Margarita ;
	skos:prefLabel "Margarita"@en .

<http://vocabulary.semantic-web.at/cocktails/2dce3576-2603-41f9-8dce-ab21f639c2a7> dcterms:contributor <http://localhost/user/blumauera> ;
	dcterms:created "2015-05-01T08:33:07Z"^^xsd:dateTime ;
	dcterms:creator <http://localhost/user/blumauera> ;
	dcterms:modified "2015-05-07T07:24:13Z"^^xsd:dateTime ;
	<http://schema.semantic-web.at/ppt/inScheme> <http://vocabulary.semantic-web.at/cocktails/f09732a9-a0e6-494a-8ce9-299ef036aaaf> ;
	<http://vocabulary.semantic-web.at/cocktail-ontology/image_2> <http://upload.wikimedia.org/wikipedia/commons/thumb/9/9f/Ofgcup.svg/32px-Ofgcup.svg.png> ;
	<http://vocabulary.semantic-web.at/cocktail-ontology/is-used-by> <http://vocabulary.semantic-web.at/cocktails/1576f08f-5936-4071-b85e-d4e85f31c303> , <http://vocabulary.semantic-web.at/cocktails/2c682ed8-e2ba-473e-8cb7-979598080e18> , <http://vocabulary.semantic-web.at/cocktails/33d9a47f-0622-4b0f-ad1b-62eb96fc6799> , <http://vocabulary.semantic-web.at/cocktails/40ab50e9-66f1-411b-8220-ef8f05273542> , <http://vocabulary.semantic-web.at/cocktails/43b786b6-a1f1-4b7f-a5d9-be43d386ffb4> , <http://vocabulary.semantic-web.at/cocktails/45788a96-1fde-486b-80fc-31ad243bba31> , <http://vocabulary.semantic-web.at/cocktails/52117ab2-dcb8-4d28-a366-ddd932e58219> , <http://vocabulary.semantic-web.at/cocktails/563bf7e0-0f40-41b6-a749-c4e94760204d> , <http://vocabulary.semantic-web.at/cocktails/76c0e55c-22df-4489-9551-4fe8a6a649f8> , <http://vocabulary.semantic-web.at/cocktails/b0885ae3-68e1-453d-8669-119e8464ff5f> , <http://vocabulary.semantic-web.at/cocktails/b33091cd-8c57-45e3-a89b-9de91ffce1e8> , <http://vocabulary.semantic-web.at/cocktails/bca7bc6d-6709-48b8-ae52-fe194c212398> , <http://vocabulary.semantic-web.at/cocktails/be3653af-d585-43f7-b8ce-ad75b1bd7aad> , <http://vocabulary.semantic-web.at/cocktails/c8f4f6bd-4ac1-456a-a3aa-595e4b93d979> , <http://vocabulary.semantic-web.at/cocktails/fb278b46-3c67-48b0-b9eb-7ea037294f5f> ;
	a <http://vocabulary.semantic-web.at/cocktail-ontology/Drinkware> , skos:Concept ;
	skos:altLabel "Lowball glass"@en , "Old-Fashioned glass"@en , "Old-fashioned glass"@en , "Rocks glass"@en , "Whiskey glass"@en , "Whisky glass"@en ;
	skos:broader <http://vocabulary.semantic-web.at/cocktails/2e839563-8037-4e59-8dbf-27736605d687> ;
	skos:definition "The Old Fashioned glass, lowball glass, or rocks glass is a short tumbler used for serving an alcoholic beverage, such as whisky, with ice cubes (“on the rocks”). It is also normally used to serve certain cocktails, such as the Old Fashioned, from which it receives its name. Old fashioned glasses typically have a wide brim, thus releasing the flavours of the drink."@en ;
	skos:exactMatch dbpedia:Old_Fashioned_glass ;
	skos:prefLabel "Old Fashioned glass"@en .

<http://vocabulary.semantic-web.at/cocktails/2e20010b-3ddb-48b9-b275-682e5c357730> dcterms:contributor <http://localhost/user/blumauera> ;
	dcterms:created "2015-05-02T19:16:34Z"^^xsd:dateTime ;
	dcterms:creator <http://localhost/user/blumauera> ;
	dcterms:modified "2015-05-05T06:39:55Z"^^xsd:dateTime ;
	<http://schema.semantic-web.at/ppt/inScheme> <http://vocabulary.semantic-web.at/cocktails/591cf89a-57af-49b8-9042-3fc77408c93e> ;
	<http://schema.semantic-web.at/ppt/inSubtree> <http://vocabulary.semantic-web.at/cocktails/403d1249-f37f-4f43-bebf-8dde9677d886> ;
	<http://vocabulary.semantic-web.at/cocktail-ontology/is-part-of> <http://vocabulary.semantic-web.at/cocktails/cd66d6ff-559f-43ea-a754-ac613a87325d> ;
	a <http://vocabulary.semantic-web.at/cocktail-ontology/Alcoholic-Beverages> , <http://vocabulary.semantic-web.at/cocktail-ontology/Beverages> , <http://vocabulary.semantic-web.at/cocktail-ontology/Ingredients> , skos:Concept ;
	skos:altLabel "Bailey's"@en , "Bailey's Cream"@en , "Bailey's Irish Cream"@en , "Baileys"@en , "Baileys Cream"@en ;
	skos:broader <http://vocabulary.semantic-web.at/cocktails/e5f9e219-d894-491c-a009-20336f5b8e7f> ;
	skos:definition "Baileys Irish Cream is an Irish whiskey and cream based liqueur, made by Gilbeys of Ireland. The trademark is currently owned by Diageo. It has a declared alcohol content of 17% alcohol by volume. It can be compared to other cream liqueurs such as Amarula, Carolans and Sangster's."@en ;
	skos:exactMatch dbpedia:Baileys_Irish_Cream ;
	skos:prefLabel "Baileys Irish Cream"@en .

<http://vocabulary.semantic-web.at/cocktails/2e839563-8037-4e59-8dbf-27736605d687> dcterms:created "2015-05-01T07:55:14Z"^^xsd:dateTime ;
	dcterms:creator <http://localhost/user/blumauera> ;
	<http://schema.semantic-web.at/ppt/inScheme> <http://vocabulary.semantic-web.at/cocktails/f09732a9-a0e6-494a-8ce9-299ef036aaaf> ;
	a <http://vocabulary.semantic-web.at/cocktail-ontology/Drinkware> , skos:Concept ;
	skos:narrower <http://vocabulary.semantic-web.at/cocktails/20d288cb-4e38-46f9-9bec-1c79d8397215> , <http://vocabulary.semantic-web.at/cocktails/2dce3576-2603-41f9-8dce-ab21f639c2a7> , <http://vocabulary.semantic-web.at/cocktails/a54d2096-6214-4006-beaf-afcc77824710> , <http://vocabulary.semantic-web.at/cocktails/bfbfb9b6-4c70-4323-a64b-4cfd533c55d8> ;
	skos:prefLabel "Tumbler"@en ;
	skos:topConceptOf <http://vocabulary.semantic-web.at/cocktails/f09732a9-a0e6-494a-8ce9-299ef036aaaf> .

<http://vocabulary.semantic-web.at/cocktails/2ea18d11-7415-4282-9608-7a3f497a0928> dcterms:contributor <http://localhost/user/blumauera> ;
	dcterms:created "2015-05-01T07:53:52Z"^^xsd:dateTime ;
	dcterms:creator <http://localhost/user/blumauera> ;
	dcterms:modified "2015-05-02T19:45:07Z"^^xsd:dateTime ;
	<http://schema.semantic-web.at/ppt/inScheme> <http://vocabulary.semantic-web.at/cocktails/f09732a9-a0e6-494a-8ce9-299ef036aaaf> ;
	a <http://vocabulary.semantic-web.at/cocktail-ontology/Drinkware> , skos:Concept ;
	skos:definition "Stemware is drinkware that stands on stems above a base. It is usually made from glass, but may be made from ceramics or metals. Stemware includes: Champagne flutes Chalices and goblets Cocktail glasses (including martini glasses and margarita glasses) Liqueur glasses Rummers Snifters Wine glasses"@en ;
	skos:exactMatch dbpedia:Stemware ;
	skos:narrower <http://vocabulary.semantic-web.at/cocktails/19dee0d8-fd30-469f-9ecd-91c902ff717c> , <http://vocabulary.semantic-web.at/cocktails/22c81328-d483-4c62-8338-cb732ee39734> , <http://vocabulary.semantic-web.at/cocktails/e576e848-0f11-4f7a-b6b3-1ff820b02023> , <http://vocabulary.semantic-web.at/cocktails/e90dfeeb-19f6-4c8f-8b2e-a230850fb35b> , <http://vocabulary.semantic-web.at/cocktails/fece03b5-ec0b-4e47-964d-cc5dc09fd7fb> ;
	skos:prefLabel "Stemware"@en ;
	skos:topConceptOf <http://vocabulary.semantic-web.at/cocktails/f09732a9-a0e6-494a-8ce9-299ef036aaaf> .

<http://vocabulary.semantic-web.at/cocktails/33d9a47f-0622-4b0f-ad1b-62eb96fc6799> dcterms:contributor <http://localhost/user/blumauera> ;
	dcterms:created "2015-05-02T07:28:48Z"^^xsd:dateTime ;
	dcterms:creator <http://localhost/user/blumauera> ;
	dcterms:modified "2015-05-06T12:27:42Z"^^xsd:dateTime ;
	<http://schema.semantic-web.at/ppt/inScheme> <http://vocabulary.semantic-web.at/cocktails/8d052dfc-44bf-4985-8ce3-4564570a161b> ;
	<http://vocabulary.semantic-web.at/cocktail-ontology/consists-of> <http://vocabulary.semantic-web.at/cocktails/22df810d-e509-4da8-979c-0758e94de3e6> , <http://vocabulary.semantic-web.at/cocktails/a12b3836-dba0-49e9-92c6-7725ccf35944> ;
	<http://vocabulary.semantic-web.at/cocktail-ontology/iba> <http://www.iba-world.com/index.php?option=com_content&id=215&Itemid=532> ;
	<http://vocabulary.semantic-web.at/cocktail-ontology/image> <http://upload.wikimedia.org/wikipedia/commons/c/c5/Blackrussian.jpg> ;
	<http://vocabulary.semantic-web.at/cocktail-ontology/preparation> "Pour the ingredients into the old fashioned-glass filled with ice cubes. Stir gently."@en ;
	<http://vocabulary.semantic-web.at/cocktail-ontology/served> "On the rocks; poured over ice"@en ;
	<http://vocabulary.semantic-web.at/cocktail-ontology/uses> <http://vocabulary.semantic-web.at/cocktails/2dce3576-2603-41f9-8dce-ab21f639c2a7> ;
	a <http://vocabulary.semantic-web.at/cocktail-ontology/Cocktail> , skos:Concept ;
	skos:altLabel "Black Russian (cocktail)"@en , "Tall Black Russian"@en , "Tall black russian"@en ;
	skos:broader <http://vocabulary.semantic-web.at/cocktails/b9bf3799-a4e4-47f7-9aea-7697cc998a34> ;
	skos:definition "The Black Russian is a cocktail of vodka and coffee liqueur. It contains either three parts vodka and two parts coffee liqueur, per the Kahlúa bottle's label, or five parts vodka to two parts coffee liqueur, per IBA specified ingredients. Traditionally the drink is made by pouring the vodka over ice cubes or cracked ice in an old-fashioned glass, followed by the coffee liqueur."@en ;
	skos:exactMatch dbpedia:Black_Russian ;
	skos:prefLabel "Black Russian"@en .

<http://vocabulary.semantic-web.at/cocktails/33df103a-03ac-4177-b620-7953fe094236> dcterms:contributor <http://localhost/user/blumauera> ;
	dcterms:created "2015-05-02T17:19:40Z"^^xsd:dateTime ;
	dcterms:creator <http://localhost/user/blumauera> ;
	dcterms:modified "2015-07-02T14:56:34Z"^^xsd:dateTime ;
	<http://schema.semantic-web.at/ppt/inScheme> <http://vocabulary.semantic-web.at/cocktails/eff672ac-6601-42c6-a3e9-0adda3b45df8> ;
	<http://schema.semantic-web.at/ppt/inSubtree> <http://vocabulary.semantic-web.at/cocktails/4f20d6bb-710d-4870-bde4-b6e835d7d13f> ;
	<http://vocabulary.semantic-web.at/cocktail-ontology/is-used-by_2> <http://vocabulary.semantic-web.at/cocktails/1576f08f-5936-4071-b85e-d4e85f31c303> , <http://vocabulary.semantic-web.at/cocktails/1d5b39cc-fcab-48b2-bb24-9840b7e34d64> , <http://vocabulary.semantic-web.at/cocktails/236b36df-93ca-4408-836c-133ace53798a> , <http://vocabulary.semantic-web.at/cocktails/268fb62f-8ef1-45cd-844f-8c7da85a6a0b> , <http://vocabulary.semantic-web.at/cocktails/36671f9c-904a-4629-937a-519d094ecefc> , <http://vocabulary.semantic-web.at/cocktails/383ea520-07b2-4dc9-8827-8fc84fb7749c> , <http://vocabulary.semantic-web.at/cocktails/44cc99c1-28ac-4c50-a55d-7244b2c5c07b> , <http://vocabulary.semantic-web.at/cocktails/4f85cadd-4fd4-4ffc-a78d-cddb0763fa4b> , <http://vocabulary.semantic-web.at/cocktails/53a05366-d473-4eb4-ac66-0d0119e0b759> , <http://vocabulary.semantic-web.at/cocktails/563bf7e0-0f40-41b6-a749-c4e94760204d> , <http://vocabulary.semantic-web.at/cocktails/72a77af2-bbee-4b75-871f-a96dcd3a452b> , <http://vocabulary.semantic-web.at/cocktails/a0fba95c-d29e-4954-8800-f5e6de1e6f86> , <http://vocabulary.semantic-web.at/cocktails/b00a123f-a2b5-49d2-8325-a81d1d26ddc6> , <http://vocabulary.semantic-web.at/cocktails/b33091cd-8c57-45e3-a89b-9de91ffce1e8> , <http://vocabulary.semantic-web.at/cocktails/be3653af-d585-43f7-b8ce-ad75b1bd7aad> , <http://vocabulary.semantic-web.at/cocktails/bee1e709-b317-4f46-b06f-a22367baefdf> , <http://vocabulary.semantic-web.at/cocktails/ce8f4591-ccd4-4d90-a761-244115d64061> , <http://vocabulary.semantic-web.at/cocktails/eddf4894-1683-44e9-9ee3-7920d3729d71> ;
	a <http://vocabulary.semantic-web.at/cocktail-ontology/Garnish> , <http://vocabulary.semantic-web.at/cocktail-ontology/Ingredients> , skos:Concept ;
	skos:altLabel "Citrus limon"@en , "Citrus x limon"@en , "Citrus × limon"@en , "Lemon (fruit)"@en , "Lemon extract"@en , "Lemon oil"@en , "Lemons"@en , "Nimbu"@en , "🍋"@en ;
	skos:broader <http://vocabulary.semantic-web.at/cocktails/4f20d6bb-710d-4870-bde4-b6e835d7d13f> ;
	skos:definition "The lemon is a small evergreen tree native to Asia, and the tree's ellipsoidal yellow fruit. The fruit is used for culinary and non-culinary purposes throughout the world, primarily for its juice, though the pulp and rind are also used in cooking and baking. The juice of the lemon is about 5% to 6% citric acid, which gives lemons a sour taste. The distinctive sour taste of lemon juice makes it a key ingredient in drinks and foods such as lemonade."@en ;
	skos:exactMatch dbpedia:Lemon ;
	skos:narrower <http://vocabulary.semantic-web.at/cocktails/7effbf10-d493-429f-aaff-04011849774d> ;
	skos:prefLabel "Lemon"@en .

<http://vocabulary.semantic-web.at/cocktails/347f5539-1dae-44fc-9e7b-a2cbe9e2e157> dcterms:contributor <http://localhost/user/blumauera> ;
	dcterms:created "2015-05-02T17:26:07Z"^^xsd:dateTime ;
	dcterms:creator <http://localhost/user/blumauera> ;
	dcterms:modified "2015-05-07T06:50:14Z"^^xsd:dateTime ;
	<http://schema.semantic-web.at/ppt/inScheme> <http://vocabulary.semantic-web.at/cocktails/f09732a9-a0e6-494a-8ce9-299ef036aaaf> ;
	<http://vocabulary.semantic-web.at/cocktail-ontology/is-used-by> <http://vocabulary.semantic-web.at/cocktails/c3b197cc-8583-4e2f-8e45-3a7fed1309c1> ;
	a <http://vocabulary.semantic-web.at/cocktail-ontology/Drinkware> , skos:Concept ;
	skos:broader <http://vocabulary.semantic-web.at/cocktails/d6c5f29f-bef7-41c5-9d39-535d83e9f750> ;
	skos:prefLabel "Irish coffee mug"@en .

<http://vocabulary.semantic-web.at/cocktails/36671f9c-904a-4629-937a-519d094ecefc> dcterms:contributor <http://localhost/user/blumauera> ;
	dcterms:created "2015-05-02T07:20:00Z"^^xsd:dateTime ;
	dcterms:creator <http://localhost/user/blumauera> ;
	dcterms:modified "2015-05-05T06:27:15Z"^^xsd:dateTime ;
	<http://schema.semantic-web.at/ppt/inScheme> <http://vocabulary.semantic-web.at/cocktails/8d052dfc-44bf-4985-8ce3-4564570a161b> ;
	<http://vocabulary.semantic-web.at/cocktail-ontology/consists-of> <http://vocabulary.semantic-web.at/cocktails/5d96c50c-ee48-4c40-bb4c-4b9a42d11de6> , <http://vocabulary.semantic-web.at/cocktails/9c2ce399-c6ae-4f4d-bf37-7fd8ffe2a19d> , <http://vocabulary.semantic-web.at/cocktails/d530df52-cc54-4be3-8409-85734e5ec67f> ;
	<http://vocabulary.semantic-web.at/cocktail-ontology/iba> <http://www.iba-world.com/index.php?option=com_content&id=212&Itemid=532> ;
	<http://vocabulary.semantic-web.at/cocktail-ontology/image> <http://www.iba-world.com/images/cocktail_drinks/white_lady.jpg> ;
	<http://vocabulary.semantic-web.at/cocktail-ontology/is-variant-of> <http://vocabulary.semantic-web.at/cocktails/e039633b-03c1-47bd-a705-a104a4323e45> ;
	<http://vocabulary.semantic-web.at/cocktail-ontology/preparation> "Add all ingredients into cocktail shaker filled with ice. Shake well and strain into large cocktail glass."@en ;
	<http://vocabulary.semantic-web.at/cocktail-ontology/served> "Straight up; without ice"@en ;
	<http://vocabulary.semantic-web.at/cocktail-ontology/uses> <http://vocabulary.semantic-web.at/cocktails/19dee0d8-fd30-469f-9ecd-91c902ff717c> ;
	<http://vocabulary.semantic-web.at/cocktail-ontology/uses_2> <http://vocabulary.semantic-web.at/cocktails/33df103a-03ac-4177-b620-7953fe094236> ;
	a <http://vocabulary.semantic-web.at/cocktail-ontology/Cocktail> , skos:Concept ;
	skos:altLabel "Chelsea Side-car"@en , "Delilah"@en , "Lillian Forever"@en ;
	skos:broader <http://vocabulary.semantic-web.at/cocktails/7516b400-963a-4151-8fdc-f6b23bad1dd5> , <http://vocabulary.semantic-web.at/cocktails/caae2ea0-7e60-400b-a2bb-14ef79720668> ;
	skos:prefLabel "White Lady"@en .

<http://vocabulary.semantic-web.at/cocktails/371797a7-e9a8-453b-8744-2e89f2fd30d2> dcterms:contributor <http://localhost/user/blumauera> ;
	dcterms:created "2015-05-03T11:38:08Z"^^xsd:dateTime ;
	dcterms:creator <http://localhost/user/blumauera> ;
	dcterms:modified "2015-05-05T07:31:49Z"^^xsd:dateTime ;
	<http://schema.semantic-web.at/ppt/inScheme> <http://vocabulary.semantic-web.at/cocktails/87384ce8-f20a-4201-b06d-3e0b8d832e5d> ;
	<http://vocabulary.semantic-web.at/cocktail-ontology/is-part-of> <http://vocabulary.semantic-web.at/cocktails/c3ae5830-1bfd-4f37-afc9-3e88849d03cf> ;
	a <http://vocabulary.semantic-web.at/cocktail-ontology/Ingredients> , skos:Concept ;
	skos:broader <http://vocabulary.semantic-web.at/cocktails/0e385475-f369-4832-b8e3-20f35028988d> ;
	skos:prefLabel "Raspberry syrup"@en .

<http://vocabulary.semantic-web.at/cocktails/372c645f-53c5-4b75-ba34-b36625f87b02> dcterms:contributor <http://localhost/user/blumauera> ;
	dcterms:created "2015-05-01T15:08:14Z"^^xsd:dateTime ;
	dcterms:creator <http://localhost/user/blumauera> ;
	dcterms:modified "2015-05-03T10:43:56Z"^^xsd:dateTime ;
	<http://schema.semantic-web.at/ppt/inScheme> <http://vocabulary.semantic-web.at/cocktails/591cf89a-57af-49b8-9042-3fc77408c93e> ;
	<http://schema.semantic-web.at/ppt/inSubtree> <http://vocabulary.semantic-web.at/cocktails/403d1249-f37f-4f43-bebf-8dde9677d886> ;
	a <http://vocabulary.semantic-web.at/cocktail-ontology/Alcoholic-Beverages> , <http://vocabulary.semantic-web.at/cocktail-ontology/Beverages> , <http://vocabulary.semantic-web.at/cocktail-ontology/Ingredients> , skos:Concept ;
	skos:altLabel "Kraeuterlikoer"@en , "Krauterlikor"@en ;
	skos:broader <http://vocabulary.semantic-web.at/cocktails/917d78d0-0938-4fe0-80c4-cfd2eb16e6a4> ;
	skos:definition "Kräuterlikör (herbal liqueur or spiced liqueur) is a kind of German liqueur that is flavored with herbs or spices and sweetened with sugar. Liqueurs of this kind normally contain 15% to 44% alcohol by volume. Widely sold brands are Jägermeister, Killepitsch, Kuemmerling and Mummelmann. The history of Kräuterlikör goes back to the Middle Ages, when mixtures of alcohol and herbs were used as medicine."@en ;
	skos:exactMatch dbpedia:Kr%C3%A4uterlik%C3%B6r ;
	skos:prefLabel "Kräuterlikör"@en .

<http://vocabulary.semantic-web.at/cocktails/383ea520-07b2-4dc9-8827-8fc84fb7749c> dcterms:contributor <http://localhost/user/blumauera> ;
	dcterms:created "2015-05-01T14:37:04Z"^^xsd:dateTime ;
	dcterms:creator <http://localhost/user/blumauera> ;
	dcterms:modified "2015-05-03T18:19:38Z"^^xsd:dateTime ;
	<http://schema.semantic-web.at/ppt/inScheme> <http://vocabulary.semantic-web.at/cocktails/8d052dfc-44bf-4985-8ce3-4564570a161b> ;
	<http://vocabulary.semantic-web.at/cocktail-ontology/consists-of> <http://vocabulary.semantic-web.at/cocktails/5d96c50c-ee48-4c40-bb4c-4b9a42d11de6> , <http://vocabulary.semantic-web.at/cocktails/71210bd1-3071-4533-8da4-fe0f7d7694a0> , <http://vocabulary.semantic-web.at/cocktails/7448dbed-7603-41f7-a316-99f754c9ae45> , <http://vocabulary.semantic-web.at/cocktails/9c2ce399-c6ae-4f4d-bf37-7fd8ffe2a19d> ;
	<http://vocabulary.semantic-web.at/cocktail-ontology/iba> <http://www.iba-world.com/index.php?option=com_content&id=197&Itemid=532> ;
	<http://vocabulary.semantic-web.at/cocktail-ontology/image> <http://www.iba-world.com/images/cocktail_drinks/john_collins.jpg> ;
	<http://vocabulary.semantic-web.at/cocktail-ontology/preparation> "Pour all ingredients directly into highball glass filled with ice. Stir gently. Garnish with lemon slice and maraschino cherry. Add a dash of Angostura bitters."@en ;
	<http://vocabulary.semantic-web.at/cocktail-ontology/uses> <http://vocabulary.semantic-web.at/cocktails/a54d2096-6214-4006-beaf-afcc77824710> ;
	<http://vocabulary.semantic-web.at/cocktail-ontology/uses_2> <http://vocabulary.semantic-web.at/cocktails/33df103a-03ac-4177-b620-7953fe094236> , <http://vocabulary.semantic-web.at/cocktails/8a5e1790-d3c0-432e-bb85-709692b14f03> ;
	a <http://vocabulary.semantic-web.at/cocktail-ontology/Cocktail> , skos:Concept ;
	skos:broader <http://vocabulary.semantic-web.at/cocktails/caae2ea0-7e60-400b-a2bb-14ef79720668> ;
	skos:prefLabel "John Collins"@en .

<http://vocabulary.semantic-web.at/cocktails/397d0ec3-98e2-47d9-a8c2-eca9702ff94d> dcterms:contributor <http://localhost/user/blumauera> ;
	dcterms:created "2015-05-01T08:36:13Z"^^xsd:dateTime ;
	dcterms:creator <http://localhost/user/blumauera> ;
	dcterms:modified "2015-05-06T12:59:08Z"^^xsd:dateTime ;
	<http://schema.semantic-web.at/ppt/inScheme> <http://vocabulary.semantic-web.at/cocktails/591cf89a-57af-49b8-9042-3fc77408c93e> ;
	<http://schema.semantic-web.at/ppt/inSubtree> <http://vocabulary.semantic-web.at/cocktails/403d1249-f37f-4f43-bebf-8dde9677d886> ;
	<http://vocabulary.semantic-web.at/cocktail-ontology/is-part-of> <http://vocabulary.semantic-web.at/cocktails/13b85b5c-7f69-4871-bb08-3cd5281f6039> , <http://vocabulary.semantic-web.at/cocktails/4f85cadd-4fd4-4ffc-a78d-cddb0763fa4b> ;
	a <http://vocabulary.semantic-web.at/cocktail-ontology/Alcoholic-Beverages> , <http://vocabulary.semantic-web.at/cocktail-ontology/Beverages> , <http://vocabulary.semantic-web.at/cocktail-ontology/Ingredients> , skos:Concept ;
	skos:broader <http://vocabulary.semantic-web.at/cocktails/2944baef-5338-421b-a5f5-0e51f75244c2> ;
	skos:narrower <http://vocabulary.semantic-web.at/cocktails/1439e6c3-a155-4c80-8a5d-723453b4d17e> , <http://vocabulary.semantic-web.at/cocktails/59848efb-dc96-4014-af09-5f89ba057df9> , <http://vocabulary.semantic-web.at/cocktails/82026d8e-0fa5-4317-8827-410133db3bbd> ;
	skos:prefLabel "Orange-flavored liqueur"@en .

<http://vocabulary.semantic-web.at/cocktails/3abfd580-0f7d-4971-9c90-3cc8a5dafc0c> dcterms:contributor <http://localhost/user/blumauera> ;
	dcterms:created "2015-05-02T19:23:07Z"^^xsd:dateTime ;
	dcterms:creator <http://localhost/user/blumauera> ;
	dcterms:modified "2015-05-05T07:25:10Z"^^xsd:dateTime ;
	<http://schema.semantic-web.at/ppt/inScheme> <http://vocabulary.semantic-web.at/cocktails/eff672ac-6601-42c6-a3e9-0adda3b45df8> ;
	<http://schema.semantic-web.at/ppt/inSubtree> <http://vocabulary.semantic-web.at/cocktails/4f20d6bb-710d-4870-bde4-b6e835d7d13f> ;
	<http://vocabulary.semantic-web.at/cocktail-ontology/is-used-by_2> <http://vocabulary.semantic-web.at/cocktails/7e5afb63-30ec-42b4-a9f5-f61fc456107d> ;
	a <http://vocabulary.semantic-web.at/cocktail-ontology/Garnish> , <http://vocabulary.semantic-web.at/cocktail-ontology/Ingredients> , skos:Concept ;
	skos:altLabel "Coffee Beans"@en , "Coffee Berry"@en , "Coffee beans"@en , "Coffee berries"@en , "Green coffee"@en , "Green coffee bean"@en ;
	skos:broader <http://vocabulary.semantic-web.at/cocktails/4f20d6bb-710d-4870-bde4-b6e835d7d13f> ;
	skos:definition "A coffee bean is a seed of the coffee plant. It is the pit inside the red or purple fruit often referred to as a cherry. Even though they are seeds, they are incorrectly referred to as 'beans' because of their resemblance to true beans. The fruits - coffee cherries or coffee berries - most commonly contain two stones with their flat sides together. A small percentage of cherries contain a single seed, instead of the usual two. This is called a peaberry."@en ;
	skos:exactMatch dbpedia:Coffee_bean ;
	skos:prefLabel "Coffee bean"@en .

<http://vocabulary.semantic-web.at/cocktails/3bc44d8c-4e94-4f84-9354-8770018e8a8d> dcterms:contributor <http://localhost/user/blumauera> ;
	dcterms:created "2015-05-02T18:53:50Z"^^xsd:dateTime ;
	dcterms:creator <http://localhost/user/blumauera> ;
	dcterms:modified "2015-05-07T07:07:23Z"^^xsd:dateTime ;
	<http://schema.semantic-web.at/ppt/inScheme> <http://vocabulary.semantic-web.at/cocktails/87384ce8-f20a-4201-b06d-3e0b8d832e5d> ;
	<http://vocabulary.semantic-web.at/cocktail-ontology/is-part-of> <http://vocabulary.semantic-web.at/cocktails/b8075344-1e6d-4348-bdee-83948203a974> ;
	a <http://vocabulary.semantic-web.at/cocktail-ontology/Ingredients> , skos:Concept ;
	skos:broader <http://vocabulary.semantic-web.at/cocktails/0e385475-f369-4832-b8e3-20f35028988d> ;
	skos:prefLabel "Strawberry syrup"@en .

<http://vocabulary.semantic-web.at/cocktails/3c3cd646-f1a4-4eac-b354-17d78b79a5d5> dcterms:contributor <http://localhost/user/blumauera> ;
	dcterms:created "2015-05-02T07:27:09Z"^^xsd:dateTime ;
	dcterms:creator <http://localhost/user/blumauera> ;
	dcterms:modified "2015-05-02T07:27:09Z"^^xsd:dateTime ;
	<http://schema.semantic-web.at/ppt/inScheme> <http://vocabulary.semantic-web.at/cocktails/87384ce8-f20a-4201-b06d-3e0b8d832e5d> ;
	a <http://vocabulary.semantic-web.at/cocktail-ontology/Ingredients> , skos:Concept ;
	skos:altLabel "Carrot puree"@en , "Carrot purée"@en , "Puree"@en , "Pureé"@en , "Puréed"@en ;
	skos:definition "Purée and (more rarely) mash are general terms for cooked food, usually vegetables or legumes, that have been ground, pressed, blended, and/or sieved to the consistency of a soft creamy paste or thick liquid. Purées of specific foods are often known by specific names, e.g. , mashed potatoes or apple sauce. The term is of French origin, where it meant in Old French (13th century) purified or refined."@en ;
	skos:exactMatch dbpedia:Pur%C3%A9e ;
	skos:narrower <http://vocabulary.semantic-web.at/cocktails/876f13e0-d873-4a11-94e1-e344b80cd53f> ;
	skos:prefLabel "Purée"@en ;
	skos:topConceptOf <http://vocabulary.semantic-web.at/cocktails/87384ce8-f20a-4201-b06d-3e0b8d832e5d> .

<http://vocabulary.semantic-web.at/cocktails/3c94f5fc-4664-4177-a880-88643c0be9c1> dcterms:contributor <http://localhost/user/blumauera> ;
	dcterms:created "2015-05-01T14:11:22Z"^^xsd:dateTime ;
	dcterms:creator <http://localhost/user/blumauera> ;
	dcterms:modified "2015-11-12T12:39:44Z"^^xsd:dateTime ;
	<http://schema.semantic-web.at/ppt/inScheme> <http://vocabulary.semantic-web.at/cocktails/87384ce8-f20a-4201-b06d-3e0b8d832e5d> ;
	<http://schema.semantic-web.at/ppt/propagateType> <http://vocabulary.semantic-web.at/cocktail-ontology/Garnish> ;
	<http://vocabulary.semantic-web.at/cocktail-ontology/is-part-of> <http://vocabulary.semantic-web.at/cocktails/1576f08f-5936-4071-b85e-d4e85f31c303> , <http://vocabulary.semantic-web.at/cocktails/61a18ebf-fd92-4ef1-8ab1-bfd3c26867b9> , <http://vocabulary.semantic-web.at/cocktails/b33091cd-8c57-45e3-a89b-9de91ffce1e8> , <http://vocabulary.semantic-web.at/cocktails/bee1e709-b317-4f46-b06f-a22367baefdf> , <http://vocabulary.semantic-web.at/cocktails/fb278b46-3c67-48b0-b9eb-7ea037294f5f> ;
	<http://vocabulary.semantic-web.at/cocktail-ontology/is-used-by_2> <http://vocabulary.semantic-web.at/cocktails/236b36df-93ca-4408-836c-133ace53798a> , <http://vocabulary.semantic-web.at/cocktails/bca7bc6d-6709-48b8-ae52-fe194c212398> ;
	a <http://vocabulary.semantic-web.at/cocktail-ontology/Garnish> , <http://vocabulary.semantic-web.at/cocktail-ontology/Ingredients> , skos:Concept ;
	skos:altLabel "-Ose"@en , "Berry sugar"@en , "Cube sugar"@en , "Foreign matter in refined sugar"@en , "Lump sugar"@en , "Molten sugar"@en , "Raw Sugar"@en , "Refined sugar"@en , "Shurger"@en , "Sugar Crystals"@en , "Sugar buzz"@en , "Sugar crops"@en , "Sugar cube"@en , "Sugar engineering"@en , "Sugar lumps"@en , "Sugar trade"@en , "Sugars"@en , "Sugary"@en , "Suggar"@en , "Sweet salt"@en , "White Sugar"@en , "White refined sugar"@en , "White sugar"@en ;
	skos:definition "Sugar is the generalised name for a class of chemically-related sweet-flavored substances, most of which are used as food. They are carbohydrates, composed of carbon, hydrogen and oxygen. There are various types of sugar derived from different sources. Simple sugars are called monosaccharides and include glucose (also known as dextrose), fructose and galactose."@en ;
	skos:exactMatch dbpedia:Sugar ;
	skos:narrower <http://vocabulary.semantic-web.at/cocktails/92e8ded1-1223-4a3f-b2d4-7ee731d6dbc7> , <http://vocabulary.semantic-web.at/cocktails/9d9fb486-a0dd-4d1a-b65e-7346a626cadf> , <http://vocabulary.semantic-web.at/cocktails/cd4b845c-d8db-4f73-9a0c-b60743c58019> ;
	skos:prefLabel "Sugar"@en ;
	skos:topConceptOf <http://vocabulary.semantic-web.at/cocktails/87384ce8-f20a-4201-b06d-3e0b8d832e5d> .

<http://vocabulary.semantic-web.at/cocktails/3e2d26b8-928b-462d-99ee-59eac11b241f> dcterms:contributor <http://localhost/user/blumauera> ;
	dcterms:created "2015-05-01T14:31:24Z"^^xsd:dateTime ;
	dcterms:creator <http://localhost/user/blumauera> ;
	dcterms:modified "2015-05-07T06:56:02Z"^^xsd:dateTime ;
	<http://schema.semantic-web.at/ppt/inScheme> <http://vocabulary.semantic-web.at/cocktails/591cf89a-57af-49b8-9042-3fc77408c93e> ;
	<http://schema.semantic-web.at/ppt/inSubtree> <http://vocabulary.semantic-web.at/cocktails/403d1249-f37f-4f43-bebf-8dde9677d886> ;
	<http://vocabulary.semantic-web.at/cocktail-ontology/is-part-of> <http://vocabulary.semantic-web.at/cocktails/1529fd23-9c55-45d7-b8c6-b0fc229a3871> , <http://vocabulary.semantic-web.at/cocktails/76c0e55c-22df-4489-9551-4fe8a6a649f8> , <http://vocabulary.semantic-web.at/cocktails/fb278b46-3c67-48b0-b9eb-7ea037294f5f> ;
	a <http://vocabulary.semantic-web.at/cocktail-ontology/Alcoholic-Beverages> , <http://vocabulary.semantic-web.at/cocktail-ontology/Beverages> , <http://vocabulary.semantic-web.at/cocktail-ontology/Ingredients> , skos:Concept ;
	skos:altLabel "Bourbon"@en , "Bourbon whisky"@en , "Kentucky Whiskey"@en ;
	skos:broader <http://vocabulary.semantic-web.at/cocktails/c4339109-ae35-4be9-a7e8-b5dfd206e960> ;
	skos:definition "Bourbon whiskey is a type of American whiskey – a barrel-aged distilled spirit made primarily from corn. The name of the spirit derives from its historical association with an area known as Old Bourbon, around what is now Bourbon County, Kentucky (which, in turn, was named after the French House of Bourbon royal family). It has been produced since the 18th century."@en ;
	skos:exactMatch dbpedia:Bourbon_whiskey ;
	skos:prefLabel "Bourbon whiskey"@en .

<http://vocabulary.semantic-web.at/cocktails/4028ce28-b682-4c06-b861-010b25f488ca> dcterms:contributor <http://localhost/user/blumauera> ;
	dcterms:created "2015-05-01T14:38:17Z"^^xsd:dateTime ;
	dcterms:creator <http://localhost/user/blumauera> ;
	dcterms:modified "2015-05-06T12:21:26Z"^^xsd:dateTime ;
	<http://schema.semantic-web.at/ppt/inScheme> <http://vocabulary.semantic-web.at/cocktails/591cf89a-57af-49b8-9042-3fc77408c93e> ;
	<http://schema.semantic-web.at/ppt/inSubtree> <http://vocabulary.semantic-web.at/cocktails/403d1249-f37f-4f43-bebf-8dde9677d886> ;
	a <http://vocabulary.semantic-web.at/cocktail-ontology/Alcoholic-Beverages> , <http://vocabulary.semantic-web.at/cocktail-ontology/Beverages> , <http://vocabulary.semantic-web.at/cocktail-ontology/Ingredients> , skos:Concept ;
	skos:altLabel "Canadian rye whisky"@en , "Canadian single malt"@en , "Canadian whiskey"@en , "Whisky/Canadian"@en ;
	skos:broader <http://vocabulary.semantic-web.at/cocktails/4f03a6ef-9631-4b6d-a005-7fbbdcb9b342> ;
	skos:definition "Canadian whisky is a type of whisky produced in Canada. Most Canadian whiskies are blended multi-grain liquors containing a large percentage of corn spirits, and are typically lighter and smoother than other whisky styles. Several hundred years ago, when Canadian distillers began adding small amounts of highly-flavorful rye grain to their mashes people began demanding this new rye-flavored whisky, referring to it simply as \"rye."@en ;
	skos:exactMatch dbpedia:Canadian_whisky ;
	skos:prefLabel "Canadian whisky"@en .

<http://vocabulary.semantic-web.at/cocktails/40362aa1-0058-4f25-ba82-74bcd2202cc4> dcterms:contributor <http://localhost/user/blumauera> ;
	dcterms:created "2015-05-03T18:49:51Z"^^xsd:dateTime ;
	dcterms:creator <http://localhost/user/blumauera> ;
	dcterms:modified "2015-05-03T18:59:23Z"^^xsd:dateTime ;
	<http://schema.semantic-web.at/ppt/inScheme> <http://vocabulary.semantic-web.at/cocktails/591cf89a-57af-49b8-9042-3fc77408c93e> ;
	<http://schema.semantic-web.at/ppt/inSubtree> <http://vocabulary.semantic-web.at/cocktails/403d1249-f37f-4f43-bebf-8dde9677d886> ;
	a <http://vocabulary.semantic-web.at/cocktail-ontology/Alcoholic-Beverages> , <http://vocabulary.semantic-web.at/cocktail-ontology/Beverages> , <http://vocabulary.semantic-web.at/cocktail-ontology/Ingredients> , skos:Concept ;
	skos:broader <http://vocabulary.semantic-web.at/cocktails/8cfd00fe-9f5a-414e-be27-858a8bc43c7c> ;
	skos:narrower <http://vocabulary.semantic-web.at/cocktails/7a2ef9c4-4083-4531-9edc-b27e0353349e> , <http://vocabulary.semantic-web.at/cocktails/92561e61-4e22-4402-bf23-3e1a1fefb530> ;
	skos:prefLabel "Sweet vermouth"@en .

<http://vocabulary.semantic-web.at/cocktails/403d1249-f37f-4f43-bebf-8dde9677d886> dcterms:contributor <http://localhost/user/blumauera> ;
	dcterms:created "2015-05-01T07:51:06Z"^^xsd:dateTime ;
	dcterms:creator <http://localhost/user/blumauera> ;
	dcterms:modified "2015-07-02T14:44:40Z"^^xsd:dateTime ;
	<http://schema.semantic-web.at/ppt/inScheme> <http://vocabulary.semantic-web.at/cocktails/591cf89a-57af-49b8-9042-3fc77408c93e> ;
	<http://schema.semantic-web.at/ppt/propagateType> <http://vocabulary.semantic-web.at/cocktail-ontology/Alcoholic-Beverages> ;
	a <http://vocabulary.semantic-web.at/cocktail-ontology/Alcoholic-Beverages> , <http://vocabulary.semantic-web.at/cocktail-ontology/Beverages> , <http://vocabulary.semantic-web.at/cocktail-ontology/Ingredients> , skos:Concept ;
	skos:altLabel "Distilled Spirit"@en , "Distilled alcoholic beverage"@en , "Distilled beverages"@en , "Distilled liquor"@en , "Distilled spirit"@en , "Distilled spirits"@en , "Fire Water"@en , "Hard alcohol"@en , "Hard liquor"@en , "Liqour"@en , "Liquor"@en , "Liquors"@en , "ליקר"@en ;
	skos:definition "A distilled beverage, spirit, or liquor is an alcoholic beverage containing ethanol that is produced by distilling ethanol produced by means of fermenting grain, fruit, or vegetables. This excludes undistilled fermented beverages such as beer, wine, and cider. Vodka, gin, baijiu, tequila, rum, whisky, brandy, and soju are examples of distilled beverages. The term hard liquor is used in North America and India to distinguish distilled beverages from undistilled ones (implicitly weaker)."@en ;
	skos:exactMatch dbpedia:Distilled_beverage ;
	skos:narrower <http://vocabulary.semantic-web.at/cocktails/22df810d-e509-4da8-979c-0758e94de3e6> , <http://vocabulary.semantic-web.at/cocktails/27c48d24-bb0b-46a3-9b0c-4b09e38a4b07> , <http://vocabulary.semantic-web.at/cocktails/2944baef-5338-421b-a5f5-0e51f75244c2> , <http://vocabulary.semantic-web.at/cocktails/5d96c50c-ee48-4c40-bb4c-4b9a42d11de6> , <http://vocabulary.semantic-web.at/cocktails/7dede323-e986-4417-b723-c9c7a7fe82ba> , <http://vocabulary.semantic-web.at/cocktails/84bf281b-95ab-4e18-a6fa-2d5156387167> , <http://vocabulary.semantic-web.at/cocktails/8f09ee6f-d5b9-4b8a-aa17-b0665fae4e83> , <http://vocabulary.semantic-web.at/cocktails/c4339109-ae35-4be9-a7e8-b5dfd206e960> , <http://vocabulary.semantic-web.at/cocktails/e98ac9a3-64f3-4cc5-8d0d-cf8684b0e7d1> ;
	skos:prefLabel "Distilled beverage"@en ;
	skos:topConceptOf <http://vocabulary.semantic-web.at/cocktails/591cf89a-57af-49b8-9042-3fc77408c93e> .

<http://vocabulary.semantic-web.at/cocktails/40ab50e9-66f1-411b-8220-ef8f05273542> dcterms:contributor <http://localhost/user/blumauera> ;
	dcterms:created "2015-05-03T10:05:34Z"^^xsd:dateTime ;
	dcterms:creator <http://localhost/user/blumauera> ;
	dcterms:modified "2015-05-04T09:45:12Z"^^xsd:dateTime ;
	<http://schema.semantic-web.at/ppt/inScheme> <http://vocabulary.semantic-web.at/cocktails/8d052dfc-44bf-4985-8ce3-4564570a161b> ;
	<http://vocabulary.semantic-web.at/cocktail-ontology/consists-of> <http://vocabulary.semantic-web.at/cocktails/5d96c50c-ee48-4c40-bb4c-4b9a42d11de6> , <http://vocabulary.semantic-web.at/cocktails/7c831f82-c54d-4d31-ab40-97e1d6226cf2> , <http://vocabulary.semantic-web.at/cocktails/8dee4eba-b6c6-4d16-b8f2-8d6cc0d9436c> ;
	<http://vocabulary.semantic-web.at/cocktail-ontology/iba> <http://www.iba-world.com/index.php?option=com_content&id=201&Itemid=532> ;
	<http://vocabulary.semantic-web.at/cocktail-ontology/image> <http://upload.wikimedia.org/wikipedia/commons/thumb/c/c6/Negroni_served_in_Vancouver_BC.jpg/440px-Negroni_served_in_Vancouver_BC.jpg> ;
	<http://vocabulary.semantic-web.at/cocktail-ontology/preparation> "Stir into glass over ice, garnish and serve."@en ;
	<http://vocabulary.semantic-web.at/cocktail-ontology/served> "On the rocks; poured over ice"@en ;
	<http://vocabulary.semantic-web.at/cocktail-ontology/uses> <http://vocabulary.semantic-web.at/cocktails/2dce3576-2603-41f9-8dce-ab21f639c2a7> ;
	<http://vocabulary.semantic-web.at/cocktail-ontology/uses_2> <http://vocabulary.semantic-web.at/cocktails/99171f20-c59f-40c4-998a-a9c8f1909168> ;
	a <http://vocabulary.semantic-web.at/cocktail-ontology/Cocktail> , skos:Concept ;
	skos:altLabel "Negroni (cocktail)"@en , "Negroni cocktail"@en ;
	skos:broader <http://vocabulary.semantic-web.at/cocktails/caae2ea0-7e60-400b-a2bb-14ef79720668> ;
	skos:definition "The Negroni cocktail is made of one part gin, one part vermouth rosso (red, semi-sweet), and one part bitters, traditionally Campari. It is considered an apéritif."@en ;
	skos:exactMatch dbpedia:Negroni ;
	skos:prefLabel "Negroni"@en .

<http://vocabulary.semantic-web.at/cocktails/43111fc3-3b59-420c-a588-024cd2d33896> dcterms:contributor <http://localhost/user/blumauera> ;
	dcterms:created "2015-05-02T18:59:28Z"^^xsd:dateTime ;
	dcterms:creator <http://localhost/user/blumauera> ;
	dcterms:modified "2015-05-07T07:15:16Z"^^xsd:dateTime ;
	<http://schema.semantic-web.at/ppt/inScheme> <http://vocabulary.semantic-web.at/cocktails/8d052dfc-44bf-4985-8ce3-4564570a161b> ;
	<http://vocabulary.semantic-web.at/cocktail-ontology/consists-of> <http://vocabulary.semantic-web.at/cocktails/12da816f-8ad3-487d-b8f9-2190e4b3e1b8> , <http://vocabulary.semantic-web.at/cocktails/1439e6c3-a155-4c80-8a5d-723453b4d17e> , <http://vocabulary.semantic-web.at/cocktails/1be6ee21-daf9-4b15-847d-6acdb88f9104> , <http://vocabulary.semantic-web.at/cocktails/44d8b702-5261-4ce9-923c-50d2acb4e0de> , <http://vocabulary.semantic-web.at/cocktails/5c291fe9-6fdb-4939-930d-dacbc67171a5> , <http://vocabulary.semantic-web.at/cocktails/5d96c50c-ee48-4c40-bb4c-4b9a42d11de6> , <http://vocabulary.semantic-web.at/cocktails/88f5de3d-3de4-4a2f-9523-50bc7bb06600> , <http://vocabulary.semantic-web.at/cocktails/ced2e755-fe48-4d7b-86ab-6b39fe359a32> ;
	<http://vocabulary.semantic-web.at/cocktail-ontology/iba> <http://www.iba-world.com/index.php?option=com_content&id=236&Itemid=532> ;
	<http://vocabulary.semantic-web.at/cocktail-ontology/image> <http://upload.wikimedia.org/wikipedia/commons/thumb/4/44/Singapore_Sling.jpg/440px-Singapore_Sling.jpg> ;
	<http://vocabulary.semantic-web.at/cocktail-ontology/preparation> "Pour all ingredients into cocktail shaker filled with ice cubes. Shake well. Strain into highball glass. Garnish with pineapple and cocktail cherry."@en ;
	<http://vocabulary.semantic-web.at/cocktail-ontology/served> "Well shaken, with ice"@en ;
	<http://vocabulary.semantic-web.at/cocktail-ontology/uses> <http://vocabulary.semantic-web.at/cocktails/a54d2096-6214-4006-beaf-afcc77824710> ;
	<http://vocabulary.semantic-web.at/cocktail-ontology/uses_2> <http://vocabulary.semantic-web.at/cocktails/8a5e1790-d3c0-432e-bb85-709692b14f03> , <http://vocabulary.semantic-web.at/cocktails/f9d7d22d-5d57-434a-b9e1-b9c8cde324e9> ;
	a <http://vocabulary.semantic-web.at/cocktail-ontology/Cocktail> , skos:Concept ;
	skos:altLabel "Gin sling"@en , "Gin slings"@en ;
	skos:broader <http://vocabulary.semantic-web.at/cocktails/54702498-ad42-4af6-b28a-2276215450da> , <http://vocabulary.semantic-web.at/cocktails/b9bf3799-a4e4-47f7-9aea-7697cc998a34> ;
	skos:definition "The Singapore Sling is a South-East Asian cocktail. This long drink was developed sometime before 1915 by Ngiam Tong Boon, a Hainanese bartender working at the Long Bar in Raffles Hotel Singapore. It was initially called the gin sling, - a sling was originally an American drink composed of spirit and water, sweetened and flavoured. D. A. Embury stated in the Fine Art of Mixing Drinks: \"Of all the recipes published for [this drink] I have never seen any two that were alike."@en ;
	skos:exactMatch dbpedia:Singapore_Sling ;
	skos:prefLabel "Singapore Sling"@en .

<http://vocabulary.semantic-web.at/cocktails/43b786b6-a1f1-4b7f-a5d9-be43d386ffb4> dcterms:contributor <http://localhost/user/blumauera> ;
	dcterms:created "2015-05-02T19:28:15Z"^^xsd:dateTime ;
	dcterms:creator <http://localhost/user/blumauera> ;
	dcterms:modified "2016-08-04T14:11:16Z"^^xsd:dateTime ;
	<http://schema.semantic-web.at/ppt/inScheme> <http://vocabulary.semantic-web.at/cocktails/8d052dfc-44bf-4985-8ce3-4564570a161b> ;
	<http://vocabulary.semantic-web.at/cocktail-ontology/consists-of> <http://vocabulary.semantic-web.at/cocktails/5c291fe9-6fdb-4939-930d-dacbc67171a5> , <http://vocabulary.semantic-web.at/cocktails/71210bd1-3071-4533-8da4-fe0f7d7694a0> , <http://vocabulary.semantic-web.at/cocktails/98f20476-57d7-46d3-b76d-6aac18b57788> , <http://vocabulary.semantic-web.at/cocktails/9c2ce399-c6ae-4f4d-bf37-7fd8ffe2a19d> , <http://vocabulary.semantic-web.at/cocktails/d9f071c0-8c44-43d1-9e4f-eef5709f5d98> ;
	<http://vocabulary.semantic-web.at/cocktail-ontology/iba> <http://www.iba-world.com/index.php?option=com_content&id=246&Itemid=532> ;
	<http://vocabulary.semantic-web.at/cocktail-ontology/image> <http://upload.wikimedia.org/wikipedia/commons/thumb/2/27/Pisco_sour_20100613b.JPG/440px-Pisco_sour_20100613b.JPG> ;
	<http://vocabulary.semantic-web.at/cocktail-ontology/preparation> "Shake and strain into a chilled champagne flute. Dash some Angostura bitters on top."@en ;
	<http://vocabulary.semantic-web.at/cocktail-ontology/uses> <http://vocabulary.semantic-web.at/cocktails/2dce3576-2603-41f9-8dce-ab21f639c2a7> ;
	a <http://vocabulary.semantic-web.at/cocktail-ontology/Cocktail> , skos:Concept ;
	skos:broader <http://vocabulary.semantic-web.at/cocktails/7516b400-963a-4151-8fdc-f6b23bad1dd5> , <http://vocabulary.semantic-web.at/cocktails/ccee1079-43df-4ff1-bef0-d15d3dc8fa6f> ;
	skos:definition "A Pisco Sour is a cocktail typical of western South American cuisine. The drink's name is a combination of the word Pisco, its base liquor, and the term sour (in reference to a lime juice and sweetener components). The Peruvian Pisco Sour requires the use of Peruvian Pisco as the base liquor and the addition of lime (or lemon) juice, syrup, ice, egg white, and Angostura bitters. The Chilean version is similar, but uses Chilean Pisco, sugar instead of syrup, and excludes the bitters."@en ;
	skos:exactMatch dbpedia:Pisco_Sour ;
	skos:prefLabel "Pisco Sour"@en .

<http://vocabulary.semantic-web.at/cocktails/441a0d9e-f4e1-434a-9cb4-503bb840e23a> dcterms:contributor <http://localhost/user/blumauera> ;
	dcterms:created "2015-05-05T07:17:54Z"^^xsd:dateTime ;
	dcterms:creator <http://localhost/user/blumauera> ;
	dcterms:modified "2015-05-05T07:18:05Z"^^xsd:dateTime ;
	<http://schema.semantic-web.at/ppt/inScheme> <http://vocabulary.semantic-web.at/cocktails/591cf89a-57af-49b8-9042-3fc77408c93e> ;
	<http://schema.semantic-web.at/ppt/inSubtree> <http://vocabulary.semantic-web.at/cocktails/e86c1671-4a67-494b-ae5d-bcb750865acc> ;
	<http://vocabulary.semantic-web.at/cocktail-ontology/is-part-of> <http://vocabulary.semantic-web.at/cocktails/11d68913-3a30-4591-bc41-25fea3f38520> ;
	a <http://vocabulary.semantic-web.at/cocktail-ontology/Beverages> , <http://vocabulary.semantic-web.at/cocktail-ontology/Ingredients> , <http://vocabulary.semantic-web.at/cocktail-ontology/Non-alcoholic-Beverages> , skos:Concept ;
	skos:broader <http://vocabulary.semantic-web.at/cocktails/6c0607a9-410d-4b65-87a1-b189a8e36352> ;
	skos:prefLabel "Olive juice"@en .

<http://vocabulary.semantic-web.at/cocktails/44cc99c1-28ac-4c50-a55d-7244b2c5c07b> dcterms:contributor <http://localhost/user/blumauera> ;
	dcterms:created "2015-05-01T14:21:50Z"^^xsd:dateTime ;
	dcterms:creator <http://localhost/user/blumauera> ;
	dcterms:modified "2015-05-03T10:42:03Z"^^xsd:dateTime ;
	<http://schema.semantic-web.at/ppt/inScheme> <http://vocabulary.semantic-web.at/cocktails/8d052dfc-44bf-4985-8ce3-4564570a161b> ;
	<http://vocabulary.semantic-web.at/cocktail-ontology/consists-of> <http://vocabulary.semantic-web.at/cocktails/224b4628-2f46-44a1-9d2f-8b5ef0b31e79> , <http://vocabulary.semantic-web.at/cocktails/5d96c50c-ee48-4c40-bb4c-4b9a42d11de6> , <http://vocabulary.semantic-web.at/cocktails/809f470a-4be7-47e8-9356-cb71009c31c2> , <http://vocabulary.semantic-web.at/cocktails/9c2ce399-c6ae-4f4d-bf37-7fd8ffe2a19d> ;
	<http://vocabulary.semantic-web.at/cocktail-ontology/iba> <http://www.iba-world.com/index.php?option=com_content&id=191&Itemid=532> ;
	<http://vocabulary.semantic-web.at/cocktail-ontology/image> <http://www.iba-world.com/images/cocktail_drinks/casino.jpg> ;
	<http://vocabulary.semantic-web.at/cocktail-ontology/preparation> "Pour all ingredients into shaker with ice cubes. Shake well. Strain into chilled cocktail glass. Garnish with a lemon twist and a maraschino cherry. Serve without a straw."@en ;
	<http://vocabulary.semantic-web.at/cocktail-ontology/served> "Straight up; without ice"@en ;
	<http://vocabulary.semantic-web.at/cocktail-ontology/uses> <http://vocabulary.semantic-web.at/cocktails/19dee0d8-fd30-469f-9ecd-91c902ff717c> ;
	<http://vocabulary.semantic-web.at/cocktail-ontology/uses_2> <http://vocabulary.semantic-web.at/cocktails/33df103a-03ac-4177-b620-7953fe094236> , <http://vocabulary.semantic-web.at/cocktails/8a5e1790-d3c0-432e-bb85-709692b14f03> ;
	a <http://vocabulary.semantic-web.at/cocktail-ontology/Cocktail> , skos:Concept ;
	skos:broader <http://vocabulary.semantic-web.at/cocktails/caae2ea0-7e60-400b-a2bb-14ef79720668> ;
	skos:definition "The Casino is an IBA official cocktail made with gin, maraschino liqueur, orange bitters and fresh lemon juice."@en ;
	skos:prefLabel "Casino"@en .

<http://vocabulary.semantic-web.at/cocktails/44d8b702-5261-4ce9-923c-50d2acb4e0de> dcterms:contributor <http://localhost/user/blumauera> ;
	dcterms:created "2015-05-02T19:01:02Z"^^xsd:dateTime ;
	dcterms:creator <http://localhost/user/blumauera> ;
	dcterms:modified "2015-05-07T07:13:39Z"^^xsd:dateTime ;
	<http://schema.semantic-web.at/ppt/inScheme> <http://vocabulary.semantic-web.at/cocktails/591cf89a-57af-49b8-9042-3fc77408c93e> ;
	<http://schema.semantic-web.at/ppt/inSubtree> <http://vocabulary.semantic-web.at/cocktails/403d1249-f37f-4f43-bebf-8dde9677d886> ;
	<http://vocabulary.semantic-web.at/cocktail-ontology/is-part-of> <http://vocabulary.semantic-web.at/cocktails/43111fc3-3b59-420c-a588-024cd2d33896> ;
	a <http://vocabulary.semantic-web.at/cocktail-ontology/Alcoholic-Beverages> , <http://vocabulary.semantic-web.at/cocktail-ontology/Beverages> , <http://vocabulary.semantic-web.at/cocktail-ontology/Ingredients> , skos:Concept ;
	skos:altLabel "Benedictine (liqueur)"@en , "Benedictine (liquor)"@en , "Benedictine liqueur"@en , "Dom Benedictine"@en ;
	skos:broader <http://vocabulary.semantic-web.at/cocktails/917d78d0-0938-4fe0-80c4-cfd2eb16e6a4> ;
	skos:definition "Bénédictine is an herbal liqueur beverage developed by Alexandre Le Grand in the 19th century and produced in France. It is claimed that at the Benedictine Abbey of Fécamp in Normandy, monks had developed a medicinal aromatic herbal beverage which was produced until the abbey's devastation during the French Revolution, but in fact Alexandre Le Grand invented the recipe himself, helped by a local chemist, and he told this story to connect the liqueur with the city history to increase sales."@en ;
	skos:exactMatch dbpedia:B%C3%A9n%C3%A9dictine ;
	skos:prefLabel "Bénédictine"@en .

<http://vocabulary.semantic-web.at/cocktails/45234a8f-9357-49d2-931b-638c48e3772e> dcterms:contributor <http://localhost/user/blumauera> ;
	dcterms:created "2015-05-01T07:58:26Z"^^xsd:dateTime ;
	dcterms:creator <http://localhost/user/blumauera> ;
	dcterms:modified "2015-05-07T07:11:26Z"^^xsd:dateTime ;
	<http://schema.semantic-web.at/ppt/inScheme> <http://vocabulary.semantic-web.at/cocktails/591cf89a-57af-49b8-9042-3fc77408c93e> ;
	<http://schema.semantic-web.at/ppt/inSubtree> <http://vocabulary.semantic-web.at/cocktails/e86c1671-4a67-494b-ae5d-bcb750865acc> ;
	<http://vocabulary.semantic-web.at/cocktail-ontology/is-part-of> <http://vocabulary.semantic-web.at/cocktails/12f4790a-560f-4e1c-b57a-53b8171ae39a> , <http://vocabulary.semantic-web.at/cocktails/4f85cadd-4fd4-4ffc-a78d-cddb0763fa4b> , <http://vocabulary.semantic-web.at/cocktails/dff0a7f4-ded0-48d5-bd31-881b70fbe36a> ;
	a <http://vocabulary.semantic-web.at/cocktail-ontology/Beverages> , <http://vocabulary.semantic-web.at/cocktail-ontology/Ingredients> , <http://vocabulary.semantic-web.at/cocktail-ontology/Non-alcoholic-Beverages> , skos:Concept ;
	skos:altLabel "Cranberry juice cocktail"@en ;
	skos:broader <http://vocabulary.semantic-web.at/cocktails/6c0607a9-410d-4b65-87a1-b189a8e36352> ;
	skos:definition "Cranberry juice is the juice of the cranberry. As a pure juice, it is quite tart; as with lime juice, it is not intended as a drink on its own. One solution is to combine it with sweeter juices, such as apple or grape. Another solution is to dilute it with water and add some sweetener, such as corn syrup or sugar, or artificial sweetener. The term, used on its own, almost always refers to a sweetened version."@en ;
	skos:exactMatch dbpedia:Cranberry_juice ;
	skos:prefLabel "Cranberry juice"@en .

<http://vocabulary.semantic-web.at/cocktails/45788a96-1fde-486b-80fc-31ad243bba31> dcterms:contributor <http://localhost/user/blumauera> ;
	dcterms:created "2015-05-02T17:11:07Z"^^xsd:dateTime ;
	dcterms:creator <http://localhost/user/blumauera> ;
	dcterms:modified "2015-05-06T12:55:21Z"^^xsd:dateTime ;
	<http://schema.semantic-web.at/ppt/inScheme> <http://vocabulary.semantic-web.at/cocktails/8d052dfc-44bf-4985-8ce3-4564570a161b> ;
	<http://vocabulary.semantic-web.at/cocktail-ontology/consists-of> <http://vocabulary.semantic-web.at/cocktails/a1c1e015-91fd-4f6e-b2a8-5edae9aa0b9d> , <http://vocabulary.semantic-web.at/cocktails/f0bfda32-3c42-457f-b6a3-bbf2a9e77b06> ;
	<http://vocabulary.semantic-web.at/cocktail-ontology/iba> <http://www.iba-world.com/index.php?option=com_content&id=266&Itemid=532> ;
	<http://vocabulary.semantic-web.at/cocktail-ontology/image> <http://upload.wikimedia.org/wikipedia/commons/thumb/8/80/Godfather_cocktail.jpg/440px-Godfather_cocktail.jpg> ;
	<http://vocabulary.semantic-web.at/cocktail-ontology/preparation> "Pour all ingredients directly into old fashioned glass filled with ice cubes. Stir gently."@en ;
	<http://vocabulary.semantic-web.at/cocktail-ontology/served> "On the rocks; poured over ice"@en ;
	<http://vocabulary.semantic-web.at/cocktail-ontology/uses> <http://vocabulary.semantic-web.at/cocktails/2dce3576-2603-41f9-8dce-ab21f639c2a7> ;
	a <http://vocabulary.semantic-web.at/cocktail-ontology/Cocktail> , skos:Concept ;
	skos:altLabel "God Father"@en ;
	skos:broader <http://vocabulary.semantic-web.at/cocktails/87cf1079-05d6-44da-acbe-c94b3ba52bd7> , <http://vocabulary.semantic-web.at/cocktails/b9bf3799-a4e4-47f7-9aea-7697cc998a34> ;
	skos:definition "The Godfather is a cocktail made of 35 mL scotch whisky and 35 mL amaretto. Typically, the liquids are poured into an old fashioned glass."@en ;
	skos:exactMatch <http://dbpedia.org/resource/Godfather_(cocktail)> ;
	skos:prefLabel "Godfather"@en ;
	skos:related <http://vocabulary.semantic-web.at/cocktails/c8f4f6bd-4ac1-456a-a3aa-595e4b93d979> .

<http://vocabulary.semantic-web.at/cocktails/457aff50-b86b-4879-8e17-41ca59cf03a7> dcterms:contributor <http://localhost/user/blumauera> ;
	dcterms:created "2015-05-02T07:16:53Z"^^xsd:dateTime ;
	dcterms:creator <http://localhost/user/blumauera> ;
	dcterms:modified "2015-07-02T14:56:10Z"^^xsd:dateTime ;
	<http://schema.semantic-web.at/ppt/inScheme> <http://vocabulary.semantic-web.at/cocktails/87384ce8-f20a-4201-b06d-3e0b8d832e5d> ;
	<http://vocabulary.semantic-web.at/cocktail-ontology/is-part-of> <http://vocabulary.semantic-web.at/cocktails/76c0e55c-22df-4489-9551-4fe8a6a649f8> , <http://vocabulary.semantic-web.at/cocktails/ce8f4591-ccd4-4d90-a761-244115d64061> ;
	a <http://vocabulary.semantic-web.at/cocktail-ontology/Ingredients> , skos:Concept ;
	skos:altLabel "Gum syrup"@en ;
	skos:broader <http://vocabulary.semantic-web.at/cocktails/0e385475-f369-4832-b8e3-20f35028988d> ;
	skos:prefLabel "Gomme syrup"@en .

<http://vocabulary.semantic-web.at/cocktails/469959a3-10dc-4539-80ff-08bf9ff2de1c> dcterms:contributor <http://localhost/user/blumauera> ;
	dcterms:created "2015-05-01T08:10:13Z"^^xsd:dateTime ;
	dcterms:creator <http://localhost/user/blumauera> ;
	dcterms:modified "2015-05-05T13:03:47Z"^^xsd:dateTime ;
	<http://schema.semantic-web.at/ppt/inScheme> <http://vocabulary.semantic-web.at/cocktails/eff672ac-6601-42c6-a3e9-0adda3b45df8> ;
	<http://schema.semantic-web.at/ppt/propagateType> <http://vocabulary.semantic-web.at/cocktail-ontology/Ingredients> ;
	a <http://vocabulary.semantic-web.at/cocktail-ontology/Garnish> , <http://vocabulary.semantic-web.at/cocktail-ontology/Ingredients> , skos:Concept ;
	skos:narrower <http://vocabulary.semantic-web.at/cocktails/1ca477d1-98d5-4a16-82e2-a4b07c34fdbe> , <http://vocabulary.semantic-web.at/cocktails/805e18b6-0f7a-4c26-b35e-9cc68a099086> , <http://vocabulary.semantic-web.at/cocktails/91b112c0-2fcc-4495-b68c-b1f09fa0a698> , <http://vocabulary.semantic-web.at/cocktails/cb1bb8c3-5013-4c5f-80e3-5267367fe2fb> , <http://vocabulary.semantic-web.at/cocktails/e2d63a1c-56e7-47d2-b01b-8cf88cac3d8b> , <http://vocabulary.semantic-web.at/cocktails/e76e4e97-260a-4eef-af34-111938241931> , <http://vocabulary.semantic-web.at/cocktails/f159e33f-fed0-4382-93b9-acfa28f23937> ;
	skos:prefLabel "Herbs and spices"@en ;
	skos:topConceptOf <http://vocabulary.semantic-web.at/cocktails/eff672ac-6601-42c6-a3e9-0adda3b45df8> .

<http://vocabulary.semantic-web.at/cocktails/47635419-edef-4b78-8da1-e58a96d96f61> dcterms:contributor <http://localhost/user/blumauera> ;
	dcterms:created "2015-05-02T19:07:54Z"^^xsd:dateTime ;
	dcterms:creator <http://localhost/user/blumauera> ;
	dcterms:modified "2015-05-02T19:08:51Z"^^xsd:dateTime ;
	<http://schema.semantic-web.at/ppt/inScheme> <http://vocabulary.semantic-web.at/cocktails/591cf89a-57af-49b8-9042-3fc77408c93e> ;
	<http://schema.semantic-web.at/ppt/inSubtree> <http://vocabulary.semantic-web.at/cocktails/403d1249-f37f-4f43-bebf-8dde9677d886> ;
	a <http://vocabulary.semantic-web.at/cocktail-ontology/Alcoholic-Beverages> , <http://vocabulary.semantic-web.at/cocktail-ontology/Beverages> , <http://vocabulary.semantic-web.at/cocktail-ontology/Ingredients> , skos:Concept ;
	skos:altLabel "Creme liqueur"@en , "Creme liqueurs"@en , "Crème liqueurs"@en ;
	skos:broader <http://vocabulary.semantic-web.at/cocktails/2944baef-5338-421b-a5f5-0e51f75244c2> ;
	skos:definition "A crème liqueur (not to be confused with cream liqueur) is a liqueur that has a great deal of additional sugar added to the point that it has a near-syrup consistency. Unlike cream liqueurs, crème liqueurs include no cream in their ingredients. \"Crème\" in this case refers to the consistency. This category includes crème de cacao (chocolate), crème de menthe (mint), crème de mûre (blackberry), and crème de cassis (black currant)."@en ;
	skos:exactMatch dbpedia:Cr%C3%A8me_liqueur ;
	skos:narrower <http://vocabulary.semantic-web.at/cocktails/2d7c2c72-a6a1-43ef-9175-02885fcf4518> , <http://vocabulary.semantic-web.at/cocktails/687a5d86-1f4e-4a6b-b5ca-3b5d74aeafcc> , <http://vocabulary.semantic-web.at/cocktails/8352ad8c-0355-4ca4-9ff7-c3dff28931c5> , <http://vocabulary.semantic-web.at/cocktails/e406119b-7637-43f9-9a62-5a8ea500ebc4> , <http://vocabulary.semantic-web.at/cocktails/f4da82d8-eaf5-451f-824c-05564bc48816> ;
	skos:prefLabel "Crème liqueur"@en .

<http://vocabulary.semantic-web.at/cocktails/4792b0b8-0046-47ca-8c2a-f3ad58922182> dcterms:contributor <http://localhost/user/blumauera> ;
	dcterms:created "2015-05-02T18:44:31Z"^^xsd:dateTime ;
	dcterms:creator <http://localhost/user/blumauera> ;
	dcterms:modified "2015-05-07T07:06:23Z"^^xsd:dateTime ;
	<http://schema.semantic-web.at/ppt/inScheme> <http://vocabulary.semantic-web.at/cocktails/8d052dfc-44bf-4985-8ce3-4564570a161b> ;
	<http://vocabulary.semantic-web.at/cocktail-ontology/consists-of> <http://vocabulary.semantic-web.at/cocktails/12da816f-8ad3-487d-b8f9-2190e4b3e1b8> , <http://vocabulary.semantic-web.at/cocktails/26ca4892-5265-4ce6-875c-ef92348ff7a4> , <http://vocabulary.semantic-web.at/cocktails/f5cd2a2b-2153-4b7e-ae79-678b939765ca> ;
	<http://vocabulary.semantic-web.at/cocktail-ontology/iba> <http://www.iba-world.com/index.php?option=com_content&id=232&Itemid=532> ;
	<http://vocabulary.semantic-web.at/cocktail-ontology/image> <http://upload.wikimedia.org/wikipedia/commons/thumb/b/b2/Pi%C3%B1a_Colada.jpg/440px-Pi%C3%B1a_Colada.jpg> ;
	<http://vocabulary.semantic-web.at/cocktail-ontology/preparation> "Mix with crushed ice until smooth. Pour into chilled glass, garnish and serve."@en ;
	<http://vocabulary.semantic-web.at/cocktail-ontology/served> "Blended with ice (frozen style)"@en ;
	<http://vocabulary.semantic-web.at/cocktail-ontology/uses> <http://vocabulary.semantic-web.at/cocktails/22c81328-d483-4c62-8338-cb732ee39734> ;
	<http://vocabulary.semantic-web.at/cocktail-ontology/uses_2> <http://vocabulary.semantic-web.at/cocktails/62fbc16f-3f84-4cc7-8c6f-5afebfc1510a> , <http://vocabulary.semantic-web.at/cocktails/f9d7d22d-5d57-434a-b9e1-b9c8cde324e9> ;
	a <http://vocabulary.semantic-web.at/cocktail-ontology/Cocktail> , skos:Concept ;
	skos:altLabel "Peanut Colada"@en , "Pina Colada"@en , "Pina colada"@en , "Pina coladas"@en , "Pina colata"@en , "Pina collada"@en , "Pinacolada"@en , "Piña coladas"@en , "Virgin Pina Colada"@en , "Virgin Piña Colada"@en , "Virgin pina colada"@en ;
	skos:broader <http://vocabulary.semantic-web.at/cocktails/b9bf3799-a4e4-47f7-9aea-7697cc998a34> ;
	skos:definition "The piña colada is a sweet, rum-based cocktail made with rum, cream of coconut, and pineapple juice, usually served either blended or shaken with ice. It may be garnished with a pineapple wedge, a maraschino cherry or both. The piña colada has been the official beverage of Puerto Rico since 1978."@en ;
	skos:exactMatch dbpedia:Pi%C3%B1a_colada ;
	skos:prefLabel "Piña colada"@en .

<http://vocabulary.semantic-web.at/cocktails/47c10a33-a7b2-44f5-9614-2bca65cff2fd> dcterms:contributor <http://localhost/user/blumauera> ;
	dcterms:created "2015-05-01T15:05:54Z"^^xsd:dateTime ;
	dcterms:creator <http://localhost/user/blumauera> ;
	dcterms:modified "2015-05-04T11:26:03Z"^^xsd:dateTime ;
	<http://schema.semantic-web.at/ppt/inScheme> <http://vocabulary.semantic-web.at/cocktails/591cf89a-57af-49b8-9042-3fc77408c93e> ;
	<http://schema.semantic-web.at/ppt/inSubtree> <http://vocabulary.semantic-web.at/cocktails/e86c1671-4a67-494b-ae5d-bcb750865acc> ;
	<http://vocabulary.semantic-web.at/cocktail-ontology/is-part-of> <http://vocabulary.semantic-web.at/cocktails/c151ee28-45d2-4128-8587-1f1b69060d9d> ;
	a <http://vocabulary.semantic-web.at/cocktail-ontology/Beverages> , <http://vocabulary.semantic-web.at/cocktail-ontology/Ingredients> , <http://vocabulary.semantic-web.at/cocktail-ontology/Non-alcoholic-Beverages> , skos:Concept ;
	skos:altLabel "Orange blossom water"@en ;
	skos:broader <http://vocabulary.semantic-web.at/cocktails/204c40af-075d-4bf6-a54e-33a60c54ac35> ;
	skos:definition "Orange flower water, or orange blossom water, is a clear, perfumed distillation of fresh bitter-orange blossoms. This essential water has traditionally been used in many French and Mediterranean dessert dishes, such as the gibassier and pompe à l'huile, but has more recently found its way into Western cuisine."@en ;
	skos:exactMatch dbpedia:Orange_flower_water ;
	skos:prefLabel "Orange flower water"@en .

<http://vocabulary.semantic-web.at/cocktails/48499a53-a687-4156-b966-1e16e3e967bd> dcterms:contributor <http://localhost/user/blumauera> ;
	dcterms:created "2015-05-02T07:31:11Z"^^xsd:dateTime ;
	dcterms:creator <http://localhost/user/blumauera> ;
	dcterms:modified "2015-05-06T12:29:32Z"^^xsd:dateTime ;
	<http://schema.semantic-web.at/ppt/inScheme> <http://vocabulary.semantic-web.at/cocktails/591cf89a-57af-49b8-9042-3fc77408c93e> ;
	<http://schema.semantic-web.at/ppt/inSubtree> <http://vocabulary.semantic-web.at/cocktails/e86c1671-4a67-494b-ae5d-bcb750865acc> ;
	<http://vocabulary.semantic-web.at/cocktail-ontology/is-part-of> <http://vocabulary.semantic-web.at/cocktails/268fb62f-8ef1-45cd-844f-8c7da85a6a0b> , <http://vocabulary.semantic-web.at/cocktails/a5db05ca-eda3-41ef-a8ab-ba77b3e4baba> ;
	a <http://vocabulary.semantic-web.at/cocktail-ontology/Beverages> , <http://vocabulary.semantic-web.at/cocktail-ontology/Ingredients> , <http://vocabulary.semantic-web.at/cocktail-ontology/Non-alcoholic-Beverages> , skos:Concept ;
	skos:broader <http://vocabulary.semantic-web.at/cocktails/6c0607a9-410d-4b65-87a1-b189a8e36352> ;
	skos:definition "Tomato juice is a juice made from tomatoes. It is usually used as a beverage, either plain or in cocktails such as a Bloody Mary or Michelada."@en ;
	skos:exactMatch dbpedia:Tomato_juice ;
	skos:prefLabel "Tomato juice"@en .

<http://vocabulary.semantic-web.at/cocktails/498283e1-6a11-43f0-b6ae-d04aea796285> dcterms:created "2016-03-09T17:26:29Z"^^xsd:dateTime ;
	dcterms:creator <http://localhost/user/blumauera> ;
	<http://schema.semantic-web.at/ppt/inScheme> <http://vocabulary.semantic-web.at/cocktails/591cf89a-57af-49b8-9042-3fc77408c93e> ;
	<http://schema.semantic-web.at/ppt/inSubtree> <http://vocabulary.semantic-web.at/cocktails/e86c1671-4a67-494b-ae5d-bcb750865acc> ;
	a <http://vocabulary.semantic-web.at/cocktail-ontology/Beverages> , <http://vocabulary.semantic-web.at/cocktail-ontology/Ingredients> , <http://vocabulary.semantic-web.at/cocktail-ontology/Non-alcoholic-Beverages> , skos:Concept ;
	skos:broader <http://vocabulary.semantic-web.at/cocktails/b6ce7a37-ceda-4e8c-86a0-fe7bc5fd0908> ;
	skos:narrower <http://vocabulary.semantic-web.at/cocktails/5238edc3-0873-4be5-8197-56c867dcc589> ;
	skos:prefLabel "dairy"@en .

<http://vocabulary.semantic-web.at/cocktails/4be1257b-f797-4ab9-a2b3-af09b958173e> dcterms:contributor <http://localhost/user/blumauera> ;
	dcterms:created "2015-05-02T17:13:21Z"^^xsd:dateTime ;
	dcterms:creator <http://localhost/user/blumauera> ;
	dcterms:modified "2015-05-07T06:34:31Z"^^xsd:dateTime ;
	<http://schema.semantic-web.at/ppt/inScheme> <http://vocabulary.semantic-web.at/cocktails/591cf89a-57af-49b8-9042-3fc77408c93e> ;
	<http://schema.semantic-web.at/ppt/inSubtree> <http://vocabulary.semantic-web.at/cocktails/403d1249-f37f-4f43-bebf-8dde9677d886> ;
	<http://vocabulary.semantic-web.at/cocktail-ontology/is-part-of> <http://vocabulary.semantic-web.at/cocktails/0f8cc862-9056-49be-b636-cd22f8d7282d> , <http://vocabulary.semantic-web.at/cocktails/13b85b5c-7f69-4871-bb08-3cd5281f6039> , <http://vocabulary.semantic-web.at/cocktails/4d15a643-f7c7-4ee5-8f56-4ebd2bcf74b5> , <http://vocabulary.semantic-web.at/cocktails/b970d408-39ca-49b0-98fc-838f96c94608> ;
	a <http://vocabulary.semantic-web.at/cocktail-ontology/Alcoholic-Beverages> , <http://vocabulary.semantic-web.at/cocktail-ontology/Beverages> , <http://vocabulary.semantic-web.at/cocktail-ontology/Ingredients> , skos:Concept ;
	skos:altLabel "Galliano (drink)"@en , "Liquore Galliano"@en ;
	skos:broader <http://vocabulary.semantic-web.at/cocktails/917d78d0-0938-4fe0-80c4-cfd2eb16e6a4> ;
	skos:definition "Liquore Galliano L'Autentico, known more commonly as Galliano, is a sweet herbal liqueur, created in 1896 by Italian distiller and brandy producer Arturo Vaccari of Livorno, Tuscany and named after Giuseppe Galliano, an Italian hero of the First Italo–Ethiopian War. Its vivid yellow color symbolizes the Gold Rushes of the 1890s. Galliano has a large number of natural ingredients including vanilla, star anise, Mediterranean anise, ginger, citrus, juniper, musk yarrow, and lavender."@en ;
	skos:exactMatch <http://dbpedia.org/resource/Galliano_(liqueur)> ;
	skos:prefLabel "Galliano"@en .

<http://vocabulary.semantic-web.at/cocktails/4c6a85a7-de2a-42a9-9664-3279e53bac48> a skos:Concept ;
	skos:broader <http://vocabulary.semantic-web.at/cocktails/2944baef-5338-421b-a5f5-0e51f75244c2> ;
	skos:prefLabel "Calvados"@en .

<http://vocabulary.semantic-web.at/cocktails/4d15a643-f7c7-4ee5-8f56-4ebd2bcf74b5> dcterms:contributor <http://localhost/user/blumauera> ;
	dcterms:created "2015-05-02T19:04:05Z"^^xsd:dateTime ;
	dcterms:creator <http://localhost/user/blumauera> ;
	dcterms:modified "2015-05-05T07:27:07Z"^^xsd:dateTime ;
	<http://schema.semantic-web.at/ppt/inScheme> <http://vocabulary.semantic-web.at/cocktails/8d052dfc-44bf-4985-8ce3-4564570a161b> ;
	<http://vocabulary.semantic-web.at/cocktail-ontology/consists-of> <http://vocabulary.semantic-web.at/cocktails/12da816f-8ad3-487d-b8f9-2190e4b3e1b8> , <http://vocabulary.semantic-web.at/cocktails/4be1257b-f797-4ab9-a2b3-af09b958173e> , <http://vocabulary.semantic-web.at/cocktails/88f5de3d-3de4-4a2f-9523-50bc7bb06600> , <http://vocabulary.semantic-web.at/cocktails/a293047d-788b-4e8c-96bc-65e62fec4b0b> , <http://vocabulary.semantic-web.at/cocktails/e98ac9a3-64f3-4cc5-8d0d-cf8684b0e7d1> ;
	<http://vocabulary.semantic-web.at/cocktail-ontology/iba> <http://www.iba-world.com/index.php?option=com_content&id=238&Itemid=532> ;
	<http://vocabulary.semantic-web.at/cocktail-ontology/image> <http://www.iba-world.com/images/cocktail_drinks/baracuda.jpg> ;
	<http://vocabulary.semantic-web.at/cocktail-ontology/preparation> "Pour all ingredients except the wine in a chilled glass. Top with the sparkling wine."@en ;
	<http://vocabulary.semantic-web.at/cocktail-ontology/uses> <http://vocabulary.semantic-web.at/cocktails/a54d2096-6214-4006-beaf-afcc77824710> ;
	a <http://vocabulary.semantic-web.at/cocktail-ontology/Cocktail> , skos:Concept ;
	skos:broader <http://vocabulary.semantic-web.at/cocktails/204cd4e7-58d7-4417-837a-7f9cc41663c8> , <http://vocabulary.semantic-web.at/cocktails/ccee1079-43df-4ff1-bef0-d15d3dc8fa6f> ;
	skos:prefLabel "Barracuda"@en .

<http://vocabulary.semantic-web.at/cocktails/4e27dba8-ce80-4246-ad19-14f72e628959> dcterms:created "2015-11-18T14:47:21Z"^^xsd:dateTime ;
	dcterms:creator <http://localhost/user/blumauera> ;
	<http://schema.semantic-web.at/ppt/inScheme> <http://vocabulary.semantic-web.at/cocktails/591cf89a-57af-49b8-9042-3fc77408c93e> ;
	<http://schema.semantic-web.at/ppt/inSubtree> <http://vocabulary.semantic-web.at/cocktails/403d1249-f37f-4f43-bebf-8dde9677d886> ;
	a <http://vocabulary.semantic-web.at/cocktail-ontology/Alcoholic-Beverages> , <http://vocabulary.semantic-web.at/cocktail-ontology/Beverages> , <http://vocabulary.semantic-web.at/cocktail-ontology/Ingredients> , skos:Concept ;
	skos:broader <http://vocabulary.semantic-web.at/cocktails/ec2452b9-849d-4750-8190-bc696f2271fa> ;
	skos:prefLabel "Fireball Cinnamon Whisky"@en .

<http://vocabulary.semantic-web.at/cocktails/4efda48d-6c56-47e5-bf98-bf8918ff58eb> dcterms:contributor <http://localhost/user/blumauera> ;
	dcterms:created "2015-11-18T14:32:32Z"^^xsd:dateTime ;
	dcterms:creator <http://localhost/user/blumauera> ;
	dcterms:modified "2015-11-18T14:37:17Z"^^xsd:dateTime ;
	<http://schema.semantic-web.at/ppt/inScheme> <http://vocabulary.semantic-web.at/cocktails/8d052dfc-44bf-4985-8ce3-4564570a161b> ;
	<http://vocabulary.semantic-web.at/cocktail-ontology/consists-of> <http://vocabulary.semantic-web.at/cocktails/5b272721-4eb2-41cd-9224-5963091fb639> , <http://vocabulary.semantic-web.at/cocktails/6420f3aa-5146-4893-b3ea-04033b26c915> , <http://vocabulary.semantic-web.at/cocktails/c96d576c-9640-4c21-af92-d6da3560c9d0> ;
	<http://vocabulary.semantic-web.at/cocktail-ontology/preparation> "Pour the absinthe in a shot glass. Float the Kummel on top using the back of  bar spoon. Using the same technique, layer the Goldschlager on top of this"@en ;
	<http://vocabulary.semantic-web.at/cocktail-ontology/uses> <http://vocabulary.semantic-web.at/cocktails/bfbfb9b6-4c70-4323-a64b-4cfd533c55d8> ;
	a <http://vocabulary.semantic-web.at/cocktail-ontology/Cocktail> , skos:Concept ;
	skos:broader <http://vocabulary.semantic-web.at/cocktails/b65b6d98-400f-47cf-94c7-d2566f10cf64> ;
	skos:definition "The Fireball is a German layered shot with a powerful punch and a green colour."@en ;
	skos:prefLabel "Fireball"@en .

<http://vocabulary.semantic-web.at/cocktails/4f03a6ef-9631-4b6d-a005-7fbbdcb9b342> dcterms:contributor <http://localhost/user/blumauera> ;
	dcterms:created "2015-05-01T14:43:03Z"^^xsd:dateTime ;
	dcterms:creator <http://localhost/user/blumauera> ;
	dcterms:modified "2015-05-06T12:21:25Z"^^xsd:dateTime ;
	<http://schema.semantic-web.at/ppt/inScheme> <http://vocabulary.semantic-web.at/cocktails/591cf89a-57af-49b8-9042-3fc77408c93e> ;
	<http://schema.semantic-web.at/ppt/inSubtree> <http://vocabulary.semantic-web.at/cocktails/403d1249-f37f-4f43-bebf-8dde9677d886> ;
	<http://vocabulary.semantic-web.at/cocktail-ontology/is-part-of> <http://vocabulary.semantic-web.at/cocktails/f632b16d-1490-4587-a637-fb393d7b1e7f> , <http://vocabulary.semantic-web.at/cocktails/fb278b46-3c67-48b0-b9eb-7ea037294f5f> ;
	a <http://vocabulary.semantic-web.at/cocktail-ontology/Alcoholic-Beverages> , <http://vocabulary.semantic-web.at/cocktail-ontology/Beverages> , <http://vocabulary.semantic-web.at/cocktail-ontology/Ingredients> , skos:Concept ;
	skos:altLabel "Rock and Rye"@en , "Rye Whisky"@en , "Rye whisky"@en ;
	skos:broader <http://vocabulary.semantic-web.at/cocktails/c4339109-ae35-4be9-a7e8-b5dfd206e960> ;
	skos:definition "Rye whiskey can refer to either of two types of whiskey: American rye whiskey, which must be distilled from at least 51 percent rye; Canadian whisky, which is often referred to (and labelled as) rye whisky for historical reasons, although it may or may not actually include any rye in its production process."@en ;
	skos:exactMatch dbpedia:Rye_whiskey ;
	skos:narrower <http://vocabulary.semantic-web.at/cocktails/4028ce28-b682-4c06-b861-010b25f488ca> ;
	skos:prefLabel "Rye whiskey"@en .

<http://vocabulary.semantic-web.at/cocktails/4f20d6bb-710d-4870-bde4-b6e835d7d13f> dcterms:contributor <http://localhost/user/blumauera> ;
	dcterms:created "2015-05-01T08:08:54Z"^^xsd:dateTime ;
	dcterms:creator <http://localhost/user/blumauera> ;
	dcterms:modified "2015-05-03T17:32:41Z"^^xsd:dateTime ;
	<http://schema.semantic-web.at/ppt/inScheme> <http://vocabulary.semantic-web.at/cocktails/eff672ac-6601-42c6-a3e9-0adda3b45df8> ;
	<http://schema.semantic-web.at/ppt/propagateType> <http://vocabulary.semantic-web.at/cocktail-ontology/Ingredients> ;
	a <http://vocabulary.semantic-web.at/cocktail-ontology/Garnish> , <http://vocabulary.semantic-web.at/cocktail-ontology/Ingredients> , skos:Concept ;
	skos:altLabel "Aggregated fruit"@en , "Bacca"@en , "Culture of fruits"@en , "Ethylene-ripened fruits"@en , "Friut"@en , "Fruiting"@en , "Fruiting Shrubs"@en , "Fruits"@en , "Fruity"@en , "Pod types"@en , "Prutas"@en , "Seed pod"@en , "Simple fruit"@en ;
	skos:definition "In botany, a fruit is a part of a flowering plant that derives from specific tissues of the flower, one or more ovaries, and in some cases accessory tissues. Fruits are the means by which these plants disseminate seeds."@en ;
	skos:exactMatch dbpedia:Fruit ;
	skos:narrower <http://vocabulary.semantic-web.at/cocktails/021c85c0-a60a-4414-8fd8-bd3383b794f1> , <http://vocabulary.semantic-web.at/cocktails/33df103a-03ac-4177-b620-7953fe094236> , <http://vocabulary.semantic-web.at/cocktails/3abfd580-0f7d-4971-9c90-3cc8a5dafc0c> , <http://vocabulary.semantic-web.at/cocktails/62fbc16f-3f84-4cc7-8c6f-5afebfc1510a> , <http://vocabulary.semantic-web.at/cocktails/78ace24b-5e26-42f8-9f4f-3106576118cc> , <http://vocabulary.semantic-web.at/cocktails/7c4a2cfe-6750-419a-87d1-dcb4919ff92b> , <http://vocabulary.semantic-web.at/cocktails/99171f20-c59f-40c4-998a-a9c8f1909168> , <http://vocabulary.semantic-web.at/cocktails/cec5e96c-41c6-4b82-ab3a-0a057a54f70a> , <http://vocabulary.semantic-web.at/cocktails/f9d7d22d-5d57-434a-b9e1-b9c8cde324e9> ;
	skos:prefLabel "Fruit"@en ;
	skos:topConceptOf <http://vocabulary.semantic-web.at/cocktails/eff672ac-6601-42c6-a3e9-0adda3b45df8> .

<http://vocabulary.semantic-web.at/cocktails/4f4bed20-5317-45f6-a070-f28267b6e961> dcterms:contributor <http://localhost/user/blumauera> ;
	dcterms:created "2015-05-02T17:22:34Z"^^xsd:dateTime ;
	dcterms:creator <http://localhost/user/blumauera> ;
	dcterms:modified "2015-05-07T06:49:06Z"^^xsd:dateTime ;
	<http://schema.semantic-web.at/ppt/inScheme> <http://vocabulary.semantic-web.at/cocktails/591cf89a-57af-49b8-9042-3fc77408c93e> ;
	<http://schema.semantic-web.at/ppt/inSubtree> <http://vocabulary.semantic-web.at/cocktails/e86c1671-4a67-494b-ae5d-bcb750865acc> ;
	<http://vocabulary.semantic-web.at/cocktail-ontology/is-part-of> <http://vocabulary.semantic-web.at/cocktails/c3b197cc-8583-4e2f-8e45-3a7fed1309c1> ;
	a <http://vocabulary.semantic-web.at/cocktail-ontology/Beverages> , <http://vocabulary.semantic-web.at/cocktail-ontology/Ingredients> , <http://vocabulary.semantic-web.at/cocktail-ontology/Non-alcoholic-Beverages> , skos:Concept ;
	skos:altLabel "Brazilian coffee"@en , "Cafe de Columbia"@en , "Caffé"@en , "Coffe"@en , "Coffee (drink)"@en , "Coffee Bags"@en , "Coffee brewing method"@en , "Coffee brews"@en , "Cup of Joe"@en , "Decaffinated Coffee"@en , "Decaffinated coffee"@en , "Gavaccino"@en , "Gourmet coffee"@en , "Hand picked coffee"@en , "Joe (coffee)"@en , "Kaffee"@en , "Kawha"@en , "Malabar (beans)"@en , "Raktajeno"@en , "Regular coffee"@en , "Roasted coffee"@en , "Specialty Coffees"@en , "Specialty coffees"@en , "Used coffee ground"@en , "Used coffee grounds"@en ;
	skos:broader <http://vocabulary.semantic-web.at/cocktails/e86c1671-4a67-494b-ae5d-bcb750865acc> ;
	skos:definition "Coffee is a brewed beverage with a distinct aroma and flavor, prepared from the roasted seeds of the Coffea plant. The seeds are found in coffee \"cherries\", which grow on trees cultivated in over 70 countries, primarily in equatorial Latin America, Southeast Asia, India and Africa. Green (unroasted) coffee is one of the most traded agricultural commodities in the world. Coffee is slightly acidic (pH 5.0–5.1) and can have a stimulating effect on humans because of its caffeine content."@en ;
	skos:exactMatch dbpedia:Coffee ;
	skos:narrower <http://vocabulary.semantic-web.at/cocktails/8ba9f3ab-d600-441c-85d3-d3aeb44678d1> ;
	skos:prefLabel "Coffee"@en .

<http://vocabulary.semantic-web.at/cocktails/4f85cadd-4fd4-4ffc-a78d-cddb0763fa4b> dcterms:contributor <http://localhost/user/blumauera> ;
	dcterms:created "2015-05-02T08:13:29Z"^^xsd:dateTime ;
	dcterms:creator <http://localhost/user/blumauera> ;
	dcterms:modified "2015-05-06T12:42:35Z"^^xsd:dateTime ;
	<http://schema.semantic-web.at/ppt/inScheme> <http://vocabulary.semantic-web.at/cocktails/8d052dfc-44bf-4985-8ce3-4564570a161b> ;
	<http://vocabulary.semantic-web.at/cocktail-ontology/consists-of> <http://vocabulary.semantic-web.at/cocktails/397d0ec3-98e2-47d9-a8c2-eca9702ff94d> , <http://vocabulary.semantic-web.at/cocktails/45234a8f-9357-49d2-931b-638c48e3772e> , <http://vocabulary.semantic-web.at/cocktails/88f5de3d-3de4-4a2f-9523-50bc7bb06600> , <http://vocabulary.semantic-web.at/cocktails/b6725284-f65d-4802-b79d-029c539a1580> ;
	<http://vocabulary.semantic-web.at/cocktail-ontology/iba> <http://www.iba-world.com/index.php?option=com_content&id=265&Itemid=532> ;
	<http://vocabulary.semantic-web.at/cocktail-ontology/image> <http://upload.wikimedia.org/wikipedia/commons/thumb/2/2b/Cosmo_drink.jpg/440px-Cosmo_drink.jpg> ;
	<http://vocabulary.semantic-web.at/cocktail-ontology/preparation> "Shake all ingredients in cocktail shaker filled with ice. Strain into a large cocktail glass Garnish with lime slice."@en ;
	<http://vocabulary.semantic-web.at/cocktail-ontology/served> "straight up"@en ;
	<http://vocabulary.semantic-web.at/cocktail-ontology/uses> <http://vocabulary.semantic-web.at/cocktails/19dee0d8-fd30-469f-9ecd-91c902ff717c> ;
	<http://vocabulary.semantic-web.at/cocktail-ontology/uses_2> <http://vocabulary.semantic-web.at/cocktails/021c85c0-a60a-4414-8fd8-bd3383b794f1> , <http://vocabulary.semantic-web.at/cocktails/33df103a-03ac-4177-b620-7953fe094236> ;
	a <http://vocabulary.semantic-web.at/cocktail-ontology/Cocktail> , skos:Concept ;
	skos:altLabel "Cosmo"@en , "Cosmopolitan (cocktail"@en , "Cosmopolitan (drink)"@en , "Cosmopolitan cocktail"@en ;
	skos:broader <http://vocabulary.semantic-web.at/cocktails/b9bf3799-a4e4-47f7-9aea-7697cc998a34> ;
	skos:definition "A cosmopolitan, or informally a cosmo, is a cocktail made with vodka, triple sec, cranberry juice, and freshly squeezed lime juice or sweetened lime juice."@en ;
	skos:exactMatch <http://dbpedia.org/resource/Cosmopolitan_(cocktail)> ;
	skos:prefLabel "Cosmopolitan"@en .

<http://vocabulary.semantic-web.at/cocktails/52117ab2-dcb8-4d28-a366-ddd932e58219> dcterms:contributor <http://localhost/user/blumauera> ;
	dcterms:created "2015-05-02T08:24:28Z"^^xsd:dateTime ;
	dcterms:creator <http://localhost/user/blumauera> ;
	dcterms:modified "2015-05-06T12:56:04Z"^^xsd:dateTime ;
	<http://schema.semantic-web.at/ppt/inScheme> <http://vocabulary.semantic-web.at/cocktails/8d052dfc-44bf-4985-8ce3-4564570a161b> ;
	<http://vocabulary.semantic-web.at/cocktail-ontology/consists-of> <http://vocabulary.semantic-web.at/cocktails/a1c1e015-91fd-4f6e-b2a8-5edae9aa0b9d> , <http://vocabulary.semantic-web.at/cocktails/fd76c5ab-be62-4c4b-a2c6-7fa9bc359f47> ;
	<http://vocabulary.semantic-web.at/cocktail-ontology/iba> <http://www.iba-world.com/index.php?option=com_content&id=269&Itemid=532> ;
	<http://vocabulary.semantic-web.at/cocktail-ontology/image> <http://www.iba-world.com/images/cocktail_drinks/french_connection.jpg> ;
	<http://vocabulary.semantic-web.at/cocktail-ontology/is-variant-of> <http://vocabulary.semantic-web.at/cocktails/45788a96-1fde-486b-80fc-31ad243bba31> ;
	<http://vocabulary.semantic-web.at/cocktail-ontology/preparation> "Pour all ingredients directly into old fashioned glass filled with ice cubes. Stir gently."@en ;
	<http://vocabulary.semantic-web.at/cocktail-ontology/served> "On the rocks; poured over ice"@en ;
	<http://vocabulary.semantic-web.at/cocktail-ontology/uses> <http://vocabulary.semantic-web.at/cocktails/2dce3576-2603-41f9-8dce-ab21f639c2a7> ;
	a <http://vocabulary.semantic-web.at/cocktail-ontology/Cocktail> , skos:Concept ;
	skos:broader <http://vocabulary.semantic-web.at/cocktails/87cf1079-05d6-44da-acbe-c94b3ba52bd7> , <http://vocabulary.semantic-web.at/cocktails/b9bf3799-a4e4-47f7-9aea-7697cc998a34> ;
	skos:definition "A French connection is a cocktail made with equal parts Cognac and Amaretto liqueur."@en ;
	skos:exactMatch <http://dbpedia.org/resource/French_Connection_(cocktail)> ;
	skos:prefLabel "French Connection"@en .

<http://vocabulary.semantic-web.at/cocktails/5238edc3-0873-4be5-8197-56c867dcc589> dcterms:created "2016-03-09T17:26:29Z"^^xsd:dateTime ;
	dcterms:creator <http://localhost/user/blumauera> ;
	<http://schema.semantic-web.at/ppt/inScheme> <http://vocabulary.semantic-web.at/cocktails/591cf89a-57af-49b8-9042-3fc77408c93e> ;
	<http://schema.semantic-web.at/ppt/inSubtree> <http://vocabulary.semantic-web.at/cocktails/e86c1671-4a67-494b-ae5d-bcb750865acc> ;
	a <http://vocabulary.semantic-web.at/cocktail-ontology/Beverages> , <http://vocabulary.semantic-web.at/cocktail-ontology/Ingredients> , <http://vocabulary.semantic-web.at/cocktail-ontology/Non-alcoholic-Beverages> , skos:Concept ;
	skos:broader <http://vocabulary.semantic-web.at/cocktails/498283e1-6a11-43f0-b6ae-d04aea796285> ;
	skos:prefLabel "Milk"@en .

<http://vocabulary.semantic-web.at/cocktails/53a05366-d473-4eb4-ac66-0d0119e0b759> dcterms:contributor <http://localhost/user/nagyhel> ;
	dcterms:created "2015-05-01T14:35:41Z"^^xsd:dateTime ;
	dcterms:creator <http://localhost/user/blumauera> ;
	dcterms:modified "2015-11-04T14:59:26Z"^^xsd:dateTime ;
	<http://schema.semantic-web.at/ppt/inScheme> <http://vocabulary.semantic-web.at/cocktails/8d052dfc-44bf-4985-8ce3-4564570a161b> ;
	<http://vocabulary.semantic-web.at/cocktail-ontology/consists-of> <http://vocabulary.semantic-web.at/cocktails/5d96c50c-ee48-4c40-bb4c-4b9a42d11de6> , <http://vocabulary.semantic-web.at/cocktails/71210bd1-3071-4533-8da4-fe0f7d7694a0> , <http://vocabulary.semantic-web.at/cocktails/7448dbed-7603-41f7-a316-99f754c9ae45> , <http://vocabulary.semantic-web.at/cocktails/9c2ce399-c6ae-4f4d-bf37-7fd8ffe2a19d> ;
	<http://vocabulary.semantic-web.at/cocktail-ontology/iba> <http://www.iba-world.com/index.php?option=com_content&id=196&Itemid=532> ;
	<http://vocabulary.semantic-web.at/cocktail-ontology/image> <http://www.iba-world.com/images/cocktail_drinks/gin_fizz.jpg> ;
	<http://vocabulary.semantic-web.at/cocktail-ontology/preparation> "A Gin Fizz contains gin, lemon juice, sugar, and carbonated water, served in a tumbler with two ice cubes."@en ;
	<http://vocabulary.semantic-web.at/cocktail-ontology/served> "On the rocks; poured over ice"@en ;
	<http://vocabulary.semantic-web.at/cocktail-ontology/uses> <http://vocabulary.semantic-web.at/cocktails/a54d2096-6214-4006-beaf-afcc77824710> ;
	<http://vocabulary.semantic-web.at/cocktail-ontology/uses_2> <http://vocabulary.semantic-web.at/cocktails/33df103a-03ac-4177-b620-7953fe094236> ;
	a <http://vocabulary.semantic-web.at/cocktail-ontology/Cocktail> , skos:Concept ;
	skos:altLabel "Sloe Gin Fizz"@en ;
	skos:broader <http://vocabulary.semantic-web.at/cocktails/7516b400-963a-4151-8fdc-f6b23bad1dd5> , <http://vocabulary.semantic-web.at/cocktails/caae2ea0-7e60-400b-a2bb-14ef79720668> ;
	skos:definition "A Fizz is a type of mixed drink—a variation on the older Sours family. The defining features of the fizz are an acidic juice (such as lemon or lime juice) and carbonated water."@en ;
	skos:exactMatch <http://dbpedia.org/resource/Fizz_(cocktail)> ;
	skos:prefLabel "Gin Fizz"@en .

<http://vocabulary.semantic-web.at/cocktails/54702498-ad42-4af6-b28a-2276215450da> dcterms:contributor <http://localhost/user/huberf> ;
	dcterms:created "2015-05-01T07:42:25Z"^^xsd:dateTime ;
	dcterms:creator <http://localhost/user/blumauera> ;
	dcterms:modified "2016-10-05T09:35:34Z"^^xsd:dateTime ;
	<http://schema.semantic-web.at/ppt/inScheme> <http://vocabulary.semantic-web.at/cocktails/8d052dfc-44bf-4985-8ce3-4564570a161b> ;
	a <http://vocabulary.semantic-web.at/cocktail-ontology/Cocktail> , skos:Concept ;
	skos:altLabel "Mixed Drinks"@en , "Mixed drinks"@en , "Sling (drink)"@en ;
	skos:definition "A mixed drink is a beverage in which two or more ingredients are mixed. Some mixed drinks are alcoholic beverages that contain liquor; others are non-alcoholic."@en ;
	skos:exactMatch dbpedia:Mixed_drink ;
	skos:narrower <http://vocabulary.semantic-web.at/cocktails/12f4790a-560f-4e1c-b57a-53b8171ae39a> , <http://vocabulary.semantic-web.at/cocktails/2c032fe6-a518-44be-851a-dbf1c253be63> , <http://vocabulary.semantic-web.at/cocktails/43111fc3-3b59-420c-a588-024cd2d33896> , <http://vocabulary.semantic-web.at/cocktails/7e5afb63-30ec-42b4-a9f5-f61fc456107d> , <http://vocabulary.semantic-web.at/cocktails/9c287d15-c699-4f56-bd65-bf8cc75a2cca> , <http://vocabulary.semantic-web.at/cocktails/b0885ae3-68e1-453d-8669-119e8464ff5f> , <http://vocabulary.semantic-web.at/cocktails/b33091cd-8c57-45e3-a89b-9de91ffce1e8> , <http://vocabulary.semantic-web.at/cocktails/b65b6d98-400f-47cf-94c7-d2566f10cf64> ;
	skos:prefLabel "Mixed drink"@en ;
	skos:topConceptOf <http://vocabulary.semantic-web.at/cocktails/8d052dfc-44bf-4985-8ce3-4564570a161b> .

<http://vocabulary.semantic-web.at/cocktails/55c40695-8b41-41ed-8c6a-70fe6930067e> dcterms:contributor <http://localhost/user/huberf> ;
	dcterms:created "2015-05-02T19:03:18Z"^^xsd:dateTime ;
	dcterms:creator <http://localhost/user/blumauera> ;
	dcterms:modified "2016-10-05T09:32:10Z"^^xsd:dateTime ;
	<http://schema.semantic-web.at/ppt/inScheme> <http://vocabulary.semantic-web.at/cocktails/8d052dfc-44bf-4985-8ce3-4564570a161b> ;
	<http://vocabulary.semantic-web.at/cocktail-ontology/consists-of> <http://vocabulary.semantic-web.at/cocktails/2ce50273-13b2-4ba1-9ff2-8cfbd835c1f2> , <http://vocabulary.semantic-web.at/cocktails/7dede323-e986-4417-b723-c9c7a7fe82ba> , <http://vocabulary.semantic-web.at/cocktails/ced2e755-fe48-4d7b-86ab-6b39fe359a32> ;
	<http://vocabulary.semantic-web.at/cocktail-ontology/iba> <http://www.iba-world.com/index.php?option=com_content&id=237&Itemid=532> ;
	<http://vocabulary.semantic-web.at/cocktail-ontology/image> <http://upload.wikimedia.org/wikipedia/commons/thumb/7/79/Tequila_Sunrise_garnished_with_orange_and_cherry_-_Evan_Swigart.jpg/440px-Tequila_Sunrise_garnished_with_orange_and_cherry_-_Evan_Swigart.jpg> ;
	<http://vocabulary.semantic-web.at/cocktail-ontology/preparation> "Pour the tequila and orange juice into glass over ice. Add the grenadine, which will sink to the bottom. Do not stir. Garnish and serve."@en ;
	<http://vocabulary.semantic-web.at/cocktail-ontology/served> "On the rocks; poured over ice"@en ;
	<http://vocabulary.semantic-web.at/cocktail-ontology/uses> <http://vocabulary.semantic-web.at/cocktails/20d288cb-4e38-46f9-9bec-1c79d8397215> , <http://vocabulary.semantic-web.at/cocktails/a54d2096-6214-4006-beaf-afcc77824710> ;
	<http://vocabulary.semantic-web.at/cocktail-ontology/uses_2> <http://vocabulary.semantic-web.at/cocktails/62fbc16f-3f84-4cc7-8c6f-5afebfc1510a> , <http://vocabulary.semantic-web.at/cocktails/99171f20-c59f-40c4-998a-a9c8f1909168> ;
	a <http://vocabulary.semantic-web.at/cocktail-ontology/Cocktail> , skos:Concept ;
	skos:broader <http://vocabulary.semantic-web.at/cocktails/b9bf3799-a4e4-47f7-9aea-7697cc998a34> ;
	skos:definition "The Tequila Sunrise is a cocktail made in two different ways, the original and the more popular concoction. Originally served at the Arizona Biltmore Hotel, where it was created by Gene Sulit in the 1930s or 1940s, the cocktail is named for the way it looks after it has been poured into a glass. The denser ingredients (cassis or grenadine) settle, creating gradations in color that mimic a sunrise."@en ;
	skos:exactMatch <http://dbpedia.org/resource/Tequila_Sunrise_(cocktail)> ;
	skos:prefLabel "Tequila Sunrise"@en .

<http://vocabulary.semantic-web.at/cocktails/563bf7e0-0f40-41b6-a749-c4e94760204d> dcterms:contributor <http://localhost/user/blumauera> ;
	dcterms:created "2015-05-02T19:05:00Z"^^xsd:dateTime ;
	dcterms:creator <http://localhost/user/blumauera> ;
	dcterms:modified "2015-05-05T07:55:54Z"^^xsd:dateTime ;
	<http://schema.semantic-web.at/ppt/inScheme> <http://vocabulary.semantic-web.at/cocktails/8d052dfc-44bf-4985-8ce3-4564570a161b> ;
	<http://vocabulary.semantic-web.at/cocktail-ontology/consists-of> <http://vocabulary.semantic-web.at/cocktails/5d96c50c-ee48-4c40-bb4c-4b9a42d11de6> , <http://vocabulary.semantic-web.at/cocktails/71210bd1-3071-4533-8da4-fe0f7d7694a0> , <http://vocabulary.semantic-web.at/cocktails/9c2ce399-c6ae-4f4d-bf37-7fd8ffe2a19d> , <http://vocabulary.semantic-web.at/cocktails/f4da82d8-eaf5-451f-824c-05564bc48816> ;
	<http://vocabulary.semantic-web.at/cocktail-ontology/iba> <http://www.iba-world.com/index.php?option=com_content&id=239&Itemid=532> ;
	<http://vocabulary.semantic-web.at/cocktail-ontology/image> <http://upload.wikimedia.org/wikipedia/commons/thumb/0/0a/A_Bramble_%286777249261%29.jpg/440px-A_Bramble_%286777249261%29.jpg> ;
	<http://vocabulary.semantic-web.at/cocktail-ontology/preparation> "Build over crushed ice, in a rock glass. Stir, then pour the blackberry liqueur over the top of the drink in a circular fashion. Garnish with a lemon slice, and two blackberries."@en ;
	<http://vocabulary.semantic-web.at/cocktail-ontology/uses> <http://vocabulary.semantic-web.at/cocktails/2dce3576-2603-41f9-8dce-ab21f639c2a7> ;
	<http://vocabulary.semantic-web.at/cocktail-ontology/uses_2> <http://vocabulary.semantic-web.at/cocktails/33df103a-03ac-4177-b620-7953fe094236> , <http://vocabulary.semantic-web.at/cocktails/7c4a2cfe-6750-419a-87d1-dcb4919ff92b> ;
	a <http://vocabulary.semantic-web.at/cocktail-ontology/Cocktail> , skos:Concept ;
	skos:broader <http://vocabulary.semantic-web.at/cocktails/ccee1079-43df-4ff1-bef0-d15d3dc8fa6f> ;
	skos:prefLabel "Bramble"@en .

<http://vocabulary.semantic-web.at/cocktails/591cf89a-57af-49b8-9042-3fc77408c93e> dcterms:contributor <http://localhost/user/blumauera> ;
	dcterms:created "2015-05-01T07:50:48Z"^^xsd:dateTime ;
	dcterms:creator <http://localhost/user/blumauera> ;
	dcterms:modified "2015-05-02T21:01:57Z"^^xsd:dateTime ;
	dcterms:publisher <http://localhost/user/Semantic-Web-Company> ;
	dcterms:title "Beverages"@en ;
	<http://schema.semantic-web.at/ppt/appliedType> <http://vocabulary.semantic-web.at/cocktail-ontology/Ingredients> ;
	a skos:ConceptScheme ;
	rdfs:label "Beverages"@en ;
	skos:hasTopConcept <http://vocabulary.semantic-web.at/cocktails/403d1249-f37f-4f43-bebf-8dde9677d886> , <http://vocabulary.semantic-web.at/cocktails/d5286375-41b3-468b-9602-8fcf698e3e83> , <http://vocabulary.semantic-web.at/cocktails/e86c1671-4a67-494b-ae5d-bcb750865acc> , <http://vocabulary.semantic-web.at/cocktails/f3000285-36b0-4ffe-af90-740c2dd8fff5> .

<http://vocabulary.semantic-web.at/cocktails/59848efb-dc96-4014-af09-5f89ba057df9> dcterms:contributor <http://localhost/user/blumauera> ;
	dcterms:created "2015-05-01T08:37:21Z"^^xsd:dateTime ;
	dcterms:creator <http://localhost/user/blumauera> ;
	dcterms:modified "2015-05-05T07:42:54Z"^^xsd:dateTime ;
	<http://schema.semantic-web.at/ppt/inScheme> <http://vocabulary.semantic-web.at/cocktails/591cf89a-57af-49b8-9042-3fc77408c93e> ;
	<http://schema.semantic-web.at/ppt/inSubtree> <http://vocabulary.semantic-web.at/cocktails/403d1249-f37f-4f43-bebf-8dde9677d886> ;
	<http://vocabulary.semantic-web.at/cocktail-ontology/image_3> <http://upload.wikimedia.org/wikipedia/commons/0/03/Grand_Marnier_Bottle.jpg> ;
	<http://vocabulary.semantic-web.at/cocktail-ontology/is-part-of> <http://vocabulary.semantic-web.at/cocktails/cd66d6ff-559f-43ea-a754-ac613a87325d> ;
	a <http://vocabulary.semantic-web.at/cocktail-ontology/Alcoholic-Beverages> , <http://vocabulary.semantic-web.at/cocktail-ontology/Beverages> , <http://vocabulary.semantic-web.at/cocktail-ontology/Ingredients> , skos:Concept ;
	skos:altLabel "Gran marnier"@en , "Grand Marinier"@en , "Grand mariner"@en ;
	skos:broader <http://vocabulary.semantic-web.at/cocktails/397d0ec3-98e2-47d9-a8c2-eca9702ff94d> ;
	skos:definition "Grand Marnier Cordon Rouge is an orange-flavored brandy liqueur created in 1880 by Alexandre Marnier-Lapostolle. It is made from a blend of Cognac brandy, distilled essence of bitter orange, and sugar. Grand Marnier Cordon Rouge is 40% alcohol (70 Proof in UK, 80 Proof in US). Aside from Cordon Rouge, the Grand Marnier line includes other liqueurs, most of which can be consumed \"neat\" as a cordial or a digestif, and can be used in mixed drinks and desserts."@en ;
	skos:exactMatch dbpedia:Grand_Marnier ;
	skos:prefLabel "Grand Marnier"@en .

<http://vocabulary.semantic-web.at/cocktails/59ccd2fc-1807-45eb-8621-8d3e898e6d37> dcterms:contributor <http://localhost/user/blumauera> ;
	dcterms:created "2015-05-01T14:58:03Z"^^xsd:dateTime ;
	dcterms:creator <http://localhost/user/blumauera> ;
	dcterms:modified "2015-05-05T07:11:40Z"^^xsd:dateTime ;
	<http://schema.semantic-web.at/ppt/inScheme> <http://vocabulary.semantic-web.at/cocktails/591cf89a-57af-49b8-9042-3fc77408c93e> ;
	<http://schema.semantic-web.at/ppt/inSubtree> <http://vocabulary.semantic-web.at/cocktails/403d1249-f37f-4f43-bebf-8dde9677d886> ;
	<http://vocabulary.semantic-web.at/cocktail-ontology/is-part-of> <http://vocabulary.semantic-web.at/cocktails/9c287d15-c699-4f56-bd65-bf8cc75a2cca> , <http://vocabulary.semantic-web.at/cocktails/bed073f2-de84-4322-a490-4f34ec54c6d1> ;
	a <http://vocabulary.semantic-web.at/cocktail-ontology/Alcoholic-Beverages> , <http://vocabulary.semantic-web.at/cocktail-ontology/Beverages> , <http://vocabulary.semantic-web.at/cocktail-ontology/Ingredients> , skos:Concept ;
	skos:broader <http://vocabulary.semantic-web.at/cocktails/e98ac9a3-64f3-4cc5-8d0d-cf8684b0e7d1> ;
	skos:prefLabel "Dark rum"@en .

<http://vocabulary.semantic-web.at/cocktails/5ac37bec-e4b9-4d43-9bcc-8d6954903c25> dcterms:contributor <http://localhost/user/blumauera> ;
	dcterms:created "2015-05-01T07:40:02Z"^^xsd:dateTime ;
	dcterms:creator <http://localhost/user/blumauera> ;
	dcterms:modified "2015-05-01T07:40:30Z"^^xsd:dateTime ;
	<http://schema.semantic-web.at/ppt/inScheme> <http://vocabulary.semantic-web.at/cocktails/8d052dfc-44bf-4985-8ce3-4564570a161b> ;
	a <http://vocabulary.semantic-web.at/cocktail-ontology/Cocktail> , skos:Concept ;
	skos:altLabel "IBA Official Cocktails"@en , "IBA cocktails"@en ;
	skos:definition "An IBA Official Cocktail is one of many cocktails selected by the International Bartenders Association for use in the annual World Cocktail Competition (WCC) in bartending. As such, these mixed drinks are some of the most notable and frequently-made cocktails by professional bartenders around the world. IBA Cocktails are specified in centilitres (cl) rather than the more commonly used millilitres (ml). 3 cl are approximately equivalent to 1 U.S. fluid ounce (1.4% more)."@en ;
	skos:exactMatch dbpedia:IBA_Official_Cocktail ;
	skos:narrower <http://vocabulary.semantic-web.at/cocktails/b9bf3799-a4e4-47f7-9aea-7697cc998a34> , <http://vocabulary.semantic-web.at/cocktails/caae2ea0-7e60-400b-a2bb-14ef79720668> , <http://vocabulary.semantic-web.at/cocktails/ccee1079-43df-4ff1-bef0-d15d3dc8fa6f> ;
	skos:prefLabel "IBA Official Cocktail"@en ;
	skos:topConceptOf <http://vocabulary.semantic-web.at/cocktails/8d052dfc-44bf-4985-8ce3-4564570a161b> .

<http://vocabulary.semantic-web.at/cocktails/5b272721-4eb2-41cd-9224-5963091fb639> dcterms:contributor <http://localhost/user/blumauera> ;
	dcterms:created "2015-11-18T14:36:51Z"^^xsd:dateTime ;
	dcterms:creator <http://localhost/user/blumauera> ;
	dcterms:modified "2015-11-18T14:37:02Z"^^xsd:dateTime ;
	<http://schema.semantic-web.at/ppt/inScheme> <http://vocabulary.semantic-web.at/cocktails/591cf89a-57af-49b8-9042-3fc77408c93e> ;
	<http://schema.semantic-web.at/ppt/inSubtree> <http://vocabulary.semantic-web.at/cocktails/403d1249-f37f-4f43-bebf-8dde9677d886> ;
	<http://vocabulary.semantic-web.at/cocktail-ontology/is-part-of> <http://vocabulary.semantic-web.at/cocktails/4efda48d-6c56-47e5-bf98-bf8918ff58eb> ;
	a <http://vocabulary.semantic-web.at/cocktail-ontology/Alcoholic-Beverages> , <http://vocabulary.semantic-web.at/cocktail-ontology/Beverages> , <http://vocabulary.semantic-web.at/cocktail-ontology/Ingredients> , skos:Concept ;
	skos:altLabel "Gilka-Kuemmel"@en , "Gilka-Kummel"@en , "Gilka-Kümmel"@en , "Kuemmel"@en , "Kummel"@en ;
	skos:broader <http://vocabulary.semantic-web.at/cocktails/917d78d0-0938-4fe0-80c4-cfd2eb16e6a4> ;
	skos:definition "Kümmel, also called kummel or kimmel, is a sweet, colorless liqueur flavored with caraway seed, cumin, and fennel. Originally, the words kümmel, kummel, and kimmel are somewhat generic terms in the German, Dutch, and Yiddish languages, respectively, meaning both caraway and cumin. For instance, in German caraway is called Echter Kümmel and cumin is called Kreuzkümmel, but the term Kümmel is also used for the liqueur flavored with these spices."@en ;
	skos:exactMatch dbpedia:K%C3%BCmmel ;
	skos:prefLabel "Kümmel"@en .

<http://vocabulary.semantic-web.at/cocktails/5b4cd5f6-19e8-4854-8c5e-0b6d58cbb702> dcterms:contributor <http://localhost/user/blumauera> ;
	dcterms:created "2015-05-02T18:41:36Z"^^xsd:dateTime ;
	dcterms:creator <http://localhost/user/blumauera> ;
	dcterms:modified "2015-05-07T07:00:56Z"^^xsd:dateTime ;
	<http://schema.semantic-web.at/ppt/inScheme> <http://vocabulary.semantic-web.at/cocktails/591cf89a-57af-49b8-9042-3fc77408c93e> ;
	<http://schema.semantic-web.at/ppt/inSubtree> <http://vocabulary.semantic-web.at/cocktails/e86c1671-4a67-494b-ae5d-bcb750865acc> ;
	<http://vocabulary.semantic-web.at/cocktail-ontology/is-part-of> <http://vocabulary.semantic-web.at/cocktails/2c032fe6-a518-44be-851a-dbf1c253be63> , <http://vocabulary.semantic-web.at/cocktails/bed073f2-de84-4322-a490-4f34ec54c6d1> ;
	a <http://vocabulary.semantic-web.at/cocktail-ontology/Beverages> , <http://vocabulary.semantic-web.at/cocktail-ontology/Ingredients> , <http://vocabulary.semantic-web.at/cocktail-ontology/Non-alcoholic-Beverages> , skos:Concept ;
	skos:altLabel "Ginger beer plant"@en , "Ginger-beer"@en ;
	skos:broader <http://vocabulary.semantic-web.at/cocktails/89ac12aa-d4f9-46d0-b127-fd8f4c21fbcc> ;
	skos:definition "Ginger beer is a carbonated drink, that is flavored primarily with ginger and sweetened with sugar or artificial sweeteners."@en ;
	skos:exactMatch dbpedia:Ginger_beer ;
	skos:prefLabel "Ginger beer"@en .

<http://vocabulary.semantic-web.at/cocktails/5c291fe9-6fdb-4939-930d-dacbc67171a5> dcterms:contributor <http://localhost/user/blumauera> ;
	dcterms:created "2015-05-01T14:41:09Z"^^xsd:dateTime ;
	dcterms:creator <http://localhost/user/blumauera> ;
	dcterms:modified "2015-05-07T07:14:09Z"^^xsd:dateTime ;
	<http://schema.semantic-web.at/ppt/inScheme> <http://vocabulary.semantic-web.at/cocktails/591cf89a-57af-49b8-9042-3fc77408c93e> ;
	<http://schema.semantic-web.at/ppt/inSubtree> <http://vocabulary.semantic-web.at/cocktails/403d1249-f37f-4f43-bebf-8dde9677d886> ;
	<http://vocabulary.semantic-web.at/cocktail-ontology/is-part-of> <http://vocabulary.semantic-web.at/cocktails/43111fc3-3b59-420c-a588-024cd2d33896> , <http://vocabulary.semantic-web.at/cocktails/43b786b6-a1f1-4b7f-a5d9-be43d386ffb4> , <http://vocabulary.semantic-web.at/cocktails/61a18ebf-fd92-4ef1-8ab1-bfd3c26867b9> , <http://vocabulary.semantic-web.at/cocktails/9c287d15-c699-4f56-bd65-bf8cc75a2cca> , <http://vocabulary.semantic-web.at/cocktails/eddf4894-1683-44e9-9ee3-7920d3729d71> , <http://vocabulary.semantic-web.at/cocktails/f632b16d-1490-4587-a637-fb393d7b1e7f> , <http://vocabulary.semantic-web.at/cocktails/fb278b46-3c67-48b0-b9eb-7ea037294f5f> ;
	a <http://vocabulary.semantic-web.at/cocktail-ontology/Alcoholic-Beverages> , <http://vocabulary.semantic-web.at/cocktail-ontology/Beverages> , <http://vocabulary.semantic-web.at/cocktail-ontology/Ingredients> , skos:Concept ;
	skos:altLabel "Angostura (flavouring)"@en , "Angostura bitter"@en ;
	skos:broader <http://vocabulary.semantic-web.at/cocktails/d40e2215-bc1b-4bae-8cf8-d10b1ad36d44> ;
	skos:definition "Angostura bitters, often simply referred to as angostura, is a concentrated bitters made of water, 44.7% alcohol, herbs and spices. by House of Angostura in Trinidad and Tobago. They are typically used for flavoring beverages, or (less often) food. The bitters were first produced in the town of Angostura (hence the name), and do not contain angostura bark. The bottle is easily recognisable by its distinctive over-sized label."@en ;
	skos:exactMatch dbpedia:Angostura_bitters ;
	skos:prefLabel "Angostura bitters"@en .

<http://vocabulary.semantic-web.at/cocktails/5caedba2-9aef-4fab-b26b-6e20cf014419> dcterms:contributor <http://localhost/user/blumauera> ;
	dcterms:created "2015-05-01T14:54:52Z"^^xsd:dateTime ;
	dcterms:creator <http://localhost/user/blumauera> ;
	dcterms:modified "2015-05-04T10:11:06Z"^^xsd:dateTime ;
	<http://schema.semantic-web.at/ppt/inScheme> <http://vocabulary.semantic-web.at/cocktails/591cf89a-57af-49b8-9042-3fc77408c93e> ;
	<http://schema.semantic-web.at/ppt/inSubtree> <http://vocabulary.semantic-web.at/cocktails/403d1249-f37f-4f43-bebf-8dde9677d886> ;
	<http://vocabulary.semantic-web.at/cocktail-ontology/is-part-of> <http://vocabulary.semantic-web.at/cocktails/2c3083d2-8650-4460-b019-cae7aea38f14> , <http://vocabulary.semantic-web.at/cocktails/b3834414-af63-4e6f-9c3c-6c353e9600ee> ;
	a <http://vocabulary.semantic-web.at/cocktail-ontology/Alcoholic-Beverages> , <http://vocabulary.semantic-web.at/cocktail-ontology/Beverages> , <http://vocabulary.semantic-web.at/cocktail-ontology/Ingredients> , skos:Concept ;
	skos:broader <http://vocabulary.semantic-web.at/cocktails/8f09ee6f-d5b9-4b8a-aa17-b0665fae4e83> ;
	skos:definition "Apricot brandy can refer to a liquor (or Eau de Vie) distilled from fermented apricot juice or a liqueur made from apricot flesh and kernels."@en ;
	skos:exactMatch dbpedia:Apricot_brandy ;
	skos:prefLabel "Apricot brandy"@en .

<http://vocabulary.semantic-web.at/cocktails/5d0fdad6-6256-4042-a1a0-709f332cf373> dcterms:contributor <http://localhost/user/blumauera> ;
	dcterms:created "2015-05-03T18:59:07Z"^^xsd:dateTime ;
	dcterms:creator <http://localhost/user/blumauera> ;
	dcterms:modified "2015-05-03T18:59:18Z"^^xsd:dateTime ;
	<http://schema.semantic-web.at/ppt/inScheme> <http://vocabulary.semantic-web.at/cocktails/591cf89a-57af-49b8-9042-3fc77408c93e> ;
	<http://schema.semantic-web.at/ppt/inSubtree> <http://vocabulary.semantic-web.at/cocktails/403d1249-f37f-4f43-bebf-8dde9677d886> ;
	a <http://vocabulary.semantic-web.at/cocktail-ontology/Alcoholic-Beverages> , <http://vocabulary.semantic-web.at/cocktail-ontology/Beverages> , <http://vocabulary.semantic-web.at/cocktail-ontology/Ingredients> , skos:Concept ;
	skos:broader <http://vocabulary.semantic-web.at/cocktails/074c3acb-bc4d-4c6e-ad8a-e553d5ec7eff> , <http://vocabulary.semantic-web.at/cocktails/1b9d9c87-9a94-465a-b7e9-feee6c77bf03> ;
	skos:prefLabel "Cinzano Extra Dry"@en .

<http://vocabulary.semantic-web.at/cocktails/5d96c50c-ee48-4c40-bb4c-4b9a42d11de6> dcterms:contributor <http://localhost/user/blumauera> ;
	dcterms:created "2015-05-01T08:35:12Z"^^xsd:dateTime ;
	dcterms:creator <http://localhost/user/blumauera> ;
	dcterms:modified "2015-08-07T15:06:42Z"^^xsd:dateTime ;
	<http://schema.semantic-web.at/ppt/inScheme> <http://vocabulary.semantic-web.at/cocktails/591cf89a-57af-49b8-9042-3fc77408c93e> ;
	<http://schema.semantic-web.at/ppt/inSubtree> <http://vocabulary.semantic-web.at/cocktails/403d1249-f37f-4f43-bebf-8dde9677d886> ;
	<http://vocabulary.semantic-web.at/cocktail-ontology/image_3> <http://preview.poolparty.biz/sparqlingCocktails/resources/images/gin.png> ;
	<http://vocabulary.semantic-web.at/cocktail-ontology/is-part-of> <http://vocabulary.semantic-web.at/cocktails/0bbdca98-077b-48d1-99d6-47eca59c442c> , <http://vocabulary.semantic-web.at/cocktails/11d68913-3a30-4591-bc41-25fea3f38520> , <http://vocabulary.semantic-web.at/cocktails/2c3083d2-8650-4460-b019-cae7aea38f14> , <http://vocabulary.semantic-web.at/cocktails/36671f9c-904a-4629-937a-519d094ecefc> , <http://vocabulary.semantic-web.at/cocktails/383ea520-07b2-4dc9-8827-8fc84fb7749c> , <http://vocabulary.semantic-web.at/cocktails/40ab50e9-66f1-411b-8220-ef8f05273542> , <http://vocabulary.semantic-web.at/cocktails/43111fc3-3b59-420c-a588-024cd2d33896> , <http://vocabulary.semantic-web.at/cocktails/44cc99c1-28ac-4c50-a55d-7244b2c5c07b> , <http://vocabulary.semantic-web.at/cocktails/53a05366-d473-4eb4-ac66-0d0119e0b759> , <http://vocabulary.semantic-web.at/cocktails/563bf7e0-0f40-41b6-a749-c4e94760204d> , <http://vocabulary.semantic-web.at/cocktails/85669fcc-a38a-4ceb-ae23-90ae3fb7e16c> , <http://vocabulary.semantic-web.at/cocktails/a0fba95c-d29e-4954-8800-f5e6de1e6f86> , <http://vocabulary.semantic-web.at/cocktails/a73d88e9-0c50-45d2-b364-9dec5abe206d> , <http://vocabulary.semantic-web.at/cocktails/b00a123f-a2b5-49d2-8325-a81d1d26ddc6> , <http://vocabulary.semantic-web.at/cocktails/b33091cd-8c57-45e3-a89b-9de91ffce1e8> , <http://vocabulary.semantic-web.at/cocktails/b3834414-af63-4e6f-9c3c-6c353e9600ee> , <http://vocabulary.semantic-web.at/cocktails/c151ee28-45d2-4128-8587-1f1b69060d9d> , <http://vocabulary.semantic-web.at/cocktails/c3ae5830-1bfd-4f37-afc9-3e88849d03cf> , <http://vocabulary.semantic-web.at/cocktails/ce8f4591-ccd4-4d90-a761-244115d64061> ;
	a <http://vocabulary.semantic-web.at/cocktail-ontology/Alcoholic-Beverages> , <http://vocabulary.semantic-web.at/cocktail-ontology/Beverages> , <http://vocabulary.semantic-web.at/cocktail-ontology/Ingredients> , skos:Concept ;
	skos:altLabel "Blue ruin"@en , "Gins"@en , "Mothers ruin"@en ;
	skos:broader <http://vocabulary.semantic-web.at/cocktails/403d1249-f37f-4f43-bebf-8dde9677d886> , <http://vocabulary.semantic-web.at/cocktails/f3000285-36b0-4ffe-af90-740c2dd8fff5> ;
	skos:definition "Gin is a spirit which derives its predominant flavour from juniper berries (Juniperus communis). From its earliest beginnings in the Middle Ages, gin has evolved over the course of a millennium from a herbal medicine to an object of commerce in the spirits industry. Today, the gin category is one of the most popular and widely distributed range of spirits, and is represented by products of various origins, styles, and flavor profiles that all revolve around juniper as a common ingredient."@en ;
	skos:exactMatch dbpedia:Gin ;
	skos:narrower <http://vocabulary.semantic-web.at/cocktails/0a9e12b8-afa5-425a-b08b-941374b3bdc4> ;
	skos:prefLabel "Gin"@en .

<http://vocabulary.semantic-web.at/cocktails/60d3a991-48d3-4e73-9d62-5961893fd311> dcterms:contributor <http://localhost/user/blumauera> ;
	dcterms:created "2015-05-01T14:08:13Z"^^xsd:dateTime ;
	dcterms:creator <http://localhost/user/blumauera> ;
	dcterms:modified "2015-05-03T10:31:58Z"^^xsd:dateTime ;
	<http://schema.semantic-web.at/ppt/inScheme> <http://vocabulary.semantic-web.at/cocktails/8d052dfc-44bf-4985-8ce3-4564570a161b> ;
	<http://vocabulary.semantic-web.at/cocktail-ontology/consists-of> <http://vocabulary.semantic-web.at/cocktails/88f5de3d-3de4-4a2f-9523-50bc7bb06600> , <http://vocabulary.semantic-web.at/cocktails/c3a50c60-ccb3-4ab4-8f9f-722acdae8d50> , <http://vocabulary.semantic-web.at/cocktails/ced2e755-fe48-4d7b-86ab-6b39fe359a32> ;
	<http://vocabulary.semantic-web.at/cocktail-ontology/iba> <http://www.iba-world.com/index.php?option=com_content&id=189&Itemid=532> ;
	<http://vocabulary.semantic-web.at/cocktail-ontology/image> <http://upload.wikimedia.org/wikipedia/commons/thumb/f/f9/Bacardi_cocktail.jpg/440px-Bacardi_cocktail.jpg> ;
	<http://vocabulary.semantic-web.at/cocktail-ontology/preparation> "Pour all ingredients into shaker with ice cubes, shake well, strain into chilled cocktail glass."@en ;
	<http://vocabulary.semantic-web.at/cocktail-ontology/served> "straight up"@en ;
	<http://vocabulary.semantic-web.at/cocktail-ontology/uses> <http://vocabulary.semantic-web.at/cocktails/19dee0d8-fd30-469f-9ecd-91c902ff717c> ;
	<http://vocabulary.semantic-web.at/cocktail-ontology/uses_2> <http://vocabulary.semantic-web.at/cocktails/021c85c0-a60a-4414-8fd8-bd3383b794f1> ;
	a <http://vocabulary.semantic-web.at/cocktail-ontology/Cocktail> , skos:Concept ;
	skos:broader <http://vocabulary.semantic-web.at/cocktails/caae2ea0-7e60-400b-a2bb-14ef79720668> ;
	skos:prefLabel "Bacardi cocktail"@en ;
	skos:related <http://vocabulary.semantic-web.at/cocktails/bab016bd-2fd5-4809-bfe7-3225d25f116d> .

<http://vocabulary.semantic-web.at/cocktails/61a18ebf-fd92-4ef1-8ab1-bfd3c26867b9> dcterms:contributor <http://localhost/user/blumauera> ;
	dcterms:created "2015-05-02T08:11:49Z"^^xsd:dateTime ;
	dcterms:creator <http://localhost/user/blumauera> ;
	dcterms:modified "2015-05-06T12:37:34Z"^^xsd:dateTime ;
	<http://schema.semantic-web.at/ppt/inScheme> <http://vocabulary.semantic-web.at/cocktails/8d052dfc-44bf-4985-8ce3-4564570a161b> ;
	<http://vocabulary.semantic-web.at/cocktail-ontology/consists-of> <http://vocabulary.semantic-web.at/cocktails/3c94f5fc-4664-4177-a880-88643c0be9c1> , <http://vocabulary.semantic-web.at/cocktails/5c291fe9-6fdb-4939-930d-dacbc67171a5> , <http://vocabulary.semantic-web.at/cocktails/cdbac85a-d5b7-40f3-9e98-4d7e176b5565> , <http://vocabulary.semantic-web.at/cocktails/fd76c5ab-be62-4c4b-a2c6-7fa9bc359f47> ;
	<http://vocabulary.semantic-web.at/cocktail-ontology/iba> <http://www.iba-world.com/index.php?option=com_content&id=217&Itemid=532> ;
	<http://vocabulary.semantic-web.at/cocktail-ontology/image> <http://www.iba-world.com/images/cocktail_drinks/champagne_cocktail.jpg> ;
	<http://vocabulary.semantic-web.at/cocktail-ontology/preparation> "Add dash of Angostura bitter onto sugar cube and drop it into champagne flute. Add cognac followed by gently pouring chilled champagne. Garnish with orange slice and maraschino cherry."@en ;
	<http://vocabulary.semantic-web.at/cocktail-ontology/served> "Straight up; without ice"@en ;
	<http://vocabulary.semantic-web.at/cocktail-ontology/uses> <http://vocabulary.semantic-web.at/cocktails/fece03b5-ec0b-4e47-964d-cc5dc09fd7fb> ;
	<http://vocabulary.semantic-web.at/cocktail-ontology/uses_2> <http://vocabulary.semantic-web.at/cocktails/8a5e1790-d3c0-432e-bb85-709692b14f03> , <http://vocabulary.semantic-web.at/cocktails/99171f20-c59f-40c4-998a-a9c8f1909168> ;
	a <http://vocabulary.semantic-web.at/cocktail-ontology/Cocktail> , skos:Concept ;
	skos:broader <http://vocabulary.semantic-web.at/cocktails/204cd4e7-58d7-4417-837a-7f9cc41663c8> , <http://vocabulary.semantic-web.at/cocktails/b9bf3799-a4e4-47f7-9aea-7697cc998a34> ;
	skos:definition "A champagne cocktail is an alcoholic drink made with sugar, Angostura bitters, champagne, and a maraschino cherry as a garnish. It is one of the IBA Official Cocktails."@en ;
	skos:exactMatch dbpedia:Champagne_cocktail ;
	skos:prefLabel "Champagne cocktail"@en .

<http://vocabulary.semantic-web.at/cocktails/61b2054a-4bb6-4dc2-8125-d69977973bed> dcterms:contributor <http://localhost/user/blumauera> ;
	dcterms:created "2015-05-01T15:02:15Z"^^xsd:dateTime ;
	dcterms:creator <http://localhost/user/blumauera> ;
	dcterms:modified "2015-05-04T11:21:41Z"^^xsd:dateTime ;
	<http://schema.semantic-web.at/ppt/inScheme> <http://vocabulary.semantic-web.at/cocktails/591cf89a-57af-49b8-9042-3fc77408c93e> ;
	<http://schema.semantic-web.at/ppt/inSubtree> <http://vocabulary.semantic-web.at/cocktails/e86c1671-4a67-494b-ae5d-bcb750865acc> ;
	<http://vocabulary.semantic-web.at/cocktail-ontology/is-part-of> <http://vocabulary.semantic-web.at/cocktails/cfa8539e-ede2-42ec-b563-d084ddb33280> ;
	a <http://vocabulary.semantic-web.at/cocktail-ontology/Beverages> , <http://vocabulary.semantic-web.at/cocktail-ontology/Ingredients> , <http://vocabulary.semantic-web.at/cocktail-ontology/Non-alcoholic-Beverages> , skos:Concept ;
	skos:altLabel "Double egg yolk"@en , "Double yolk"@en , "Double yolk egg"@en , "Double yolk eggs"@en , "Double yolked"@en , "Double yolked egg"@en , "Double yolked eggs"@en , "Double yolker"@en , "Double yolkers"@en , "Double yolking"@en , "Double yolks"@en , "Double-yolk"@en , "Double-yolk egg"@en , "Double-yolk eggs"@en , "Double-yolked"@en , "Double-yolked egg"@en , "Double-yolked eggs"@en , "Double-yolker"@en , "Double-yolkers"@en , "Double-yolking"@en , "Double-yolks"@en , "Doubleyolk"@en , "Doubleyolk egg"@en , "Doubleyolk eggs"@en , "Doubleyolked"@en , "Doubleyolked egg"@en , "Doubleyolked eggs"@en , "Doubleyolker"@en , "Doubleyolkers"@en , "Doubleyolking"@en , "Doubleyolks"@en , "Egg yolks"@en , "Egg-yolk"@en , "Vitellus"@en , "Yellow of the egg"@en , "Yolk"@en , "Yolkier"@en , "Yolkiest"@en , "Yolks"@en , "Yolky"@en ;
	skos:broader <http://vocabulary.semantic-web.at/cocktails/de17b6c7-513a-4fe2-a8ee-4fdc6069ae27> ;
	skos:definition "An egg yolk is a part of an egg which feeds the developing embryo. The egg yolk is suspended in the egg white (known alternatively as albumen or glair/glaire) by one or two spiral bands of tissue called the chalazae. Prior to fertilization, the yolk together with the germinal disc is a single cell, one of the few single cells that can be seen by the naked eye. As a food, yolks are a major source of vitamins and minerals."@en ;
	skos:exactMatch dbpedia:Egg_yolk ;
	skos:prefLabel "Egg yolk"@en .

<http://vocabulary.semantic-web.at/cocktails/62fbc16f-3f84-4cc7-8c6f-5afebfc1510a> dcterms:contributor <http://localhost/user/blumauera> ;
	dcterms:created "2015-05-01T08:45:06Z"^^xsd:dateTime ;
	dcterms:creator <http://localhost/user/blumauera> ;
	dcterms:modified "2015-05-07T07:16:47Z"^^xsd:dateTime ;
	<http://schema.semantic-web.at/ppt/inScheme> <http://vocabulary.semantic-web.at/cocktails/eff672ac-6601-42c6-a3e9-0adda3b45df8> ;
	<http://schema.semantic-web.at/ppt/inSubtree> <http://vocabulary.semantic-web.at/cocktails/4f20d6bb-710d-4870-bde4-b6e835d7d13f> ;
	<http://vocabulary.semantic-web.at/cocktail-ontology/is-used-by_2> <http://vocabulary.semantic-web.at/cocktails/0bbdca98-077b-48d1-99d6-47eca59c442c> , <http://vocabulary.semantic-web.at/cocktails/0f8cc862-9056-49be-b636-cd22f8d7282d> , <http://vocabulary.semantic-web.at/cocktails/1d5b39cc-fcab-48b2-bb24-9840b7e34d64> , <http://vocabulary.semantic-web.at/cocktails/4792b0b8-0046-47ca-8c2a-f3ad58922182> , <http://vocabulary.semantic-web.at/cocktails/55c40695-8b41-41ed-8c6a-70fe6930067e> , <http://vocabulary.semantic-web.at/cocktails/9c287d15-c699-4f56-bd65-bf8cc75a2cca> , <http://vocabulary.semantic-web.at/cocktails/fb278b46-3c67-48b0-b9eb-7ea037294f5f> ;
	a <http://vocabulary.semantic-web.at/cocktail-ontology/Garnish> , <http://vocabulary.semantic-web.at/cocktail-ontology/Ingredients> , skos:Concept ;
	skos:altLabel "Cherise"@en , "Cherries"@en , "Cherry pit"@en , "Cocktail cherry"@en , "Razzcherries"@en , "Razzcherry"@en , "Wild cherry"@en , "🍒"@en ;
	skos:broader <http://vocabulary.semantic-web.at/cocktails/4f20d6bb-710d-4870-bde4-b6e835d7d13f> ;
	skos:definition "The cherry is the fruit of many plants of the genus Prunus, and is a fleshy drupe (stone fruit). The cherry fruits of commerce are usually obtained from a limited number of species, including especially cultivars of the sweet cherry, Prunus avium. The name 'cherry' also refers to the cherry tree, and is sometimes applied to almonds and visually similar flowering trees in the genus Prunus, as in \"ornamental cherry\", \"cherry blossom\", etc."@en ;
	skos:exactMatch dbpedia:Cherry ;
	skos:narrower <http://vocabulary.semantic-web.at/cocktails/8a5e1790-d3c0-432e-bb85-709692b14f03> ;
	skos:prefLabel "Cherry"@en .

<http://vocabulary.semantic-web.at/cocktails/6420f3aa-5146-4893-b3ea-04033b26c915> dcterms:contributor <http://localhost/user/blumauera> ;
	dcterms:created "2015-11-18T14:35:44Z"^^xsd:dateTime ;
	dcterms:creator <http://localhost/user/blumauera> ;
	dcterms:modified "2015-11-18T14:35:59Z"^^xsd:dateTime ;
	<http://schema.semantic-web.at/ppt/inScheme> <http://vocabulary.semantic-web.at/cocktails/591cf89a-57af-49b8-9042-3fc77408c93e> ;
	<http://schema.semantic-web.at/ppt/inSubtree> <http://vocabulary.semantic-web.at/cocktails/403d1249-f37f-4f43-bebf-8dde9677d886> ;
	<http://vocabulary.semantic-web.at/cocktail-ontology/is-part-of> <http://vocabulary.semantic-web.at/cocktails/4efda48d-6c56-47e5-bf98-bf8918ff58eb> ;
	a <http://vocabulary.semantic-web.at/cocktail-ontology/Alcoholic-Beverages> , <http://vocabulary.semantic-web.at/cocktail-ontology/Beverages> , <http://vocabulary.semantic-web.at/cocktail-ontology/Ingredients> , skos:Concept ;
	skos:altLabel "Goldschlaeger"@en , "Goldschlager"@en , "Goldschlagger"@en , "Goldshlager"@en ;
	skos:broader <http://vocabulary.semantic-web.at/cocktails/9cbe0ac7-b97d-431c-8ea6-a1d7ccc44d4f> ;
	skos:definition "Goldschläger is a Swiss cinnamon schnapps (43.5% alcohol by volume or 87 proof; originally it was 53.5% alcohol or 107 proof), a liqueur with very thin, yet visible flakes of gold floating in it. The actual amount of gold has been measured at approximately 13 mg in a 1 Litre bottle of Goldschläger. As of November 2012 this amounts to €0.56 EUR or lower on the international gold market."@en ;
	skos:exactMatch dbpedia:Goldschl%C3%A4ger ;
	skos:prefLabel "Goldschläger"@en .

<http://vocabulary.semantic-web.at/cocktails/680c7429-30a7-4044-b32f-e28c99dcb9f4> dcterms:contributor <http://localhost/user/blumauera> ;
	dcterms:created "2015-05-02T19:26:40Z"^^xsd:dateTime ;
	dcterms:creator <http://localhost/user/blumauera> ;
	dcterms:modified "2015-05-05T07:36:54Z"^^xsd:dateTime ;
	<http://schema.semantic-web.at/ppt/inScheme> <http://vocabulary.semantic-web.at/cocktails/8d052dfc-44bf-4985-8ce3-4564570a161b> ;
	<http://vocabulary.semantic-web.at/cocktail-ontology/consists-of> <http://vocabulary.semantic-web.at/cocktails/12da816f-8ad3-487d-b8f9-2190e4b3e1b8> , <http://vocabulary.semantic-web.at/cocktails/22df810d-e509-4da8-979c-0758e94de3e6> , <http://vocabulary.semantic-web.at/cocktails/7effbf10-d493-429f-aaff-04011849774d> , <http://vocabulary.semantic-web.at/cocktails/ee61817b-0d10-4862-b44b-740c990e676e> ;
	<http://vocabulary.semantic-web.at/cocktail-ontology/iba> <http://www.iba-world.com/index.php?option=com_content&id=243&Itemid=532> ;
	<http://vocabulary.semantic-web.at/cocktail-ontology/image> <http://www.iba-world.com/images/cocktail_drinks/french_martini.jpg> ;
	<http://vocabulary.semantic-web.at/cocktail-ontology/preparation> "Pour all ingredients into mixing glass with ice cubes. Stir well. Strain in chilled cocktail glass.  Squeeze oil from lemon peel onto the drink."@en ;
	<http://vocabulary.semantic-web.at/cocktail-ontology/uses> <http://vocabulary.semantic-web.at/cocktails/19dee0d8-fd30-469f-9ecd-91c902ff717c> ;
	<http://vocabulary.semantic-web.at/cocktail-ontology/uses_2> <http://vocabulary.semantic-web.at/cocktails/7c4a2cfe-6750-419a-87d1-dcb4919ff92b> ;
	a <http://vocabulary.semantic-web.at/cocktail-ontology/Cocktail> , skos:Concept ;
	skos:broader <http://vocabulary.semantic-web.at/cocktails/ccee1079-43df-4ff1-bef0-d15d3dc8fa6f> ;
	skos:prefLabel "French Martini"@en .

<http://vocabulary.semantic-web.at/cocktails/687a5d86-1f4e-4a6b-b5ca-3b5d74aeafcc> dcterms:contributor <http://localhost/user/blumauera> ;
	dcterms:created "2015-05-02T17:29:53Z"^^xsd:dateTime ;
	dcterms:creator <http://localhost/user/blumauera> ;
	dcterms:modified "2015-05-05T07:53:07Z"^^xsd:dateTime ;
	<http://schema.semantic-web.at/ppt/inScheme> <http://vocabulary.semantic-web.at/cocktails/591cf89a-57af-49b8-9042-3fc77408c93e> ;
	<http://schema.semantic-web.at/ppt/inSubtree> <http://vocabulary.semantic-web.at/cocktails/403d1249-f37f-4f43-bebf-8dde9677d886> ;
	<http://vocabulary.semantic-web.at/cocktail-ontology/is-part-of> <http://vocabulary.semantic-web.at/cocktails/72a77af2-bbee-4b75-871f-a96dcd3a452b> , <http://vocabulary.semantic-web.at/cocktails/ea946e07-e812-4492-a0ed-124d73bfbba7> ;
	a <http://vocabulary.semantic-web.at/cocktail-ontology/Alcoholic-Beverages> , <http://vocabulary.semantic-web.at/cocktail-ontology/Beverages> , <http://vocabulary.semantic-web.at/cocktail-ontology/Ingredients> , skos:Concept ;
	skos:altLabel "Cassis de Dijon"@en , "Cassis de dijon"@en , "Cream of blackcurrant"@en , "Creme De Cassis"@en , "Creme de Cassis"@en , "Creme de cassis"@en ;
	skos:broader <http://vocabulary.semantic-web.at/cocktails/0f6d360f-af24-4d66-8f70-760c927ed0a7> , <http://vocabulary.semantic-web.at/cocktails/47635419-edef-4b78-8da1-e58a96d96f61> ;
	skos:definition "Crème de cassis is a sweet, dark red liqueur made from blackcurrants. Several cocktails are made with crème de cassis, including the very popular wine cocktail, kir. It may also be served as an after-dinner liqueur or as a frappé."@en ;
	skos:exactMatch dbpedia:Cr%C3%A8me_de_cassis ;
	skos:prefLabel "Crème de cassis"@en .

<http://vocabulary.semantic-web.at/cocktails/698723d7-e8b8-410e-91a8-9bdc867b3f8a> dcterms:contributor <http://localhost/user/blumauera> ;
	dcterms:created "2015-05-01T07:41:10Z"^^xsd:dateTime ;
	dcterms:creator <http://localhost/user/blumauera> ;
	dcterms:modified "2015-11-13T14:27:46Z"^^xsd:dateTime ;
	<http://schema.semantic-web.at/ppt/inScheme> <http://vocabulary.semantic-web.at/cocktails/8d052dfc-44bf-4985-8ce3-4564570a161b> ;
	<http://vocabulary.semantic-web.at/cocktail-ontology/consists-of> <http://vocabulary.semantic-web.at/cocktails/876f13e0-d873-4a11-94e1-e344b80cd53f> , <http://vocabulary.semantic-web.at/cocktails/a293047d-788b-4e8c-96bc-65e62fec4b0b> ;
	<http://vocabulary.semantic-web.at/cocktail-ontology/iba> <http://www.iba-world.com/index.php?option=com_content&id=214&Itemid=532> ;
	<http://vocabulary.semantic-web.at/cocktail-ontology/image> <http://upload.wikimedia.org/wikipedia/commons/thumb/d/d5/Bellini_Cipriani%2C_Macaroni_Grill%2C_Dunwoody_GA.jpg/440px-Bellini_Cipriani%2C_Macaroni_Grill%2C_Dunwoody_GA.jpg> ;
	<http://vocabulary.semantic-web.at/cocktail-ontology/preparation> "Pour peach puree into chilled glass and add sparkling wine. Stir gently."@en ;
	<http://vocabulary.semantic-web.at/cocktail-ontology/served> "Straight up; without ice"@en ;
	<http://vocabulary.semantic-web.at/cocktail-ontology/uses> <http://vocabulary.semantic-web.at/cocktails/fece03b5-ec0b-4e47-964d-cc5dc09fd7fb> ;
	a <http://vocabulary.semantic-web.at/cocktail-ontology/Cocktail> , skos:Concept ;
	skos:altLabel "Bellini (drink)"@en , "Bellini cocktail"@en ;
	skos:broader <http://vocabulary.semantic-web.at/cocktails/204cd4e7-58d7-4417-837a-7f9cc41663c8> , <http://vocabulary.semantic-web.at/cocktails/b9bf3799-a4e4-47f7-9aea-7697cc998a34> ;
	skos:definition "A Bellini cocktail is a mixture of Prosecco sparkling wine and peach purée. Originating in Venice, it is one of Italy's most popular long drinks."@en ;
	skos:exactMatch <http://dbpedia.org/resource/Bellini_(cocktail)> ;
	skos:prefLabel "Bellini"@en .

<http://vocabulary.semantic-web.at/cocktails/6c0607a9-410d-4b65-87a1-b189a8e36352> dcterms:contributor <http://localhost/user/blumauera> ;
	dcterms:created "2015-05-01T07:57:02Z"^^xsd:dateTime ;
	dcterms:creator <http://localhost/user/blumauera> ;
	dcterms:modified "2015-05-05T07:17:47Z"^^xsd:dateTime ;
	<http://schema.semantic-web.at/ppt/inScheme> <http://vocabulary.semantic-web.at/cocktails/591cf89a-57af-49b8-9042-3fc77408c93e> ;
	<http://schema.semantic-web.at/ppt/inSubtree> <http://vocabulary.semantic-web.at/cocktails/e86c1671-4a67-494b-ae5d-bcb750865acc> ;
	a <http://vocabulary.semantic-web.at/cocktail-ontology/Beverages> , <http://vocabulary.semantic-web.at/cocktail-ontology/Ingredients> , <http://vocabulary.semantic-web.at/cocktail-ontology/Non-alcoholic-Beverages> , skos:Concept ;
	skos:altLabel "Bottled juice"@en , "Fruit drink"@en , "Fruit extract"@en , "Fruit juice"@en , "Fruit juices"@en , "Fruitextract"@en , "Juice bar"@en , "Juicebar"@en , "Juices"@en ;
	skos:broader <http://vocabulary.semantic-web.at/cocktails/e86c1671-4a67-494b-ae5d-bcb750865acc> ;
	skos:definition "Juice is a liquid that is naturally contained in fruit and vegetables. It can also refer to liquids that are flavored with these or other biological food sources such as meat and seafood. It is commonly consumed as a beverage or used as an ingredient or flavoring in foods. Juice is prepared by mechanically squeezing or macerating fruit or vegetable flesh without the application of heat or solvents."@en ;
	skos:exactMatch dbpedia:Juice ;
	skos:narrower <http://vocabulary.semantic-web.at/cocktails/12da816f-8ad3-487d-b8f9-2190e4b3e1b8> , <http://vocabulary.semantic-web.at/cocktails/2ce50273-13b2-4ba1-9ff2-8cfbd835c1f2> , <http://vocabulary.semantic-web.at/cocktails/441a0d9e-f4e1-434a-9cb4-503bb840e23a> , <http://vocabulary.semantic-web.at/cocktails/45234a8f-9357-49d2-931b-638c48e3772e> , <http://vocabulary.semantic-web.at/cocktails/48499a53-a687-4156-b966-1e16e3e967bd> , <http://vocabulary.semantic-web.at/cocktails/88f5de3d-3de4-4a2f-9523-50bc7bb06600> , <http://vocabulary.semantic-web.at/cocktails/9c2ce399-c6ae-4f4d-bf37-7fd8ffe2a19d> , <http://vocabulary.semantic-web.at/cocktails/abe8b872-3a29-49a3-9a8e-1b71db770a3f> ;
	skos:prefLabel "Juice"@en .

<http://vocabulary.semantic-web.at/cocktails/6f6c504d-2272-4561-b46b-35bbccad8355> dcterms:contributor <http://localhost/user/blumauera> ;
	dcterms:created "2015-05-06T12:31:06Z"^^xsd:dateTime ;
	dcterms:creator <http://localhost/user/blumauera> ;
	dcterms:modified "2015-05-06T12:31:34Z"^^xsd:dateTime ;
	<http://schema.semantic-web.at/ppt/inScheme> <http://vocabulary.semantic-web.at/cocktails/eff672ac-6601-42c6-a3e9-0adda3b45df8> ;
	<http://schema.semantic-web.at/ppt/inSubtree> <http://vocabulary.semantic-web.at/cocktails/469959a3-10dc-4539-80ff-08bf9ff2de1c> ;
	<http://vocabulary.semantic-web.at/cocktail-ontology/is-part-of> <http://vocabulary.semantic-web.at/cocktails/268fb62f-8ef1-45cd-844f-8c7da85a6a0b> ;
	a <http://vocabulary.semantic-web.at/cocktail-ontology/Garnish> , <http://vocabulary.semantic-web.at/cocktail-ontology/Ingredients> , skos:Concept ;
	skos:broader <http://vocabulary.semantic-web.at/cocktails/e2d63a1c-56e7-47d2-b01b-8cf88cac3d8b> ;
	skos:definition "Celery salt is a flavored salt used as a food seasoning, made from ground seeds, which may come from celery or its relative lovage. These ground seeds are mixed with salt, either table salt or sea salt. Celery salt is an ingredient of the Bloody Mary cocktail and the Caesar cocktail. It is also commonly used to season the famous Chicago-style hot dog, the New York System wiener, salads, and stews. It can also be used to liven up a coleslaw. It is a primary ingredient in Old Bay brand seasoning."@en ;
	skos:exactMatch dbpedia:Celery_salt ;
	skos:prefLabel "Celery salt"@en .

<http://vocabulary.semantic-web.at/cocktails/6fe33361-f993-416d-bc13-cb36c326736b> dcterms:contributor <http://localhost/user/blumauera> ;
	dcterms:created "2015-05-02T08:21:31Z"^^xsd:dateTime ;
	dcterms:creator <http://localhost/user/Andreas-Blumauer> ;
	dcterms:description "Sauces used to mix Cocktails"@en ;
	dcterms:modified "2015-05-05T13:02:39Z"^^xsd:dateTime ;
	dcterms:publisher <http://localhost/user/Semantic-Web-Company> ;
	dcterms:subject "How to mix the best Cocktails"@en ;
	dcterms:title "Sauces"@en ;
	<http://schema.semantic-web.at/ppt/appliedType> <http://vocabulary.semantic-web.at/cocktail-ontology/Ingredients> ;
	a skos:ConceptScheme ;
	rdfs:label "Saueces"@en ;
	skos:hasTopConcept <http://vocabulary.semantic-web.at/cocktails/105184cf-c7fa-4e7c-b668-b4db7a689ab7> , <http://vocabulary.semantic-web.at/cocktails/790d1a2d-d20b-4ecd-a3d0-f9a931156e14> .

<http://vocabulary.semantic-web.at/cocktails/70bf85cb-53bb-4ebd-8bcb-e5efe304e5e2> dcterms:contributor <http://localhost/user/blumauera> ;
	dcterms:created "2015-05-02T17:33:37Z"^^xsd:dateTime ;
	dcterms:creator <http://localhost/user/blumauera> ;
	dcterms:modified "2015-05-02T17:33:37Z"^^xsd:dateTime ;
	<http://schema.semantic-web.at/ppt/inScheme> <http://vocabulary.semantic-web.at/cocktails/87384ce8-f20a-4201-b06d-3e0b8d832e5d> ;
	a <http://vocabulary.semantic-web.at/cocktail-ontology/Ingredients> , skos:Concept ;
	skos:altLabel "Orgeat"@en , "Soumada"@en , "Soumatha"@en ;
	skos:broader <http://vocabulary.semantic-web.at/cocktails/0e385475-f369-4832-b8e3-20f35028988d> ;
	skos:definition "Orgeat syrup is a sweet syrup made from almonds, sugar and rose water or orange flower water. It was, however, originally made with a barley-almond blend. It has a pronounced almond taste and is used to flavor many cocktails, perhaps the most famous of which is the Mai Tai. The word \"orgeat\" is derived from the Latin hordeata \"made with barley\" through the French, where barley is called orge. The Spanish word horchata has the same origin, though today the two drinks have little else in common."@en ;
	skos:exactMatch dbpedia:Orgeat_syrup ;
	skos:prefLabel "Orgeat syrup"@en .

<http://vocabulary.semantic-web.at/cocktails/70c69ab8-78ab-41b8-a93c-314cdeda1da4> dcterms:created "2015-05-02T19:49:40Z"^^xsd:dateTime ;
	dcterms:creator <http://localhost/user/blumauera> ;
	<http://schema.semantic-web.at/ppt/inScheme> <http://vocabulary.semantic-web.at/cocktails/591cf89a-57af-49b8-9042-3fc77408c93e> ;
	<http://schema.semantic-web.at/ppt/inSubtree> <http://vocabulary.semantic-web.at/cocktails/d5286375-41b3-468b-9602-8fcf698e3e83> ;
	a <http://vocabulary.semantic-web.at/cocktail-ontology/Alcoholic-Beverages> , <http://vocabulary.semantic-web.at/cocktail-ontology/Beverages> , <http://vocabulary.semantic-web.at/cocktail-ontology/Ingredients> , skos:Concept ;
	skos:broader <http://vocabulary.semantic-web.at/cocktails/d5286375-41b3-468b-9602-8fcf698e3e83> ;
	skos:narrower <http://vocabulary.semantic-web.at/cocktails/108f19eb-a64b-47ce-b25f-c15049a0f4be> ;
	skos:prefLabel "Aperitif wine"@en .

<http://vocabulary.semantic-web.at/cocktails/71210bd1-3071-4533-8da4-fe0f7d7694a0> dcterms:contributor <http://localhost/user/blumauera> ;
	dcterms:created "2015-05-01T14:27:55Z"^^xsd:dateTime ;
	dcterms:creator <http://localhost/user/blumauera> ;
	dcterms:modified "2015-05-06T12:50:16Z"^^xsd:dateTime ;
	<http://schema.semantic-web.at/ppt/inScheme> <http://vocabulary.semantic-web.at/cocktails/87384ce8-f20a-4201-b06d-3e0b8d832e5d> ;
	<http://vocabulary.semantic-web.at/cocktail-ontology/is-part-of> <http://vocabulary.semantic-web.at/cocktails/383ea520-07b2-4dc9-8827-8fc84fb7749c> , <http://vocabulary.semantic-web.at/cocktails/43b786b6-a1f1-4b7f-a5d9-be43d386ffb4> , <http://vocabulary.semantic-web.at/cocktails/53a05366-d473-4eb4-ac66-0d0119e0b759> , <http://vocabulary.semantic-web.at/cocktails/563bf7e0-0f40-41b6-a749-c4e94760204d> , <http://vocabulary.semantic-web.at/cocktails/72a77af2-bbee-4b75-871f-a96dcd3a452b> , <http://vocabulary.semantic-web.at/cocktails/7e5afb63-30ec-42b4-a9f5-f61fc456107d> , <http://vocabulary.semantic-web.at/cocktails/9c287d15-c699-4f56-bd65-bf8cc75a2cca> , <http://vocabulary.semantic-web.at/cocktails/a73d88e9-0c50-45d2-b364-9dec5abe206d> , <http://vocabulary.semantic-web.at/cocktails/bab016bd-2fd5-4809-bfe7-3225d25f116d> , <http://vocabulary.semantic-web.at/cocktails/c151ee28-45d2-4128-8587-1f1b69060d9d> ;
	a <http://vocabulary.semantic-web.at/cocktail-ontology/Ingredients> , skos:Concept ;
	skos:altLabel "Simple syrup"@en ;
	skos:broader <http://vocabulary.semantic-web.at/cocktails/0e385475-f369-4832-b8e3-20f35028988d> ;
	skos:prefLabel "Sugar syrup"@en .

<http://vocabulary.semantic-web.at/cocktails/71399fc3-e67c-4b55-88a7-64c6b96128bc> dcterms:contributor <http://localhost/user/blumauera> ;
	dcterms:created "2015-05-02T07:25:18Z"^^xsd:dateTime ;
	dcterms:creator <http://localhost/user/blumauera> ;
	dcterms:modified "2015-05-02T07:25:19Z"^^xsd:dateTime ;
	<http://schema.semantic-web.at/ppt/inScheme> <http://vocabulary.semantic-web.at/cocktails/591cf89a-57af-49b8-9042-3fc77408c93e> ;
	<http://schema.semantic-web.at/ppt/inSubtree> <http://vocabulary.semantic-web.at/cocktails/d5286375-41b3-468b-9602-8fcf698e3e83> ;
	a <http://vocabulary.semantic-web.at/cocktail-ontology/Alcoholic-Beverages> , <http://vocabulary.semantic-web.at/cocktail-ontology/Beverages> , <http://vocabulary.semantic-web.at/cocktail-ontology/Ingredients> , skos:Concept ;
	skos:altLabel "Brut (sparkling wine)"@en , "Brut (wine)"@en , "Brut zero"@en , "Cap Classique"@en , "Cremant"@en , "Cremant de Bourgogne"@en , "Cremant de Loire"@en , "Cremants"@en , "Crémant"@en , "Crémant de Bordeaux"@en , "Crémant de Bourgogne"@en , "Crémant de Loire"@en , "Demi-sec"@en , "Extra dry"@en , "Extra sec"@en , "Frizzante"@en , "Frizzantino"@en , "History of Spumante"@en , "Methode Cap Classique"@en , "Mousseux"@en , "Perlant"@en , "Petillant"@en , "Pezsgő"@en , "Pétillant"@en , "Sekt"@en , "Semi Sparkling Wine"@en , "Semi Sparkling wine"@en , "Semi-Sparkling wine"@en , "Semi-Sparkling wines"@en , "Semi-sparkling"@en , "Semi-sparkling wine"@en , "Semi-sparkling wines"@en , "Slightly sparkling (wine)"@en , "Sparkling (wine)"@en , "Sparkling red wine"@en , "Sparkling white wine champagne"@en , "Sparkling wines"@en , "Spritz (wine)"@en , "Spumante"@en , "Spumanti"@en , "The Steven the Great Cellars"@en , "Vino de Aguja"@en , "Vino spumante"@en , "Zero brut"@en ;
	skos:broader <http://vocabulary.semantic-web.at/cocktails/d5286375-41b3-468b-9602-8fcf698e3e83> ;
	skos:definition "Sparkling wine is a wine with significant levels of carbon dioxide in it making it fizzy. The carbon dioxide may result from natural fermentation, either in a bottle, as with the méthode champenoise, in a large tank designed to withstand the pressures involved (as in the Charmat process), or as a result of carbon dioxide injection. Sparkling wine is usually white or rosé but there are many examples of red sparkling wines such as Italian Brachetto and Australian sparkling Shiraz."@en ;
	skos:exactMatch dbpedia:Sparkling_wine ;
	skos:narrower <http://vocabulary.semantic-web.at/cocktails/a293047d-788b-4e8c-96bc-65e62fec4b0b> , <http://vocabulary.semantic-web.at/cocktails/cdbac85a-d5b7-40f3-9e98-4d7e176b5565> ;
	skos:prefLabel "Sparkling wine"@en .

<http://vocabulary.semantic-web.at/cocktails/72a77af2-bbee-4b75-871f-a96dcd3a452b> dcterms:contributor <http://localhost/user/blumauera> ;
	dcterms:created "2015-05-02T19:31:43Z"^^xsd:dateTime ;
	dcterms:creator <http://localhost/user/blumauera> ;
	dcterms:modified "2015-05-05T07:54:08Z"^^xsd:dateTime ;
	<http://schema.semantic-web.at/ppt/inScheme> <http://vocabulary.semantic-web.at/cocktails/8d052dfc-44bf-4985-8ce3-4564570a161b> ;
	<http://vocabulary.semantic-web.at/cocktail-ontology/consists-of> <http://vocabulary.semantic-web.at/cocktails/22df810d-e509-4da8-979c-0758e94de3e6> , <http://vocabulary.semantic-web.at/cocktails/687a5d86-1f4e-4a6b-b5ca-3b5d74aeafcc> , <http://vocabulary.semantic-web.at/cocktails/71210bd1-3071-4533-8da4-fe0f7d7694a0> , <http://vocabulary.semantic-web.at/cocktails/9c2ce399-c6ae-4f4d-bf37-7fd8ffe2a19d> ;
	<http://vocabulary.semantic-web.at/cocktail-ontology/iba> <http://www.iba-world.com/index.php?option=com_content&id=247&Itemid=532> ;
	<http://vocabulary.semantic-web.at/cocktail-ontology/image> <http://www.iba-world.com/images/cocktail_drinks/russian_spring.jpg> ;
	<http://vocabulary.semantic-web.at/cocktail-ontology/preparation> "Shake the ingredients and pour into highball glass. Top with Sparkling wine. Garnish with a lemon slice and a blackberry."@en ;
	<http://vocabulary.semantic-web.at/cocktail-ontology/uses> <http://vocabulary.semantic-web.at/cocktails/a54d2096-6214-4006-beaf-afcc77824710> ;
	<http://vocabulary.semantic-web.at/cocktail-ontology/uses_2> <http://vocabulary.semantic-web.at/cocktails/33df103a-03ac-4177-b620-7953fe094236> , <http://vocabulary.semantic-web.at/cocktails/7c4a2cfe-6750-419a-87d1-dcb4919ff92b> ;
	a <http://vocabulary.semantic-web.at/cocktail-ontology/Cocktail> , skos:Concept ;
	skos:broader <http://vocabulary.semantic-web.at/cocktails/ccee1079-43df-4ff1-bef0-d15d3dc8fa6f> ;
	skos:prefLabel "Russian Spring Punch"@en .

<http://vocabulary.semantic-web.at/cocktails/72cf9c86-734f-4954-b4c2-f02ee89373e8> dcterms:contributor <http://localhost/user/blumauera> ;
	dcterms:created "2015-05-05T08:05:00Z"^^xsd:dateTime ;
	dcterms:creator <http://localhost/user/blumauera> ;
	dcterms:modified "2015-05-05T12:57:23Z"^^xsd:dateTime ;
	<http://schema.semantic-web.at/ppt/inScheme> <http://vocabulary.semantic-web.at/cocktails/87384ce8-f20a-4201-b06d-3e0b8d832e5d> ;
	<http://vocabulary.semantic-web.at/cocktail-ontology/is-part-of> <http://vocabulary.semantic-web.at/cocktails/7e4a73d5-f73d-4890-972c-f3dfd6952fd8> ;
	a <http://vocabulary.semantic-web.at/cocktail-ontology/Ingredients> , skos:Concept ;
	skos:altLabel "Agave honey"@en , "Agave sweetener"@en , "Agave syrup"@en ;
	skos:broader <http://vocabulary.semantic-web.at/cocktails/0e385475-f369-4832-b8e3-20f35028988d> ;
	skos:definition "Agave nectar (also called agave syrup) is a sweetener commercially produced from several species of agave, including Agave tequilana (blue agave) and. Agave nectar is sweeter than honey and tends to be thinner and flow more freely than honey. Most agave nectar comes from Mexico and South Africa."@en ;
	skos:exactMatch dbpedia:Agave_nectar ;
	skos:prefLabel "Agave nectar"@en .

<http://vocabulary.semantic-web.at/cocktails/7448dbed-7603-41f7-a316-99f754c9ae45> dcterms:contributor <http://localhost/user/blumauera> ;
	dcterms:created "2015-05-01T08:34:11Z"^^xsd:dateTime ;
	dcterms:creator <http://localhost/user/blumauera> ;
	dcterms:modified "2015-05-07T06:58:48Z"^^xsd:dateTime ;
	<http://schema.semantic-web.at/ppt/inScheme> <http://vocabulary.semantic-web.at/cocktails/591cf89a-57af-49b8-9042-3fc77408c93e> ;
	<http://schema.semantic-web.at/ppt/inSubtree> <http://vocabulary.semantic-web.at/cocktails/e86c1671-4a67-494b-ae5d-bcb750865acc> ;
	<http://vocabulary.semantic-web.at/cocktail-ontology/is-part-of> <http://vocabulary.semantic-web.at/cocktails/2c682ed8-e2ba-473e-8cb7-979598080e18> , <http://vocabulary.semantic-web.at/cocktails/383ea520-07b2-4dc9-8827-8fc84fb7749c> , <http://vocabulary.semantic-web.at/cocktails/53a05366-d473-4eb4-ac66-0d0119e0b759> , <http://vocabulary.semantic-web.at/cocktails/b0885ae3-68e1-453d-8669-119e8464ff5f> , <http://vocabulary.semantic-web.at/cocktails/bee1e709-b317-4f46-b06f-a22367baefdf> , <http://vocabulary.semantic-web.at/cocktails/c151ee28-45d2-4128-8587-1f1b69060d9d> ;
	a <http://vocabulary.semantic-web.at/cocktail-ontology/Beverages> , <http://vocabulary.semantic-web.at/cocktail-ontology/Ingredients> , <http://vocabulary.semantic-web.at/cocktail-ontology/Non-alcoholic-Beverages> , skos:Concept ;
	skos:altLabel "Bubbly water"@en , "Carbonate water"@en , "Carbonated water"@en , "Carbonated waters"@en , "Club Soda"@en , "Club soda"@en , "Eau avec gaz"@en , "Fizzy water"@en , "L'eau avec gaz"@en , "Seltzer water"@en , "Soda-water"@en , "Sparkling Water"@en , "Sparkling water"@en , "Two Cents Plain"@en , "Unflavored Soda"@en ;
	skos:broader <http://vocabulary.semantic-web.at/cocktails/84c72e0e-7830-46ef-ac35-44cad56d27ec> ;
	skos:definition "Carbonated water (also known as club soda, soda water, sparkling water, seltzer water, or fizzy water) is water into which carbon dioxide gas under pressure has been dissolved, a process that causes the water to become effervescent. Carbonated water is the defining ingredient of carbonated soft drinks. The process of dissolving carbon dioxide in water is called carbonation."@en ;
	skos:exactMatch dbpedia:Carbonated_water ;
	skos:prefLabel "Soda water"@en .

<http://vocabulary.semantic-web.at/cocktails/7516b400-963a-4151-8fdc-f6b23bad1dd5> dcterms:contributor <http://localhost/user/blumauera> ;
	dcterms:created "2015-05-01T14:35:10Z"^^xsd:dateTime ;
	dcterms:creator <http://localhost/user/blumauera> ;
	dcterms:modified "2016-08-04T14:12:47Z"^^xsd:dateTime ;
	<http://schema.semantic-web.at/ppt/inScheme> <http://vocabulary.semantic-web.at/cocktails/8d052dfc-44bf-4985-8ce3-4564570a161b> ;
	a <http://vocabulary.semantic-web.at/cocktail-ontology/Cocktail> , skos:Concept ;
	skos:altLabel "Sour Cocktail"@en ;
	skos:definition "A sour is a traditional family of mixed drinks; the word itself is often used as a post-positive adjective when in the name of a drink. Common examples of sours are the margarita and the sidecar. Sours belong to one of the old families of original cocktails and are described by Jerry Thomas in his 1862 book How to Mix Drinks. Sours are mixed drinks containing a base liquor (bourbon or some other whiskey in the case of a whiskey sour), lemon or lime juice, egg white, and a sweetener."@en ;
	skos:exactMatch <http://dbpedia.org/resource/Sour_(cocktail)> ;
	skos:narrower <http://vocabulary.semantic-web.at/cocktails/2d85fb1b-96cb-4c48-8df5-707032f34e71> , <http://vocabulary.semantic-web.at/cocktails/36671f9c-904a-4629-937a-519d094ecefc> , <http://vocabulary.semantic-web.at/cocktails/43b786b6-a1f1-4b7f-a5d9-be43d386ffb4> , <http://vocabulary.semantic-web.at/cocktails/53a05366-d473-4eb4-ac66-0d0119e0b759> , <http://vocabulary.semantic-web.at/cocktails/76c0e55c-22df-4489-9551-4fe8a6a649f8> , <http://vocabulary.semantic-web.at/cocktails/7e4a73d5-f73d-4890-972c-f3dfd6952fd8> , <http://vocabulary.semantic-web.at/cocktails/a47e8f08-057a-45f2-8398-9be51ed351fc> , <http://vocabulary.semantic-web.at/cocktails/b33091cd-8c57-45e3-a89b-9de91ffce1e8> , <http://vocabulary.semantic-web.at/cocktails/bab016bd-2fd5-4809-bfe7-3225d25f116d> , <http://vocabulary.semantic-web.at/cocktails/bca7bc6d-6709-48b8-ae52-fe194c212398> , <http://vocabulary.semantic-web.at/cocktails/c151ee28-45d2-4128-8587-1f1b69060d9d> , <http://vocabulary.semantic-web.at/cocktails/e039633b-03c1-47bd-a705-a104a4323e45> ;
	skos:prefLabel "Sour"@en ;
	skos:topConceptOf <http://vocabulary.semantic-web.at/cocktails/8d052dfc-44bf-4985-8ce3-4564570a161b> .

<http://vocabulary.semantic-web.at/cocktails/76c0e55c-22df-4489-9551-4fe8a6a649f8> dcterms:contributor <http://localhost/user/huberf> ;
	dcterms:created "2015-05-02T07:14:54Z"^^xsd:dateTime ;
	dcterms:creator <http://localhost/user/blumauera> ;
	dcterms:modified "2016-10-05T09:32:33Z"^^xsd:dateTime ;
	<http://schema.semantic-web.at/ppt/inScheme> <http://vocabulary.semantic-web.at/cocktails/8d052dfc-44bf-4985-8ce3-4564570a161b> ;
	<http://vocabulary.semantic-web.at/cocktail-ontology/consists-of> <http://vocabulary.semantic-web.at/cocktails/3e2d26b8-928b-462d-99ee-59eac11b241f> , <http://vocabulary.semantic-web.at/cocktails/457aff50-b86b-4879-8e17-41ca59cf03a7> , <http://vocabulary.semantic-web.at/cocktails/98f20476-57d7-46d3-b76d-6aac18b57788> , <http://vocabulary.semantic-web.at/cocktails/9c2ce399-c6ae-4f4d-bf37-7fd8ffe2a19d> ;
	<http://vocabulary.semantic-web.at/cocktail-ontology/iba> <http://www.iba-world.com/index.php?option=com_content&id=211&Itemid=532> ;
	<http://vocabulary.semantic-web.at/cocktail-ontology/image> <http://upload.wikimedia.org/wikipedia/commons/thumb/5/59/Whiskey_Sour.jpg/440px-Whiskey_Sour.jpg> ;
	<http://vocabulary.semantic-web.at/cocktail-ontology/preparation> "Shake with ice. Strain into ice-filled old-fashioned glass to serve 'on the rocks.'"@en ;
	<http://vocabulary.semantic-web.at/cocktail-ontology/served> "shaken"@en ;
	<http://vocabulary.semantic-web.at/cocktail-ontology/uses> <http://vocabulary.semantic-web.at/cocktails/2dce3576-2603-41f9-8dce-ab21f639c2a7> ;
	<http://vocabulary.semantic-web.at/cocktail-ontology/uses_2> <http://vocabulary.semantic-web.at/cocktails/8a5e1790-d3c0-432e-bb85-709692b14f03> , <http://vocabulary.semantic-web.at/cocktails/99171f20-c59f-40c4-998a-a9c8f1909168> ;
	a <http://vocabulary.semantic-web.at/cocktail-ontology/Cocktail> , skos:Concept ;
	skos:altLabel "Boston sour"@en , "Whiskey Sour (cocktail)"@en , "Whiskey sour (cocktail)"@en , "Whisky Sour"@en , "Whisky sour"@en ;
	skos:broader <http://vocabulary.semantic-web.at/cocktails/7516b400-963a-4151-8fdc-f6b23bad1dd5> , <http://vocabulary.semantic-web.at/cocktails/caae2ea0-7e60-400b-a2bb-14ef79720668> ;
	skos:definition "The whiskey sour is a mixed drink containing whiskey, lemon juice, sugar, and optionally, a dash of egg white to make it a Boston Sour. It is shaken and served either straight or over ice. The traditional garnish is half an orange slice and a maraschino cherry. A notable variant of the whiskey sour is the Ward 8, which often is based either in Bourbon or rye whiskey, with both lemon and orange juices, and grenadine syrup as the sweetener."@en ;
	skos:exactMatch dbpedia:Whiskey_sour ;
	skos:prefLabel "Whiskey sour"@en .

<http://vocabulary.semantic-web.at/cocktails/7738a6e2-84c2-4ae3-b605-8bb6420e6e28> dcterms:contributor <http://localhost/user/blumauera> ;
	dcterms:created "2015-05-02T18:58:45Z"^^xsd:dateTime ;
	dcterms:creator <http://localhost/user/blumauera> ;
	dcterms:modified "2015-05-07T07:11:22Z"^^xsd:dateTime ;
	<http://schema.semantic-web.at/ppt/inScheme> <http://vocabulary.semantic-web.at/cocktails/591cf89a-57af-49b8-9042-3fc77408c93e> ;
	<http://schema.semantic-web.at/ppt/inSubtree> <http://vocabulary.semantic-web.at/cocktails/403d1249-f37f-4f43-bebf-8dde9677d886> ;
	<http://vocabulary.semantic-web.at/cocktail-ontology/is-part-of> <http://vocabulary.semantic-web.at/cocktails/dff0a7f4-ded0-48d5-bd31-881b70fbe36a> ;
	a <http://vocabulary.semantic-web.at/cocktail-ontology/Alcoholic-Beverages> , <http://vocabulary.semantic-web.at/cocktail-ontology/Beverages> , <http://vocabulary.semantic-web.at/cocktail-ontology/Ingredients> , skos:Concept ;
	skos:broader <http://vocabulary.semantic-web.at/cocktails/27c48d24-bb0b-46a3-9b0c-4b09e38a4b07> ;
	skos:prefLabel "Peach schnapps"@en .

<http://vocabulary.semantic-web.at/cocktails/785b30fd-1eb4-445b-8247-7e1e57b35b0f> dcterms:contributor <http://localhost/user/turdeant> ;
	dcterms:created "2015-05-01T14:45:03Z"^^xsd:dateTime ;
	dcterms:creator <http://localhost/user/blumauera> ;
	dcterms:modified "2015-09-04T22:17:31Z"^^xsd:dateTime ;
	<http://schema.semantic-web.at/ppt/inScheme> <http://vocabulary.semantic-web.at/cocktails/8d052dfc-44bf-4985-8ce3-4564570a161b> ;
	<http://vocabulary.semantic-web.at/cocktail-ontology/consists-of> <http://vocabulary.semantic-web.at/cocktails/12da816f-8ad3-487d-b8f9-2190e4b3e1b8> , <http://vocabulary.semantic-web.at/cocktails/224b4628-2f46-44a1-9d2f-8b5ef0b31e79> , <http://vocabulary.semantic-web.at/cocktails/ced2e755-fe48-4d7b-86ab-6b39fe359a32> , <http://vocabulary.semantic-web.at/cocktails/f5cd2a2b-2153-4b7e-ae79-678b939765ca> ;
	<http://vocabulary.semantic-web.at/cocktail-ontology/iba> <http://www.iba-world.com/index.php?option=com_content&id=199&Itemid=532> ;
	<http://vocabulary.semantic-web.at/cocktail-ontology/image> <http://az659704.vo.msecnd.net/v1/image/c_lpad,w_1500,h_1500/v1400600711/cocktail_mary_pickford-1.png> ;
	<http://vocabulary.semantic-web.at/cocktail-ontology/preparation> "Shake and strain into a chilled large cocktail glass."@en ;
	<http://vocabulary.semantic-web.at/cocktail-ontology/uses> <http://vocabulary.semantic-web.at/cocktails/19dee0d8-fd30-469f-9ecd-91c902ff717c> ;
	<http://vocabulary.semantic-web.at/cocktail-ontology/uses_2> <http://vocabulary.semantic-web.at/cocktails/8a5e1790-d3c0-432e-bb85-709692b14f03> ;
	a <http://vocabulary.semantic-web.at/cocktail-ontology/Cocktail> , skos:Concept ;
	skos:broader <http://vocabulary.semantic-web.at/cocktails/caae2ea0-7e60-400b-a2bb-14ef79720668> ;
	skos:prefLabel "Mary Pickford"@en .

<http://vocabulary.semantic-web.at/cocktails/78ace24b-5e26-42f8-9f4f-3106576118cc> dcterms:contributor <http://localhost/user/blumauera> ;
	dcterms:created "2015-05-02T18:32:15Z"^^xsd:dateTime ;
	dcterms:creator <http://localhost/user/blumauera> ;
	dcterms:modified "2015-05-02T18:32:15Z"^^xsd:dateTime ;
	<http://schema.semantic-web.at/ppt/inScheme> <http://vocabulary.semantic-web.at/cocktails/eff672ac-6601-42c6-a3e9-0adda3b45df8> ;
	<http://schema.semantic-web.at/ppt/inSubtree> <http://vocabulary.semantic-web.at/cocktails/4f20d6bb-710d-4870-bde4-b6e835d7d13f> ;
	a <http://vocabulary.semantic-web.at/cocktail-ontology/Garnish> , <http://vocabulary.semantic-web.at/cocktail-ontology/Ingredients> , skos:Concept ;
	skos:altLabel "Ananas strawberry"@en , "Culture of strawberry"@en , "Fragaria ananassa"@en , "Fragaria x ananassa"@en , "Fragaria xananassa"@en , "Fragaria × ananassa"@en , "Fragaria ×ananassa"@en , "Fragraria"@en , "Garden Strawberry"@en , "Garden strawberries"@en , "Garden strawberry"@en , "Gariguette"@en , "Pineapple strawberry"@en , "Strawbarry"@en , "Strawberries"@en , "Strawberrys"@en , "🍓"@en ;
	skos:broader <http://vocabulary.semantic-web.at/cocktails/4f20d6bb-710d-4870-bde4-b6e835d7d13f> ;
	skos:definition "Fragaria × ananassa, commonly known as strawberry or garden strawberry, is a hybrid species that is cultivated worldwide for its fruit. The fruit (which is not a botanical berry, but an aggregate accessory fruit) is widely appreciated for its characteristic aroma, bright red color, juicy texture, and sweetness. It is consumed in large quantities, either fresh or in prepared foods such as preserves, fruit juice, pies, ice creams, milkshakes, and chocolates."@en ;
	skos:exactMatch dbpedia:Strawberry ;
	skos:prefLabel "Strawberry"@en .

<http://vocabulary.semantic-web.at/cocktails/790d1a2d-d20b-4ecd-a3d0-f9a931156e14> dcterms:contributor <http://localhost/user/huberf> ;
	dcterms:created "2015-05-05T13:01:30Z"^^xsd:dateTime ;
	dcterms:creator <http://localhost/user/blumauera> ;
	dcterms:modified "2015-11-19T15:22:43Z"^^xsd:dateTime ;
	<http://schema.semantic-web.at/ppt/inScheme> <http://vocabulary.semantic-web.at/cocktails/6fe33361-f993-416d-bc13-cb36c326736b> ;
	<http://vocabulary.semantic-web.at/cocktail-ontology/is-part-of> <http://vocabulary.semantic-web.at/cocktails/268fb62f-8ef1-45cd-844f-8c7da85a6a0b> , <http://vocabulary.semantic-web.at/cocktails/a5db05ca-eda3-41ef-a8ab-ba77b3e4baba> ;
	a <http://vocabulary.semantic-web.at/cocktail-ontology/Ingredients> , skos:Concept ;
	skos:altLabel "Salsa inglesa"@en , "Tonkatsu sauce"@en , "Wooster sauce"@en , "Worcester Sauce"@en , "Worcester Sause"@en , "Worcester sauce"@en , "Worcesterchire sauce"@en , "Worchestershire sauce"@en , "Worchestire sauce"@en , "Worstershire"@en , "Worstershire sauce"@en ;
	skos:definition "Worcestershire sauce, sometimes known as Worcester sauce, is a fermented liquid condiment, primarily used to flavour meat or fish dishes. First made at 60 Broad Street, Worcester, England, by two dispensing chemists, John Wheeley Lea and William Henry Perrins, the Lea & Perrins brand was commercialised in 1837 and has been produced in the current Midlands Road factory in Worcester since 16 October 1897. It was purchased by H.J."@en ;
	skos:exactMatch dbpedia:Worcestershire_sauce ;
	skos:prefLabel "Worcestershire sauce"@en ;
	skos:topConceptOf <http://vocabulary.semantic-web.at/cocktails/6fe33361-f993-416d-bc13-cb36c326736b> .

<http://vocabulary.semantic-web.at/cocktails/79d4686d-4f5b-4067-a2ef-99beccc51242> dcterms:contributor <http://localhost/user/blumauera> ;
	dcterms:created "2015-05-01T15:15:45Z"^^xsd:dateTime ;
	dcterms:creator <http://localhost/user/blumauera> ;
	dcterms:modified "2015-05-04T11:41:54Z"^^xsd:dateTime ;
	<http://schema.semantic-web.at/ppt/inScheme> <http://vocabulary.semantic-web.at/cocktails/8d052dfc-44bf-4985-8ce3-4564570a161b> ;
	<http://vocabulary.semantic-web.at/cocktail-ontology/consists-of> <http://vocabulary.semantic-web.at/cocktails/22df810d-e509-4da8-979c-0758e94de3e6> , <http://vocabulary.semantic-web.at/cocktails/2ce50273-13b2-4ba1-9ff2-8cfbd835c1f2> ;
	<http://vocabulary.semantic-web.at/cocktail-ontology/iba> <http://www.iba-world.com/index.php?option=com_content&id=262&Itemid=532> ;
	<http://vocabulary.semantic-web.at/cocktail-ontology/image> <http://www.iba-world.com/images/cocktail_drinks/screwdriver.jpg> ;
	<http://vocabulary.semantic-web.at/cocktail-ontology/preparation> "Mix in a highball glass with ice. Garnish and serve."@en ;
	<http://vocabulary.semantic-web.at/cocktail-ontology/served> "On the rocks; poured over ice"@en ;
	<http://vocabulary.semantic-web.at/cocktail-ontology/uses> <http://vocabulary.semantic-web.at/cocktails/a54d2096-6214-4006-beaf-afcc77824710> ;
	<http://vocabulary.semantic-web.at/cocktail-ontology/uses_2> <http://vocabulary.semantic-web.at/cocktails/99171f20-c59f-40c4-998a-a9c8f1909168> ;
	a <http://vocabulary.semantic-web.at/cocktail-ontology/Cocktail> , skos:Concept ;
	skos:altLabel "Cosmonaut (cocktail)"@en , "Hi-Fi (cocktail)"@en , "Screwdriver (drink)"@en , "Screwdriver cocktail"@en , "Screwdriver drink"@en , "Slow comfortable screw"@en , "Vodka Orange"@en , "Vodka and orange"@en ;
	skos:broader <http://vocabulary.semantic-web.at/cocktails/caae2ea0-7e60-400b-a2bb-14ef79720668> ;
	skos:definition "A screwdriver is a popular highball drink made with fresh orange juice and vodka. Outside the US, it is often referred to as \"vodka and orange\". While the basic drink is simply the two ingredients, there are many variations. Many of the variations have different names in different parts of the world. The International Bartender Association has designated this cocktail as an IBA Official Cocktail."@en ;
	skos:exactMatch <http://dbpedia.org/resource/Screwdriver_(cocktail)> ;
	skos:prefLabel "Screwdriver"@en .

<http://vocabulary.semantic-web.at/cocktails/7a2ef9c4-4083-4531-9edc-b27e0353349e> dcterms:contributor <http://localhost/user/blumauera> ;
	dcterms:created "2015-05-03T18:59:00Z"^^xsd:dateTime ;
	dcterms:creator <http://localhost/user/blumauera> ;
	dcterms:modified "2015-05-03T18:59:23Z"^^xsd:dateTime ;
	<http://schema.semantic-web.at/ppt/inScheme> <http://vocabulary.semantic-web.at/cocktails/591cf89a-57af-49b8-9042-3fc77408c93e> ;
	<http://schema.semantic-web.at/ppt/inSubtree> <http://vocabulary.semantic-web.at/cocktails/403d1249-f37f-4f43-bebf-8dde9677d886> ;
	a <http://vocabulary.semantic-web.at/cocktail-ontology/Alcoholic-Beverages> , <http://vocabulary.semantic-web.at/cocktail-ontology/Beverages> , <http://vocabulary.semantic-web.at/cocktail-ontology/Ingredients> , skos:Concept ;
	skos:broader <http://vocabulary.semantic-web.at/cocktails/1b9d9c87-9a94-465a-b7e9-feee6c77bf03> , <http://vocabulary.semantic-web.at/cocktails/40362aa1-0058-4f25-ba82-74bcd2202cc4> ;
	skos:prefLabel "Cinzano Bianco"@en .

<http://vocabulary.semantic-web.at/cocktails/7c4a2cfe-6750-419a-87d1-dcb4919ff92b> dcterms:contributor <http://localhost/user/blumauera> ;
	dcterms:created "2015-05-05T07:09:05Z"^^xsd:dateTime ;
	dcterms:creator <http://localhost/user/blumauera> ;
	dcterms:modified "2016-04-06T11:49:35Z"^^xsd:dateTime ;
	<http://schema.semantic-web.at/ppt/inScheme> <http://vocabulary.semantic-web.at/cocktails/eff672ac-6601-42c6-a3e9-0adda3b45df8> ;
	<http://schema.semantic-web.at/ppt/inSubtree> <http://vocabulary.semantic-web.at/cocktails/4f20d6bb-710d-4870-bde4-b6e835d7d13f> ;
	<http://vocabulary.semantic-web.at/cocktail-ontology/is-used-by_2> <http://vocabulary.semantic-web.at/cocktails/563bf7e0-0f40-41b6-a749-c4e94760204d> , <http://vocabulary.semantic-web.at/cocktails/680c7429-30a7-4044-b32f-e28c99dcb9f4> , <http://vocabulary.semantic-web.at/cocktails/72a77af2-bbee-4b75-871f-a96dcd3a452b> ;
	a <http://vocabulary.semantic-web.at/cocktail-ontology/Garnish> , <http://vocabulary.semantic-web.at/cocktail-ontology/Ingredients> , skos:Concept ;
	skos:altLabel "Black Berry"@en , "Black-berry"@en , "Blackberries"@en , "Blackberry (fruit)"@en , "Blackberry Vines"@en , "Blackberry bush"@en , "Bramble Raspberry"@en , "Bramble raspberry"@en , "Bush Blackberry"@en , "Bush blackberry"@en , "Culture of blackberry"@en , "Rubus fruticosus"@en ;
	skos:broader <http://vocabulary.semantic-web.at/cocktails/4f20d6bb-710d-4870-bde4-b6e835d7d13f> ;
	skos:definition "The blackberry is an edible fruit produced by many species in the Rubus genus in the Rosaceae family, hybrids among these species within the Rubus subgenus, as well as hybrids between the Rubus and Idaeobatus subgenera. What distinguishes blackberries from its raspberry relatives is whether the torus (receptacle) picks with the fruit, a blackberry, or remains on the plant when picked leaving a hole in the fruit, a raspberry."@en ;
	skos:exactMatch dbpedia:Blackberry ;
	skos:prefLabel "Blackberry"@en .

<http://vocabulary.semantic-web.at/cocktails/7c831f82-c54d-4d31-ab40-97e1d6226cf2> dcterms:contributor <http://localhost/user/blumauera> ;
	dcterms:created "2015-05-01T08:32:37Z"^^xsd:dateTime ;
	dcterms:creator <http://localhost/user/blumauera> ;
	dcterms:modified "2015-05-04T09:43:36Z"^^xsd:dateTime ;
	<http://schema.semantic-web.at/ppt/inScheme> <http://vocabulary.semantic-web.at/cocktails/591cf89a-57af-49b8-9042-3fc77408c93e> ;
	<http://schema.semantic-web.at/ppt/inSubtree> <http://vocabulary.semantic-web.at/cocktails/403d1249-f37f-4f43-bebf-8dde9677d886> ;
	<http://vocabulary.semantic-web.at/cocktail-ontology/is-part-of> <http://vocabulary.semantic-web.at/cocktails/40ab50e9-66f1-411b-8220-ef8f05273542> , <http://vocabulary.semantic-web.at/cocktails/b0885ae3-68e1-453d-8669-119e8464ff5f> ;
	a <http://vocabulary.semantic-web.at/cocktail-ontology/Alcoholic-Beverages> , <http://vocabulary.semantic-web.at/cocktail-ontology/Beverages> , <http://vocabulary.semantic-web.at/cocktail-ontology/Ingredients> , skos:Concept ;
	skos:broader <http://vocabulary.semantic-web.at/cocktails/d40e2215-bc1b-4bae-8cf8-d10b1ad36d44> ;
	skos:definition "Campari is an alcoholic apéritif (20.5%, 21%, 24%, 25%, or 28% ABV, depending on the country in which it is sold) obtained from the infusion of herbs and fruit in alcohol and water. It is a bitters characterized by its dark red color. Campari is often used in cocktails and is commonly served with soda water, wine, or citrus juice. It is produced by the Campari Group, a multi-national company based in Italy."@en ;
	skos:exactMatch dbpedia:Campari ;
	skos:prefLabel "Campari"@en .

<http://vocabulary.semantic-web.at/cocktails/7dede323-e986-4417-b723-c9c7a7fe82ba> dcterms:contributor <http://localhost/user/blumauera> ;
	dcterms:created "2015-05-02T17:31:39Z"^^xsd:dateTime ;
	dcterms:creator <http://localhost/user/blumauera> ;
	dcterms:modified "2015-08-07T15:06:50Z"^^xsd:dateTime ;
	<http://schema.semantic-web.at/ppt/inScheme> <http://vocabulary.semantic-web.at/cocktails/591cf89a-57af-49b8-9042-3fc77408c93e> ;
	<http://schema.semantic-web.at/ppt/inSubtree> <http://vocabulary.semantic-web.at/cocktails/403d1249-f37f-4f43-bebf-8dde9677d886> ;
	<http://vocabulary.semantic-web.at/cocktail-ontology/image_3> <http://preview.poolparty.biz/sparqlingCocktails/resources/images/tequila.png> ;
	<http://vocabulary.semantic-web.at/cocktail-ontology/is-part-of> <http://vocabulary.semantic-web.at/cocktails/2d85fb1b-96cb-4c48-8df5-707032f34e71> , <http://vocabulary.semantic-web.at/cocktails/55c40695-8b41-41ed-8c6a-70fe6930067e> , <http://vocabulary.semantic-web.at/cocktails/7e4a73d5-f73d-4890-972c-f3dfd6952fd8> , <http://vocabulary.semantic-web.at/cocktails/a5db05ca-eda3-41ef-a8ab-ba77b3e4baba> , <http://vocabulary.semantic-web.at/cocktails/ce8f4591-ccd4-4d90-a761-244115d64061> ;
	a <http://vocabulary.semantic-web.at/cocktail-ontology/Alcoholic-Beverages> , <http://vocabulary.semantic-web.at/cocktail-ontology/Beverages> , <http://vocabulary.semantic-web.at/cocktail-ontology/Ingredients> , skos:Concept ;
	skos:altLabel "100% agave"@en , "Extra Añejo"@en , "List of Tequila brands"@en , "Mixtos"@en , "Reposado"@en , "Tequila Manhattan"@en , "Tequila fruit"@en , "Tequilla"@en ;
	skos:broader <http://vocabulary.semantic-web.at/cocktails/403d1249-f37f-4f43-bebf-8dde9677d886> , <http://vocabulary.semantic-web.at/cocktails/f3000285-36b0-4ffe-af90-740c2dd8fff5> ;
	skos:definition "Tequila is a distilled beverage made from the blue agave plant, primarily in the area surrounding the city of Tequila, 65 kilometres northwest of Guadalajara, and in the highlands of the western Mexican state of Jalisco. The blue volcanic soil in the surrounding region is particularly well suited to the growing of the blue agave, and more than 300 million of the plants are harvested there each year. Agave tequila grows differently depending on the region."@en ;
	skos:exactMatch dbpedia:Tequila ;
	skos:prefLabel "Tequila"@en .

<http://vocabulary.semantic-web.at/cocktails/7e4a73d5-f73d-4890-972c-f3dfd6952fd8> dcterms:contributor <http://localhost/user/blumauera> ;
	dcterms:created "2015-05-02T19:43:11Z"^^xsd:dateTime ;
	dcterms:creator <http://localhost/user/blumauera> ;
	dcterms:modified "2015-05-05T12:57:52Z"^^xsd:dateTime ;
	<http://schema.semantic-web.at/ppt/inScheme> <http://vocabulary.semantic-web.at/cocktails/8d052dfc-44bf-4985-8ce3-4564570a161b> ;
	<http://vocabulary.semantic-web.at/cocktail-ontology/consists-of> <http://vocabulary.semantic-web.at/cocktails/72cf9c86-734f-4954-b4c2-f02ee89373e8> , <http://vocabulary.semantic-web.at/cocktails/7dede323-e986-4417-b723-c9c7a7fe82ba> , <http://vocabulary.semantic-web.at/cocktails/88f5de3d-3de4-4a2f-9523-50bc7bb06600> ;
	<http://vocabulary.semantic-web.at/cocktail-ontology/iba> <http://www.iba-world.com/index.php?option=com_content&id=249&Itemid=532> ;
	<http://vocabulary.semantic-web.at/cocktail-ontology/image> <http://www.iba-world.com/images/cocktail_drinks/tommy_margarita.jpg> ;
	<http://vocabulary.semantic-web.at/cocktail-ontology/is-variant-of> <http://vocabulary.semantic-web.at/cocktails/2d85fb1b-96cb-4c48-8df5-707032f34e71> ;
	<http://vocabulary.semantic-web.at/cocktail-ontology/preparation> "Shake and strain into a chilled cocktail glass."@en ;
	<http://vocabulary.semantic-web.at/cocktail-ontology/uses> <http://vocabulary.semantic-web.at/cocktails/19dee0d8-fd30-469f-9ecd-91c902ff717c> ;
	<http://vocabulary.semantic-web.at/cocktail-ontology/uses_2> <http://vocabulary.semantic-web.at/cocktails/021c85c0-a60a-4414-8fd8-bd3383b794f1> ;
	a <http://vocabulary.semantic-web.at/cocktail-ontology/Cocktail> , skos:Concept ;
	skos:broader <http://vocabulary.semantic-web.at/cocktails/7516b400-963a-4151-8fdc-f6b23bad1dd5> , <http://vocabulary.semantic-web.at/cocktails/ccee1079-43df-4ff1-bef0-d15d3dc8fa6f> ;
	skos:prefLabel "Tommy's Margarita"@en .

<http://vocabulary.semantic-web.at/cocktails/7e5afb63-30ec-42b4-a9f5-f61fc456107d> dcterms:contributor <http://localhost/user/blumauera> ;
	dcterms:created "2015-05-02T19:21:59Z"^^xsd:dateTime ;
	dcterms:creator <http://localhost/user/blumauera> ;
	dcterms:modified "2015-05-05T07:25:59Z"^^xsd:dateTime ;
	<http://schema.semantic-web.at/ppt/inScheme> <http://vocabulary.semantic-web.at/cocktails/8d052dfc-44bf-4985-8ce3-4564570a161b> ;
	<http://vocabulary.semantic-web.at/cocktail-ontology/consists-of> <http://vocabulary.semantic-web.at/cocktails/22df810d-e509-4da8-979c-0758e94de3e6> , <http://vocabulary.semantic-web.at/cocktails/71210bd1-3071-4533-8da4-fe0f7d7694a0> , <http://vocabulary.semantic-web.at/cocktails/8ba9f3ab-d600-441c-85d3-d3aeb44678d1> , <http://vocabulary.semantic-web.at/cocktails/8d5e2abc-6280-42b7-8e21-8bbc30f7509f> ;
	<http://vocabulary.semantic-web.at/cocktail-ontology/iba> <http://www.iba-world.com/index.php?option=com_content&id=242&Itemid=532> ;
	<http://vocabulary.semantic-web.at/cocktail-ontology/image> <http://upload.wikimedia.org/wikipedia/commons/thumb/8/8c/Espresso-martini.jpg/440px-Espresso-martini.jpg> ;
	<http://vocabulary.semantic-web.at/cocktail-ontology/preparation> "Pour ingredients into shaker filled with ice, shake vigorously, and strain into chilled martini glass"@en ;
	<http://vocabulary.semantic-web.at/cocktail-ontology/served> "Straight-up"@en ;
	<http://vocabulary.semantic-web.at/cocktail-ontology/uses> <http://vocabulary.semantic-web.at/cocktails/19dee0d8-fd30-469f-9ecd-91c902ff717c> ;
	<http://vocabulary.semantic-web.at/cocktail-ontology/uses_2> <http://vocabulary.semantic-web.at/cocktails/3abfd580-0f7d-4971-9c90-3cc8a5dafc0c> ;
	a <http://vocabulary.semantic-web.at/cocktail-ontology/Cocktail> , skos:Concept ;
	skos:broader <http://vocabulary.semantic-web.at/cocktails/54702498-ad42-4af6-b28a-2276215450da> , <http://vocabulary.semantic-web.at/cocktails/ccee1079-43df-4ff1-bef0-d15d3dc8fa6f> ;
	skos:definition "Espresso Martini is a coffee flavored variation of Martini and is made with coffee liqueur and vodka."@en ;
	skos:prefLabel "Espresso Martini"@en .

<http://vocabulary.semantic-web.at/cocktails/7effbf10-d493-429f-aaff-04011849774d> dcterms:contributor <http://localhost/user/blumauera> ;
	dcterms:created "2015-05-02T17:19:48Z"^^xsd:dateTime ;
	dcterms:creator <http://localhost/user/blumauera> ;
	dcterms:modified "2015-05-05T07:36:40Z"^^xsd:dateTime ;
	<http://schema.semantic-web.at/ppt/inScheme> <http://vocabulary.semantic-web.at/cocktails/eff672ac-6601-42c6-a3e9-0adda3b45df8> ;
	<http://schema.semantic-web.at/ppt/inSubtree> <http://vocabulary.semantic-web.at/cocktails/4f20d6bb-710d-4870-bde4-b6e835d7d13f> ;
	<http://vocabulary.semantic-web.at/cocktail-ontology/is-part-of> <http://vocabulary.semantic-web.at/cocktails/680c7429-30a7-4044-b32f-e28c99dcb9f4> ;
	a <http://vocabulary.semantic-web.at/cocktail-ontology/Garnish> , <http://vocabulary.semantic-web.at/cocktail-ontology/Ingredients> , skos:Concept ;
	skos:altLabel "Citrus zest"@en , "Lemon peel"@en , "Lemon zest"@en , "Orange zest"@en ;
	skos:broader <http://vocabulary.semantic-web.at/cocktails/33df103a-03ac-4177-b620-7953fe094236> ;
	skos:definition "Zest is a food ingredient that is prepared by scraping or cutting from the outer, colorful skin of citrus fruits such as lemon, orange, citron, and lime. Zest is used to add flavor (\"zest\") to foods. In terms of fruit anatomy, zest is obtained from the flavedo. The flavedo and white pith of a citrus fruit together makes up its peel. The amounts of both flavedo and pith are variable among citrus fruits, and may be adjusted by the manner in which they are prepared."@en ;
	skos:exactMatch <http://dbpedia.org/resource/Zest_(ingredient)> ;
	skos:prefLabel "Zest"@en .

<http://vocabulary.semantic-web.at/cocktails/805e18b6-0f7a-4c26-b35e-9cc68a099086> dcterms:contributor <http://localhost/user/blumauera> ;
	dcterms:created "2015-05-04T11:27:19Z"^^xsd:dateTime ;
	dcterms:creator <http://localhost/user/blumauera> ;
	dcterms:modified "2015-05-04T11:27:19Z"^^xsd:dateTime ;
	<http://schema.semantic-web.at/ppt/inScheme> <http://vocabulary.semantic-web.at/cocktails/eff672ac-6601-42c6-a3e9-0adda3b45df8> ;
	<http://schema.semantic-web.at/ppt/inSubtree> <http://vocabulary.semantic-web.at/cocktails/469959a3-10dc-4539-80ff-08bf9ff2de1c> ;
	a <http://vocabulary.semantic-web.at/cocktail-ontology/Garnish> , <http://vocabulary.semantic-web.at/cocktail-ontology/Ingredients> , skos:Concept ;
	skos:altLabel "Bourbon vanilla"@en , "French Vanilla"@en , "French vanilla"@en , "Vanila"@en , "Vanilla Beans"@en , "Vanilla bean"@en ;
	skos:broader <http://vocabulary.semantic-web.at/cocktails/469959a3-10dc-4539-80ff-08bf9ff2de1c> ;
	skos:definition "Vanilla is a flavoring derived from orchids of the genus Vanilla, primarily from the Mexican species, flat-leaved vanilla. The word vanilla, derived from the diminutive of the Spanish word vaina (vaina itself meaning sheath or pod), simply translates as little pod. Pre-Columbian Mesoamerican peoples cultivated the vine of the vanilla orchid, called tlilxochitl by the Aztecs, and Spanish conquistador Hernán Cortés is credited with introducing both vanilla and chocolate to Europe in the 1520s."@en ;
	skos:exactMatch dbpedia:Vanilla ;
	skos:narrower <http://vocabulary.semantic-web.at/cocktails/cc32e2f5-d1ae-4506-b000-86fbfee4a3e7> ;
	skos:prefLabel "Vanilla"@en .

<http://vocabulary.semantic-web.at/cocktails/809f470a-4be7-47e8-9356-cb71009c31c2> dcterms:contributor <http://localhost/user/blumauera> ;
	dcterms:created "2015-05-03T10:37:30Z"^^xsd:dateTime ;
	dcterms:creator <http://localhost/user/blumauera> ;
	dcterms:modified "2015-05-05T06:19:11Z"^^xsd:dateTime ;
	<http://schema.semantic-web.at/ppt/inScheme> <http://vocabulary.semantic-web.at/cocktails/591cf89a-57af-49b8-9042-3fc77408c93e> ;
	<http://schema.semantic-web.at/ppt/inSubtree> <http://vocabulary.semantic-web.at/cocktails/403d1249-f37f-4f43-bebf-8dde9677d886> ;
	<http://vocabulary.semantic-web.at/cocktail-ontology/is-part-of> <http://vocabulary.semantic-web.at/cocktails/1d5b39cc-fcab-48b2-bb24-9840b7e34d64> , <http://vocabulary.semantic-web.at/cocktails/44cc99c1-28ac-4c50-a55d-7244b2c5c07b> ;
	a <http://vocabulary.semantic-web.at/cocktail-ontology/Alcoholic-Beverages> , <http://vocabulary.semantic-web.at/cocktail-ontology/Beverages> , <http://vocabulary.semantic-web.at/cocktail-ontology/Ingredients> , skos:Concept ;
	skos:broader <http://vocabulary.semantic-web.at/cocktails/d40e2215-bc1b-4bae-8cf8-d10b1ad36d44> ;
	skos:definition "Orange bitters is a cocktail flavoring made from the peels of Seville oranges, cardamon, caraway seed, coriander and burnt sugar in an alcohol base. Orange bitters, which are not to be confused with standard Angostura bitters, are currently enjoying a resurgence among cocktail enthusiasts. For many years, it was difficult to find orange bitters in the United States and elsewhere. Because of this, some cocktail recipes which traditionally contained orange bitters may now exclude that ingredient."@en ;
	skos:exactMatch dbpedia:Orange_bitters ;
	skos:prefLabel "Orange bitters"@en .

<http://vocabulary.semantic-web.at/cocktails/80baac32-dfeb-461d-89cf-decf60f0709a> dcterms:contributor <http://localhost/user/blumauera> ;
	dcterms:created "2015-05-02T08:26:11Z"^^xsd:dateTime ;
	dcterms:creator <http://localhost/user/blumauera> ;
	dcterms:modified "2015-05-06T12:48:44Z"^^xsd:dateTime ;
	<http://schema.semantic-web.at/ppt/inScheme> <http://vocabulary.semantic-web.at/cocktails/591cf89a-57af-49b8-9042-3fc77408c93e> ;
	<http://schema.semantic-web.at/ppt/inSubtree> <http://vocabulary.semantic-web.at/cocktails/403d1249-f37f-4f43-bebf-8dde9677d886> ;
	a <http://vocabulary.semantic-web.at/cocktail-ontology/Alcoholic-Beverages> , <http://vocabulary.semantic-web.at/cocktail-ontology/Beverages> , <http://vocabulary.semantic-web.at/cocktail-ontology/Ingredients> , skos:Concept ;
	skos:altLabel "Disaronno Originale"@en ;
	skos:broader <http://vocabulary.semantic-web.at/cocktails/a1c1e015-91fd-4f6e-b2a8-5edae9aa0b9d> ;
	skos:definition "Disaronno Originale is a brand of fruity amaretto, with a characteristic bittersweet almond taste. Disaronno claims its \"originale\" amaretto's \"secret formula\" is unchanged from the year 1525, and claims the Luini tale as its own particular history. Its production remains in Saronno, but the product is sold worldwide."@en ;
	skos:exactMatch dbpedia:Disaronno ;
	skos:prefLabel "Disaronno"@en .

<http://vocabulary.semantic-web.at/cocktails/82026d8e-0fa5-4317-8827-410133db3bbd> dcterms:contributor <http://localhost/user/blumauera> ;
	dcterms:created "2015-05-01T14:19:45Z"^^xsd:dateTime ;
	dcterms:creator <http://localhost/user/blumauera> ;
	dcterms:modified "2015-05-01T14:20:39Z"^^xsd:dateTime ;
	<http://schema.semantic-web.at/ppt/inScheme> <http://vocabulary.semantic-web.at/cocktails/591cf89a-57af-49b8-9042-3fc77408c93e> ;
	<http://schema.semantic-web.at/ppt/inSubtree> <http://vocabulary.semantic-web.at/cocktails/403d1249-f37f-4f43-bebf-8dde9677d886> ;
	a <http://vocabulary.semantic-web.at/cocktail-ontology/Alcoholic-Beverages> , <http://vocabulary.semantic-web.at/cocktail-ontology/Beverages> , <http://vocabulary.semantic-web.at/cocktail-ontology/Ingredients> , skos:Concept ;
	skos:altLabel "Blue Curacao"@en , "Blue Curaçao"@en , "Blue curacao"@en , "Curacao (liqueur)"@en , "Curacao liqueur"@en , "Curacao liqueurs"@en , "Curaçao liqueur"@en , "Curaçao liqueurs"@en , "Orange Curacao"@en ;
	skos:broader <http://vocabulary.semantic-web.at/cocktails/397d0ec3-98e2-47d9-a8c2-eca9702ff94d> ;
	skos:definition "Curaçao is a liqueur flavored with the dried peel of the laraha citrus fruit, grown on the island of Curaçao. A non-native plant similar to an orange, the laraha developed from the sweet Valencia orange transplanted by Spanish explorers. The nutrient-poor soil and arid climate of Curaçao proved unsuitable to Valencia cultivation, resulting in small bitter fruit on the trees."@en ;
	skos:exactMatch <http://dbpedia.org/resource/Cura%C3%A7ao_(liqueur)> ;
	skos:narrower <http://vocabulary.semantic-web.at/cocktails/d530df52-cc54-4be3-8409-85734e5ec67f> ;
	skos:prefLabel "Curaçao"@en .

<http://vocabulary.semantic-web.at/cocktails/8352ad8c-0355-4ca4-9ff7-c3dff28931c5> dcterms:contributor <http://localhost/user/blumauera> ;
	dcterms:created "2015-05-02T17:15:49Z"^^xsd:dateTime ;
	dcterms:creator <http://localhost/user/blumauera> ;
	dcterms:modified "2015-05-07T06:27:27Z"^^xsd:dateTime ;
	<http://schema.semantic-web.at/ppt/inScheme> <http://vocabulary.semantic-web.at/cocktails/591cf89a-57af-49b8-9042-3fc77408c93e> ;
	<http://schema.semantic-web.at/ppt/inSubtree> <http://vocabulary.semantic-web.at/cocktails/403d1249-f37f-4f43-bebf-8dde9677d886> ;
	<http://vocabulary.semantic-web.at/cocktail-ontology/is-part-of> <http://vocabulary.semantic-web.at/cocktails/117bd4d2-6da3-4d69-8c79-bc1d873b5010> , <http://vocabulary.semantic-web.at/cocktails/21b94d69-280e-4546-be1a-fdd1d9aa5d32> ;
	a <http://vocabulary.semantic-web.at/cocktail-ontology/Alcoholic-Beverages> , <http://vocabulary.semantic-web.at/cocktail-ontology/Beverages> , <http://vocabulary.semantic-web.at/cocktail-ontology/Ingredients> , skos:Concept ;
	skos:broader <http://vocabulary.semantic-web.at/cocktails/19316511-1d42-4516-9504-873c3fd8fb85> , <http://vocabulary.semantic-web.at/cocktails/47635419-edef-4b78-8da1-e58a96d96f61> ;
	skos:prefLabel "Crème de cacao"@en .

<http://vocabulary.semantic-web.at/cocktails/84bf281b-95ab-4e18-a6fa-2d5156387167> dcterms:contributor <http://localhost/user/blumauera> ;
	dcterms:created "2015-05-01T08:31:23Z"^^xsd:dateTime ;
	dcterms:creator <http://localhost/user/blumauera> ;
	dcterms:modified "2015-08-07T15:06:39Z"^^xsd:dateTime ;
	<http://schema.semantic-web.at/ppt/inScheme> <http://vocabulary.semantic-web.at/cocktails/591cf89a-57af-49b8-9042-3fc77408c93e> ;
	<http://schema.semantic-web.at/ppt/inSubtree> <http://vocabulary.semantic-web.at/cocktails/403d1249-f37f-4f43-bebf-8dde9677d886> ;
	<http://vocabulary.semantic-web.at/cocktail-ontology/image_3> <http://preview.poolparty.biz/sparqlingCocktails/resources/images/fortifiedWine.png> ;
	a <http://vocabulary.semantic-web.at/cocktail-ontology/Alcoholic-Beverages> , <http://vocabulary.semantic-web.at/cocktail-ontology/Beverages> , <http://vocabulary.semantic-web.at/cocktail-ontology/Ingredients> , skos:Concept ;
	skos:altLabel "British fortified wine"@en , "Fortification (wine)"@en , "Fortification of wine"@en , "Fortified (wine)"@en , "Fortified (wines)"@en , "Fortified wines"@en , "Liqueur wine"@en , "Liquoroso"@en , "Mistela"@en , "Mistella"@en , "Mistelle"@en , "Mistelles"@en , "Street wine"@en , "Street wines"@en , "VDN"@en , "Vin Doux Naturel"@en , "Vin doux naturel"@en , "Vins Doux Naturels"@en , "Vins doux naturel"@en , "Vins doux naturels"@en , "Wine fortification"@en ;
	skos:broader <http://vocabulary.semantic-web.at/cocktails/403d1249-f37f-4f43-bebf-8dde9677d886> , <http://vocabulary.semantic-web.at/cocktails/f3000285-36b0-4ffe-af90-740c2dd8fff5> ;
	skos:definition "Fortified wine is wine with an added distilled beverage. Fortified wine is distinguished from spirits made from wine in that spirits are produced by means of distillation, while fortified wine is simply wine that has had a spirit added to it. Many different styles of fortified wine have been developed, including Port, Sherry, Madeira, Marsala, Commandaria wine and the aromatized wine Vermouth."@en ;
	skos:exactMatch dbpedia:Fortified_wine ;
	skos:narrower <http://vocabulary.semantic-web.at/cocktails/8cfd00fe-9f5a-414e-be27-858a8bc43c7c> , <http://vocabulary.semantic-web.at/cocktails/ef0fb33b-cf31-4acb-aeb8-cff4ab5411d2> ;
	skos:prefLabel "Fortified wine"@en .

<http://vocabulary.semantic-web.at/cocktails/84c72e0e-7830-46ef-ac35-44cad56d27ec> dcterms:contributor <http://localhost/user/blumauera> ;
	dcterms:created "2015-05-02T18:36:10Z"^^xsd:dateTime ;
	dcterms:creator <http://localhost/user/blumauera> ;
	dcterms:modified "2015-05-07T06:56:32Z"^^xsd:dateTime ;
	<http://schema.semantic-web.at/ppt/inScheme> <http://vocabulary.semantic-web.at/cocktails/591cf89a-57af-49b8-9042-3fc77408c93e> ;
	<http://schema.semantic-web.at/ppt/inSubtree> <http://vocabulary.semantic-web.at/cocktails/e86c1671-4a67-494b-ae5d-bcb750865acc> ;
	<http://vocabulary.semantic-web.at/cocktail-ontology/is-part-of> <http://vocabulary.semantic-web.at/cocktails/1529fd23-9c55-45d7-b8c6-b0fc229a3871> , <http://vocabulary.semantic-web.at/cocktails/fb278b46-3c67-48b0-b9eb-7ea037294f5f> ;
	a <http://vocabulary.semantic-web.at/cocktail-ontology/Beverages> , <http://vocabulary.semantic-web.at/cocktail-ontology/Ingredients> , <http://vocabulary.semantic-web.at/cocktail-ontology/Non-alcoholic-Beverages> , skos:Concept ;
	skos:broader <http://vocabulary.semantic-web.at/cocktails/a2b8e0e7-0dd0-40e2-a9a4-6178c7728cd0> ;
	skos:narrower <http://vocabulary.semantic-web.at/cocktails/7448dbed-7603-41f7-a316-99f754c9ae45> ;
	skos:prefLabel "Water"@en .

<http://vocabulary.semantic-web.at/cocktails/85669fcc-a38a-4ceb-ae23-90ae3fb7e16c> dcterms:contributor <http://localhost/user/blumauera> ;
	dcterms:created "2015-05-01T14:28:36Z"^^xsd:dateTime ;
	dcterms:creator <http://localhost/user/blumauera> ;
	dcterms:modified "2016-03-09T17:13:39Z"^^xsd:dateTime ;
	<http://schema.semantic-web.at/ppt/inScheme> <http://vocabulary.semantic-web.at/cocktails/8d052dfc-44bf-4985-8ce3-4564570a161b> ;
	<http://vocabulary.semantic-web.at/cocktail-ontology/consists-of> <http://vocabulary.semantic-web.at/cocktails/1d8d3cdc-91a7-421d-ad66-4814f475eddc> , <http://vocabulary.semantic-web.at/cocktails/5d96c50c-ee48-4c40-bb4c-4b9a42d11de6> , <http://vocabulary.semantic-web.at/cocktails/91b112c0-2fcc-4495-b68c-b1f09fa0a698> ;
	<http://vocabulary.semantic-web.at/cocktail-ontology/iba> <http://www.iba-world.com/index.php?option=com_content&id=194&Itemid=532> ;
	<http://vocabulary.semantic-web.at/cocktail-ontology/image> <http://www.iba-world.com/images/cocktail_drinks/derby.jpg> ;
	<http://vocabulary.semantic-web.at/cocktail-ontology/preparation> "Pour all ingredients into a mixing glass with ice. Stir.  Strain into a cocktail glass.  Garnish with a fresh mint leaves in the drink."@en ;
	<http://vocabulary.semantic-web.at/cocktail-ontology/uses> <http://vocabulary.semantic-web.at/cocktails/19dee0d8-fd30-469f-9ecd-91c902ff717c> ;
	<http://vocabulary.semantic-web.at/cocktail-ontology/uses_2> <http://vocabulary.semantic-web.at/cocktails/91b112c0-2fcc-4495-b68c-b1f09fa0a698> ;
	a <http://vocabulary.semantic-web.at/cocktail-ontology/Cocktail> , skos:Concept ;
	skos:broader <http://vocabulary.semantic-web.at/cocktails/caae2ea0-7e60-400b-a2bb-14ef79720668> ;
	skos:prefLabel "Derby"@en .

<http://vocabulary.semantic-web.at/cocktails/87384ce8-f20a-4201-b06d-3e0b8d832e5d> dcterms:contributor <http://localhost/user/blumauera> ;
	dcterms:created "2015-05-01T14:10:02Z"^^xsd:dateTime ;
	dcterms:creator <http://localhost/user/Andreas-Blumauer> ;
	dcterms:description "Sweeteners used to mix Cocktails"@en ;
	dcterms:modified "2015-05-02T21:03:41Z"^^xsd:dateTime ;
	dcterms:publisher <http://localhost/user/Semantic-Web-Company> ;
	dcterms:subject "How to mix the best Cocktails"@en ;
	dcterms:title "Sweeteners"@en ;
	<http://schema.semantic-web.at/ppt/appliedType> <http://vocabulary.semantic-web.at/cocktail-ontology/Ingredients> ;
	a skos:ConceptScheme ;
	rdfs:label "Sweeteners"@en ;
	skos:hasTopConcept <http://vocabulary.semantic-web.at/cocktails/0e385475-f369-4832-b8e3-20f35028988d> , <http://vocabulary.semantic-web.at/cocktails/3c3cd646-f1a4-4eac-b354-17d78b79a5d5> , <http://vocabulary.semantic-web.at/cocktails/3c94f5fc-4664-4177-a880-88643c0be9c1> , <http://vocabulary.semantic-web.at/cocktails/a3fcf23f-e2e0-4ba6-873a-bc6ae2870011> .

<http://vocabulary.semantic-web.at/cocktails/876f13e0-d873-4a11-94e1-e344b80cd53f> dcterms:contributor <http://localhost/user/huberf> ;
	dcterms:created "2015-05-02T07:27:25Z"^^xsd:dateTime ;
	dcterms:creator <http://localhost/user/blumauera> ;
	dcterms:modified "2015-11-19T15:22:44Z"^^xsd:dateTime ;
	<http://schema.semantic-web.at/ppt/inScheme> <http://vocabulary.semantic-web.at/cocktails/87384ce8-f20a-4201-b06d-3e0b8d832e5d> ;
	<http://vocabulary.semantic-web.at/cocktail-ontology/is-part-of> <http://vocabulary.semantic-web.at/cocktails/698723d7-e8b8-410e-91a8-9bdc867b3f8a> ;
	a <http://vocabulary.semantic-web.at/cocktail-ontology/Ingredients> , skos:Concept ;
	skos:broader <http://vocabulary.semantic-web.at/cocktails/3c3cd646-f1a4-4eac-b354-17d78b79a5d5> ;
	skos:prefLabel "Peach puree"@en .

<http://vocabulary.semantic-web.at/cocktails/87cf1079-05d6-44da-acbe-c94b3ba52bd7> dcterms:contributor <http://localhost/user/blumauera> ;
	dcterms:created "2015-05-01T15:18:55Z"^^xsd:dateTime ;
	dcterms:creator <http://localhost/user/blumauera> ;
	dcterms:modified "2016-04-04T09:13:39Z"^^xsd:dateTime ;
	<http://schema.semantic-web.at/ppt/inScheme> <http://vocabulary.semantic-web.at/cocktails/8d052dfc-44bf-4985-8ce3-4564570a161b> ;
	a <http://vocabulary.semantic-web.at/cocktail-ontology/Cocktail> , skos:Concept ;
	skos:altLabel "Colorado Bulldog"@en , "Duo (cocktail)"@en , "List of duos and trios"@en , "Panama (cocktail)"@en , "Panama (drink)"@en , "Trio (cocktail)"@en , "Vodka stinger"@en ;
	skos:definition "Duos and trios are a family of mixed drinks. A duo contains a spirit and a liqueur; a trio additionally contains a creamy ingredient, commonly cream or Irish cream. This family of drinks is named in Gary Regan's The Joy of Mixology. There is much variation in their ingredients, but their defining feature is that they are sweet due to their liqueur content."@en ;
	skos:exactMatch dbpedia:List_of_duo_and_trio_cocktails ;
	skos:narrower <http://vocabulary.semantic-web.at/cocktails/099726a2-ec4b-4b0f-b4e4-e6f25cdfd685> , <http://vocabulary.semantic-web.at/cocktails/45788a96-1fde-486b-80fc-31ad243bba31> , <http://vocabulary.semantic-web.at/cocktails/52117ab2-dcb8-4d28-a366-ddd932e58219> ;
	skos:prefLabel "Duo and trio cocktails"@en ;
	skos:topConceptOf <http://vocabulary.semantic-web.at/cocktails/8d052dfc-44bf-4985-8ce3-4564570a161b> .

<http://vocabulary.semantic-web.at/cocktails/88f5de3d-3de4-4a2f-9523-50bc7bb06600> dcterms:contributor <http://localhost/user/blumauera> ;
	dcterms:created "2015-05-01T08:08:03Z"^^xsd:dateTime ;
	dcterms:creator <http://localhost/user/blumauera> ;
	dcterms:modified "2015-05-07T07:13:55Z"^^xsd:dateTime ;
	<http://schema.semantic-web.at/ppt/inScheme> <http://vocabulary.semantic-web.at/cocktails/591cf89a-57af-49b8-9042-3fc77408c93e> ;
	<http://schema.semantic-web.at/ppt/inSubtree> <http://vocabulary.semantic-web.at/cocktails/e86c1671-4a67-494b-ae5d-bcb750865acc> ;
	<http://vocabulary.semantic-web.at/cocktail-ontology/is-part-of> <http://vocabulary.semantic-web.at/cocktails/2c032fe6-a518-44be-851a-dbf1c253be63> , <http://vocabulary.semantic-web.at/cocktails/2d85fb1b-96cb-4c48-8df5-707032f34e71> , <http://vocabulary.semantic-web.at/cocktails/43111fc3-3b59-420c-a588-024cd2d33896> , <http://vocabulary.semantic-web.at/cocktails/4d15a643-f7c7-4ee5-8f56-4ebd2bcf74b5> , <http://vocabulary.semantic-web.at/cocktails/4f85cadd-4fd4-4ffc-a78d-cddb0763fa4b> , <http://vocabulary.semantic-web.at/cocktails/60d3a991-48d3-4e73-9d62-5961893fd311> , <http://vocabulary.semantic-web.at/cocktails/7e4a73d5-f73d-4890-972c-f3dfd6952fd8> , <http://vocabulary.semantic-web.at/cocktails/926b14fe-1b83-4f46-bbf9-f946be1889aa> , <http://vocabulary.semantic-web.at/cocktails/a47e8f08-057a-45f2-8398-9be51ed351fc> , <http://vocabulary.semantic-web.at/cocktails/a5db05ca-eda3-41ef-a8ab-ba77b3e4baba> , <http://vocabulary.semantic-web.at/cocktails/b970d408-39ca-49b0-98fc-838f96c94608> , <http://vocabulary.semantic-web.at/cocktails/bab016bd-2fd5-4809-bfe7-3225d25f116d> , <http://vocabulary.semantic-web.at/cocktails/bee1e709-b317-4f46-b06f-a22367baefdf> , <http://vocabulary.semantic-web.at/cocktails/c151ee28-45d2-4128-8587-1f1b69060d9d> , <http://vocabulary.semantic-web.at/cocktails/f01f6a10-01a5-4810-860f-d3a52fd36b1b> ;
	a <http://vocabulary.semantic-web.at/cocktail-ontology/Beverages> , <http://vocabulary.semantic-web.at/cocktail-ontology/Ingredients> , <http://vocabulary.semantic-web.at/cocktail-ontology/Non-alcoholic-Beverages> , skos:Concept ;
	skos:broader <http://vocabulary.semantic-web.at/cocktails/6c0607a9-410d-4b65-87a1-b189a8e36352> ;
	skos:prefLabel "Lime juice"@en .

<http://vocabulary.semantic-web.at/cocktails/89ac12aa-d4f9-46d0-b127-fd8f4c21fbcc> dcterms:contributor <http://localhost/user/blumauera> ;
	dcterms:created "2015-05-02T17:20:19Z"^^xsd:dateTime ;
	dcterms:creator <http://localhost/user/blumauera> ;
	dcterms:modified "2015-05-07T06:44:27Z"^^xsd:dateTime ;
	<http://schema.semantic-web.at/ppt/inScheme> <http://vocabulary.semantic-web.at/cocktails/591cf89a-57af-49b8-9042-3fc77408c93e> ;
	<http://schema.semantic-web.at/ppt/inSubtree> <http://vocabulary.semantic-web.at/cocktails/e86c1671-4a67-494b-ae5d-bcb750865acc> ;
	<http://vocabulary.semantic-web.at/cocktail-ontology/is-part-of> <http://vocabulary.semantic-web.at/cocktails/eddf4894-1683-44e9-9ee3-7920d3729d71> ;
	a <http://vocabulary.semantic-web.at/cocktail-ontology/Beverages> , <http://vocabulary.semantic-web.at/cocktail-ontology/Ingredients> , <http://vocabulary.semantic-web.at/cocktail-ontology/Non-alcoholic-Beverages> , skos:Concept ;
	skos:altLabel "Gingerale"@en ;
	skos:broader <http://vocabulary.semantic-web.at/cocktails/a2b8e0e7-0dd0-40e2-a9a4-6178c7728cd0> ;
	skos:definition "Ginger ale is a carbonated soft drink flavored with ginger in either the Golden-style, closer to the ginger beer original, credited to the American doctor Thomas Cantrell, and the (Pale) Dry-style created by Canadian John McLaughlin, which is a paler drink with a much milder ginger-flavor to it."@en ;
	skos:exactMatch dbpedia:Ginger_ale ;
	skos:narrower <http://vocabulary.semantic-web.at/cocktails/5b4cd5f6-19e8-4854-8c5e-0b6d58cbb702> ;
	skos:prefLabel "Ginger ale"@en .

<http://vocabulary.semantic-web.at/cocktails/8a5e1790-d3c0-432e-bb85-709692b14f03> dcterms:contributor <http://localhost/user/blumauera> ;
	dcterms:created "2015-05-01T14:22:48Z"^^xsd:dateTime ;
	dcterms:creator <http://localhost/user/blumauera> ;
	dcterms:modified "2015-05-07T07:15:01Z"^^xsd:dateTime ;
	<http://schema.semantic-web.at/ppt/inScheme> <http://vocabulary.semantic-web.at/cocktails/eff672ac-6601-42c6-a3e9-0adda3b45df8> ;
	<http://schema.semantic-web.at/ppt/inSubtree> <http://vocabulary.semantic-web.at/cocktails/4f20d6bb-710d-4870-bde4-b6e835d7d13f> ;
	<http://vocabulary.semantic-web.at/cocktail-ontology/is-used-by_2> <http://vocabulary.semantic-web.at/cocktails/383ea520-07b2-4dc9-8827-8fc84fb7749c> , <http://vocabulary.semantic-web.at/cocktails/43111fc3-3b59-420c-a588-024cd2d33896> , <http://vocabulary.semantic-web.at/cocktails/44cc99c1-28ac-4c50-a55d-7244b2c5c07b> , <http://vocabulary.semantic-web.at/cocktails/61a18ebf-fd92-4ef1-8ab1-bfd3c26867b9> , <http://vocabulary.semantic-web.at/cocktails/76c0e55c-22df-4489-9551-4fe8a6a649f8> , <http://vocabulary.semantic-web.at/cocktails/785b30fd-1eb4-445b-8247-7e1e57b35b0f> , <http://vocabulary.semantic-web.at/cocktails/b33091cd-8c57-45e3-a89b-9de91ffce1e8> , <http://vocabulary.semantic-web.at/cocktails/b8075344-1e6d-4348-bdee-83948203a974> , <http://vocabulary.semantic-web.at/cocktails/b970d408-39ca-49b0-98fc-838f96c94608> , <http://vocabulary.semantic-web.at/cocktails/f632b16d-1490-4587-a637-fb393d7b1e7f> ;
	a <http://vocabulary.semantic-web.at/cocktail-ontology/Garnish> , <http://vocabulary.semantic-web.at/cocktail-ontology/Ingredients> , skos:Concept ;
	skos:altLabel "Maraschino berry"@en , "Maraschino cherries"@en ;
	skos:broader <http://vocabulary.semantic-web.at/cocktails/62fbc16f-3f84-4cc7-8c6f-5afebfc1510a> ;
	skos:definition "A maraschino cherry is a preserved, sweetened cherry, typically made from light-colored sweet cherries such as the Royal Ann, Rainier, or Gold varieties. In their modern form, the cherries are first preserved in a brine solution usually containing sulfur dioxide and calcium chloride to bleach the fruit, then soaked in a suspension of food coloring (common red food dye, FD&C Red 40), sugar syrup, and other components. Green maraschino cherries use a mint flavoring."@en ;
	skos:exactMatch dbpedia:Maraschino_cherry ;
	skos:prefLabel "Maraschino cherry"@en .

<http://vocabulary.semantic-web.at/cocktails/8ba9f3ab-d600-441c-85d3-d3aeb44678d1> dcterms:contributor <http://localhost/user/blumauera> ;
	dcterms:created "2015-05-02T19:26:11Z"^^xsd:dateTime ;
	dcterms:creator <http://localhost/user/blumauera> ;
	dcterms:modified "2015-05-05T07:24:24Z"^^xsd:dateTime ;
	<http://schema.semantic-web.at/ppt/inScheme> <http://vocabulary.semantic-web.at/cocktails/591cf89a-57af-49b8-9042-3fc77408c93e> ;
	<http://schema.semantic-web.at/ppt/inSubtree> <http://vocabulary.semantic-web.at/cocktails/e86c1671-4a67-494b-ae5d-bcb750865acc> ;
	<http://vocabulary.semantic-web.at/cocktail-ontology/is-part-of> <http://vocabulary.semantic-web.at/cocktails/7e5afb63-30ec-42b4-a9f5-f61fc456107d> ;
	a <http://vocabulary.semantic-web.at/cocktail-ontology/Beverages> , <http://vocabulary.semantic-web.at/cocktail-ontology/Ingredients> , <http://vocabulary.semantic-web.at/cocktail-ontology/Non-alcoholic-Beverages> , skos:Concept ;
	skos:altLabel "Caffe Espresso"@en , "Caffè Espresso"@en , "Caffè espresso"@en , "Crema (coffee)"@en , "Crema foam"@en , "Espreso"@en , "Espresso Coffee"@en , "Espresso-based drinks"@en , "Esspreso"@en , "Esspresso"@en , "Esxpresso"@en , "Petit noir"@en , "Schiuma"@en ;
	skos:broader <http://vocabulary.semantic-web.at/cocktails/4f4bed20-5317-45f6-a070-f28267b6e961> ;
	skos:definition "Espresso is a concentrated beverage brewed by forcing a small amount of nearly boiling water under pressure through finely ground coffee beans. Espresso often has a thicker consistency than coffee brewed by other methods, a higher concentration of suspended and dissolved solids, and crema (meaning cream, but being a reference to the foam with a creamy texture that forms as a result of the pressure)."@en ;
	skos:exactMatch dbpedia:Espresso ;
	skos:prefLabel "Espresso"@en .

<http://vocabulary.semantic-web.at/cocktails/8cfd00fe-9f5a-414e-be27-858a8bc43c7c> dcterms:contributor <http://localhost/user/blumauera> ;
	dcterms:created "2015-05-01T08:31:46Z"^^xsd:dateTime ;
	dcterms:creator <http://localhost/user/blumauera> ;
	dcterms:modified "2015-05-03T18:54:33Z"^^xsd:dateTime ;
	<http://schema.semantic-web.at/ppt/inScheme> <http://vocabulary.semantic-web.at/cocktails/591cf89a-57af-49b8-9042-3fc77408c93e> ;
	<http://schema.semantic-web.at/ppt/inSubtree> <http://vocabulary.semantic-web.at/cocktails/403d1249-f37f-4f43-bebf-8dde9677d886> ;
	<http://vocabulary.semantic-web.at/cocktail-ontology/is-part-of> <http://vocabulary.semantic-web.at/cocktails/b0885ae3-68e1-453d-8669-119e8464ff5f> ;
	a <http://vocabulary.semantic-web.at/cocktail-ontology/Alcoholic-Beverages> , <http://vocabulary.semantic-web.at/cocktail-ontology/Beverages> , <http://vocabulary.semantic-web.at/cocktail-ontology/Ingredients> , skos:Concept ;
	skos:broader <http://vocabulary.semantic-web.at/cocktails/84bf281b-95ab-4e18-a6fa-2d5156387167> ;
	skos:definition "Vermouth is an aromatized fortified wine flavored with various botanicals (roots, barks, flowers, seeds, herbs, spices). The modern versions of the beverage were first produced in 1757 in Turin, Italy. Vermouth was consumed as a medicinal libation until the later 19th century when it became an important ingredient in many of the first classic cocktails, such as the martini, the Manhattan, and the Negroni."@en ;
	skos:exactMatch dbpedia:Vermouth ;
	skos:narrower <http://vocabulary.semantic-web.at/cocktails/074c3acb-bc4d-4c6e-ad8a-e553d5ec7eff> , <http://vocabulary.semantic-web.at/cocktails/1b9d9c87-9a94-465a-b7e9-feee6c77bf03> , <http://vocabulary.semantic-web.at/cocktails/40362aa1-0058-4f25-ba82-74bcd2202cc4> , <http://vocabulary.semantic-web.at/cocktails/8dee4eba-b6c6-4d16-b8f2-8d6cc0d9436c> , <http://vocabulary.semantic-web.at/cocktails/9ca4c18b-03f7-4c4f-802e-e18299702bad> ;
	skos:prefLabel "Vermouth"@en .

<http://vocabulary.semantic-web.at/cocktails/8d052dfc-44bf-4985-8ce3-4564570a161b> dcterms:contributor <http://localhost/user/blumauera> ;
	dcterms:created "2015-05-01T07:39:15Z"^^xsd:dateTime ;
	dcterms:creator <http://localhost/user/Andreas-Blumauer> ;
	dcterms:modified "2015-05-02T21:02:13Z"^^xsd:dateTime ;
	dcterms:publisher <http://localhost/user/Semantic-Web-Company> ;
	dcterms:title "Cocktails"@en ;
	<http://schema.semantic-web.at/ppt/appliedType> <http://vocabulary.semantic-web.at/cocktail-ontology/Cocktail> ;
	a skos:ConceptScheme ;
	rdfs:label "All about Cocktails"@en ;
	skos:hasTopConcept <http://vocabulary.semantic-web.at/cocktails/204cd4e7-58d7-4417-837a-7f9cc41663c8> , <http://vocabulary.semantic-web.at/cocktails/54702498-ad42-4af6-b28a-2276215450da> , <http://vocabulary.semantic-web.at/cocktails/5ac37bec-e4b9-4d43-9bcc-8d6954903c25> , <http://vocabulary.semantic-web.at/cocktails/7516b400-963a-4151-8fdc-f6b23bad1dd5> , <http://vocabulary.semantic-web.at/cocktails/87cf1079-05d6-44da-acbe-c94b3ba52bd7> , <http://vocabulary.semantic-web.at/cocktails/b523727e-7f49-4e1b-9c09-55002ee3a81e> .

<http://vocabulary.semantic-web.at/cocktails/8d5e2abc-6280-42b7-8e21-8bbc30f7509f> dcterms:contributor <http://localhost/user/blumauera> ;
	dcterms:created "2015-05-02T07:29:39Z"^^xsd:dateTime ;
	dcterms:creator <http://localhost/user/blumauera> ;
	dcterms:modified "2015-10-16T07:53:32Z"^^xsd:dateTime ;
	<http://schema.semantic-web.at/ppt/inScheme> <http://vocabulary.semantic-web.at/cocktails/591cf89a-57af-49b8-9042-3fc77408c93e> ;
	<http://schema.semantic-web.at/ppt/inSubtree> <http://vocabulary.semantic-web.at/cocktails/403d1249-f37f-4f43-bebf-8dde9677d886> ;
	<http://vocabulary.semantic-web.at/cocktail-ontology/is-part-of> <http://vocabulary.semantic-web.at/cocktails/7e5afb63-30ec-42b4-a9f5-f61fc456107d> , <http://vocabulary.semantic-web.at/cocktails/cd66d6ff-559f-43ea-a754-ac613a87325d> ;
	a <http://vocabulary.semantic-web.at/cocktail-ontology/Alcoholic-Beverages> , <http://vocabulary.semantic-web.at/cocktail-ontology/Beverages> , <http://vocabulary.semantic-web.at/cocktail-ontology/Ingredients> , skos:Concept ;
	skos:altLabel "Kahlua"@en , "Khalua"@en , "Kuhlua"@en ;
	skos:broader <http://vocabulary.semantic-web.at/cocktails/a12b3836-dba0-49e9-92c6-7725ccf35944> ;
	skos:definition "Kahlúa is a Mexican coffee-flavored rum-based liqueur. It is dense and sweet, with the distinct taste of coffee, from which it is made. Kahlúa also contains sugar, corn syrup and vanilla bean."@en ;
	skos:exactMatch dbpedia:Kahl%C3%BAa ;
	skos:prefLabel "Kahlúa"@en .

<http://vocabulary.semantic-web.at/cocktails/8dee4eba-b6c6-4d16-b8f2-8d6cc0d9436c> dcterms:contributor <http://localhost/user/blumauera> ;
	dcterms:created "2015-05-01T14:50:22Z"^^xsd:dateTime ;
	dcterms:creator <http://localhost/user/blumauera> ;
	dcterms:modified "2015-05-06T12:18:48Z"^^xsd:dateTime ;
	<http://schema.semantic-web.at/ppt/inScheme> <http://vocabulary.semantic-web.at/cocktails/591cf89a-57af-49b8-9042-3fc77408c93e> ;
	<http://schema.semantic-web.at/ppt/inSubtree> <http://vocabulary.semantic-web.at/cocktails/403d1249-f37f-4f43-bebf-8dde9677d886> ;
	<http://vocabulary.semantic-web.at/cocktail-ontology/is-part-of> <http://vocabulary.semantic-web.at/cocktails/40ab50e9-66f1-411b-8220-ef8f05273542> , <http://vocabulary.semantic-web.at/cocktails/f632b16d-1490-4587-a637-fb393d7b1e7f> ;
	a <http://vocabulary.semantic-web.at/cocktail-ontology/Alcoholic-Beverages> , <http://vocabulary.semantic-web.at/cocktail-ontology/Beverages> , <http://vocabulary.semantic-web.at/cocktail-ontology/Ingredients> , skos:Concept ;
	skos:broader <http://vocabulary.semantic-web.at/cocktails/8cfd00fe-9f5a-414e-be27-858a8bc43c7c> ;
	skos:prefLabel "Red vermouth"@en .

<http://vocabulary.semantic-web.at/cocktails/8f09ee6f-d5b9-4b8a-aa17-b0665fae4e83> dcterms:contributor <http://localhost/user/blumauera> ;
	dcterms:created "2015-05-01T08:25:40Z"^^xsd:dateTime ;
	dcterms:creator <http://localhost/user/blumauera> ;
	dcterms:modified "2015-08-07T15:06:34Z"^^xsd:dateTime ;
	<http://schema.semantic-web.at/ppt/inScheme> <http://vocabulary.semantic-web.at/cocktails/591cf89a-57af-49b8-9042-3fc77408c93e> ;
	<http://schema.semantic-web.at/ppt/inSubtree> <http://vocabulary.semantic-web.at/cocktails/403d1249-f37f-4f43-bebf-8dde9677d886> ;
	<http://vocabulary.semantic-web.at/cocktail-ontology/image_3> <http://preview.poolparty.biz/sparqlingCocktails/resources/images/brandy.png> ;
	<http://vocabulary.semantic-web.at/cocktail-ontology/is-part-of> <http://vocabulary.semantic-web.at/cocktails/cfa8539e-ede2-42ec-b563-d084ddb33280> , <http://vocabulary.semantic-web.at/cocktails/eddf4894-1683-44e9-9ee3-7920d3729d71> ;
	a <http://vocabulary.semantic-web.at/cocktail-ontology/Alcoholic-Beverages> , <http://vocabulary.semantic-web.at/cocktail-ontology/Beverages> , <http://vocabulary.semantic-web.at/cocktail-ontology/Ingredients> , skos:Concept ;
	skos:altLabel "Apple brandy"@en , "Blackberry brandy"@en , "Brandewijn"@en , "Brandies"@en , "Brandy (wine)"@en , "Cherry B"@en , "Cider Brandy"@en , "Cider brandy"@en , "Fruit brandy"@en , "Grape spirit"@en , "Grape spirits"@en , "Obstwasser"@en , "Peach brandy"@en , "Weinbrand"@en ;
	skos:broader <http://vocabulary.semantic-web.at/cocktails/403d1249-f37f-4f43-bebf-8dde9677d886> , <http://vocabulary.semantic-web.at/cocktails/f3000285-36b0-4ffe-af90-740c2dd8fff5> ;
	skos:definition "Brandy (from brandywine, derived from Dutch brandewijn—\"burnt wine\") is a spirit produced by distilling wine. Brandy generally contains 35–60% alcohol by volume and is typically taken as an after-dinner drink. Some brandies are aged in wooden casks, some are coloured with caramel colouring to imitate the effect of aging, and some brandies are produced using a combination of both aging and colouring."@en ;
	skos:exactMatch dbpedia:Brandy ;
	skos:narrower <http://vocabulary.semantic-web.at/cocktails/16b625c5-3930-4cf8-a75b-b25e72f2bfb6> , <http://vocabulary.semantic-web.at/cocktails/1c6b25d5-2b8e-49f9-8d26-5d26438cb1aa> , <http://vocabulary.semantic-web.at/cocktails/5caedba2-9aef-4fab-b26b-6e20cf014419> , <http://vocabulary.semantic-web.at/cocktails/c532e86c-01cc-40d4-b2d6-1f959e72d9da> , <http://vocabulary.semantic-web.at/cocktails/d9f071c0-8c44-43d1-9e4f-eef5709f5d98> , <http://vocabulary.semantic-web.at/cocktails/fd76c5ab-be62-4c4b-a2c6-7fa9bc359f47> ;
	skos:prefLabel "Brandy"@en .

<http://vocabulary.semantic-web.at/cocktails/8ff588a8-d5ad-4e34-aee9-8f6de16ca30c> dcterms:contributor <http://localhost/user/turdeant> ;
	dcterms:created "2015-05-01T14:46:08Z"^^xsd:dateTime ;
	dcterms:creator <http://localhost/user/blumauera> ;
	dcterms:modified "2015-09-04T22:18:35Z"^^xsd:dateTime ;
	<http://schema.semantic-web.at/ppt/inScheme> <http://vocabulary.semantic-web.at/cocktails/8d052dfc-44bf-4985-8ce3-4564570a161b> ;
	<http://vocabulary.semantic-web.at/cocktail-ontology/image> <http://thehoochlife.com/wp-content/uploads/2012/02/monkey_gland-266x399.jpg> ;
	a <http://vocabulary.semantic-web.at/cocktail-ontology/Cocktail> , skos:Concept ;
	skos:altLabel "Monkey glands"@en ;
	skos:broader <http://vocabulary.semantic-web.at/cocktails/caae2ea0-7e60-400b-a2bb-14ef79720668> ;
	skos:definition "The Monkey Gland is a cocktail of gin, orange juice, grenadine and absinthe named after a surgical technique of grafting monkey testicle tissue into humans. The practice was started by Dr Serge Voronoff, and was intended to produce longevity. The Monkey Gland was created in the 1920s by Harry MacElhone, owner of Harry's New York Bar in Paris, France. Rachel Maddow prepared this drink during her guest appearance on the Jimmy Fallon Show on March 25, 2011."@en ;
	skos:exactMatch dbpedia:The_Monkey_Gland ;
	skos:prefLabel "The Monkey Gland"@en .

<http://vocabulary.semantic-web.at/cocktails/917d78d0-0938-4fe0-80c4-cfd2eb16e6a4> dcterms:contributor <http://localhost/user/blumauera> ;
	dcterms:created "2015-05-01T15:12:11Z"^^xsd:dateTime ;
	dcterms:creator <http://localhost/user/blumauera> ;
	dcterms:modified "2015-05-01T15:12:16Z"^^xsd:dateTime ;
	<http://schema.semantic-web.at/ppt/inScheme> <http://vocabulary.semantic-web.at/cocktails/591cf89a-57af-49b8-9042-3fc77408c93e> ;
	<http://schema.semantic-web.at/ppt/inSubtree> <http://vocabulary.semantic-web.at/cocktails/403d1249-f37f-4f43-bebf-8dde9677d886> ;
	a <http://vocabulary.semantic-web.at/cocktail-ontology/Alcoholic-Beverages> , <http://vocabulary.semantic-web.at/cocktail-ontology/Beverages> , <http://vocabulary.semantic-web.at/cocktail-ontology/Ingredients> , skos:Concept ;
	skos:broader <http://vocabulary.semantic-web.at/cocktails/2944baef-5338-421b-a5f5-0e51f75244c2> ;
	skos:narrower <http://vocabulary.semantic-web.at/cocktails/05a0d86b-79fc-4d75-91e4-dc77e8167db9> , <http://vocabulary.semantic-web.at/cocktails/372c645f-53c5-4b75-ba34-b36625f87b02> , <http://vocabulary.semantic-web.at/cocktails/44d8b702-5261-4ce9-923c-50d2acb4e0de> , <http://vocabulary.semantic-web.at/cocktails/4be1257b-f797-4ab9-a2b3-af09b958173e> , <http://vocabulary.semantic-web.at/cocktails/5b272721-4eb2-41cd-9224-5963091fb639> , <http://vocabulary.semantic-web.at/cocktails/c5c70695-d939-4f4d-8ae7-394f2f66ccbb> , <http://vocabulary.semantic-web.at/cocktails/e406119b-7637-43f9-9a62-5a8ea500ebc4> ;
	skos:prefLabel "Herbal liqueur"@en .

<http://vocabulary.semantic-web.at/cocktails/91b112c0-2fcc-4495-b68c-b1f09fa0a698> dcterms:contributor <http://localhost/user/blumauera> ;
	dcterms:created "2015-05-01T08:10:40Z"^^xsd:dateTime ;
	dcterms:creator <http://localhost/user/blumauera> ;
	dcterms:modified "2015-05-07T06:59:07Z"^^xsd:dateTime ;
	<http://schema.semantic-web.at/ppt/inScheme> <http://vocabulary.semantic-web.at/cocktails/eff672ac-6601-42c6-a3e9-0adda3b45df8> ;
	<http://schema.semantic-web.at/ppt/inSubtree> <http://vocabulary.semantic-web.at/cocktails/469959a3-10dc-4539-80ff-08bf9ff2de1c> ;
	<http://vocabulary.semantic-web.at/cocktail-ontology/is-part-of> <http://vocabulary.semantic-web.at/cocktails/1529fd23-9c55-45d7-b8c6-b0fc229a3871> , <http://vocabulary.semantic-web.at/cocktails/85669fcc-a38a-4ceb-ae23-90ae3fb7e16c> , <http://vocabulary.semantic-web.at/cocktails/bee1e709-b317-4f46-b06f-a22367baefdf> ;
	<http://vocabulary.semantic-web.at/cocktail-ontology/is-used-by_2> <http://vocabulary.semantic-web.at/cocktails/1529fd23-9c55-45d7-b8c6-b0fc229a3871> , <http://vocabulary.semantic-web.at/cocktails/85669fcc-a38a-4ceb-ae23-90ae3fb7e16c> , <http://vocabulary.semantic-web.at/cocktails/bee1e709-b317-4f46-b06f-a22367baefdf> ;
	a <http://vocabulary.semantic-web.at/cocktail-ontology/Garnish> , <http://vocabulary.semantic-web.at/cocktail-ontology/Ingredients> , skos:Concept ;
	skos:altLabel "Hīoi"@en , "Mendra"@en , "Mendër"@en , "Mentha nemorosa"@en , "Mint (botany)"@en , "Mint (herb)"@en , "Mint (plant)"@en , "Mint jam"@en , "Mint jelly"@en , "Mint leaf"@en , "Mint leaves"@en , "Mint plant"@en , "Pudine"@en ;
	skos:broader <http://vocabulary.semantic-web.at/cocktails/469959a3-10dc-4539-80ff-08bf9ff2de1c> ;
	skos:definition "Mentha (also known as Mint, from Greek míntha, Linear B mi-ta) is a genus of flowering plants in the family Lamiaceae (mint family). The species are not clearly distinct and estimates of the number of species varies from 13 to 18. Hybridization between some of the species occurs naturally. Many other hybrids as well as numerous cultivars are known in cultivation. The genus has a subcosmopolitan distribution across Europe, Africa, Asia, Australia, and North America."@en ;
	skos:exactMatch dbpedia:Mentha ;
	skos:prefLabel "Mentha"@en .

<http://vocabulary.semantic-web.at/cocktails/92561e61-4e22-4402-bf23-3e1a1fefb530> dcterms:created "2015-05-03T18:58:11Z"^^xsd:dateTime ;
	dcterms:creator <http://localhost/user/blumauera> ;
	<http://schema.semantic-web.at/ppt/inScheme> <http://vocabulary.semantic-web.at/cocktails/591cf89a-57af-49b8-9042-3fc77408c93e> ;
	<http://schema.semantic-web.at/ppt/inSubtree> <http://vocabulary.semantic-web.at/cocktails/403d1249-f37f-4f43-bebf-8dde9677d886> ;
	a <http://vocabulary.semantic-web.at/cocktail-ontology/Alcoholic-Beverages> , <http://vocabulary.semantic-web.at/cocktail-ontology/Beverages> , <http://vocabulary.semantic-web.at/cocktail-ontology/Ingredients> , skos:Concept ;
	skos:broader <http://vocabulary.semantic-web.at/cocktails/40362aa1-0058-4f25-ba82-74bcd2202cc4> ;
	skos:prefLabel "Martini Bianco"@en .

<http://vocabulary.semantic-web.at/cocktails/926b14fe-1b83-4f46-bbf9-f946be1889aa> dcterms:contributor <http://localhost/user/blumauera> ;
	dcterms:created "2015-05-02T17:16:58Z"^^xsd:dateTime ;
	dcterms:creator <http://localhost/user/blumauera> ;
	dcterms:modified "2015-05-07T06:42:57Z"^^xsd:dateTime ;
	<http://schema.semantic-web.at/ppt/inScheme> <http://vocabulary.semantic-web.at/cocktails/8d052dfc-44bf-4985-8ce3-4564570a161b> ;
	<http://vocabulary.semantic-web.at/cocktail-ontology/consists-of> <http://vocabulary.semantic-web.at/cocktails/224b4628-2f46-44a1-9d2f-8b5ef0b31e79> , <http://vocabulary.semantic-web.at/cocktails/88f5de3d-3de4-4a2f-9523-50bc7bb06600> , <http://vocabulary.semantic-web.at/cocktails/abe8b872-3a29-49a3-9a8e-1b71db770a3f> , <http://vocabulary.semantic-web.at/cocktails/f5cd2a2b-2153-4b7e-ae79-678b939765ca> ;
	<http://vocabulary.semantic-web.at/cocktail-ontology/iba> <http://www.iba-world.com/index.php?option=com_content&id=222&Itemid=532> ;
	<http://vocabulary.semantic-web.at/cocktail-ontology/image> <http://www.iba-world.com/images/cocktail_drinks/hemingway_special.jpg> ;
	<http://vocabulary.semantic-web.at/cocktail-ontology/preparation> "Pour all ingredients into a shaker with ice. Shake. Strain into a double cocktail glass."@en ;
	<http://vocabulary.semantic-web.at/cocktail-ontology/uses> <http://vocabulary.semantic-web.at/cocktails/19dee0d8-fd30-469f-9ecd-91c902ff717c> ;
	a <http://vocabulary.semantic-web.at/cocktail-ontology/Cocktail> , skos:Concept ;
	skos:broader <http://vocabulary.semantic-web.at/cocktails/b9bf3799-a4e4-47f7-9aea-7697cc998a34> ;
	skos:prefLabel "Hemingway Special"@en .

<http://vocabulary.semantic-web.at/cocktails/92e8ded1-1223-4a3f-b2d4-7ee731d6dbc7> dcterms:contributor <http://localhost/user/blumauera> ;
	dcterms:created "2015-05-02T17:22:02Z"^^xsd:dateTime ;
	dcterms:creator <http://localhost/user/blumauera> ;
	dcterms:modified "2015-05-07T06:49:20Z"^^xsd:dateTime ;
	<http://schema.semantic-web.at/ppt/inScheme> <http://vocabulary.semantic-web.at/cocktails/87384ce8-f20a-4201-b06d-3e0b8d832e5d> ;
	<http://schema.semantic-web.at/ppt/inSubtree> <http://vocabulary.semantic-web.at/cocktails/3c94f5fc-4664-4177-a880-88643c0be9c1> ;
	<http://vocabulary.semantic-web.at/cocktail-ontology/is-part-of> <http://vocabulary.semantic-web.at/cocktails/bca7bc6d-6709-48b8-ae52-fe194c212398> , <http://vocabulary.semantic-web.at/cocktails/c3b197cc-8583-4e2f-8e45-3a7fed1309c1> ;
	a <http://vocabulary.semantic-web.at/cocktail-ontology/Garnish> , <http://vocabulary.semantic-web.at/cocktail-ontology/Ingredients> , skos:Concept ;
	skos:altLabel "Black sugar"@en , "Brown (sugar)"@en , "Brown sugars"@en , "Demerara (sugar)"@en , "Demerara sugar"@en , "Demerera sugar"@en , "Natural Brown Sugar"@en , "Natural brown sugar"@en , "Sugar in the Raw"@en , "Turbinado"@en , "Turbinado sugar"@en , "Whole cane sugar"@en ;
	skos:broader <http://vocabulary.semantic-web.at/cocktails/3c94f5fc-4664-4177-a880-88643c0be9c1> ;
	skos:definition "Brown sugar is a sucrose sugar product with a distinctive brown colour due to the presence of molasses. It is either an unrefined or partially refined soft sugar consisting of sugar crystals with some residual molasses content, or it is produced by the addition of molasses to refined white sugar. Brown sugar contains from 3.5% molasses (light brown sugar) to 6.5% molasses (dark brown sugar) based on total volume. Based on total weight, regular brown sugar contains up to 10% molasses."@en ;
	skos:exactMatch dbpedia:Brown_sugar ;
	skos:prefLabel "Brown sugar"@en .

<http://vocabulary.semantic-web.at/cocktails/94cca1b4-3603-472b-9c78-6d6a43b6b4ca> dcterms:contributor <http://localhost/user/blumauera> ;
	dcterms:created "2015-05-06T12:30:33Z"^^xsd:dateTime ;
	dcterms:creator <http://localhost/user/blumauera> ;
	dcterms:modified "2015-05-06T12:30:54Z"^^xsd:dateTime ;
	<http://schema.semantic-web.at/ppt/inScheme> <http://vocabulary.semantic-web.at/cocktails/6fe33361-f993-416d-bc13-cb36c326736b> ;
	<http://vocabulary.semantic-web.at/cocktail-ontology/is-part-of> <http://vocabulary.semantic-web.at/cocktails/268fb62f-8ef1-45cd-844f-8c7da85a6a0b> ;
	a <http://vocabulary.semantic-web.at/cocktail-ontology/Ingredients> , skos:Concept ;
	skos:altLabel "E. McIlhenny"@en , "McIlhenny Company"@en , "Mcilhenny company"@en , "TABASCO"@en , "Tobacco sauce"@en , "Tobasco Sauce"@en ;
	skos:broader <http://vocabulary.semantic-web.at/cocktails/105184cf-c7fa-4e7c-b668-b4db7a689ab7> ;
	skos:definition "Tabasco sauce is a hot sauce made from tabasco peppers (Capsicum frutescens var. tabasco), vinegar and salt. It has a hot, spicy flavor. The sauce is produced by US-based McIlhenny Company to whom the \"Tabasco sauce\" brand name belongs."@en ;
	skos:exactMatch dbpedia:Tabasco_sauce ;
	skos:prefLabel "Tabasco sauce"@en .

<http://vocabulary.semantic-web.at/cocktails/96c173d1-f047-4811-8950-45b071588fdc> dcterms:contributor <http://localhost/user/blumauera> ;
	dcterms:created "2015-05-03T18:55:08Z"^^xsd:dateTime ;
	dcterms:creator <http://localhost/user/blumauera> ;
	dcterms:modified "2015-05-03T18:55:24Z"^^xsd:dateTime ;
	<http://schema.semantic-web.at/ppt/inScheme> <http://vocabulary.semantic-web.at/cocktails/591cf89a-57af-49b8-9042-3fc77408c93e> ;
	<http://schema.semantic-web.at/ppt/inSubtree> <http://vocabulary.semantic-web.at/cocktails/403d1249-f37f-4f43-bebf-8dde9677d886> ;
	a <http://vocabulary.semantic-web.at/cocktail-ontology/Alcoholic-Beverages> , <http://vocabulary.semantic-web.at/cocktail-ontology/Beverages> , <http://vocabulary.semantic-web.at/cocktail-ontology/Ingredients> , skos:Concept ;
	skos:broader <http://vocabulary.semantic-web.at/cocktails/074c3acb-bc4d-4c6e-ad8a-e553d5ec7eff> , <http://vocabulary.semantic-web.at/cocktails/9ca4c18b-03f7-4c4f-802e-e18299702bad> ;
	skos:prefLabel "Martini Extra Dry"@en .

<http://vocabulary.semantic-web.at/cocktails/98f20476-57d7-46d3-b76d-6aac18b57788> dcterms:contributor <http://localhost/user/blumauera> ;
	dcterms:created "2015-05-01T14:26:44Z"^^xsd:dateTime ;
	dcterms:creator <http://localhost/user/blumauera> ;
	dcterms:modified "2015-05-05T07:49:58Z"^^xsd:dateTime ;
	<http://schema.semantic-web.at/ppt/inScheme> <http://vocabulary.semantic-web.at/cocktails/591cf89a-57af-49b8-9042-3fc77408c93e> ;
	<http://schema.semantic-web.at/ppt/inSubtree> <http://vocabulary.semantic-web.at/cocktails/e86c1671-4a67-494b-ae5d-bcb750865acc> ;
	<http://vocabulary.semantic-web.at/cocktail-ontology/is-part-of> <http://vocabulary.semantic-web.at/cocktails/43b786b6-a1f1-4b7f-a5d9-be43d386ffb4> , <http://vocabulary.semantic-web.at/cocktails/76c0e55c-22df-4489-9551-4fe8a6a649f8> , <http://vocabulary.semantic-web.at/cocktails/c151ee28-45d2-4128-8587-1f1b69060d9d> , <http://vocabulary.semantic-web.at/cocktails/c3ae5830-1bfd-4f37-afc9-3e88849d03cf> ;
	a <http://vocabulary.semantic-web.at/cocktail-ontology/Beverages> , <http://vocabulary.semantic-web.at/cocktail-ontology/Ingredients> , <http://vocabulary.semantic-web.at/cocktail-ontology/Non-alcoholic-Beverages> , skos:Concept ;
	skos:altLabel "Albumen"@en , "Egg albumen"@en , "Egg albumin"@en , "Egg whites"@en , "Egg-white"@en , "Eggwhite"@en , "Glair"@en , "Glairy"@en , "Ovoglobulin G2"@en , "White of an egg"@en ;
	skos:broader <http://vocabulary.semantic-web.at/cocktails/de17b6c7-513a-4fe2-a8ee-4fdc6069ae27> ;
	skos:definition "Egg white is the common name for the clear liquid (also called the albumen or the glair/glaire) contained within an egg. In chickens it is formed from the layers of secretions of the anterior section of the hen's oviduct during the passage of the egg. It forms around either fertilized or unfertilized egg yolks. The primary natural purpose of egg white is to protect the yolk and provide additional nutrition for the growth of the embryo (when fertilized)."@en ;
	skos:exactMatch dbpedia:Egg_white ;
	skos:prefLabel "Egg white"@en .

<http://vocabulary.semantic-web.at/cocktails/99171f20-c59f-40c4-998a-a9c8f1909168> dcterms:contributor <http://localhost/user/blumauera> ;
	dcterms:created "2015-05-01T08:20:37Z"^^xsd:dateTime ;
	dcterms:creator <http://localhost/user/blumauera> ;
	dcterms:modified "2015-05-07T07:16:38Z"^^xsd:dateTime ;
	<http://schema.semantic-web.at/ppt/inScheme> <http://vocabulary.semantic-web.at/cocktails/eff672ac-6601-42c6-a3e9-0adda3b45df8> ;
	<http://schema.semantic-web.at/ppt/inSubtree> <http://vocabulary.semantic-web.at/cocktails/4f20d6bb-710d-4870-bde4-b6e835d7d13f> ;
	<http://vocabulary.semantic-web.at/cocktail-ontology/is-used-by_2> <http://vocabulary.semantic-web.at/cocktails/0f8cc862-9056-49be-b636-cd22f8d7282d> , <http://vocabulary.semantic-web.at/cocktails/2c682ed8-e2ba-473e-8cb7-979598080e18> , <http://vocabulary.semantic-web.at/cocktails/40ab50e9-66f1-411b-8220-ef8f05273542> , <http://vocabulary.semantic-web.at/cocktails/55c40695-8b41-41ed-8c6a-70fe6930067e> , <http://vocabulary.semantic-web.at/cocktails/61a18ebf-fd92-4ef1-8ab1-bfd3c26867b9> , <http://vocabulary.semantic-web.at/cocktails/76c0e55c-22df-4489-9551-4fe8a6a649f8> , <http://vocabulary.semantic-web.at/cocktails/79d4686d-4f5b-4067-a2ef-99beccc51242> , <http://vocabulary.semantic-web.at/cocktails/b0885ae3-68e1-453d-8669-119e8464ff5f> , <http://vocabulary.semantic-web.at/cocktails/c151ee28-45d2-4128-8587-1f1b69060d9d> , <http://vocabulary.semantic-web.at/cocktails/c2249dc0-0529-4a11-ad82-5d710b5e9c31> , <http://vocabulary.semantic-web.at/cocktails/dff0a7f4-ded0-48d5-bd31-881b70fbe36a> , <http://vocabulary.semantic-web.at/cocktails/fb278b46-3c67-48b0-b9eb-7ea037294f5f> ;
	a <http://vocabulary.semantic-web.at/cocktail-ontology/Garnish> , <http://vocabulary.semantic-web.at/cocktail-ontology/Ingredients> , skos:Concept ;
	skos:altLabel "Appelsina"@en , "Appelsína"@en , "Citrus sinensis"@en , "Citrus x sinensis"@en , "Citrus × sinensis"@en , "Citrus ×sinensis"@en , "Culture of orange"@en , "Navel Orange"@en , "Navel orange"@en , "Orange (botany)"@en , "Orange (flavor)"@en , "Orange (plant)"@en , "Orange (tree)"@en , "Orange fruit"@en , "Orange tree"@en , "Orange trees"@en , "Orange wood"@en , "Orange(fruit)"@en , "Orangewood"@en , "Sweet Orange"@en , "Sweet orange"@en , "Sweet oranges"@en ;
	skos:broader <http://vocabulary.semantic-web.at/cocktails/4f20d6bb-710d-4870-bde4-b6e835d7d13f> ;
	skos:definition "The orange (specifically, the sweet orange) is the fruit of the citrus species Citrus × ​sinensis in the family Rutaceae. The fruit of the Citrus sinensis is called sweet orange to distinguish it from that of the Citrus aurantium, the bitter orange. The orange is a hybrid, possibly between pomelo (Citrus maxima) and mandarin (Citrus reticulata), cultivated since ancient times. Probably originated in Southeast Asia, oranges were already cultivated in China as far back as 2500 BC."@en ;
	skos:exactMatch <http://dbpedia.org/resource/Orange_(fruit)> ;
	skos:prefLabel "Orange"@en .

<http://vocabulary.semantic-web.at/cocktails/9c287d15-c699-4f56-bd65-bf8cc75a2cca> dcterms:contributor <http://localhost/user/blumauera> ;
	dcterms:created "2015-05-01T14:59:01Z"^^xsd:dateTime ;
	dcterms:creator <http://localhost/user/blumauera> ;
	dcterms:modified "2016-03-09T17:13:39Z"^^xsd:dateTime ;
	<http://schema.semantic-web.at/ppt/inScheme> <http://vocabulary.semantic-web.at/cocktails/8d052dfc-44bf-4985-8ce3-4564570a161b> ;
	<http://vocabulary.semantic-web.at/cocktail-ontology/consists-of> <http://vocabulary.semantic-web.at/cocktails/12da816f-8ad3-487d-b8f9-2190e4b3e1b8> , <http://vocabulary.semantic-web.at/cocktails/2ce50273-13b2-4ba1-9ff2-8cfbd835c1f2> , <http://vocabulary.semantic-web.at/cocktails/59ccd2fc-1807-45eb-8621-8d3e898e6d37> , <http://vocabulary.semantic-web.at/cocktails/5c291fe9-6fdb-4939-930d-dacbc67171a5> , <http://vocabulary.semantic-web.at/cocktails/71210bd1-3071-4533-8da4-fe0f7d7694a0> , <http://vocabulary.semantic-web.at/cocktails/9c2ce399-c6ae-4f4d-bf37-7fd8ffe2a19d> , <http://vocabulary.semantic-web.at/cocktails/ced2e755-fe48-4d7b-86ab-6b39fe359a32> ;
	<http://vocabulary.semantic-web.at/cocktail-ontology/iba> <http://www.iba-world.com/index.php?option=com_content&id=204&Itemid=532> ;
	<http://vocabulary.semantic-web.at/cocktail-ontology/image> <http://upload.wikimedia.org/wikipedia/commons/thumb/1/10/Planters_Punch_2.jpg/440px-Planters_Punch_2.jpg> ;
	<http://vocabulary.semantic-web.at/cocktail-ontology/preparation> "Pour all ingredients, except the bitters, into shaker filled with ice. Shake well. Pour into large glass, filled with ice. Add Angostura bitters, “on top”. Garnish with cocktail cherry and pineapple."@en ;
	<http://vocabulary.semantic-web.at/cocktail-ontology/served> "On the rocks; poured over ice"@en ;
	<http://vocabulary.semantic-web.at/cocktail-ontology/uses> <http://vocabulary.semantic-web.at/cocktails/a54d2096-6214-4006-beaf-afcc77824710> ;
	<http://vocabulary.semantic-web.at/cocktail-ontology/uses_2> <http://vocabulary.semantic-web.at/cocktails/62fbc16f-3f84-4cc7-8c6f-5afebfc1510a> , <http://vocabulary.semantic-web.at/cocktails/f9d7d22d-5d57-434a-b9e1-b9c8cde324e9> ;
	a <http://vocabulary.semantic-web.at/cocktail-ontology/Cocktail> , skos:Concept ;
	skos:broader <http://vocabulary.semantic-web.at/cocktails/54702498-ad42-4af6-b28a-2276215450da> , <http://vocabulary.semantic-web.at/cocktails/caae2ea0-7e60-400b-a2bb-14ef79720668> ;
	skos:prefLabel "Planter's Punch"@en .

<http://vocabulary.semantic-web.at/cocktails/9c2ce399-c6ae-4f4d-bf37-7fd8ffe2a19d> dcterms:contributor <http://localhost/user/blumauera> ;
	dcterms:created "2015-05-01T08:47:30Z"^^xsd:dateTime ;
	dcterms:creator <http://localhost/user/blumauera> ;
	dcterms:modified "2015-07-02T14:55:55Z"^^xsd:dateTime ;
	<http://schema.semantic-web.at/ppt/inScheme> <http://vocabulary.semantic-web.at/cocktails/591cf89a-57af-49b8-9042-3fc77408c93e> ;
	<http://schema.semantic-web.at/ppt/inSubtree> <http://vocabulary.semantic-web.at/cocktails/e86c1671-4a67-494b-ae5d-bcb750865acc> ;
	<http://vocabulary.semantic-web.at/cocktail-ontology/is-part-of> <http://vocabulary.semantic-web.at/cocktails/0bbdca98-077b-48d1-99d6-47eca59c442c> , <http://vocabulary.semantic-web.at/cocktails/22f838ea-3c2b-4b63-99d1-fdb6280b5705> , <http://vocabulary.semantic-web.at/cocktails/236b36df-93ca-4408-836c-133ace53798a> , <http://vocabulary.semantic-web.at/cocktails/268fb62f-8ef1-45cd-844f-8c7da85a6a0b> , <http://vocabulary.semantic-web.at/cocktails/36671f9c-904a-4629-937a-519d094ecefc> , <http://vocabulary.semantic-web.at/cocktails/383ea520-07b2-4dc9-8827-8fc84fb7749c> , <http://vocabulary.semantic-web.at/cocktails/43b786b6-a1f1-4b7f-a5d9-be43d386ffb4> , <http://vocabulary.semantic-web.at/cocktails/44cc99c1-28ac-4c50-a55d-7244b2c5c07b> , <http://vocabulary.semantic-web.at/cocktails/53a05366-d473-4eb4-ac66-0d0119e0b759> , <http://vocabulary.semantic-web.at/cocktails/563bf7e0-0f40-41b6-a749-c4e94760204d> , <http://vocabulary.semantic-web.at/cocktails/72a77af2-bbee-4b75-871f-a96dcd3a452b> , <http://vocabulary.semantic-web.at/cocktails/76c0e55c-22df-4489-9551-4fe8a6a649f8> , <http://vocabulary.semantic-web.at/cocktails/9c287d15-c699-4f56-bd65-bf8cc75a2cca> , <http://vocabulary.semantic-web.at/cocktails/a73d88e9-0c50-45d2-b364-9dec5abe206d> , <http://vocabulary.semantic-web.at/cocktails/b33091cd-8c57-45e3-a89b-9de91ffce1e8> , <http://vocabulary.semantic-web.at/cocktails/c151ee28-45d2-4128-8587-1f1b69060d9d> , <http://vocabulary.semantic-web.at/cocktails/c3ae5830-1bfd-4f37-afc9-3e88849d03cf> , <http://vocabulary.semantic-web.at/cocktails/ce8f4591-ccd4-4d90-a761-244115d64061> , <http://vocabulary.semantic-web.at/cocktails/e039633b-03c1-47bd-a705-a104a4323e45> ;
	a <http://vocabulary.semantic-web.at/cocktail-ontology/Beverages> , <http://vocabulary.semantic-web.at/cocktail-ontology/Ingredients> , <http://vocabulary.semantic-web.at/cocktail-ontology/Non-alcoholic-Beverages> , skos:Concept ;
	skos:broader <http://vocabulary.semantic-web.at/cocktails/6c0607a9-410d-4b65-87a1-b189a8e36352> ;
	skos:prefLabel "Lemon juice"@en .

<http://vocabulary.semantic-web.at/cocktails/9ca4c18b-03f7-4c4f-802e-e18299702bad> dcterms:contributor <http://localhost/user/blumauera> ;
	dcterms:created "2015-05-01T14:33:26Z"^^xsd:dateTime ;
	dcterms:creator <http://localhost/user/blumauera> ;
	dcterms:modified "2015-05-05T07:17:13Z"^^xsd:dateTime ;
	<http://schema.semantic-web.at/ppt/inScheme> <http://vocabulary.semantic-web.at/cocktails/591cf89a-57af-49b8-9042-3fc77408c93e> ;
	<http://schema.semantic-web.at/ppt/inSubtree> <http://vocabulary.semantic-web.at/cocktails/403d1249-f37f-4f43-bebf-8dde9677d886> ;
	<http://vocabulary.semantic-web.at/cocktail-ontology/is-part-of> <http://vocabulary.semantic-web.at/cocktails/a0fba95c-d29e-4954-8800-f5e6de1e6f86> ;
	a <http://vocabulary.semantic-web.at/cocktail-ontology/Alcoholic-Beverages> , <http://vocabulary.semantic-web.at/cocktail-ontology/Beverages> , <http://vocabulary.semantic-web.at/cocktail-ontology/Ingredients> , skos:Concept ;
	skos:altLabel "Martini vermouth"@en ;
	skos:broader <http://vocabulary.semantic-web.at/cocktails/8cfd00fe-9f5a-414e-be27-858a8bc43c7c> ;
	skos:definition "Martini is a brand of Italian vermouth, named after the Martini & Rossi Distilleria Nazionale di Spirito di Vino, in Turin. From within the Distilleria emerged Alessandro Martini, Luigi Rossi and Teofilo Sola. They changed the company name to Martini, Sola & Cia in 1863 and it was in 1879 that the Sola family sold its interests to the remaining partners who renamed the company Martini & Rossi, as it stands today."@en ;
	skos:exactMatch <http://dbpedia.org/resource/Martini_(vermouth)> ;
	skos:narrower <http://vocabulary.semantic-web.at/cocktails/96c173d1-f047-4811-8950-45b071588fdc> ;
	skos:prefLabel "Martini"@en .

<http://vocabulary.semantic-web.at/cocktails/9cbe0ac7-b97d-431c-8ea6-a1d7ccc44d4f> dcterms:created "2015-11-18T14:35:36Z"^^xsd:dateTime ;
	dcterms:creator <http://localhost/user/blumauera> ;
	<http://schema.semantic-web.at/ppt/inScheme> <http://vocabulary.semantic-web.at/cocktails/591cf89a-57af-49b8-9042-3fc77408c93e> ;
	<http://schema.semantic-web.at/ppt/inSubtree> <http://vocabulary.semantic-web.at/cocktails/403d1249-f37f-4f43-bebf-8dde9677d886> ;
	a <http://vocabulary.semantic-web.at/cocktail-ontology/Alcoholic-Beverages> , <http://vocabulary.semantic-web.at/cocktail-ontology/Beverages> , <http://vocabulary.semantic-web.at/cocktail-ontology/Ingredients> , skos:Concept ;
	skos:broader <http://vocabulary.semantic-web.at/cocktails/27c48d24-bb0b-46a3-9b0c-4b09e38a4b07> ;
	skos:narrower <http://vocabulary.semantic-web.at/cocktails/6420f3aa-5146-4893-b3ea-04033b26c915> ;
	skos:prefLabel "Cinnamon schnapps"@en .

<http://vocabulary.semantic-web.at/cocktails/9d9fb486-a0dd-4d1a-b65e-7346a626cadf> dcterms:contributor <http://localhost/user/blumauera> ;
	dcterms:created "2015-05-03T17:30:11Z"^^xsd:dateTime ;
	dcterms:creator <http://localhost/user/blumauera> ;
	dcterms:modified "2015-05-03T17:32:12Z"^^xsd:dateTime ;
	<http://schema.semantic-web.at/ppt/inScheme> <http://vocabulary.semantic-web.at/cocktails/87384ce8-f20a-4201-b06d-3e0b8d832e5d> ;
	<http://schema.semantic-web.at/ppt/inSubtree> <http://vocabulary.semantic-web.at/cocktails/3c94f5fc-4664-4177-a880-88643c0be9c1> ;
	<http://vocabulary.semantic-web.at/cocktail-ontology/is-used-by_2> <http://vocabulary.semantic-web.at/cocktails/bca7bc6d-6709-48b8-ae52-fe194c212398> ;
	a <http://vocabulary.semantic-web.at/cocktail-ontology/Garnish> , <http://vocabulary.semantic-web.at/cocktail-ontology/Ingredients> , skos:Concept ;
	skos:altLabel "Cane sugar"@en , "Caña de Azucar"@en , "Saccharum"@en , "Saccharum officinarum L"@en , "Sugar Cane"@en , "Sugar cane"@en , "Sugar canes"@en , "Sugar-cane"@en , "Sugercane"@en ;
	skos:broader <http://vocabulary.semantic-web.at/cocktails/3c94f5fc-4664-4177-a880-88643c0be9c1> ;
	skos:definition "Sugarcane, or Sugar cane, is any of six to 37 species (depending on which taxonomic system is used) of tall perennial true grasses of the genus Saccharum, tribe Andropogoneae, native to the warm temperate to tropical regions of South Asia. They have stout jointed fibrous stalks that are rich in sugar, and measure two to six metres (6 to 19 feet) tall. All sugar cane species interbreed, and the major commercial cultivars are complex hybrids."@en ;
	skos:exactMatch dbpedia:Sugarcane ;
	skos:prefLabel "Sugarcane"@en .

<http://vocabulary.semantic-web.at/cocktails/a0fba95c-d29e-4954-8800-f5e6de1e6f86> dcterms:contributor <http://localhost/user/blumauera> ;
	dcterms:created "2015-05-01T14:32:05Z"^^xsd:dateTime ;
	dcterms:creator <http://localhost/user/blumauera> ;
	dcterms:modified "2016-03-25T12:28:05Z"^^xsd:dateTime ;
	<http://schema.semantic-web.at/ppt/inScheme> <http://vocabulary.semantic-web.at/cocktails/8d052dfc-44bf-4985-8ce3-4564570a161b> ;
	<http://vocabulary.semantic-web.at/cocktail-ontology/consists-of> <http://vocabulary.semantic-web.at/cocktails/5d96c50c-ee48-4c40-bb4c-4b9a42d11de6> , <http://vocabulary.semantic-web.at/cocktails/9ca4c18b-03f7-4c4f-802e-e18299702bad> ;
	<http://vocabulary.semantic-web.at/cocktail-ontology/iba> <http://www.iba-world.com/index.php?option=com_content&id=195&Itemid=532> ;
	<http://vocabulary.semantic-web.at/cocktail-ontology/image> <http://upload.wikimedia.org/wikipedia/commons/1/10/Dry_Martini-2.jpg> ;
	<http://vocabulary.semantic-web.at/cocktail-ontology/preparation> "Straight: Pour all ingredients into mixing glass with ice cubes. Stir well. Strain in chilled martini cocktail glass. Squeeze oil from lemon peel onto the drink, or garnish with olive."@en ;
	<http://vocabulary.semantic-web.at/cocktail-ontology/served> "straight (or on the rocks)"@en ;
	<http://vocabulary.semantic-web.at/cocktail-ontology/uses> <http://vocabulary.semantic-web.at/cocktails/19dee0d8-fd30-469f-9ecd-91c902ff717c> ;
	<http://vocabulary.semantic-web.at/cocktail-ontology/uses_2> <http://vocabulary.semantic-web.at/cocktails/33df103a-03ac-4177-b620-7953fe094236> , <http://vocabulary.semantic-web.at/cocktails/cec5e96c-41c6-4b82-ab3a-0a057a54f70a> ;
	a <http://vocabulary.semantic-web.at/cocktail-ontology/Cocktail> , skos:Concept ;
	skos:altLabel "Bradford (beverage)"@en , "Dry Martini"@en , "Martini cocktail"@en , "Montgomery cocktail"@en , "Perfect Martini"@en , "Tamatini"@en ;
	skos:broader <http://vocabulary.semantic-web.at/cocktails/caae2ea0-7e60-400b-a2bb-14ef79720668> ;
	skos:definition "The martini is a cocktail made with gin and vermouth, and garnished with an olive or a lemon twist. Over the years, the martini has become one of the best-known mixed alcoholic beverages. H. L. Mencken called the martini \"the only American invention as perfect as the sonnet\" and E. B. White called it \"the elixir of quietude\"."@en ;
	skos:exactMatch <http://dbpedia.org/resource/Martini_(cocktail)> ;
	skos:prefLabel "Martini"@en .

<http://vocabulary.semantic-web.at/cocktails/a12b3836-dba0-49e9-92c6-7725ccf35944> dcterms:contributor <http://localhost/user/blumauera> ;
	dcterms:created "2015-05-02T07:28:25Z"^^xsd:dateTime ;
	dcterms:creator <http://localhost/user/blumauera> ;
	dcterms:modified "2015-05-06T12:27:10Z"^^xsd:dateTime ;
	<http://schema.semantic-web.at/ppt/inScheme> <http://vocabulary.semantic-web.at/cocktails/591cf89a-57af-49b8-9042-3fc77408c93e> ;
	<http://schema.semantic-web.at/ppt/inSubtree> <http://vocabulary.semantic-web.at/cocktails/403d1249-f37f-4f43-bebf-8dde9677d886> ;
	<http://vocabulary.semantic-web.at/cocktail-ontology/is-part-of> <http://vocabulary.semantic-web.at/cocktails/33d9a47f-0622-4b0f-ad1b-62eb96fc6799> ;
	a <http://vocabulary.semantic-web.at/cocktail-ontology/Alcoholic-Beverages> , <http://vocabulary.semantic-web.at/cocktail-ontology/Beverages> , <http://vocabulary.semantic-web.at/cocktail-ontology/Ingredients> , skos:Concept ;
	skos:broader <http://vocabulary.semantic-web.at/cocktails/2944baef-5338-421b-a5f5-0e51f75244c2> ;
	skos:narrower <http://vocabulary.semantic-web.at/cocktails/8d5e2abc-6280-42b7-8e21-8bbc30f7509f> ;
	skos:prefLabel "Coffee liqueur"@en .

<http://vocabulary.semantic-web.at/cocktails/a1c1e015-91fd-4f6e-b2a8-5edae9aa0b9d> dcterms:contributor <http://localhost/user/blumauera> ;
	dcterms:created "2015-05-02T08:25:08Z"^^xsd:dateTime ;
	dcterms:creator <http://localhost/user/blumauera> ;
	dcterms:modified "2015-05-06T12:56:24Z"^^xsd:dateTime ;
	<http://schema.semantic-web.at/ppt/inScheme> <http://vocabulary.semantic-web.at/cocktails/591cf89a-57af-49b8-9042-3fc77408c93e> ;
	<http://schema.semantic-web.at/ppt/inSubtree> <http://vocabulary.semantic-web.at/cocktails/403d1249-f37f-4f43-bebf-8dde9677d886> ;
	<http://vocabulary.semantic-web.at/cocktail-ontology/is-part-of> <http://vocabulary.semantic-web.at/cocktails/45788a96-1fde-486b-80fc-31ad243bba31> , <http://vocabulary.semantic-web.at/cocktails/52117ab2-dcb8-4d28-a366-ddd932e58219> , <http://vocabulary.semantic-web.at/cocktails/c8f4f6bd-4ac1-456a-a3aa-595e4b93d979> ;
	a <http://vocabulary.semantic-web.at/cocktail-ontology/Alcoholic-Beverages> , <http://vocabulary.semantic-web.at/cocktail-ontology/Beverages> , <http://vocabulary.semantic-web.at/cocktail-ontology/Ingredients> , skos:Concept ;
	skos:broader <http://vocabulary.semantic-web.at/cocktails/2944baef-5338-421b-a5f5-0e51f75244c2> ;
	skos:narrower <http://vocabulary.semantic-web.at/cocktails/80baac32-dfeb-461d-89cf-decf60f0709a> , <http://vocabulary.semantic-web.at/cocktails/ca113086-9563-4831-8a14-f9eb5cbaa49e> ;
	skos:prefLabel "Almond-flavored liqueur"@en .

<http://vocabulary.semantic-web.at/cocktails/a293047d-788b-4e8c-96bc-65e62fec4b0b> dcterms:contributor <http://localhost/user/blumauera> ;
	dcterms:created "2015-05-02T07:25:41Z"^^xsd:dateTime ;
	dcterms:creator <http://localhost/user/blumauera> ;
	dcterms:modified "2015-05-27T12:48:42Z"^^xsd:dateTime ;
	<http://schema.semantic-web.at/ppt/inScheme> <http://vocabulary.semantic-web.at/cocktails/591cf89a-57af-49b8-9042-3fc77408c93e> ;
	<http://schema.semantic-web.at/ppt/inSubtree> <http://vocabulary.semantic-web.at/cocktails/d5286375-41b3-468b-9602-8fcf698e3e83> ;
	<http://vocabulary.semantic-web.at/cocktail-ontology/is-part-of> <http://vocabulary.semantic-web.at/cocktails/2c682ed8-e2ba-473e-8cb7-979598080e18> , <http://vocabulary.semantic-web.at/cocktails/4d15a643-f7c7-4ee5-8f56-4ebd2bcf74b5> , <http://vocabulary.semantic-web.at/cocktails/698723d7-e8b8-410e-91a8-9bdc867b3f8a> ;
	a <http://vocabulary.semantic-web.at/cocktail-ontology/Alcoholic-Beverages> , <http://vocabulary.semantic-web.at/cocktail-ontology/Beverages> , <http://vocabulary.semantic-web.at/cocktail-ontology/Ingredients> , skos:Concept ;
	skos:altLabel "Ghera"@en , "Grappolo spargolo"@en , "Prosecco balbi"@en , "Prosecco tondo"@en , "Proseko"@en , "Sciorina"@en , "Serprina"@en , "sparkling"@en ;
	skos:broader <http://vocabulary.semantic-web.at/cocktails/71399fc3-e67c-4b55-88a7-64c6b96128bc> ;
	skos:definition "Prosecco is an Italian sparkling wine; generally a Dry or Extra Dry ; normally made from Glera (\"Prosecco\") grapes. DOC prosecco is produced in the regions of Veneto and Friuli Venezia Giulia in Italy, and traditionally mainly in the areas near Conegliano and Valdobbiadene, in the hills north of Treviso. Prosecco is known as the main ingredient of the Bellini cocktail and has more recently become popular as a less expensive substitute for Champagne."@en ;
	skos:exactMatch dbpedia:Prosecco ;
	skos:prefLabel "Prosecco"@en .

<http://vocabulary.semantic-web.at/cocktails/a2b8e0e7-0dd0-40e2-a9a4-6178c7728cd0> dcterms:contributor <http://localhost/user/blumauera> ;
	dcterms:created "2015-05-01T08:33:50Z"^^xsd:dateTime ;
	dcterms:creator <http://localhost/user/blumauera> ;
	dcterms:modified "2015-05-03T11:29:52Z"^^xsd:dateTime ;
	<http://schema.semantic-web.at/ppt/inScheme> <http://vocabulary.semantic-web.at/cocktails/591cf89a-57af-49b8-9042-3fc77408c93e> ;
	<http://schema.semantic-web.at/ppt/inSubtree> <http://vocabulary.semantic-web.at/cocktails/e86c1671-4a67-494b-ae5d-bcb750865acc> ;
	a <http://vocabulary.semantic-web.at/cocktail-ontology/Beverages> , <http://vocabulary.semantic-web.at/cocktail-ontology/Ingredients> , <http://vocabulary.semantic-web.at/cocktail-ontology/Non-alcoholic-Beverages> , skos:Concept ;
	skos:altLabel "Carbonated Glucosic Beverage"@en , "Carbonated beverage"@en , "Carbonated beverages"@en , "Carbonated soda"@en , "Carbonated soft drink"@en , "Citrus soda"@en , "Cool drink"@en , "Fizzy drink"@en , "Fizzy drinks"@en , "Fizzy pop"@en , "Flavored water"@en , "Flavoured water"@en , "Graveyard Drink"@en , "High-sugar drink"@en , "Non-alcoholic"@en , "Non-alcoholic drink"@en , "Non-alcoholic drinks"@en , "Pop drinks"@en , "Seedrink"@en , "Soda (soft drink)"@en , "Soda and the body"@en , "Soda drinking"@en , "Soda names"@en , "Soda pop"@en , "Sodapop"@en , "Soft drinks"@en , "Soft-drink"@en , "Softdrink"@en , "Sugar drink"@en , "Sugary drink"@en , "Sweet drink"@en , "The effects of soda"@en ;
	skos:broader <http://vocabulary.semantic-web.at/cocktails/e86c1671-4a67-494b-ae5d-bcb750865acc> ;
	skos:definition "A soft drink (also called soda, pop, coke, soda pop, fizzy drink, tonic, seltzer, mineral, sparkling water, or carbonated beverage) is a beverage that typically contains water (often, but not always carbonated water), usually a sweetener, and usually a flavoring agent. The sweetener may be sugar, high-fructose corn syrup, fruit juice, sugar substitutes (in the case of diet drinks) or some combination of these."@en ;
	skos:exactMatch dbpedia:Soft_drink ;
	skos:narrower <http://vocabulary.semantic-web.at/cocktails/0f11bcdf-a69e-451f-b824-48b1743c5916> , <http://vocabulary.semantic-web.at/cocktails/84c72e0e-7830-46ef-ac35-44cad56d27ec> , <http://vocabulary.semantic-web.at/cocktails/89ac12aa-d4f9-46d0-b127-fd8f4c21fbcc> ;
	skos:prefLabel "Soft drink"@en .

<http://vocabulary.semantic-web.at/cocktails/a3fcf23f-e2e0-4ba6-873a-bc6ae2870011> dcterms:contributor <http://localhost/user/blumauera> ;
	dcterms:created "2015-05-05T12:59:42Z"^^xsd:dateTime ;
	dcterms:creator <http://localhost/user/blumauera> ;
	dcterms:modified "2016-03-09T17:13:38Z"^^xsd:dateTime ;
	<http://schema.semantic-web.at/ppt/inScheme> <http://vocabulary.semantic-web.at/cocktails/87384ce8-f20a-4201-b06d-3e0b8d832e5d> ;
	<http://vocabulary.semantic-web.at/cocktail-ontology/is-part-of> <http://vocabulary.semantic-web.at/cocktails/a5db05ca-eda3-41ef-a8ab-ba77b3e4baba> ;
	a <http://vocabulary.semantic-web.at/cocktail-ontology/Ingredients> , skos:Concept ;
	skos:altLabel "Antibacterial effects of honey"@en , "Bastard honey"@en , "Bee vomit"@en , "Clover Honey"@en , "Clover honey"@en , "Finland Honey"@en , "Finland honey"@en , "Heather honey"@en , "Himalayan honey"@en , "Honey dipper"@en , "Honey usage in recovering the wounds"@en , "Honeydipper"@en , "Honeyed"@en , "Honeyed water"@en , "Honeying"@en , "Honeys"@en , "Honied"@en , "Oxymellin"@en , "Philippines Honey"@en , "Philippines honey"@en , "Raw honey"@en , "Wild honeys"@en , "🍯"@en ;
	skos:definition "Honey is a sweet food made by bees using nectar from flowers. The variety produced by honey bees is the one most commonly referred to, as it is the type of honey collected by beekeepers and consumed by humans. Honey produced by other bees and insects has distinctly different properties. Honey bees transform nectar into honey by a process of regurgitation and evaporation. They store it as a primary food source in wax honeycombs inside the beehive."@en ;
	skos:exactMatch dbpedia:Honey ;
	skos:prefLabel "Honey"@en ;
	skos:topConceptOf <http://vocabulary.semantic-web.at/cocktails/87384ce8-f20a-4201-b06d-3e0b8d832e5d> .

<http://vocabulary.semantic-web.at/cocktails/a47e8f08-057a-45f2-8398-9be51ed351fc> dcterms:contributor <http://localhost/user/blumauera> ;
	dcterms:created "2015-05-02T19:27:02Z"^^xsd:dateTime ;
	dcterms:creator <http://localhost/user/blumauera> ;
	dcterms:modified "2015-05-07T06:47:48Z"^^xsd:dateTime ;
	<http://schema.semantic-web.at/ppt/inScheme> <http://vocabulary.semantic-web.at/cocktails/8d052dfc-44bf-4985-8ce3-4564570a161b> ;
	<http://vocabulary.semantic-web.at/cocktail-ontology/consists-of> <http://vocabulary.semantic-web.at/cocktails/22df810d-e509-4da8-979c-0758e94de3e6> , <http://vocabulary.semantic-web.at/cocktails/88f5de3d-3de4-4a2f-9523-50bc7bb06600> , <http://vocabulary.semantic-web.at/cocktails/d530df52-cc54-4be3-8409-85734e5ec67f> ;
	<http://vocabulary.semantic-web.at/cocktail-ontology/iba> <http://www.iba-world.com/index.php?option=com_content&id=244&Itemid=532> ;
	<http://vocabulary.semantic-web.at/cocktail-ontology/image> <http://upload.wikimedia.org/wikipedia/commons/6/61/Kamikaze.jpg> ;
	<http://vocabulary.semantic-web.at/cocktail-ontology/preparation> "Shake and strain into a chilled cocktail glass."@en ;
	<http://vocabulary.semantic-web.at/cocktail-ontology/served> "Straight up; without ice"@en ;
	<http://vocabulary.semantic-web.at/cocktail-ontology/uses> <http://vocabulary.semantic-web.at/cocktails/19dee0d8-fd30-469f-9ecd-91c902ff717c> ;
	<http://vocabulary.semantic-web.at/cocktail-ontology/uses_2> <http://vocabulary.semantic-web.at/cocktails/021c85c0-a60a-4414-8fd8-bd3383b794f1> ;
	a <http://vocabulary.semantic-web.at/cocktail-ontology/Cocktail> , skos:Concept ;
	skos:altLabel "Kamikaze (drink)"@en , "Vodka sour"@en ;
	skos:broader <http://vocabulary.semantic-web.at/cocktails/7516b400-963a-4151-8fdc-f6b23bad1dd5> , <http://vocabulary.semantic-web.at/cocktails/ccee1079-43df-4ff1-bef0-d15d3dc8fa6f> ;
	skos:definition "The Kamikaze is made of equal parts vodka, triple sec and lime juice. According to the International Bartenders Association, it is served straight up in a cocktail glass. Garnish is typically a wedge or twist of lime."@en ;
	skos:exactMatch <http://dbpedia.org/resource/Kamikaze_(cocktail)> ;
	skos:prefLabel "Kamikaze"@en .

<http://vocabulary.semantic-web.at/cocktails/a54d2096-6214-4006-beaf-afcc77824710> dcterms:contributor <http://localhost/user/blumauera> ;
	dcterms:created "2015-05-01T07:56:01Z"^^xsd:dateTime ;
	dcterms:creator <http://localhost/user/blumauera> ;
	dcterms:modified "2015-07-02T15:03:46Z"^^xsd:dateTime ;
	<http://schema.semantic-web.at/ppt/inScheme> <http://vocabulary.semantic-web.at/cocktails/f09732a9-a0e6-494a-8ce9-299ef036aaaf> ;
	<http://vocabulary.semantic-web.at/cocktail-ontology/image_2> <http://upload.wikimedia.org/wikipedia/commons/thumb/d/db/Highball_glass_silhouette.svg/31px-Highball_glass_silhouette.svg.png> ;
	<http://vocabulary.semantic-web.at/cocktail-ontology/is-used-by> <http://vocabulary.semantic-web.at/cocktails/0f8cc862-9056-49be-b636-cd22f8d7282d> , <http://vocabulary.semantic-web.at/cocktails/12f4790a-560f-4e1c-b57a-53b8171ae39a> , <http://vocabulary.semantic-web.at/cocktails/1529fd23-9c55-45d7-b8c6-b0fc229a3871> , <http://vocabulary.semantic-web.at/cocktails/268fb62f-8ef1-45cd-844f-8c7da85a6a0b> , <http://vocabulary.semantic-web.at/cocktails/2c032fe6-a518-44be-851a-dbf1c253be63> , <http://vocabulary.semantic-web.at/cocktails/383ea520-07b2-4dc9-8827-8fc84fb7749c> , <http://vocabulary.semantic-web.at/cocktails/43111fc3-3b59-420c-a588-024cd2d33896> , <http://vocabulary.semantic-web.at/cocktails/4d15a643-f7c7-4ee5-8f56-4ebd2bcf74b5> , <http://vocabulary.semantic-web.at/cocktails/53a05366-d473-4eb4-ac66-0d0119e0b759> , <http://vocabulary.semantic-web.at/cocktails/55c40695-8b41-41ed-8c6a-70fe6930067e> , <http://vocabulary.semantic-web.at/cocktails/72a77af2-bbee-4b75-871f-a96dcd3a452b> , <http://vocabulary.semantic-web.at/cocktails/79d4686d-4f5b-4067-a2ef-99beccc51242> , <http://vocabulary.semantic-web.at/cocktails/9c287d15-c699-4f56-bd65-bf8cc75a2cca> , <http://vocabulary.semantic-web.at/cocktails/a5db05ca-eda3-41ef-a8ab-ba77b3e4baba> , <http://vocabulary.semantic-web.at/cocktails/bed073f2-de84-4322-a490-4f34ec54c6d1> , <http://vocabulary.semantic-web.at/cocktails/c151ee28-45d2-4128-8587-1f1b69060d9d> , <http://vocabulary.semantic-web.at/cocktails/ce8f4591-ccd4-4d90-a761-244115d64061> , <http://vocabulary.semantic-web.at/cocktails/dff0a7f4-ded0-48d5-bd31-881b70fbe36a> , <http://vocabulary.semantic-web.at/cocktails/eddf4894-1683-44e9-9ee3-7920d3729d71> , <http://vocabulary.semantic-web.at/cocktails/f01f6a10-01a5-4810-860f-d3a52fd36b1b> ;
	a <http://vocabulary.semantic-web.at/cocktail-ontology/Drinkware> , skos:Concept ;
	skos:altLabel "Hi-Ball"@en , "Hiball"@en ;
	skos:broader <http://vocabulary.semantic-web.at/cocktails/2e839563-8037-4e59-8dbf-27736605d687> ;
	skos:definition "A highball glass, a glass tumbler, contains 8 to 12 fluid ounces (240 to 350 ml). It is used to serve highball cocktails and other mixed drinks. A highball glass is taller than an Old Fashioned glass, and shorter and wider than a Collins glass."@en ;
	skos:exactMatch dbpedia:Highball_glass ;
	skos:prefLabel "Highball glass"@en .

<http://vocabulary.semantic-web.at/cocktails/a5db05ca-eda3-41ef-a8ab-ba77b3e4baba> dcterms:contributor <http://localhost/user/blumauera> ;
	dcterms:created "2015-05-02T19:43:36Z"^^xsd:dateTime ;
	dcterms:creator <http://localhost/user/blumauera> ;
	dcterms:modified "2015-05-05T13:06:43Z"^^xsd:dateTime ;
	<http://schema.semantic-web.at/ppt/inScheme> <http://vocabulary.semantic-web.at/cocktails/8d052dfc-44bf-4985-8ce3-4564570a161b> ;
	<http://vocabulary.semantic-web.at/cocktail-ontology/consists-of> <http://vocabulary.semantic-web.at/cocktails/2ce50273-13b2-4ba1-9ff2-8cfbd835c1f2> , <http://vocabulary.semantic-web.at/cocktails/48499a53-a687-4156-b966-1e16e3e967bd> , <http://vocabulary.semantic-web.at/cocktails/790d1a2d-d20b-4ecd-a3d0-f9a931156e14> , <http://vocabulary.semantic-web.at/cocktails/7dede323-e986-4417-b723-c9c7a7fe82ba> , <http://vocabulary.semantic-web.at/cocktails/88f5de3d-3de4-4a2f-9523-50bc7bb06600> , <http://vocabulary.semantic-web.at/cocktails/a3fcf23f-e2e0-4ba6-873a-bc6ae2870011> , <http://vocabulary.semantic-web.at/cocktails/e2d63a1c-56e7-47d2-b01b-8cf88cac3d8b> , <http://vocabulary.semantic-web.at/cocktails/f159e33f-fed0-4382-93b9-acfa28f23937> ;
	<http://vocabulary.semantic-web.at/cocktail-ontology/iba> <http://www.iba-world.com/index.php?option=com_content&id=250&Itemid=532> ;
	<http://vocabulary.semantic-web.at/cocktail-ontology/image> <http://www.iba-world.com/images/cocktail_drinks/vampiro.jpg> ;
	<http://vocabulary.semantic-web.at/cocktail-ontology/preparation> "Pour all ingredients into a shaker filled with ice. Shake well, to relaese the flavour of the chili.  Strain into a highball glass, filled with ice.  Garnish with a wedge of lime and a chili (green or red)."@en ;
	<http://vocabulary.semantic-web.at/cocktail-ontology/uses> <http://vocabulary.semantic-web.at/cocktails/a54d2096-6214-4006-beaf-afcc77824710> ;
	<http://vocabulary.semantic-web.at/cocktail-ontology/uses_2> <http://vocabulary.semantic-web.at/cocktails/e76e4e97-260a-4eef-af34-111938241931> ;
	a <http://vocabulary.semantic-web.at/cocktail-ontology/Cocktail> , skos:Concept ;
	skos:broader <http://vocabulary.semantic-web.at/cocktails/ccee1079-43df-4ff1-bef0-d15d3dc8fa6f> ;
	skos:prefLabel "Vampiro"@en .

<http://vocabulary.semantic-web.at/cocktails/a62bc4d7-b07a-4e32-9254-9facbeb8831d> dcterms:contributor <http://localhost/user/blumauera> ;
	dcterms:created "2015-05-02T19:13:44Z"^^xsd:dateTime ;
	dcterms:creator <http://localhost/user/blumauera> ;
	dcterms:modified "2015-05-02T19:13:44Z"^^xsd:dateTime ;
	<http://schema.semantic-web.at/ppt/inScheme> <http://vocabulary.semantic-web.at/cocktails/591cf89a-57af-49b8-9042-3fc77408c93e> ;
	<http://schema.semantic-web.at/ppt/inSubtree> <http://vocabulary.semantic-web.at/cocktails/403d1249-f37f-4f43-bebf-8dde9677d886> ;
	a <http://vocabulary.semantic-web.at/cocktail-ontology/Alcoholic-Beverages> , <http://vocabulary.semantic-web.at/cocktail-ontology/Beverages> , <http://vocabulary.semantic-web.at/cocktail-ontology/Ingredients> , skos:Concept ;
	skos:broader <http://vocabulary.semantic-web.at/cocktails/2944baef-5338-421b-a5f5-0e51f75244c2> ;
	skos:definition "A cream liqueur (not be confused with crème liqueur) is a liqueur that includes dairy cream among its ingredients."@en ;
	skos:exactMatch dbpedia:Cream_liqueur ;
	skos:narrower <http://vocabulary.semantic-web.at/cocktails/e5f9e219-d894-491c-a009-20336f5b8e7f> ;
	skos:prefLabel "Cream liqueur"@en .

<http://vocabulary.semantic-web.at/cocktails/a73d88e9-0c50-45d2-b364-9dec5abe206d> dcterms:contributor <http://localhost/user/blumauera> ;
	dcterms:created "2015-05-02T17:10:28Z"^^xsd:dateTime ;
	dcterms:creator <http://localhost/user/blumauera> ;
	dcterms:modified "2015-05-06T12:51:15Z"^^xsd:dateTime ;
	<http://schema.semantic-web.at/ppt/inScheme> <http://vocabulary.semantic-web.at/cocktails/8d052dfc-44bf-4985-8ce3-4564570a161b> ;
	<http://vocabulary.semantic-web.at/cocktail-ontology/consists-of> <http://vocabulary.semantic-web.at/cocktails/5d96c50c-ee48-4c40-bb4c-4b9a42d11de6> , <http://vocabulary.semantic-web.at/cocktails/71210bd1-3071-4533-8da4-fe0f7d7694a0> , <http://vocabulary.semantic-web.at/cocktails/9c2ce399-c6ae-4f4d-bf37-7fd8ffe2a19d> , <http://vocabulary.semantic-web.at/cocktails/cdbac85a-d5b7-40f3-9e98-4d7e176b5565> ;
	<http://vocabulary.semantic-web.at/cocktail-ontology/iba> <http://www.iba-world.com/index.php?option=com_content&id=221&Itemid=532> ;
	<http://vocabulary.semantic-web.at/cocktail-ontology/image> <http://upload.wikimedia.org/wikipedia/commons/thumb/0/0b/French_75.jpg/440px-French_75.jpg> ;
	<http://vocabulary.semantic-web.at/cocktail-ontology/preparation> "Pour all the ingredients, except champagne, into a shaker. Shake. Strain into a champagne flute.  Top up with champagne. Stir gently."@en ;
	<http://vocabulary.semantic-web.at/cocktail-ontology/uses> <http://vocabulary.semantic-web.at/cocktails/fece03b5-ec0b-4e47-964d-cc5dc09fd7fb> ;
	a <http://vocabulary.semantic-web.at/cocktail-ontology/Cocktail> , skos:Concept ;
	skos:broader <http://vocabulary.semantic-web.at/cocktails/204cd4e7-58d7-4417-837a-7f9cc41663c8> , <http://vocabulary.semantic-web.at/cocktails/b9bf3799-a4e4-47f7-9aea-7697cc998a34> ;
	skos:definition "French 75 is a cocktail made from gin, Champagne, lemon juice, and sugar. The drink was created in 1915 at the New York Bar in Paris---later Harry's New York Bar---by barman Harry MacElhone. The combination was said to have such a kick that it felt like being shelled with the powerful French 75mm field gun, also called a \"75 Cocktail\", or \"Soixante Quinze\" in French. The French 75 was popularized in America at the Stork Club in New York."@en ;
	skos:exactMatch <http://dbpedia.org/resource/French_75_(cocktail)> ;
	skos:prefLabel "French 75"@en .

<http://vocabulary.semantic-web.at/cocktails/abe8b872-3a29-49a3-9a8e-1b71db770a3f> dcterms:contributor <http://localhost/user/blumauera> ;
	dcterms:created "2015-05-01T08:02:10Z"^^xsd:dateTime ;
	dcterms:creator <http://localhost/user/blumauera> ;
	dcterms:modified "2015-05-07T06:36:50Z"^^xsd:dateTime ;
	<http://schema.semantic-web.at/ppt/inScheme> <http://vocabulary.semantic-web.at/cocktails/591cf89a-57af-49b8-9042-3fc77408c93e> ;
	<http://schema.semantic-web.at/ppt/inSubtree> <http://vocabulary.semantic-web.at/cocktails/e86c1671-4a67-494b-ae5d-bcb750865acc> ;
	<http://vocabulary.semantic-web.at/cocktail-ontology/is-part-of> <http://vocabulary.semantic-web.at/cocktails/12f4790a-560f-4e1c-b57a-53b8171ae39a> , <http://vocabulary.semantic-web.at/cocktails/926b14fe-1b83-4f46-bbf9-f946be1889aa> ;
	a <http://vocabulary.semantic-web.at/cocktail-ontology/Beverages> , <http://vocabulary.semantic-web.at/cocktail-ontology/Ingredients> , <http://vocabulary.semantic-web.at/cocktail-ontology/Non-alcoholic-Beverages> , skos:Concept ;
	skos:broader <http://vocabulary.semantic-web.at/cocktails/6c0607a9-410d-4b65-87a1-b189a8e36352> ;
	skos:definition "Grapefruit juice is the fruit juice from grapefruits. It is rich in Vitamin C and ranges from sweet-tart to very sour. Variations include white grapefruit, pink grapefruit and ruby red grapefruit juice."@en ;
	skos:exactMatch dbpedia:Grapefruit_juice ;
	skos:prefLabel "Grapefruit juice"@en .

<http://vocabulary.semantic-web.at/cocktails/af5df232-948a-4dc9-8dd1-1d7bfbf523f1> dcterms:created "2015-05-01T14:48:20Z"^^xsd:dateTime ;
	dcterms:creator <http://localhost/user/blumauera> ;
	<http://schema.semantic-web.at/ppt/inScheme> <http://vocabulary.semantic-web.at/cocktails/591cf89a-57af-49b8-9042-3fc77408c93e> ;
	<http://schema.semantic-web.at/ppt/inSubtree> <http://vocabulary.semantic-web.at/cocktails/403d1249-f37f-4f43-bebf-8dde9677d886> ;
	a <http://vocabulary.semantic-web.at/cocktail-ontology/Alcoholic-Beverages> , <http://vocabulary.semantic-web.at/cocktail-ontology/Beverages> , <http://vocabulary.semantic-web.at/cocktail-ontology/Ingredients> , skos:Concept ;
	skos:broader <http://vocabulary.semantic-web.at/cocktails/2944baef-5338-421b-a5f5-0e51f75244c2> ;
	skos:narrower <http://vocabulary.semantic-web.at/cocktails/c96d576c-9640-4c21-af92-d6da3560c9d0> ;
	skos:prefLabel "Anise-flavored liqueur"@en .

<http://vocabulary.semantic-web.at/cocktails/b00a123f-a2b5-49d2-8325-a81d1d26ddc6> dcterms:contributor <http://localhost/user/blumauera> ;
	dcterms:created "2015-05-02T19:43:49Z"^^xsd:dateTime ;
	dcterms:creator <http://localhost/user/blumauera> ;
	dcterms:modified "2015-05-05T13:09:09Z"^^xsd:dateTime ;
	<http://schema.semantic-web.at/ppt/inScheme> <http://vocabulary.semantic-web.at/cocktails/8d052dfc-44bf-4985-8ce3-4564570a161b> ;
	<http://vocabulary.semantic-web.at/cocktail-ontology/consists-of> <http://vocabulary.semantic-web.at/cocktails/108f19eb-a64b-47ce-b25f-c15049a0f4be> , <http://vocabulary.semantic-web.at/cocktails/22df810d-e509-4da8-979c-0758e94de3e6> , <http://vocabulary.semantic-web.at/cocktails/5d96c50c-ee48-4c40-bb4c-4b9a42d11de6> ;
	<http://vocabulary.semantic-web.at/cocktail-ontology/iba> <http://www.iba-world.com/index.php?option=com_content&id=251&Itemid=532> ;
	<http://vocabulary.semantic-web.at/cocktail-ontology/image> <http://upload.wikimedia.org/wikipedia/commons/thumb/b/be/%22Vesper_Martini_%28corrected%29.jpg%22.jpg/440px-%22Vesper_Martini_%28corrected%29.jpg%22.jpg> ;
	<http://vocabulary.semantic-web.at/cocktail-ontology/preparation> "Shake over ice until well chilled, then strain into a deep goblet and garnish with a thin slice of lemon peel."@en ;
	<http://vocabulary.semantic-web.at/cocktail-ontology/served> "Straight up; without ice"@en ;
	<http://vocabulary.semantic-web.at/cocktail-ontology/uses> <http://vocabulary.semantic-web.at/cocktails/fece03b5-ec0b-4e47-964d-cc5dc09fd7fb> ;
	<http://vocabulary.semantic-web.at/cocktail-ontology/uses_2> <http://vocabulary.semantic-web.at/cocktails/33df103a-03ac-4177-b620-7953fe094236> ;
	a <http://vocabulary.semantic-web.at/cocktail-ontology/Cocktail> , skos:Concept ;
	skos:altLabel "Green Vesper (Cocktail)"@en , "Green Vesper (cocktail)"@en , "Vesper Martini"@en , "Vesper cocktail"@en , "Vesper martini"@en ;
	skos:broader <http://vocabulary.semantic-web.at/cocktails/ccee1079-43df-4ff1-bef0-d15d3dc8fa6f> ;
	skos:definition "The Vesper or Vesper Martini is a cocktail that was originally made of gin, vodka, and Kina Lillet."@en ;
	skos:exactMatch <http://dbpedia.org/resource/Vesper_(cocktail)> ;
	skos:prefLabel "Vesper"@en .

<http://vocabulary.semantic-web.at/cocktails/b0885ae3-68e1-453d-8669-119e8464ff5f> dcterms:contributor <http://localhost/user/blumauera> ;
	dcterms:created "2015-05-01T08:30:28Z"^^xsd:dateTime ;
	dcterms:creator <http://localhost/user/blumauera> ;
	dcterms:modified "2015-05-03T10:07:36Z"^^xsd:dateTime ;
	<http://schema.semantic-web.at/ppt/inScheme> <http://vocabulary.semantic-web.at/cocktails/8d052dfc-44bf-4985-8ce3-4564570a161b> ;
	<http://vocabulary.semantic-web.at/cocktail-ontology/consists-of> <http://vocabulary.semantic-web.at/cocktails/7448dbed-7603-41f7-a316-99f754c9ae45> , <http://vocabulary.semantic-web.at/cocktails/7c831f82-c54d-4d31-ab40-97e1d6226cf2> , <http://vocabulary.semantic-web.at/cocktails/8cfd00fe-9f5a-414e-be27-858a8bc43c7c> ;
	<http://vocabulary.semantic-web.at/cocktail-ontology/iba> <http://www.iba-world.com/index.php?option=com_content&id=186> ;
	<http://vocabulary.semantic-web.at/cocktail-ontology/image> <http://upload.wikimedia.org/wikipedia/commons/2/2b/Americano_cocktail_at_Nightwood_Restaurant.jpg> ;
	<http://vocabulary.semantic-web.at/cocktail-ontology/is-variant-of> <http://vocabulary.semantic-web.at/cocktails/40ab50e9-66f1-411b-8220-ef8f05273542> ;
	<http://vocabulary.semantic-web.at/cocktail-ontology/preparation> "Pour the Campari and vermouth over ice into glass, add a splash of soda water and garnish with half orange slice."@en ;
	<http://vocabulary.semantic-web.at/cocktail-ontology/served> "On the rocks; poured over ice"@en ;
	<http://vocabulary.semantic-web.at/cocktail-ontology/uses> <http://vocabulary.semantic-web.at/cocktails/2dce3576-2603-41f9-8dce-ab21f639c2a7> ;
	<http://vocabulary.semantic-web.at/cocktail-ontology/uses_2> <http://vocabulary.semantic-web.at/cocktails/99171f20-c59f-40c4-998a-a9c8f1909168> ;
	a <http://vocabulary.semantic-web.at/cocktail-ontology/Cocktail> , skos:Concept ;
	skos:altLabel "Americano cocktail"@en ;
	skos:broader <http://vocabulary.semantic-web.at/cocktails/54702498-ad42-4af6-b28a-2276215450da> , <http://vocabulary.semantic-web.at/cocktails/caae2ea0-7e60-400b-a2bb-14ef79720668> ;
	skos:definition "The Americano is an IBA Official Cocktail composed of Campari, sweet vermouth, and club soda. The cocktail was first served in creator Gaspare Campari's bar, Caffè Campari, in the 1860s. It was originally known as the \"Milano-Torino\" because of its ingredients: Campari, the bitter liqueur, is from Milan and Cinzano, the vermouth, is from Turin (Torino). It is popular belief that in the early 1900s, the Italians noticed a surge of Americans who enjoyed the cocktail."@en ;
	skos:exactMatch <http://dbpedia.org/resource/Americano_(cocktail)> ;
	skos:prefLabel "Americano"@en .

<http://vocabulary.semantic-web.at/cocktails/b33091cd-8c57-45e3-a89b-9de91ffce1e8> dcterms:contributor <http://localhost/user/blumauera> ;
	dcterms:created "2015-05-03T10:21:29Z"^^xsd:dateTime ;
	dcterms:creator <http://localhost/user/blumauera> ;
	dcterms:modified "2015-05-03T10:26:05Z"^^xsd:dateTime ;
	<http://schema.semantic-web.at/ppt/inScheme> <http://vocabulary.semantic-web.at/cocktails/8d052dfc-44bf-4985-8ce3-4564570a161b> ;
	<http://vocabulary.semantic-web.at/cocktail-ontology/consists-of> <http://vocabulary.semantic-web.at/cocktails/3c94f5fc-4664-4177-a880-88643c0be9c1> , <http://vocabulary.semantic-web.at/cocktails/5d96c50c-ee48-4c40-bb4c-4b9a42d11de6> , <http://vocabulary.semantic-web.at/cocktails/9c2ce399-c6ae-4f4d-bf37-7fd8ffe2a19d> ;
	<http://vocabulary.semantic-web.at/cocktail-ontology/image> <http://assets.absolutdrinks.com/drinks/solid-background-black/soft-shadow/floor-reflection/415x655/gin-sour(85).jpg> ;
	<http://vocabulary.semantic-web.at/cocktail-ontology/preparation> "Fill a shaker with ice cubes. Add all ingredients. Shake and strain into a chilled rocks glass filled with ice cubes. Garnish with lemon and a maraschino berry."@en ;
	<http://vocabulary.semantic-web.at/cocktail-ontology/uses> <http://vocabulary.semantic-web.at/cocktails/2dce3576-2603-41f9-8dce-ab21f639c2a7> ;
	<http://vocabulary.semantic-web.at/cocktail-ontology/uses_2> <http://vocabulary.semantic-web.at/cocktails/33df103a-03ac-4177-b620-7953fe094236> , <http://vocabulary.semantic-web.at/cocktails/8a5e1790-d3c0-432e-bb85-709692b14f03> ;
	a <http://vocabulary.semantic-web.at/cocktail-ontology/Cocktail> , skos:Concept ;
	skos:broader <http://vocabulary.semantic-web.at/cocktails/54702498-ad42-4af6-b28a-2276215450da> , <http://vocabulary.semantic-web.at/cocktails/7516b400-963a-4151-8fdc-f6b23bad1dd5> ;
	skos:prefLabel "Gin sour"@en .

<http://vocabulary.semantic-web.at/cocktails/b3834414-af63-4e6f-9c3c-6c353e9600ee> dcterms:contributor <http://localhost/user/blumauera> ;
	dcterms:created "2015-05-01T14:07:34Z"^^xsd:dateTime ;
	dcterms:creator <http://localhost/user/blumauera> ;
	dcterms:modified "2015-05-03T10:13:56Z"^^xsd:dateTime ;
	<http://schema.semantic-web.at/ppt/inScheme> <http://vocabulary.semantic-web.at/cocktails/8d052dfc-44bf-4985-8ce3-4564570a161b> ;
	<http://vocabulary.semantic-web.at/cocktail-ontology/consists-of> <http://vocabulary.semantic-web.at/cocktails/16b625c5-3930-4cf8-a75b-b25e72f2bfb6> , <http://vocabulary.semantic-web.at/cocktails/5caedba2-9aef-4fab-b26b-6e20cf014419> , <http://vocabulary.semantic-web.at/cocktails/5d96c50c-ee48-4c40-bb4c-4b9a42d11de6> ;
	<http://vocabulary.semantic-web.at/cocktail-ontology/iba> <http://www.iba-world.com/index.php?option=com_content&id=187&Itemid=532> ;
	<http://vocabulary.semantic-web.at/cocktail-ontology/image> <http://www.iba-world.com/images/cocktail_drinks/angel_face.jpg> ;
	<http://vocabulary.semantic-web.at/cocktail-ontology/preparation> "Shake all ingredients with ice and strain contents into a cocktail glass."@en ;
	<http://vocabulary.semantic-web.at/cocktail-ontology/served> "Straight up; without ice"@en ;
	<http://vocabulary.semantic-web.at/cocktail-ontology/uses> <http://vocabulary.semantic-web.at/cocktails/19dee0d8-fd30-469f-9ecd-91c902ff717c> ;
	a <http://vocabulary.semantic-web.at/cocktail-ontology/Cocktail> , skos:Concept ;
	skos:broader <http://vocabulary.semantic-web.at/cocktails/caae2ea0-7e60-400b-a2bb-14ef79720668> ;
	skos:prefLabel "Angel Face"@en .

<http://vocabulary.semantic-web.at/cocktails/b523727e-7f49-4e1b-9c09-55002ee3a81e> dcterms:contributor <http://localhost/user/blumauera> ;
	dcterms:created "2015-05-01T14:53:30Z"^^xsd:dateTime ;
	dcterms:creator <http://localhost/user/blumauera> ;
	dcterms:modified "2015-05-05T07:58:39Z"^^xsd:dateTime ;
	<http://schema.semantic-web.at/ppt/inScheme> <http://vocabulary.semantic-web.at/cocktails/8d052dfc-44bf-4985-8ce3-4564570a161b> ;
	a <http://vocabulary.semantic-web.at/cocktail-ontology/Cocktail> , skos:Concept ;
	skos:altLabel "After-dinner drink"@en , "Aperitif"@en , "Aperitif and digestif"@en , "Aperitifs"@en , "Aperitivo"@en , "Apero"@en , "Apertif"@en , "Apéritif"@en , "Apéro"@en , "Digestif"@en , "Digestivo"@en ;
	skos:definition "Apéritifs and digestifs are alcoholic drinks that are normally served before (aperitif) or after (digestif) a meal."@en ;
	skos:exactMatch dbpedia:Ap%C3%A9ritif_and_digestif ;
	skos:narrower <http://vocabulary.semantic-web.at/cocktails/2c3083d2-8650-4460-b019-cae7aea38f14> , <http://vocabulary.semantic-web.at/cocktails/2c682ed8-e2ba-473e-8cb7-979598080e18> , <http://vocabulary.semantic-web.at/cocktails/ea946e07-e812-4492-a0ed-124d73bfbba7> ;
	skos:prefLabel "Apéritif and digestif"@en ;
	skos:topConceptOf <http://vocabulary.semantic-web.at/cocktails/8d052dfc-44bf-4985-8ce3-4564570a161b> .

<http://vocabulary.semantic-web.at/cocktails/b65b6d98-400f-47cf-94c7-d2566f10cf64> dcterms:contributor <http://localhost/user/blumauera> ;
	dcterms:created "2015-05-02T19:12:05Z"^^xsd:dateTime ;
	dcterms:creator <http://localhost/user/blumauera> ;
	dcterms:modified "2015-05-02T19:12:26Z"^^xsd:dateTime ;
	<http://schema.semantic-web.at/ppt/inScheme> <http://vocabulary.semantic-web.at/cocktails/8d052dfc-44bf-4985-8ce3-4564570a161b> ;
	a <http://vocabulary.semantic-web.at/cocktail-ontology/Cocktail> , skos:Concept ;
	skos:altLabel "Captain Kinger"@en , "Cocktail shooter"@en , "Cocktail shooters"@en , "Cocktail shot"@en , "Cocktail shots"@en , "Do a shot"@en , "Doing shots"@en , "Drink shot"@en , "Drink shots"@en , "Mixed drink shooters"@en , "Mixed drink shooters and drink shots"@en , "Molotov Cocktail (shot)"@en , "Shooter (beverage)"@en , "Shooters (beverage)"@en , "Shot (drink)"@en , "Shot/shooter"@en , "Shots (alcohol)"@en ;
	skos:broader <http://vocabulary.semantic-web.at/cocktails/54702498-ad42-4af6-b28a-2276215450da> ;
	skos:definition "A shooter is a neologism for an alcoholic mixed drink that contains one ounce (33 ml) of two or more spirits. Some shooters also have a non-alcoholic ingredient. They are generally drunk quickly, rather than being sipped. Shooters can be shaken, stirred, blended, layered, or simply poured. Shot glasses or sherry glasses are the usual drinkware in which shooters are served. They are most commonly served at bars, and some bartenders have their own \"signature\" shooter."@en ;
	skos:exactMatch <http://dbpedia.org/resource/Shooter_(mixed_drink)> ;
	skos:narrower <http://vocabulary.semantic-web.at/cocktails/4efda48d-6c56-47e5-bf98-bf8918ff58eb> , <http://vocabulary.semantic-web.at/cocktails/cd66d6ff-559f-43ea-a754-ac613a87325d> ;
	skos:prefLabel "Shooter"@en .

<http://vocabulary.semantic-web.at/cocktails/b6725284-f65d-4802-b79d-029c539a1580> dcterms:contributor <http://localhost/user/blumauera> ;
	dcterms:created "2015-05-05T07:47:14Z"^^xsd:dateTime ;
	dcterms:creator <http://localhost/user/blumauera> ;
	dcterms:modified "2015-05-06T12:38:07Z"^^xsd:dateTime ;
	<http://schema.semantic-web.at/ppt/inScheme> <http://vocabulary.semantic-web.at/cocktails/591cf89a-57af-49b8-9042-3fc77408c93e> ;
	<http://schema.semantic-web.at/ppt/inSubtree> <http://vocabulary.semantic-web.at/cocktails/403d1249-f37f-4f43-bebf-8dde9677d886> ;
	<http://vocabulary.semantic-web.at/cocktail-ontology/is-part-of> <http://vocabulary.semantic-web.at/cocktails/236b36df-93ca-4408-836c-133ace53798a> , <http://vocabulary.semantic-web.at/cocktails/4f85cadd-4fd4-4ffc-a78d-cddb0763fa4b> ;
	a <http://vocabulary.semantic-web.at/cocktail-ontology/Alcoholic-Beverages> , <http://vocabulary.semantic-web.at/cocktail-ontology/Beverages> , <http://vocabulary.semantic-web.at/cocktail-ontology/Ingredients> , skos:Concept ;
	skos:broader <http://vocabulary.semantic-web.at/cocktails/22df810d-e509-4da8-979c-0758e94de3e6> ;
	skos:prefLabel "Vodka Citron"@en .

<http://vocabulary.semantic-web.at/cocktails/b6ce7a37-ceda-4e8c-86a0-fe7bc5fd0908> dcterms:contributor <http://localhost/user/blumauera> ;
	dcterms:created "2015-05-01T08:28:57Z"^^xsd:dateTime ;
	dcterms:creator <http://localhost/user/blumauera> ;
	dcterms:modified "2015-05-01T08:28:58Z"^^xsd:dateTime ;
	<http://schema.semantic-web.at/ppt/inScheme> <http://vocabulary.semantic-web.at/cocktails/591cf89a-57af-49b8-9042-3fc77408c93e> ;
	<http://schema.semantic-web.at/ppt/inSubtree> <http://vocabulary.semantic-web.at/cocktails/e86c1671-4a67-494b-ae5d-bcb750865acc> ;
	a <http://vocabulary.semantic-web.at/cocktail-ontology/Beverages> , <http://vocabulary.semantic-web.at/cocktail-ontology/Ingredients> , <http://vocabulary.semantic-web.at/cocktail-ontology/Non-alcoholic-Beverages> , skos:Concept ;
	skos:altLabel "Dairy Products"@en , "Dairy food"@en , "Dairy foods"@en , "Dairy produce"@en , "Dairy products"@en , "Diary products"@en , "Milk products"@en ;
	skos:broader <http://vocabulary.semantic-web.at/cocktails/e86c1671-4a67-494b-ae5d-bcb750865acc> ;
	skos:definition "Dairy products are generally defined as food produced from the milk of mammals (the Food Standards Agency of the United Kingdom defines dairy as \"foodstuffs made from mammalian milk\"). They are usually high energy-yielding food products. A production plant for the processing of milk is called a dairy or a dairy factory."@en ;
	skos:exactMatch dbpedia:Dairy_product ;
	skos:narrower <http://vocabulary.semantic-web.at/cocktails/038615ab-5b6e-4293-a8ca-53cf0fb92340> , <http://vocabulary.semantic-web.at/cocktails/498283e1-6a11-43f0-b6ae-d04aea796285> ;
	skos:prefLabel "Dairy product"@en .

<http://vocabulary.semantic-web.at/cocktails/b8075344-1e6d-4348-bdee-83948203a974> dcterms:contributor <http://localhost/user/blumauera> ;
	dcterms:created "2015-05-02T18:51:57Z"^^xsd:dateTime ;
	dcterms:creator <http://localhost/user/blumauera> ;
	dcterms:modified "2015-05-07T07:08:14Z"^^xsd:dateTime ;
	<http://schema.semantic-web.at/ppt/inScheme> <http://vocabulary.semantic-web.at/cocktails/8d052dfc-44bf-4985-8ce3-4564570a161b> ;
	<http://vocabulary.semantic-web.at/cocktail-ontology/consists-of> <http://vocabulary.semantic-web.at/cocktails/074c3acb-bc4d-4c6e-ad8a-e553d5ec7eff> , <http://vocabulary.semantic-web.at/cocktails/3bc44d8c-4e94-4f84-9354-8770018e8a8d> , <http://vocabulary.semantic-web.at/cocktails/c532e86c-01cc-40d4-b2d6-1f959e72d9da> ;
	<http://vocabulary.semantic-web.at/cocktail-ontology/iba> <http://www.iba-world.com/index.php?option=com_content&id=233&Itemid=532> ;
	<http://vocabulary.semantic-web.at/cocktail-ontology/image> <http://upload.wikimedia.org/wikipedia/commons/thumb/b/b8/Rose_%28cocktail%29.jpg/440px-Rose_%28cocktail%29.jpg> ;
	<http://vocabulary.semantic-web.at/cocktail-ontology/preparation> "Shake together in a cocktail shaker, then strain into chilled glass. Garnish and serve."@en ;
	<http://vocabulary.semantic-web.at/cocktail-ontology/served> "Straight up; without ice"@en ;
	<http://vocabulary.semantic-web.at/cocktail-ontology/uses> <http://vocabulary.semantic-web.at/cocktails/19dee0d8-fd30-469f-9ecd-91c902ff717c> ;
	<http://vocabulary.semantic-web.at/cocktail-ontology/uses_2> <http://vocabulary.semantic-web.at/cocktails/8a5e1790-d3c0-432e-bb85-709692b14f03> ;
	a <http://vocabulary.semantic-web.at/cocktail-ontology/Cocktail> , skos:Concept ;
	skos:broader <http://vocabulary.semantic-web.at/cocktails/204cd4e7-58d7-4417-837a-7f9cc41663c8> , <http://vocabulary.semantic-web.at/cocktails/b9bf3799-a4e4-47f7-9aea-7697cc998a34> ;
	skos:definition "Rose is a cocktail made of vermouth and cherry eau de vie."@en ;
	skos:exactMatch <http://dbpedia.org/resource/Rose_(cocktail)> ;
	skos:prefLabel "Rose"@en .

<http://vocabulary.semantic-web.at/cocktails/b970d408-39ca-49b0-98fc-838f96c94608> dcterms:contributor <http://localhost/user/blumauera> ;
	dcterms:created "2015-05-02T19:51:12Z"^^xsd:dateTime ;
	dcterms:creator <http://localhost/user/blumauera> ;
	dcterms:modified "2015-05-05T13:11:05Z"^^xsd:dateTime ;
	<http://schema.semantic-web.at/ppt/inScheme> <http://vocabulary.semantic-web.at/cocktails/8d052dfc-44bf-4985-8ce3-4564570a161b> ;
	<http://vocabulary.semantic-web.at/cocktail-ontology/consists-of> <http://vocabulary.semantic-web.at/cocktails/4be1257b-f797-4ab9-a2b3-af09b958173e> , <http://vocabulary.semantic-web.at/cocktails/88f5de3d-3de4-4a2f-9523-50bc7bb06600> , <http://vocabulary.semantic-web.at/cocktails/d530df52-cc54-4be3-8409-85734e5ec67f> , <http://vocabulary.semantic-web.at/cocktails/f5cd2a2b-2153-4b7e-ae79-678b939765ca> ;
	<http://vocabulary.semantic-web.at/cocktail-ontology/iba> <http://www.iba-world.com/index.php?option=com_content&id=252&Itemid=532> ;
	<http://vocabulary.semantic-web.at/cocktail-ontology/image> <http://www.iba-world.com/images/cocktail_drinks/yellow_bird.jpg> ;
	<http://vocabulary.semantic-web.at/cocktail-ontology/preparation> "Shake and strain into a chilled cocktail glass"@en ;
	<http://vocabulary.semantic-web.at/cocktail-ontology/uses> <http://vocabulary.semantic-web.at/cocktails/19dee0d8-fd30-469f-9ecd-91c902ff717c> ;
	<http://vocabulary.semantic-web.at/cocktail-ontology/uses_2> <http://vocabulary.semantic-web.at/cocktails/8a5e1790-d3c0-432e-bb85-709692b14f03> ;
	a <http://vocabulary.semantic-web.at/cocktail-ontology/Cocktail> , skos:Concept ;
	skos:broader <http://vocabulary.semantic-web.at/cocktails/ccee1079-43df-4ff1-bef0-d15d3dc8fa6f> ;
	skos:prefLabel "Yellow Bird"@en .

<http://vocabulary.semantic-web.at/cocktails/b9bf3799-a4e4-47f7-9aea-7697cc998a34> dcterms:contributor <http://localhost/user/blumauera> ;
	dcterms:created "2015-05-01T07:35:30Z"^^xsd:dateTime ;
	dcterms:creator <http://localhost/user/blumauera> ;
	dcterms:modified "2016-08-26T07:17:38Z"^^xsd:dateTime ;
	<http://schema.semantic-web.at/ppt/inScheme> <http://vocabulary.semantic-web.at/cocktails/8d052dfc-44bf-4985-8ce3-4564570a161b> ;
	a <http://vocabulary.semantic-web.at/cocktail-ontology/Cocktail> , skos:Concept ;
	skos:broader <http://vocabulary.semantic-web.at/cocktails/5ac37bec-e4b9-4d43-9bcc-8d6954903c25> ;
	skos:narrower <http://vocabulary.semantic-web.at/cocktails/0f8cc862-9056-49be-b636-cd22f8d7282d> , <http://vocabulary.semantic-web.at/cocktails/117bd4d2-6da3-4d69-8c79-bc1d873b5010> , <http://vocabulary.semantic-web.at/cocktails/12f4790a-560f-4e1c-b57a-53b8171ae39a> , <http://vocabulary.semantic-web.at/cocktails/13b85b5c-7f69-4871-bb08-3cd5281f6039> , <http://vocabulary.semantic-web.at/cocktails/1529fd23-9c55-45d7-b8c6-b0fc229a3871> , <http://vocabulary.semantic-web.at/cocktails/268fb62f-8ef1-45cd-844f-8c7da85a6a0b> , <http://vocabulary.semantic-web.at/cocktails/2c032fe6-a518-44be-851a-dbf1c253be63> , <http://vocabulary.semantic-web.at/cocktails/2d85fb1b-96cb-4c48-8df5-707032f34e71> , <http://vocabulary.semantic-web.at/cocktails/33d9a47f-0622-4b0f-ad1b-62eb96fc6799> , <http://vocabulary.semantic-web.at/cocktails/43111fc3-3b59-420c-a588-024cd2d33896> , <http://vocabulary.semantic-web.at/cocktails/45788a96-1fde-486b-80fc-31ad243bba31> , <http://vocabulary.semantic-web.at/cocktails/4792b0b8-0046-47ca-8c2a-f3ad58922182> , <http://vocabulary.semantic-web.at/cocktails/4f85cadd-4fd4-4ffc-a78d-cddb0763fa4b> , <http://vocabulary.semantic-web.at/cocktails/52117ab2-dcb8-4d28-a366-ddd932e58219> , <http://vocabulary.semantic-web.at/cocktails/55c40695-8b41-41ed-8c6a-70fe6930067e> , <http://vocabulary.semantic-web.at/cocktails/61a18ebf-fd92-4ef1-8ab1-bfd3c26867b9> , <http://vocabulary.semantic-web.at/cocktails/698723d7-e8b8-410e-91a8-9bdc867b3f8a> , <http://vocabulary.semantic-web.at/cocktails/926b14fe-1b83-4f46-bbf9-f946be1889aa> , <http://vocabulary.semantic-web.at/cocktails/a73d88e9-0c50-45d2-b364-9dec5abe206d> , <http://vocabulary.semantic-web.at/cocktails/b8075344-1e6d-4348-bdee-83948203a974> , <http://vocabulary.semantic-web.at/cocktails/bca7bc6d-6709-48b8-ae52-fe194c212398> , <http://vocabulary.semantic-web.at/cocktails/bee1e709-b317-4f46-b06f-a22367baefdf> , <http://vocabulary.semantic-web.at/cocktails/c2249dc0-0529-4a11-ad82-5d710b5e9c31> , <http://vocabulary.semantic-web.at/cocktails/c3b197cc-8583-4e2f-8e45-3a7fed1309c1> , <http://vocabulary.semantic-web.at/cocktails/c8f4f6bd-4ac1-456a-a3aa-595e4b93d979> , <http://vocabulary.semantic-web.at/cocktails/ce8f4591-ccd4-4d90-a761-244115d64061> , <http://vocabulary.semantic-web.at/cocktails/dff0a7f4-ded0-48d5-bd31-881b70fbe36a> , <http://vocabulary.semantic-web.at/cocktails/ea946e07-e812-4492-a0ed-124d73bfbba7> , <http://vocabulary.semantic-web.at/cocktails/eddf4894-1683-44e9-9ee3-7920d3729d71> , <http://vocabulary.semantic-web.at/cocktails/f01f6a10-01a5-4810-860f-d3a52fd36b1b> ;
	skos:prefLabel "Contemporary Classics"@en .

<http://vocabulary.semantic-web.at/cocktails/bab016bd-2fd5-4809-bfe7-3225d25f116d> dcterms:contributor <http://localhost/user/blumauera> ;
	dcterms:created "2015-05-01T14:27:12Z"^^xsd:dateTime ;
	dcterms:creator <http://localhost/user/blumauera> ;
	dcterms:modified "2016-04-04T09:13:39Z"^^xsd:dateTime ;
	<http://schema.semantic-web.at/ppt/inScheme> <http://vocabulary.semantic-web.at/cocktails/8d052dfc-44bf-4985-8ce3-4564570a161b> ;
	<http://vocabulary.semantic-web.at/cocktail-ontology/consists-of> <http://vocabulary.semantic-web.at/cocktails/71210bd1-3071-4533-8da4-fe0f7d7694a0> , <http://vocabulary.semantic-web.at/cocktails/88f5de3d-3de4-4a2f-9523-50bc7bb06600> , <http://vocabulary.semantic-web.at/cocktails/f5cd2a2b-2153-4b7e-ae79-678b939765ca> ;
	<http://vocabulary.semantic-web.at/cocktail-ontology/iba> <http://www.iba-world.com/index.php?option=com_content&id=193&Itemid=532> ;
	<http://vocabulary.semantic-web.at/cocktail-ontology/image> <http://upload.wikimedia.org/wikipedia/commons/thumb/7/7a/Daiquiri_drink.jpg/440px-Daiquiri_drink.jpg> ;
	<http://vocabulary.semantic-web.at/cocktail-ontology/preparation> "Pour all ingredients into shaker with ice cubes. Shake well. Strain in chilled cocktail glass."@en ;
	<http://vocabulary.semantic-web.at/cocktail-ontology/served> "Straight up; without ice"@en ;
	<http://vocabulary.semantic-web.at/cocktail-ontology/uses> <http://vocabulary.semantic-web.at/cocktails/19dee0d8-fd30-469f-9ecd-91c902ff717c> ;
	<http://vocabulary.semantic-web.at/cocktail-ontology/uses_2> <http://vocabulary.semantic-web.at/cocktails/021c85c0-a60a-4414-8fd8-bd3383b794f1> ;
	a <http://vocabulary.semantic-web.at/cocktail-ontology/Cocktail> , skos:Concept ;
	skos:altLabel "Banana daikiri"@en , "Banana daiquiri"@en , "Daikiri"@en , "Daiquiri (cocktail)"@en , "Daiquiris"@en , "Daquari"@en , "Daquiri"@en , "Strawberry daiquiri"@en ;
	skos:broader <http://vocabulary.semantic-web.at/cocktails/7516b400-963a-4151-8fdc-f6b23bad1dd5> , <http://vocabulary.semantic-web.at/cocktails/caae2ea0-7e60-400b-a2bb-14ef79720668> ;
	skos:definition "Daiquiri is a family of cocktails whose main ingredients are rum, citrus, and sugar or other sweetener. The Daiquirí is one of six basic drinks listed in David A. Embury's classic The Fine Art of Mixing Drinks. In the book, he also suggests some variations."@en ;
	skos:exactMatch dbpedia:Daiquiri ;
	skos:prefLabel "Daiquiri"@en ;
	skos:related <http://vocabulary.semantic-web.at/cocktails/60d3a991-48d3-4e73-9d62-5961893fd311> , <http://vocabulary.semantic-web.at/cocktails/bca7bc6d-6709-48b8-ae52-fe194c212398> , <http://vocabulary.semantic-web.at/cocktails/bee1e709-b317-4f46-b06f-a22367baefdf> .

<http://vocabulary.semantic-web.at/cocktails/bca7bc6d-6709-48b8-ae52-fe194c212398> dcterms:contributor <http://localhost/user/huberf> ;
	dcterms:created "2015-05-03T17:26:44Z"^^xsd:dateTime ;
	dcterms:creator <http://localhost/user/blumauera> ;
	dcterms:modified "2016-10-05T09:33:22Z"^^xsd:dateTime ;
	<http://schema.semantic-web.at/ppt/inScheme> <http://vocabulary.semantic-web.at/cocktails/8d052dfc-44bf-4985-8ce3-4564570a161b> ;
	<http://vocabulary.semantic-web.at/cocktail-ontology/consists-of> <http://vocabulary.semantic-web.at/cocktails/021c85c0-a60a-4414-8fd8-bd3383b794f1> , <http://vocabulary.semantic-web.at/cocktails/92e8ded1-1223-4a3f-b2d4-7ee731d6dbc7> , <http://vocabulary.semantic-web.at/cocktails/e67b1621-7be7-471d-ac8d-a368d8c68115> ;
	<http://vocabulary.semantic-web.at/cocktail-ontology/iba> <http://www.iba-world.com/index.php?option=com_content&id=260&Itemid=532> ;
	<http://vocabulary.semantic-web.at/cocktail-ontology/image> <http://upload.wikimedia.org/wikipedia/commons/thumb/0/0c/Caipirinha2.jpg/440px-Caipirinha2.jpg> ;
	<http://vocabulary.semantic-web.at/cocktail-ontology/preparation> "Place lime and sugar into old fashioned glass and muddle (mash the two ingredients together using a muddler or a wooden spoon). Fill the glass with crushed ice and add the Cachaça."@en ;
	<http://vocabulary.semantic-web.at/cocktail-ontology/served> "On the rocks; poured over ice"@en ;
	<http://vocabulary.semantic-web.at/cocktail-ontology/uses> <http://vocabulary.semantic-web.at/cocktails/2dce3576-2603-41f9-8dce-ab21f639c2a7> ;
	<http://vocabulary.semantic-web.at/cocktail-ontology/uses_2> <http://vocabulary.semantic-web.at/cocktails/3c94f5fc-4664-4177-a880-88643c0be9c1> , <http://vocabulary.semantic-web.at/cocktails/9d9fb486-a0dd-4d1a-b65e-7346a626cadf> ;
	a <http://vocabulary.semantic-web.at/cocktail-ontology/Cocktail> , skos:Concept ;
	skos:altLabel "Caipi"@en , "Capirina"@en , "Capirinha"@en ;
	skos:broader <http://vocabulary.semantic-web.at/cocktails/7516b400-963a-4151-8fdc-f6b23bad1dd5> , <http://vocabulary.semantic-web.at/cocktails/b9bf3799-a4e4-47f7-9aea-7697cc998a34> ;
	skos:definition "Caipirinha is Brazil's national cocktail, made with cachaça (sugar cane hard liquor), sugar and lime. Cachaça is Brazil's most common distilled alcoholic beverage (also known as Pinga or Caninha). Both rum and cachaça are made from sugarcane-derived products. Specifically with cachaça, the alcohol results from the fermentation of sugarcane juice that is afterwards distilled."@en ;
	skos:exactMatch dbpedia:Caipirinha ;
	skos:prefLabel "Caipirinha"@en ;
	skos:related <http://vocabulary.semantic-web.at/cocktails/bab016bd-2fd5-4809-bfe7-3225d25f116d> , <http://vocabulary.semantic-web.at/cocktails/bee1e709-b317-4f46-b06f-a22367baefdf> .

<http://vocabulary.semantic-web.at/cocktails/be3653af-d585-43f7-b8ce-ad75b1bd7aad> dcterms:contributor <http://localhost/user/blumauera> ;
	dcterms:created "2015-05-01T15:07:00Z"^^xsd:dateTime ;
	dcterms:creator <http://localhost/user/blumauera> ;
	dcterms:modified "2015-05-04T11:35:30Z"^^xsd:dateTime ;
	<http://schema.semantic-web.at/ppt/inScheme> <http://vocabulary.semantic-web.at/cocktails/8d052dfc-44bf-4985-8ce3-4564570a161b> ;
	<http://vocabulary.semantic-web.at/cocktail-ontology/consists-of> <http://vocabulary.semantic-web.at/cocktails/c5c70695-d939-4f4d-8ae7-394f2f66ccbb> , <http://vocabulary.semantic-web.at/cocktails/f0bfda32-3c42-457f-b6a3-bbf2a9e77b06> ;
	<http://vocabulary.semantic-web.at/cocktail-ontology/iba> <http://www.iba-world.com/index.php?option=com_content&id=207&Itemid=532> ;
	<http://vocabulary.semantic-web.at/cocktail-ontology/image> <http://www.iba-world.com/images/cocktail_drinks/rusty_nail.jpg> ;
	<http://vocabulary.semantic-web.at/cocktail-ontology/preparation> "Pour all ingredients directly into old-fashioned glass filled with ice. Stir gently. Garnish with a lemon twist. Serve."@en ;
	<http://vocabulary.semantic-web.at/cocktail-ontology/served> "On the rocks; poured over ice"@en ;
	<http://vocabulary.semantic-web.at/cocktail-ontology/uses> <http://vocabulary.semantic-web.at/cocktails/2dce3576-2603-41f9-8dce-ab21f639c2a7> ;
	<http://vocabulary.semantic-web.at/cocktail-ontology/uses_2> <http://vocabulary.semantic-web.at/cocktails/33df103a-03ac-4177-b620-7953fe094236> ;
	a <http://vocabulary.semantic-web.at/cocktail-ontology/Cocktail> , skos:Concept ;
	skos:broader <http://vocabulary.semantic-web.at/cocktails/caae2ea0-7e60-400b-a2bb-14ef79720668> ;
	skos:definition "A Rusty Nail is made by mixing Drambuie and Scotch whisky. Many prefer less Drambuie to decrease the sweetness of the drink. Scotch whisky has a fairly biting and hot taste that is counterbalanced by the honeyed, herbal overtones of the Drambuie. A Rusty Nail can be served in an old-fashioned glass on the rocks, neat, or \"up\" in a stemmed glass. It is most commonly served over ice. A Rusty Nail served without ice is sometimes called a Straight Up Nail."@en ;
	skos:exactMatch <http://dbpedia.org/resource/Rusty_Nail_(cocktail)> ;
	skos:prefLabel "Rusty Nail"@en .

<http://vocabulary.semantic-web.at/cocktails/bed073f2-de84-4322-a490-4f34ec54c6d1> dcterms:contributor <http://localhost/user/blumauera> ;
	dcterms:created "2015-05-02T19:18:05Z"^^xsd:dateTime ;
	dcterms:creator <http://localhost/user/blumauera> ;
	dcterms:modified "2015-05-05T07:11:49Z"^^xsd:dateTime ;
	<http://schema.semantic-web.at/ppt/inScheme> <http://vocabulary.semantic-web.at/cocktails/8d052dfc-44bf-4985-8ce3-4564570a161b> ;
	<http://vocabulary.semantic-web.at/cocktail-ontology/consists-of> <http://vocabulary.semantic-web.at/cocktails/59ccd2fc-1807-45eb-8621-8d3e898e6d37> , <http://vocabulary.semantic-web.at/cocktails/5b4cd5f6-19e8-4854-8c5e-0b6d58cbb702> ;
	<http://vocabulary.semantic-web.at/cocktail-ontology/iba> <http://www.iba-world.com/index.php?option=com_content&id=240&Itemid=532> ;
	<http://vocabulary.semantic-web.at/cocktail-ontology/image> <http://upload.wikimedia.org/wikipedia/commons/thumb/0/00/Dark_n_Stormy.jpg/440px-Dark_n_Stormy.jpg> ;
	<http://vocabulary.semantic-web.at/cocktail-ontology/preparation> "In a highball glass filled with ice add 6cl dark rum and top with ginger beer. Garnish with lime wedge."@en ;
	<http://vocabulary.semantic-web.at/cocktail-ontology/served> "On the rocks; poured over ice"@en ;
	<http://vocabulary.semantic-web.at/cocktail-ontology/uses> <http://vocabulary.semantic-web.at/cocktails/a54d2096-6214-4006-beaf-afcc77824710> ;
	<http://vocabulary.semantic-web.at/cocktail-ontology/uses_2> <http://vocabulary.semantic-web.at/cocktails/021c85c0-a60a-4414-8fd8-bd3383b794f1> ;
	a <http://vocabulary.semantic-web.at/cocktail-ontology/Cocktail> , skos:Concept ;
	skos:broader <http://vocabulary.semantic-web.at/cocktails/ccee1079-43df-4ff1-bef0-d15d3dc8fa6f> ;
	skos:definition "A Dark 'N Stormy is a highball cocktail made with Gosling's Black rum (the dark) and ginger beer (the stormy) served over ice and garnished with a slice of lime."@en ;
	skos:exactMatch <http://dbpedia.org/resource/Dark_'N'_Stormy> ;
	skos:prefLabel "Dark 'N' Stormy"@en .

<http://vocabulary.semantic-web.at/cocktails/bee1e709-b317-4f46-b06f-a22367baefdf> dcterms:contributor <http://localhost/user/blumauera> ;
	dcterms:created "2015-05-02T18:37:14Z"^^xsd:dateTime ;
	dcterms:creator <http://localhost/user/blumauera> ;
	dcterms:modified "2015-05-07T06:59:47Z"^^xsd:dateTime ;
	<http://schema.semantic-web.at/ppt/inScheme> <http://vocabulary.semantic-web.at/cocktails/8d052dfc-44bf-4985-8ce3-4564570a161b> ;
	<http://vocabulary.semantic-web.at/cocktail-ontology/consists-of> <http://vocabulary.semantic-web.at/cocktails/3c94f5fc-4664-4177-a880-88643c0be9c1> , <http://vocabulary.semantic-web.at/cocktails/7448dbed-7603-41f7-a316-99f754c9ae45> , <http://vocabulary.semantic-web.at/cocktails/88f5de3d-3de4-4a2f-9523-50bc7bb06600> , <http://vocabulary.semantic-web.at/cocktails/91b112c0-2fcc-4495-b68c-b1f09fa0a698> , <http://vocabulary.semantic-web.at/cocktails/f5cd2a2b-2153-4b7e-ae79-678b939765ca> ;
	<http://vocabulary.semantic-web.at/cocktail-ontology/iba> <http://www.iba-world.com/index.php?option=com_content&id=229&Itemid=532> ;
	<http://vocabulary.semantic-web.at/cocktail-ontology/image> <http://upload.wikimedia.org/wikipedia/commons/f/f2/Mojito.jpg> ;
	<http://vocabulary.semantic-web.at/cocktail-ontology/preparation> "Muddle mint springs with sugar and lime juice. Add splash of soda water and fill glass with cracked ice. Pour rum and top with soda water. Garnish with spring of mint leaves and lemon slice. Serve with straw."@en ;
	<http://vocabulary.semantic-web.at/cocktail-ontology/served> "On the rocks; poured over ice"@en ;
	<http://vocabulary.semantic-web.at/cocktail-ontology/uses> <http://vocabulary.semantic-web.at/cocktails/20d288cb-4e38-46f9-9bec-1c79d8397215> ;
	<http://vocabulary.semantic-web.at/cocktail-ontology/uses_2> <http://vocabulary.semantic-web.at/cocktails/33df103a-03ac-4177-b620-7953fe094236> , <http://vocabulary.semantic-web.at/cocktails/91b112c0-2fcc-4495-b68c-b1f09fa0a698> ;
	a <http://vocabulary.semantic-web.at/cocktail-ontology/Cocktail> , skos:Concept ;
	skos:altLabel "Mohito"@en , "Mojito Royal"@en , "Mojitos"@en , "Nojito"@en , "Virgin Mojito"@en ;
	skos:broader <http://vocabulary.semantic-web.at/cocktails/b9bf3799-a4e4-47f7-9aea-7697cc998a34> ;
	skos:definition "Mojito is a traditional Cuban highball. Traditionally, a mojito is a cocktail that consists of five ingredients: white rum, sugar, lime juice, sparkling water and mint. The original Cuban recipe uses spearmint or yerba buena, a mint variety very popular on the island. Its combination of sweetness, refreshing citrus and mint flavors is intended to complement the potent kick of the rum, and have made this clear highball a popular summer drink."@en ;
	skos:exactMatch dbpedia:Mojito ;
	skos:prefLabel "Mojito"@en ;
	skos:related <http://vocabulary.semantic-web.at/cocktails/bab016bd-2fd5-4809-bfe7-3225d25f116d> , <http://vocabulary.semantic-web.at/cocktails/bca7bc6d-6709-48b8-ae52-fe194c212398> .

<http://vocabulary.semantic-web.at/cocktails/bfbfb9b6-4c70-4323-a64b-4cfd533c55d8> dcterms:contributor <http://localhost/user/blumauera> ;
	dcterms:created "2015-05-02T19:15:51Z"^^xsd:dateTime ;
	dcterms:creator <http://localhost/user/blumauera> ;
	dcterms:modified "2015-11-18T14:37:17Z"^^xsd:dateTime ;
	<http://schema.semantic-web.at/ppt/inScheme> <http://vocabulary.semantic-web.at/cocktails/f09732a9-a0e6-494a-8ce9-299ef036aaaf> ;
	<http://vocabulary.semantic-web.at/cocktail-ontology/image_2> <http://upload.wikimedia.org/wikipedia/commons/thumb/4/40/Shot_glass.svg/32px-Shot_glass.svg.png> ;
	<http://vocabulary.semantic-web.at/cocktail-ontology/is-used-by> <http://vocabulary.semantic-web.at/cocktails/4efda48d-6c56-47e5-bf98-bf8918ff58eb> , <http://vocabulary.semantic-web.at/cocktails/cd66d6ff-559f-43ea-a754-ac613a87325d> ;
	a <http://vocabulary.semantic-web.at/cocktail-ontology/Drinkware> , skos:Concept ;
	skos:altLabel "Double jigger"@en , "Jigger (bartending)"@en , "Jigger (unit)"@en , "Measure (bartending)"@en , "Shooter glass"@en , "Shot (alcohol)"@en , "Shot (unit)"@en , "Shot glasses"@en , "Shotglass"@en ;
	skos:broader <http://vocabulary.semantic-web.at/cocktails/2e839563-8037-4e59-8dbf-27736605d687> ;
	skos:definition "A shot glass is a small glass designed to hold or measure spirits or liquor, which is either drunk straight from the glass (\"a shot\") or poured into a cocktail. A \"shot\" of liquor is not the same as a \"shooter. \" Shot glasses decorated with a wide variety of toasts, advertisements and humorous pictures are popular souvenirs and collectibles."@en ;
	skos:exactMatch dbpedia:Shot_glass ;
	skos:prefLabel "Shot glass"@en .

<http://vocabulary.semantic-web.at/cocktails/c151ee28-45d2-4128-8587-1f1b69060d9d> dcterms:contributor <http://localhost/user/blumauera> ;
	dcterms:created "2015-05-01T15:06:16Z"^^xsd:dateTime ;
	dcterms:creator <http://localhost/user/blumauera> ;
	dcterms:modified "2015-05-04T11:31:48Z"^^xsd:dateTime ;
	<http://schema.semantic-web.at/ppt/inScheme> <http://vocabulary.semantic-web.at/cocktails/8d052dfc-44bf-4985-8ce3-4564570a161b> ;
	<http://vocabulary.semantic-web.at/cocktail-ontology/consists-of> <http://vocabulary.semantic-web.at/cocktails/038615ab-5b6e-4293-a8ca-53cf0fb92340> , <http://vocabulary.semantic-web.at/cocktails/47c10a33-a7b2-44f5-9614-2bca65cff2fd> , <http://vocabulary.semantic-web.at/cocktails/5d96c50c-ee48-4c40-bb4c-4b9a42d11de6> , <http://vocabulary.semantic-web.at/cocktails/71210bd1-3071-4533-8da4-fe0f7d7694a0> , <http://vocabulary.semantic-web.at/cocktails/7448dbed-7603-41f7-a316-99f754c9ae45> , <http://vocabulary.semantic-web.at/cocktails/88f5de3d-3de4-4a2f-9523-50bc7bb06600> , <http://vocabulary.semantic-web.at/cocktails/98f20476-57d7-46d3-b76d-6aac18b57788> , <http://vocabulary.semantic-web.at/cocktails/9c2ce399-c6ae-4f4d-bf37-7fd8ffe2a19d> , <http://vocabulary.semantic-web.at/cocktails/cc32e2f5-d1ae-4506-b000-86fbfee4a3e7> ;
	<http://vocabulary.semantic-web.at/cocktail-ontology/iba> <http://www.iba-world.com/index.php?option=com_content&id=206&Itemid=532> ;
	<http://vocabulary.semantic-web.at/cocktail-ontology/image> <http://upload.wikimedia.org/wikipedia/commons/thumb/8/80/RamosGinFizzRooseveltNOLAJuly2009.JPG/440px-RamosGinFizzRooseveltNOLAJuly2009.JPG> ;
	<http://vocabulary.semantic-web.at/cocktail-ontology/is-variant-of> <http://vocabulary.semantic-web.at/cocktails/53a05366-d473-4eb4-ac66-0d0119e0b759> ;
	<http://vocabulary.semantic-web.at/cocktail-ontology/preparation> "Pour all ingredients (except soda) in a mixing glass, dry shake (no ice) for two minutes, add ice and hard shake for another minute. Strain into a highball glass without ice, top with soda."@en ;
	<http://vocabulary.semantic-web.at/cocktail-ontology/served> "Straight up; without ice"@en ;
	<http://vocabulary.semantic-web.at/cocktail-ontology/uses> <http://vocabulary.semantic-web.at/cocktails/20d288cb-4e38-46f9-9bec-1c79d8397215> , <http://vocabulary.semantic-web.at/cocktails/a54d2096-6214-4006-beaf-afcc77824710> ;
	<http://vocabulary.semantic-web.at/cocktail-ontology/uses_2> <http://vocabulary.semantic-web.at/cocktails/99171f20-c59f-40c4-998a-a9c8f1909168> ;
	a <http://vocabulary.semantic-web.at/cocktail-ontology/Cocktail> , skos:Concept ;
	skos:broader <http://vocabulary.semantic-web.at/cocktails/7516b400-963a-4151-8fdc-f6b23bad1dd5> , <http://vocabulary.semantic-web.at/cocktails/caae2ea0-7e60-400b-a2bb-14ef79720668> ;
	skos:definition "A Ramos gin fizz (also known as a Ramos fizz or New Orleans fizz) contains gin, lemon juice, lime juice, egg white, sugar, cream, orange flower water, and soda water. It is served in a large non-tapered 12 to 14 ounce Collins glass. The orange flower water and egg significantly affect the flavor and texture of a Ramos, compared to a regular Gin Fizz. "@en ;
	skos:prefLabel "Ramos Gin Fizz"@en .

<http://vocabulary.semantic-web.at/cocktails/c2249dc0-0529-4a11-ad82-5d710b5e9c31> dcterms:contributor <http://localhost/user/superadmin> ;
	dcterms:created "2015-05-02T18:29:29Z"^^xsd:dateTime ;
	dcterms:creator <http://localhost/user/blumauera> ;
	dcterms:modified "2016-08-26T12:43:05Z"^^xsd:dateTime ;
	<http://schema.semantic-web.at/ppt/inScheme> <http://vocabulary.semantic-web.at/cocktails/8d052dfc-44bf-4985-8ce3-4564570a161b> ;
	<http://vocabulary.semantic-web.at/cocktail-ontology/consists-of> <http://vocabulary.semantic-web.at/cocktails/2ce50273-13b2-4ba1-9ff2-8cfbd835c1f2> , <http://vocabulary.semantic-web.at/cocktails/cdbac85a-d5b7-40f3-9e98-4d7e176b5565> ;
	<http://vocabulary.semantic-web.at/cocktail-ontology/iba> <http://www.iba-world.com/index.php?option=com_content&id=228&Itemid=532> ;
	<http://vocabulary.semantic-web.at/cocktail-ontology/image> <http://upload.wikimedia.org/wikipedia/commons/thumb/3/3a/Pool-side_Mimosas_at_The_Standard_Hotel.jpg/440px-Pool-side_Mimosas_at_The_Standard_Hotel.jpg> ;
	<http://vocabulary.semantic-web.at/cocktail-ontology/preparation> "Ensure both ingredients are well chilled, then mix into the glass. Serve cold."@en ;
	<http://vocabulary.semantic-web.at/cocktail-ontology/served> "stirred not shaken"@en ;
	<http://vocabulary.semantic-web.at/cocktail-ontology/uses> <http://vocabulary.semantic-web.at/cocktails/fece03b5-ec0b-4e47-964d-cc5dc09fd7fb> ;
	<http://vocabulary.semantic-web.at/cocktail-ontology/uses_2> <http://vocabulary.semantic-web.at/cocktails/99171f20-c59f-40c4-998a-a9c8f1909168> ;
	a <http://vocabulary.semantic-web.at/cocktail-ontology/Cocktail> , skos:Concept ;
	skos:altLabel "Buck's Fizz"@en , "Hibiscus (cocktail)"@en , "Lilosa"@en ;
	skos:broader <http://vocabulary.semantic-web.at/cocktails/204cd4e7-58d7-4417-837a-7f9cc41663c8> , <http://vocabulary.semantic-web.at/cocktails/b9bf3799-a4e4-47f7-9aea-7697cc998a34> ;
	skos:definition "A Mimosa is a cocktail-like drink composed of one part champagne and one part thoroughly chilled citrus fruit juice, usually orange juice unless otherwise specified (e.g. , \"grapefruit mimosa\"). It is traditionally served in a tall champagne flute with a morning brunch as hair of the dog or to guests at weddings. It is probably named after the yellow flowers of Acacia dealbata. A Buck's Fizz is a similar cocktail, but with twice as much orange juice as champagne."@en ;
	skos:exactMatch <http://dbpedia.org/resource/Mimosa_(cocktail)> ;
	skos:prefLabel "Mimosa"@en .

<http://vocabulary.semantic-web.at/cocktails/c3a50c60-ccb3-4ab4-8f9f-722acdae8d50> dcterms:contributor <http://localhost/user/blumauera> ;
	dcterms:created "2015-05-03T10:28:02Z"^^xsd:dateTime ;
	dcterms:creator <http://localhost/user/blumauera> ;
	dcterms:modified "2015-05-03T10:29:24Z"^^xsd:dateTime ;
	<http://schema.semantic-web.at/ppt/inScheme> <http://vocabulary.semantic-web.at/cocktails/591cf89a-57af-49b8-9042-3fc77408c93e> ;
	<http://schema.semantic-web.at/ppt/inSubtree> <http://vocabulary.semantic-web.at/cocktails/403d1249-f37f-4f43-bebf-8dde9677d886> ;
	<http://vocabulary.semantic-web.at/cocktail-ontology/is-part-of> <http://vocabulary.semantic-web.at/cocktails/60d3a991-48d3-4e73-9d62-5961893fd311> ;
	a <http://vocabulary.semantic-web.at/cocktail-ontology/Alcoholic-Beverages> , <http://vocabulary.semantic-web.at/cocktail-ontology/Beverages> , <http://vocabulary.semantic-web.at/cocktail-ontology/Ingredients> , skos:Concept ;
	skos:broader <http://vocabulary.semantic-web.at/cocktails/f5cd2a2b-2153-4b7e-ae79-678b939765ca> ;
	skos:definition "Bacardi Superior is rum made by the Bacardi Company. In the US it is 80 proof, containing 40% abv (37.5% abv in the UK and Continental Europe). It is colourless and easy flowing and is thin in the body. This rum is mostly used to make cocktails calling for a white rum such as Cuba Libre, Daiquiri, Piña Colada, and Bacardi cocktail. Energy provided by a glass of Bacardi is around 118 calories."@en ;
	skos:exactMatch dbpedia:Bacardi_Superior ;
	skos:prefLabel "Bacardi Superior"@en .

<http://vocabulary.semantic-web.at/cocktails/c3ae5830-1bfd-4f37-afc9-3e88849d03cf> dcterms:contributor <http://localhost/user/blumauera> ;
	dcterms:created "2015-05-01T14:23:41Z"^^xsd:dateTime ;
	dcterms:creator <http://localhost/user/blumauera> ;
	dcterms:modified "2015-05-03T11:45:59Z"^^xsd:dateTime ;
	<http://schema.semantic-web.at/ppt/inScheme> <http://vocabulary.semantic-web.at/cocktails/8d052dfc-44bf-4985-8ce3-4564570a161b> ;
	<http://vocabulary.semantic-web.at/cocktail-ontology/consists-of> <http://vocabulary.semantic-web.at/cocktails/371797a7-e9a8-453b-8744-2e89f2fd30d2> , <http://vocabulary.semantic-web.at/cocktails/5d96c50c-ee48-4c40-bb4c-4b9a42d11de6> , <http://vocabulary.semantic-web.at/cocktails/98f20476-57d7-46d3-b76d-6aac18b57788> , <http://vocabulary.semantic-web.at/cocktails/9c2ce399-c6ae-4f4d-bf37-7fd8ffe2a19d> ;
	<http://vocabulary.semantic-web.at/cocktail-ontology/iba> <http://www.iba-world.com/index.php?option=com_content&id=192&Itemid=532> ;
	<http://vocabulary.semantic-web.at/cocktail-ontology/image> <http://upload.wikimedia.org/wikipedia/en/thumb/9/99/Cloverclub.jpg/440px-Cloverclub.jpg> ;
	<http://vocabulary.semantic-web.at/cocktail-ontology/preparation> "Dry shake ingredients to emulsify, add ice, shake and served straight up."@en ;
	<http://vocabulary.semantic-web.at/cocktail-ontology/served> "Straight up; without ice"@en ;
	<http://vocabulary.semantic-web.at/cocktail-ontology/uses> <http://vocabulary.semantic-web.at/cocktails/19dee0d8-fd30-469f-9ecd-91c902ff717c> ;
	a <http://vocabulary.semantic-web.at/cocktail-ontology/Cocktail> , skos:Concept ;
	skos:altLabel "Clover Club"@en ;
	skos:broader <http://vocabulary.semantic-web.at/cocktails/caae2ea0-7e60-400b-a2bb-14ef79720668> ;
	skos:definition "The Clover Club Cocktail is a cocktail consisting of Gin, Lemon Juice, Raspberry Syrup, and an Egg white. The Egg white is not added for the purpose of giving the drink flavor, but rather acts as an emulsifier. Thus when the drink is shaken a characteristic foamy head is formed."@en ;
	skos:exactMatch dbpedia:Clover_Club_Cocktail ;
	skos:prefLabel "Clover Club Cocktail"@en .

<http://vocabulary.semantic-web.at/cocktails/c3b197cc-8583-4e2f-8e45-3a7fed1309c1> dcterms:contributor <http://localhost/user/blumauera> ;
	dcterms:created "2015-05-02T17:21:07Z"^^xsd:dateTime ;
	dcterms:creator <http://localhost/user/blumauera> ;
	dcterms:modified "2015-05-07T06:50:14Z"^^xsd:dateTime ;
	<http://schema.semantic-web.at/ppt/inScheme> <http://vocabulary.semantic-web.at/cocktails/8d052dfc-44bf-4985-8ce3-4564570a161b> ;
	<http://vocabulary.semantic-web.at/cocktail-ontology/consists-of> <http://vocabulary.semantic-web.at/cocktails/038615ab-5b6e-4293-a8ca-53cf0fb92340> , <http://vocabulary.semantic-web.at/cocktails/4f4bed20-5317-45f6-a070-f28267b6e961> , <http://vocabulary.semantic-web.at/cocktails/92e8ded1-1223-4a3f-b2d4-7ee731d6dbc7> , <http://vocabulary.semantic-web.at/cocktails/d14f3ba1-9350-49a9-a9df-4d97c61f9d87> ;
	<http://vocabulary.semantic-web.at/cocktail-ontology/iba> <http://www.iba-world.com/index.php?option=com_content&id=224&Itemid=532> ;
	<http://vocabulary.semantic-web.at/cocktail-ontology/image> <http://upload.wikimedia.org/wikipedia/commons/thumb/6/61/Irish_coffee_glass.jpg/440px-Irish_coffee_glass.jpg> ;
	<http://vocabulary.semantic-web.at/cocktail-ontology/preparation> "Heat the coffee, whiskey and sugar; do not boil. Pour into glass and top with cream; serve hot."@en ;
	<http://vocabulary.semantic-web.at/cocktail-ontology/served> "Hot"@en ;
	<http://vocabulary.semantic-web.at/cocktail-ontology/uses> <http://vocabulary.semantic-web.at/cocktails/347f5539-1dae-44fc-9e7b-a2cbe9e2e157> ;
	a <http://vocabulary.semantic-web.at/cocktail-ontology/Cocktail> , skos:Concept ;
	skos:altLabel "Baileys coffee"@en ;
	skos:broader <http://vocabulary.semantic-web.at/cocktails/b9bf3799-a4e4-47f7-9aea-7697cc998a34> ;
	skos:definition "Irish coffee is a cocktail consisting of hot coffee, Irish whiskey, and sugar (some recipes specify that brown sugar should be used), stirred, and topped with thick cream. The coffee is drunk through the cream. The original recipe explicitly uses cream that has not been whipped, although drinks made with whipped cream are often sold as \"Irish coffee\"."@en ;
	skos:exactMatch dbpedia:Irish_coffee ;
	skos:prefLabel "Irish coffee"@en .

<http://vocabulary.semantic-web.at/cocktails/c4339109-ae35-4be9-a7e8-b5dfd206e960> dcterms:contributor <http://localhost/user/blumauera> ;
	dcterms:created "2015-05-01T14:30:54Z"^^xsd:dateTime ;
	dcterms:creator <http://localhost/user/blumauera> ;
	dcterms:modified "2015-08-07T15:06:54Z"^^xsd:dateTime ;
	<http://schema.semantic-web.at/ppt/inScheme> <http://vocabulary.semantic-web.at/cocktails/591cf89a-57af-49b8-9042-3fc77408c93e> ;
	<http://schema.semantic-web.at/ppt/inSubtree> <http://vocabulary.semantic-web.at/cocktails/403d1249-f37f-4f43-bebf-8dde9677d886> ;
	<http://vocabulary.semantic-web.at/cocktail-ontology/image_3> <http://preview.poolparty.biz/sparqlingCocktails/resources/images/whiskey.png> ;
	a <http://vocabulary.semantic-web.at/cocktail-ontology/Alcoholic-Beverages> , <http://vocabulary.semantic-web.at/cocktail-ontology/Beverages> , <http://vocabulary.semantic-web.at/cocktail-ontology/Ingredients> , skos:Concept ;
	skos:altLabel "Craythur"@en , "Hot whiskey"@en , "Tarantula juice"@en , "Uisge beatha"@en , "Usquebaugh"@en , "Usquebeathe"@en , "Whiskey"@en , "Whiskies"@en , "Wiskey"@en ;
	skos:broader <http://vocabulary.semantic-web.at/cocktails/403d1249-f37f-4f43-bebf-8dde9677d886> , <http://vocabulary.semantic-web.at/cocktails/f3000285-36b0-4ffe-af90-740c2dd8fff5> ;
	skos:definition "Whisky or whiskey is a type of distilled alcoholic beverage made from fermented grain mash. Different grains are used for different varieties, including barley, malted barley, rye, malted rye, wheat, and corn. Whisky is typically aged in wooden casks, made generally of charred white oak. Whisky is a strictly regulated spirit worldwide with many classes and types."@en ;
	skos:exactMatch dbpedia:Whisky ;
	skos:narrower <http://vocabulary.semantic-web.at/cocktails/3e2d26b8-928b-462d-99ee-59eac11b241f> , <http://vocabulary.semantic-web.at/cocktails/4f03a6ef-9631-4b6d-a005-7fbbdcb9b342> , <http://vocabulary.semantic-web.at/cocktails/d14f3ba1-9350-49a9-a9df-4d97c61f9d87> , <http://vocabulary.semantic-web.at/cocktails/f0bfda32-3c42-457f-b6a3-bbf2a9e77b06> ;
	skos:prefLabel "Whisky"@en .

<http://vocabulary.semantic-web.at/cocktails/c532e86c-01cc-40d4-b2d6-1f959e72d9da> dcterms:contributor <http://localhost/user/blumauera> ;
	dcterms:created "2015-05-02T18:55:56Z"^^xsd:dateTime ;
	dcterms:creator <http://localhost/user/blumauera> ;
	dcterms:modified "2015-05-07T07:07:11Z"^^xsd:dateTime ;
	<http://schema.semantic-web.at/ppt/inScheme> <http://vocabulary.semantic-web.at/cocktails/591cf89a-57af-49b8-9042-3fc77408c93e> ;
	<http://schema.semantic-web.at/ppt/inSubtree> <http://vocabulary.semantic-web.at/cocktails/403d1249-f37f-4f43-bebf-8dde9677d886> ;
	<http://vocabulary.semantic-web.at/cocktail-ontology/is-part-of> <http://vocabulary.semantic-web.at/cocktails/b8075344-1e6d-4348-bdee-83948203a974> ;
	a <http://vocabulary.semantic-web.at/cocktail-ontology/Alcoholic-Beverages> , <http://vocabulary.semantic-web.at/cocktail-ontology/Beverages> , <http://vocabulary.semantic-web.at/cocktail-ontology/Ingredients> , skos:Concept ;
	skos:altLabel "Cherry Brandy"@en , "Kirschwasser"@en ;
	skos:broader <http://vocabulary.semantic-web.at/cocktails/8f09ee6f-d5b9-4b8a-aa17-b0665fae4e83> ;
	skos:definition "A kirschwasser or kirsch is a clear, colorless fruit brandy traditionally made from double distillation of morello cherries, a dark-colored cultivar of the sour cherry. However, it is now also made from other kinds of cherries. The cherries are fermented complete (that is, including their stones). Unlike cherry liqueurs and so-called “cherry brandies”, kirschwasser is not sweet."@en ;
	skos:exactMatch dbpedia:Kirsch ;
	skos:prefLabel "Kirsch"@en .

<http://vocabulary.semantic-web.at/cocktails/c5c70695-d939-4f4d-8ae7-394f2f66ccbb> dcterms:contributor <http://localhost/user/blumauera> ;
	dcterms:created "2015-05-01T15:12:26Z"^^xsd:dateTime ;
	dcterms:creator <http://localhost/user/blumauera> ;
	dcterms:modified "2015-05-04T11:32:36Z"^^xsd:dateTime ;
	<http://schema.semantic-web.at/ppt/inScheme> <http://vocabulary.semantic-web.at/cocktails/591cf89a-57af-49b8-9042-3fc77408c93e> ;
	<http://schema.semantic-web.at/ppt/inSubtree> <http://vocabulary.semantic-web.at/cocktails/403d1249-f37f-4f43-bebf-8dde9677d886> ;
	<http://vocabulary.semantic-web.at/cocktail-ontology/is-part-of> <http://vocabulary.semantic-web.at/cocktails/be3653af-d585-43f7-b8ce-ad75b1bd7aad> ;
	a <http://vocabulary.semantic-web.at/cocktail-ontology/Alcoholic-Beverages> , <http://vocabulary.semantic-web.at/cocktail-ontology/Beverages> , <http://vocabulary.semantic-web.at/cocktail-ontology/Ingredients> , skos:Concept ;
	skos:altLabel "Drambooie"@en , "Drambui"@en ;
	skos:broader <http://vocabulary.semantic-web.at/cocktails/917d78d0-0938-4fe0-80c4-cfd2eb16e6a4> ;
	skos:definition "Drambuie is a sweet, golden coloured 40% ABV liqueur made from malt whisky, honey, herbs, and spices. Produced in Broxburn, West Lothian, Scotland, it is served straight, on the rocks, or added to mixed drinks such as the Rusty Nail. In 2009, Drambuie launched The Royal Legacy of 1745, an upscale malt whisky liqueur. The 40% alcohol by volume spirit won the Drinks International Travel Retail Award for Best Travel Retail Drinks Launch at the TFWA, Cannes, France in October 2009."@en ;
	skos:exactMatch dbpedia:Drambuie ;
	skos:prefLabel "Drambuie"@en .

<http://vocabulary.semantic-web.at/cocktails/c8f4f6bd-4ac1-456a-a3aa-595e4b93d979> dcterms:contributor <http://localhost/user/blumauera> ;
	dcterms:created "2015-05-02T17:12:00Z"^^xsd:dateTime ;
	dcterms:creator <http://localhost/user/blumauera> ;
	dcterms:modified "2015-05-06T12:57:28Z"^^xsd:dateTime ;
	<http://schema.semantic-web.at/ppt/inScheme> <http://vocabulary.semantic-web.at/cocktails/8d052dfc-44bf-4985-8ce3-4564570a161b> ;
	<http://vocabulary.semantic-web.at/cocktail-ontology/consists-of> <http://vocabulary.semantic-web.at/cocktails/22df810d-e509-4da8-979c-0758e94de3e6> , <http://vocabulary.semantic-web.at/cocktails/a1c1e015-91fd-4f6e-b2a8-5edae9aa0b9d> ;
	<http://vocabulary.semantic-web.at/cocktail-ontology/iba> <http://www.iba-world.com/index.php?option=com_content&id=268&Itemid=532> ;
	<http://vocabulary.semantic-web.at/cocktail-ontology/image> <http://upload.wikimedia.org/wikipedia/commons/thumb/8/80/Godfather_cocktail.jpg/440px-Godfather_cocktail.jpg> ;
	<http://vocabulary.semantic-web.at/cocktail-ontology/is-variant-of> <http://vocabulary.semantic-web.at/cocktails/45788a96-1fde-486b-80fc-31ad243bba31> ;
	<http://vocabulary.semantic-web.at/cocktail-ontology/preparation> "Pour all ingredients directly into old fashioned glass filled with ice cubes. Stir gently."@en ;
	<http://vocabulary.semantic-web.at/cocktail-ontology/served> "On the rocks; poured over ice"@en ;
	<http://vocabulary.semantic-web.at/cocktail-ontology/uses> <http://vocabulary.semantic-web.at/cocktails/2dce3576-2603-41f9-8dce-ab21f639c2a7> ;
	a <http://vocabulary.semantic-web.at/cocktail-ontology/Cocktail> , skos:Concept ;
	skos:altLabel "God Mother"@en ;
	skos:broader <http://vocabulary.semantic-web.at/cocktails/b9bf3799-a4e4-47f7-9aea-7697cc998a34> ;
	skos:prefLabel "Godmother"@en ;
	skos:related <http://vocabulary.semantic-web.at/cocktails/45788a96-1fde-486b-80fc-31ad243bba31> .

<http://vocabulary.semantic-web.at/cocktails/c96d576c-9640-4c21-af92-d6da3560c9d0> dcterms:contributor <http://localhost/user/blumauera> ;
	dcterms:created "2015-05-01T14:48:28Z"^^xsd:dateTime ;
	dcterms:creator <http://localhost/user/blumauera> ;
	dcterms:modified "2015-11-18T14:34:41Z"^^xsd:dateTime ;
	<http://schema.semantic-web.at/ppt/inScheme> <http://vocabulary.semantic-web.at/cocktails/591cf89a-57af-49b8-9042-3fc77408c93e> ;
	<http://schema.semantic-web.at/ppt/inSubtree> <http://vocabulary.semantic-web.at/cocktails/403d1249-f37f-4f43-bebf-8dde9677d886> ;
	<http://vocabulary.semantic-web.at/cocktail-ontology/is-part-of> <http://vocabulary.semantic-web.at/cocktails/1576f08f-5936-4071-b85e-d4e85f31c303> , <http://vocabulary.semantic-web.at/cocktails/1d5b39cc-fcab-48b2-bb24-9840b7e34d64> , <http://vocabulary.semantic-web.at/cocktails/4efda48d-6c56-47e5-bf98-bf8918ff58eb> ;
	a <http://vocabulary.semantic-web.at/cocktail-ontology/Alcoholic-Beverages> , <http://vocabulary.semantic-web.at/cocktail-ontology/Beverages> , <http://vocabulary.semantic-web.at/cocktail-ontology/Ingredients> , skos:Concept ;
	skos:altLabel "Abasinthe"@en , "Absenta"@en , "Absenthe"@en , "Absinth"@en , "Absinthism"@en , "Absinthisme"@en , "Abstinthe"@en , "Apsenth"@en , "Apsinth"@en , "Green Fairy"@en , "Green fairy"@en , "La fee verte"@en ;
	skos:broader <http://vocabulary.semantic-web.at/cocktails/af5df232-948a-4dc9-8dd1-1d7bfbf523f1> ;
	skos:definition "Absinthe is historically described as a distilled, highly alcoholic beverage. It is an anise-flavoured spirit derived from botanicals, including the flowers and leaves of Artemisia absinthium (a.k.a. \"grand wormwood\"), together with green anise, sweet fennel, and other medicinal and culinary herbs. Absinthe traditionally has a natural green colour but may also be colourless. It is commonly referred to in historical literature as \"la fée verte\" (the green fairy)."@en ;
	skos:exactMatch dbpedia:Absinthe ;
	skos:prefLabel "Absinthe"@en .

<http://vocabulary.semantic-web.at/cocktails/ca113086-9563-4831-8a14-f9eb5cbaa49e> dcterms:contributor <http://localhost/user/blumauera> ;
	dcterms:created "2015-05-02T08:25:15Z"^^xsd:dateTime ;
	dcterms:creator <http://localhost/user/blumauera> ;
	dcterms:modified "2015-05-02T08:25:16Z"^^xsd:dateTime ;
	<http://schema.semantic-web.at/ppt/inScheme> <http://vocabulary.semantic-web.at/cocktails/591cf89a-57af-49b8-9042-3fc77408c93e> ;
	<http://schema.semantic-web.at/ppt/inSubtree> <http://vocabulary.semantic-web.at/cocktails/403d1249-f37f-4f43-bebf-8dde9677d886> ;
	a <http://vocabulary.semantic-web.at/cocktail-ontology/Alcoholic-Beverages> , <http://vocabulary.semantic-web.at/cocktail-ontology/Beverages> , <http://vocabulary.semantic-web.at/cocktail-ontology/Ingredients> , skos:Concept ;
	skos:altLabel "Almond flavor"@en , "Amaretto Sour (cocktail)"@en , "Amaretto sour"@en , "Amaretto sour (cocktail)"@en , "Ameretto"@en , "Cafe Zuerich"@en , "Cafe Zuerich (cocktail)"@en , "Cafe Zurich"@en , "Cafe Zurich (cocktail)"@en , "Cafe Zürich"@en , "Cafe Zürich (cocktail)"@en , "Disarono"@en , "God Father (cocktail)"@en , "God Mother (cocktail)"@en , "God father (cocktail)"@en , "God mother (cocktail)"@en , "Godmother (cocktail)"@en , "List of cocktails with amaretto"@en , "Silverlake Slip (cocktail)"@en , "Silverlake slip"@en , "Silverlake slip (cocktail)"@en ;
	skos:broader <http://vocabulary.semantic-web.at/cocktails/a1c1e015-91fd-4f6e-b2a8-5edae9aa0b9d> ;
	skos:definition "Amaretto is a sweet, almond-flavoured, Italian liqueur. It is made from a base of apricot pits or almonds, sometimes both."@en ;
	skos:exactMatch dbpedia:Amaretto ;
	skos:prefLabel "Amaretto"@en .

<http://vocabulary.semantic-web.at/cocktails/caae2ea0-7e60-400b-a2bb-14ef79720668> dcterms:contributor <http://localhost/user/blumauera> ;
	dcterms:created "2015-05-01T07:35:23Z"^^xsd:dateTime ;
	dcterms:creator <http://localhost/user/blumauera> ;
	dcterms:modified "2015-05-04T10:13:59Z"^^xsd:dateTime ;
	<http://schema.semantic-web.at/ppt/inScheme> <http://vocabulary.semantic-web.at/cocktails/8d052dfc-44bf-4985-8ce3-4564570a161b> ;
	a <http://vocabulary.semantic-web.at/cocktail-ontology/Cocktail> , skos:Concept ;
	skos:broader <http://vocabulary.semantic-web.at/cocktails/5ac37bec-e4b9-4d43-9bcc-8d6954903c25> ;
	skos:narrower <http://vocabulary.semantic-web.at/cocktails/099726a2-ec4b-4b0f-b4e4-e6f25cdfd685> , <http://vocabulary.semantic-web.at/cocktails/0bbdca98-077b-48d1-99d6-47eca59c442c> , <http://vocabulary.semantic-web.at/cocktails/1576f08f-5936-4071-b85e-d4e85f31c303> , <http://vocabulary.semantic-web.at/cocktails/1d5b39cc-fcab-48b2-bb24-9840b7e34d64> , <http://vocabulary.semantic-web.at/cocktails/21b94d69-280e-4546-be1a-fdd1d9aa5d32> , <http://vocabulary.semantic-web.at/cocktails/22f838ea-3c2b-4b63-99d1-fdb6280b5705> , <http://vocabulary.semantic-web.at/cocktails/2c3083d2-8650-4460-b019-cae7aea38f14> , <http://vocabulary.semantic-web.at/cocktails/36671f9c-904a-4629-937a-519d094ecefc> , <http://vocabulary.semantic-web.at/cocktails/383ea520-07b2-4dc9-8827-8fc84fb7749c> , <http://vocabulary.semantic-web.at/cocktails/40ab50e9-66f1-411b-8220-ef8f05273542> , <http://vocabulary.semantic-web.at/cocktails/44cc99c1-28ac-4c50-a55d-7244b2c5c07b> , <http://vocabulary.semantic-web.at/cocktails/53a05366-d473-4eb4-ac66-0d0119e0b759> , <http://vocabulary.semantic-web.at/cocktails/60d3a991-48d3-4e73-9d62-5961893fd311> , <http://vocabulary.semantic-web.at/cocktails/76c0e55c-22df-4489-9551-4fe8a6a649f8> , <http://vocabulary.semantic-web.at/cocktails/785b30fd-1eb4-445b-8247-7e1e57b35b0f> , <http://vocabulary.semantic-web.at/cocktails/79d4686d-4f5b-4067-a2ef-99beccc51242> , <http://vocabulary.semantic-web.at/cocktails/85669fcc-a38a-4ceb-ae23-90ae3fb7e16c> , <http://vocabulary.semantic-web.at/cocktails/8ff588a8-d5ad-4e34-aee9-8f6de16ca30c> , <http://vocabulary.semantic-web.at/cocktails/9c287d15-c699-4f56-bd65-bf8cc75a2cca> , <http://vocabulary.semantic-web.at/cocktails/a0fba95c-d29e-4954-8800-f5e6de1e6f86> , <http://vocabulary.semantic-web.at/cocktails/b0885ae3-68e1-453d-8669-119e8464ff5f> , <http://vocabulary.semantic-web.at/cocktails/b3834414-af63-4e6f-9c3c-6c353e9600ee> , <http://vocabulary.semantic-web.at/cocktails/bab016bd-2fd5-4809-bfe7-3225d25f116d> , <http://vocabulary.semantic-web.at/cocktails/be3653af-d585-43f7-b8ce-ad75b1bd7aad> , <http://vocabulary.semantic-web.at/cocktails/c151ee28-45d2-4128-8587-1f1b69060d9d> , <http://vocabulary.semantic-web.at/cocktails/c3ae5830-1bfd-4f37-afc9-3e88849d03cf> , <http://vocabulary.semantic-web.at/cocktails/cfa8539e-ede2-42ec-b563-d084ddb33280> , <http://vocabulary.semantic-web.at/cocktails/e039633b-03c1-47bd-a705-a104a4323e45> , <http://vocabulary.semantic-web.at/cocktails/f632b16d-1490-4587-a637-fb393d7b1e7f> , <http://vocabulary.semantic-web.at/cocktails/fb278b46-3c67-48b0-b9eb-7ea037294f5f> ;
	skos:prefLabel "The Unforgettables"@en .

<http://vocabulary.semantic-web.at/cocktails/cb1bb8c3-5013-4c5f-80e3-5267367fe2fb> dcterms:contributor <http://localhost/user/blumauera> ;
	dcterms:created "2015-05-01T08:27:45Z"^^xsd:dateTime ;
	dcterms:creator <http://localhost/user/blumauera> ;
	dcterms:modified "2015-05-04T11:21:21Z"^^xsd:dateTime ;
	<http://schema.semantic-web.at/ppt/inScheme> <http://vocabulary.semantic-web.at/cocktails/eff672ac-6601-42c6-a3e9-0adda3b45df8> ;
	<http://schema.semantic-web.at/ppt/inSubtree> <http://vocabulary.semantic-web.at/cocktails/469959a3-10dc-4539-80ff-08bf9ff2de1c> ;
	<http://vocabulary.semantic-web.at/cocktail-ontology/is-used-by_2> <http://vocabulary.semantic-web.at/cocktails/21b94d69-280e-4546-be1a-fdd1d9aa5d32> , <http://vocabulary.semantic-web.at/cocktails/cfa8539e-ede2-42ec-b563-d084ddb33280> ;
	a <http://vocabulary.semantic-web.at/cocktail-ontology/Garnish> , <http://vocabulary.semantic-web.at/cocktail-ontology/Ingredients> , skos:Concept ;
	skos:altLabel "Jaiphal"@en , "Jaiphar"@en , "Mace (botany and cooking)"@en , "Mace (spice)"@en , "Myristica"@en , "Myristica fragans"@en , "Myristica fragrans"@en , "Nutmeg butter"@en , "Nutmeg psychosis"@en , "Nutmeg seed"@en ;
	skos:broader <http://vocabulary.semantic-web.at/cocktails/469959a3-10dc-4539-80ff-08bf9ff2de1c> ;
	skos:definition "The nutmeg tree is any of several species of trees in genus Myristica. The most important commercial species is Myristica fragrans, an evergreen tree indigenous to the Banda Islands in the Moluccas (or Spice Islands) of Indonesia. The nutmeg tree is important for two spices derived from the fruit: nutmeg and mace."@en ;
	skos:exactMatch dbpedia:Nutmeg ;
	skos:prefLabel "Nutmeg"@en .

<http://vocabulary.semantic-web.at/cocktails/cc32e2f5-d1ae-4506-b000-86fbfee4a3e7> dcterms:contributor <http://localhost/user/blumauera> ;
	dcterms:created "2015-05-04T11:27:31Z"^^xsd:dateTime ;
	dcterms:creator <http://localhost/user/blumauera> ;
	dcterms:modified "2015-05-04T11:27:48Z"^^xsd:dateTime ;
	<http://schema.semantic-web.at/ppt/inScheme> <http://vocabulary.semantic-web.at/cocktails/eff672ac-6601-42c6-a3e9-0adda3b45df8> ;
	<http://schema.semantic-web.at/ppt/inSubtree> <http://vocabulary.semantic-web.at/cocktails/469959a3-10dc-4539-80ff-08bf9ff2de1c> ;
	<http://vocabulary.semantic-web.at/cocktail-ontology/is-part-of> <http://vocabulary.semantic-web.at/cocktails/c151ee28-45d2-4128-8587-1f1b69060d9d> ;
	a <http://vocabulary.semantic-web.at/cocktail-ontology/Garnish> , <http://vocabulary.semantic-web.at/cocktail-ontology/Ingredients> , skos:Concept ;
	skos:altLabel "Clear vanilla extract"@en , "Pure vanilla extract"@en , "Vanilla essence"@en ;
	skos:broader <http://vocabulary.semantic-web.at/cocktails/805e18b6-0f7a-4c26-b35e-9cc68a099086> ;
	skos:definition "Vanilla extract is a solution containing the flavor compound vanillin as the primary ingredient. Pure vanilla extract is made by macerating and percolating vanilla beans in a solution of ethyl alcohol and water. In the United States, in order for a vanilla extract to be called pure, the U.S. Food and Drug Administration requires that the solution contains a minimum 35% of alcohol and 13.35 ounces of vanilla bean per gallon."@en ;
	skos:exactMatch dbpedia:Vanilla_extract ;
	skos:prefLabel "Vanilla extract"@en .

<http://vocabulary.semantic-web.at/cocktails/ccee1079-43df-4ff1-bef0-d15d3dc8fa6f> dcterms:contributor <http://localhost/user/blumauera> ;
	dcterms:created "2015-05-01T07:35:16Z"^^xsd:dateTime ;
	dcterms:creator <http://localhost/user/blumauera> ;
	dcterms:modified "2015-05-04T10:14:03Z"^^xsd:dateTime ;
	<http://schema.semantic-web.at/ppt/inScheme> <http://vocabulary.semantic-web.at/cocktails/8d052dfc-44bf-4985-8ce3-4564570a161b> ;
	a <http://vocabulary.semantic-web.at/cocktail-ontology/Cocktail> , skos:Concept ;
	skos:broader <http://vocabulary.semantic-web.at/cocktails/5ac37bec-e4b9-4d43-9bcc-8d6954903c25> ;
	skos:narrower <http://vocabulary.semantic-web.at/cocktails/11d68913-3a30-4591-bc41-25fea3f38520> , <http://vocabulary.semantic-web.at/cocktails/236b36df-93ca-4408-836c-133ace53798a> , <http://vocabulary.semantic-web.at/cocktails/2c682ed8-e2ba-473e-8cb7-979598080e18> , <http://vocabulary.semantic-web.at/cocktails/43b786b6-a1f1-4b7f-a5d9-be43d386ffb4> , <http://vocabulary.semantic-web.at/cocktails/4d15a643-f7c7-4ee5-8f56-4ebd2bcf74b5> , <http://vocabulary.semantic-web.at/cocktails/563bf7e0-0f40-41b6-a749-c4e94760204d> , <http://vocabulary.semantic-web.at/cocktails/680c7429-30a7-4044-b32f-e28c99dcb9f4> , <http://vocabulary.semantic-web.at/cocktails/72a77af2-bbee-4b75-871f-a96dcd3a452b> , <http://vocabulary.semantic-web.at/cocktails/7e4a73d5-f73d-4890-972c-f3dfd6952fd8> , <http://vocabulary.semantic-web.at/cocktails/7e5afb63-30ec-42b4-a9f5-f61fc456107d> , <http://vocabulary.semantic-web.at/cocktails/a47e8f08-057a-45f2-8398-9be51ed351fc> , <http://vocabulary.semantic-web.at/cocktails/a5db05ca-eda3-41ef-a8ab-ba77b3e4baba> , <http://vocabulary.semantic-web.at/cocktails/b00a123f-a2b5-49d2-8325-a81d1d26ddc6> , <http://vocabulary.semantic-web.at/cocktails/b970d408-39ca-49b0-98fc-838f96c94608> , <http://vocabulary.semantic-web.at/cocktails/bed073f2-de84-4322-a490-4f34ec54c6d1> , <http://vocabulary.semantic-web.at/cocktails/cd66d6ff-559f-43ea-a754-ac613a87325d> ;
	skos:prefLabel "New Era Drinks"@en .

<http://vocabulary.semantic-web.at/cocktails/cd4b845c-d8db-4f73-9a0c-b60743c58019> dcterms:contributor <http://localhost/user/blumauera> ;
	dcterms:created "2015-05-02T18:35:30Z"^^xsd:dateTime ;
	dcterms:creator <http://localhost/user/blumauera> ;
	dcterms:modified "2015-05-07T06:56:19Z"^^xsd:dateTime ;
	<http://schema.semantic-web.at/ppt/inScheme> <http://vocabulary.semantic-web.at/cocktails/87384ce8-f20a-4201-b06d-3e0b8d832e5d> ;
	<http://schema.semantic-web.at/ppt/inSubtree> <http://vocabulary.semantic-web.at/cocktails/3c94f5fc-4664-4177-a880-88643c0be9c1> ;
	<http://vocabulary.semantic-web.at/cocktail-ontology/is-part-of> <http://vocabulary.semantic-web.at/cocktails/1529fd23-9c55-45d7-b8c6-b0fc229a3871> ;
	a <http://vocabulary.semantic-web.at/cocktail-ontology/Garnish> , <http://vocabulary.semantic-web.at/cocktail-ontology/Ingredients> , skos:Concept ;
	skos:altLabel "CONFECTIONER'S SUGAR"@en , "CONFECTIONER’S SUGAR"@en , "Confectioner's sugar"@en , "Confectioners' sugar"@en , "Confectionery sugar"@en , "Icing Sugar"@en , "Icing sugar"@en , "Powder sugar"@en ;
	skos:broader <http://vocabulary.semantic-web.at/cocktails/3c94f5fc-4664-4177-a880-88643c0be9c1> ;
	skos:definition "Powdered sugar, also known as confectioners' sugar or icing sugar, is very fine sugar. When intended for home use, it typically contains a small amount of anti-caking agent. In industrial food production, it is used where a quick dissolving sugar is required. Domestically, it is principally used to make icing or frosting and other cake decorations. It is often lightly dusted onto baked goods to add a light sweetness and subtle decoration."@en ;
	skos:exactMatch dbpedia:Powdered_sugar ;
	skos:prefLabel "Powdered sugar"@en .

<http://vocabulary.semantic-web.at/cocktails/cd66d6ff-559f-43ea-a754-ac613a87325d> dcterms:contributor <http://localhost/user/nagyhel> ;
	dcterms:created "2015-05-02T19:09:44Z"^^xsd:dateTime ;
	dcterms:creator <http://localhost/user/blumauera> ;
	dcterms:modified "2015-11-03T14:54:18Z"^^xsd:dateTime ;
	<http://schema.semantic-web.at/ppt/inScheme> <http://vocabulary.semantic-web.at/cocktails/8d052dfc-44bf-4985-8ce3-4564570a161b> ;
	<http://vocabulary.semantic-web.at/cocktail-ontology/consists-of> <http://vocabulary.semantic-web.at/cocktails/2e20010b-3ddb-48b9-b275-682e5c357730> , <http://vocabulary.semantic-web.at/cocktails/59848efb-dc96-4014-af09-5f89ba057df9> , <http://vocabulary.semantic-web.at/cocktails/8d5e2abc-6280-42b7-8e21-8bbc30f7509f> ;
	<http://vocabulary.semantic-web.at/cocktail-ontology/iba> <http://www.iba-world.com/index.php?option=com_content&id=261&Itemid=532> ;
	<http://vocabulary.semantic-web.at/cocktail-ontology/image> <http://upload.wikimedia.org/wikipedia/commons/3/3a/Cocktail_B52.jpg> ;
	<http://vocabulary.semantic-web.at/cocktail-ontology/preparation> "Layer ingredients one at a time starting with Kahlua, followed by Bailey's Irish Cream and top with Grand Marnier. Flame the Grand Marnier, serve while the flame is still on, accompanied with a straw on side plate."@en ;
	<http://vocabulary.semantic-web.at/cocktail-ontology/served> "Neat; undiluted and without ice"@en ;
	<http://vocabulary.semantic-web.at/cocktail-ontology/uses> <http://vocabulary.semantic-web.at/cocktails/bfbfb9b6-4c70-4323-a64b-4cfd533c55d8> ;
	a <http://vocabulary.semantic-web.at/cocktail-ontology/Cocktail> , skos:Concept ;
	skos:altLabel "B 52 drink"@en , "B-52 (drink)"@en , "B-52 shooter"@en , "B52"@en , "B52 (Cocktail)"@en , "B52 cocktail"@en , "B52 drink"@en , "Bifi"@en ;
	skos:broader <http://vocabulary.semantic-web.at/cocktails/b65b6d98-400f-47cf-94c7-d2566f10cf64> , <http://vocabulary.semantic-web.at/cocktails/ccee1079-43df-4ff1-bef0-d15d3dc8fa6f> ;
	skos:definition "The B-52 (also B52 or Bifi) cocktail is a layered shot composed of a coffee liqueur, an Irish Cream, and a triple sec. When prepared properly, the ingredients separate into three distinctly visible layering (due to their relative densities)."@en ;
	skos:exactMatch <http://dbpedia.org/resource/B-52_(cocktail)> ;
	skos:prefLabel "B-52"@en .

<http://vocabulary.semantic-web.at/cocktails/cdbac85a-d5b7-40f3-9e98-4d7e176b5565> dcterms:contributor <http://localhost/user/blumauera> ;
	dcterms:created "2015-05-02T08:12:09Z"^^xsd:dateTime ;
	dcterms:creator <http://localhost/user/blumauera> ;
	dcterms:modified "2015-05-07T06:53:51Z"^^xsd:dateTime ;
	<http://schema.semantic-web.at/ppt/inScheme> <http://vocabulary.semantic-web.at/cocktails/591cf89a-57af-49b8-9042-3fc77408c93e> ;
	<http://schema.semantic-web.at/ppt/inSubtree> <http://vocabulary.semantic-web.at/cocktails/d5286375-41b3-468b-9602-8fcf698e3e83> ;
	<http://vocabulary.semantic-web.at/cocktail-ontology/is-part-of> <http://vocabulary.semantic-web.at/cocktails/61a18ebf-fd92-4ef1-8ab1-bfd3c26867b9> , <http://vocabulary.semantic-web.at/cocktails/a73d88e9-0c50-45d2-b364-9dec5abe206d> , <http://vocabulary.semantic-web.at/cocktails/c2249dc0-0529-4a11-ad82-5d710b5e9c31> ;
	a <http://vocabulary.semantic-web.at/cocktail-ontology/Alcoholic-Beverages> , <http://vocabulary.semantic-web.at/cocktail-ontology/Beverages> , <http://vocabulary.semantic-web.at/cocktail-ontology/Ingredients> , skos:Concept ;
	skos:altLabel "Blanc de Noirs"@en , "Blanc de blanc"@en , "Blanc de blancs"@en , "Blanc de noir"@en , "Blanc de noirs"@en , "Brut champagne"@en , "Champagne (beverage)"@en , "Champagne (wine)"@en , "Champagne Blues"@en , "Champagne Classic"@en , "Champagne bottle"@en , "Champagne bottles"@en , "Champagne wine"@en , "Champagnes (wine)"@en , "Champaigne"@en , "French Champagne"@en , "Giggle water"@en , "Grandes marques"@en , "Methode Champagnoise"@en , "Prestige cuvée"@en , "Rosé champagne"@en ;
	skos:broader <http://vocabulary.semantic-web.at/cocktails/71399fc3-e67c-4b55-88a7-64c6b96128bc> ;
	skos:definition "Champagne is a sparkling wine produced from grapes grown in the Champagne region of France following rules that demand secondary fermentation of the wine in the bottle to create carbonation. Some use the term champagne as a generic term for sparkling wine, but many countries reserve the term exclusively for sparkling wines that come from Champagne and are produced under the rules of the appellation."@en ;
	skos:exactMatch dbpedia:Champagne ;
	skos:prefLabel "Champagne"@en .

<http://vocabulary.semantic-web.at/cocktails/ce8f4591-ccd4-4d90-a761-244115d64061> dcterms:contributor <http://localhost/user/blumauera> ;
	dcterms:created "2015-06-11T13:02:14Z"^^xsd:dateTime ;
	dcterms:creator <http://localhost/user/blumauera> ;
	dcterms:modified "2015-07-02T15:00:21Z"^^xsd:dateTime ;
	<http://schema.semantic-web.at/ppt/inScheme> <http://vocabulary.semantic-web.at/cocktails/8d052dfc-44bf-4985-8ce3-4564570a161b> ;
	<http://vocabulary.semantic-web.at/cocktail-ontology/consists-of> <http://vocabulary.semantic-web.at/cocktails/0f11bcdf-a69e-451f-b824-48b1743c5916> , <http://vocabulary.semantic-web.at/cocktails/22df810d-e509-4da8-979c-0758e94de3e6> , <http://vocabulary.semantic-web.at/cocktails/457aff50-b86b-4879-8e17-41ca59cf03a7> , <http://vocabulary.semantic-web.at/cocktails/5d96c50c-ee48-4c40-bb4c-4b9a42d11de6> , <http://vocabulary.semantic-web.at/cocktails/7dede323-e986-4417-b723-c9c7a7fe82ba> , <http://vocabulary.semantic-web.at/cocktails/9c2ce399-c6ae-4f4d-bf37-7fd8ffe2a19d> , <http://vocabulary.semantic-web.at/cocktails/d530df52-cc54-4be3-8409-85734e5ec67f> , <http://vocabulary.semantic-web.at/cocktails/f5cd2a2b-2153-4b7e-ae79-678b939765ca> ;
	<http://vocabulary.semantic-web.at/cocktail-ontology/iba> <http://www.iba-world.com/index.php?option=com_content&id=226&Itemid=532> ;
	<http://vocabulary.semantic-web.at/cocktail-ontology/image> <https://upload.wikimedia.org/wikipedia/commons/thumb/2/2d/Long_Island_Ice_Tea.jpg/512px-Long_Island_Ice_Tea.jpg> ;
	<http://vocabulary.semantic-web.at/cocktail-ontology/preparation> "Add all ingredients into highball glass filled with ice. Stir gently. Garnish with lemon spiral. Serve with straw."@en ;
	<http://vocabulary.semantic-web.at/cocktail-ontology/served> "On the rocks; poured over ice"@en ;
	<http://vocabulary.semantic-web.at/cocktail-ontology/uses> <http://vocabulary.semantic-web.at/cocktails/a54d2096-6214-4006-beaf-afcc77824710> ;
	<http://vocabulary.semantic-web.at/cocktail-ontology/uses_2> <http://vocabulary.semantic-web.at/cocktails/33df103a-03ac-4177-b620-7953fe094236> ;
	a <http://vocabulary.semantic-web.at/cocktail-ontology/Cocktail> , skos:Concept ;
	skos:broader <http://vocabulary.semantic-web.at/cocktails/b9bf3799-a4e4-47f7-9aea-7697cc998a34> ;
	skos:hiddenLabel "Long Island Ice Tea"@en ;
	skos:prefLabel "Long Island Iced Tea"@en .

<http://vocabulary.semantic-web.at/cocktails/cec5e96c-41c6-4b82-ab3a-0a057a54f70a> dcterms:contributor <http://localhost/user/blumauera> ;
	dcterms:created "2015-05-03T17:48:31Z"^^xsd:dateTime ;
	dcterms:creator <http://localhost/user/blumauera> ;
	dcterms:modified "2015-05-05T07:13:18Z"^^xsd:dateTime ;
	<http://schema.semantic-web.at/ppt/inScheme> <http://vocabulary.semantic-web.at/cocktails/eff672ac-6601-42c6-a3e9-0adda3b45df8> ;
	<http://schema.semantic-web.at/ppt/inSubtree> <http://vocabulary.semantic-web.at/cocktails/4f20d6bb-710d-4870-bde4-b6e835d7d13f> ;
	<http://vocabulary.semantic-web.at/cocktail-ontology/is-used-by_2> <http://vocabulary.semantic-web.at/cocktails/11d68913-3a30-4591-bc41-25fea3f38520> , <http://vocabulary.semantic-web.at/cocktails/a0fba95c-d29e-4954-8800-f5e6de1e6f86> ;
	a <http://vocabulary.semantic-web.at/cocktail-ontology/Garnish> , <http://vocabulary.semantic-web.at/cocktail-ontology/Ingredients> , skos:Concept ;
	skos:altLabel "Back olive"@en , "Black olive"@en , "Black olives"@en , "Colossal olive"@en , "Empeltre"@en , "Empeltre olives"@en , "European Olive"@en , "Green olive"@en , "Green olives"@en , "Kalamon (olive)"@en , "List of olive cultivars"@en , "Olea europaea"@en , "Olea europea"@en , "Olive (fruit)"@en , "Olive (tree)"@en , "Olive Tree"@en , "Olive grove"@en , "Olive groves"@en , "Olive tree"@en , "Olive trees"@en , "Olive wood"@en , "Olive-tree"@en , "Olive-trees"@en , "Olive-wood"@en , "Olives"@en , "Olivetree"@en , "Olivetrees"@en , "Olivey"@en , "The Olive Tree"@en ;
	skos:broader <http://vocabulary.semantic-web.at/cocktails/4f20d6bb-710d-4870-bde4-b6e835d7d13f> ;
	skos:definition "The olive is a species of small tree in the family Oleaceae, native to the coastal areas of the eastern Mediterranean Basin as well as northern Iraq, and northern Iran at the south of the Caspian Sea. Its fruit, also called the olive, is of major agricultural importance in the Mediterranean region as the source of olive oil. The tree and its fruit give its name to the plant family, which also includes species such as lilacs, jasmine, Forsythia and the true ash trees."@en ;
	skos:exactMatch dbpedia:Olive ;
	skos:prefLabel "Olive"@en .

<http://vocabulary.semantic-web.at/cocktails/ced2e755-fe48-4d7b-86ab-6b39fe359a32> dcterms:contributor <http://localhost/user/blumauera> ;
	dcterms:created "2015-05-01T14:12:13Z"^^xsd:dateTime ;
	dcterms:creator <http://localhost/user/blumauera> ;
	dcterms:modified "2015-05-07T07:16:02Z"^^xsd:dateTime ;
	<http://schema.semantic-web.at/ppt/inScheme> <http://vocabulary.semantic-web.at/cocktails/87384ce8-f20a-4201-b06d-3e0b8d832e5d> ;
	<http://vocabulary.semantic-web.at/cocktail-ontology/is-part-of> <http://vocabulary.semantic-web.at/cocktails/43111fc3-3b59-420c-a588-024cd2d33896> , <http://vocabulary.semantic-web.at/cocktails/55c40695-8b41-41ed-8c6a-70fe6930067e> , <http://vocabulary.semantic-web.at/cocktails/60d3a991-48d3-4e73-9d62-5961893fd311> , <http://vocabulary.semantic-web.at/cocktails/785b30fd-1eb4-445b-8247-7e1e57b35b0f> , <http://vocabulary.semantic-web.at/cocktails/9c287d15-c699-4f56-bd65-bf8cc75a2cca> ;
	a <http://vocabulary.semantic-web.at/cocktail-ontology/Ingredients> , skos:Concept ;
	skos:altLabel "Grenadin"@en , "Grenadin syrup"@en , "Grenadine syrup"@en , "Red fruit syrup"@en ;
	skos:broader <http://vocabulary.semantic-web.at/cocktails/0e385475-f369-4832-b8e3-20f35028988d> ;
	skos:definition "Grenadine is a commonly used bar syrup, characterized by a flavor that is both tart and sweet, and a deep red color. It is popular as an ingredient in cocktails, both for its flavor and to give a reddish/pink tint to mixed drinks."@en ;
	skos:exactMatch dbpedia:Grenadine ;
	skos:prefLabel "Grenadine"@en .

<http://vocabulary.semantic-web.at/cocktails/cfa8539e-ede2-42ec-b563-d084ddb33280> dcterms:contributor <http://localhost/user/blumauera> ;
	dcterms:created "2015-05-01T15:00:01Z"^^xsd:dateTime ;
	dcterms:creator <http://localhost/user/blumauera> ;
	dcterms:modified "2015-05-04T11:23:20Z"^^xsd:dateTime ;
	<http://schema.semantic-web.at/ppt/inScheme> <http://vocabulary.semantic-web.at/cocktails/8d052dfc-44bf-4985-8ce3-4564570a161b> ;
	<http://vocabulary.semantic-web.at/cocktail-ontology/consists-of> <http://vocabulary.semantic-web.at/cocktails/61b2054a-4bb6-4dc2-8125-d69977973bed> , <http://vocabulary.semantic-web.at/cocktails/8f09ee6f-d5b9-4b8a-aa17-b0665fae4e83> , <http://vocabulary.semantic-web.at/cocktails/ef0fb33b-cf31-4acb-aeb8-cff4ab5411d2> ;
	<http://vocabulary.semantic-web.at/cocktail-ontology/iba> <http://www.iba-world.com/index.php?option=com_content&id=205&Itemid=532> ;
	<http://vocabulary.semantic-web.at/cocktail-ontology/image> <http://upload.wikimedia.org/wikipedia/commons/thumb/d/d2/Porto_Flip.jpg/440px-Porto_Flip.jpg> ;
	<http://vocabulary.semantic-web.at/cocktail-ontology/preparation> "Shake ingredients together in a mixer with ice. Strain into glass, garnish and serve"@en ;
	<http://vocabulary.semantic-web.at/cocktail-ontology/served> "Straight up; without ice"@en ;
	<http://vocabulary.semantic-web.at/cocktail-ontology/uses> <http://vocabulary.semantic-web.at/cocktails/19dee0d8-fd30-469f-9ecd-91c902ff717c> ;
	<http://vocabulary.semantic-web.at/cocktail-ontology/uses_2> <http://vocabulary.semantic-web.at/cocktails/cb1bb8c3-5013-4c5f-80e3-5267367fe2fb> ;
	a <http://vocabulary.semantic-web.at/cocktail-ontology/Cocktail> , skos:Concept ;
	skos:broader <http://vocabulary.semantic-web.at/cocktails/caae2ea0-7e60-400b-a2bb-14ef79720668> ;
	skos:definition "A Porto flip is a type of alcoholic beverage. It is typically made with brandy, ruby port, and one egg yolk."@en ;
	skos:exactMatch dbpedia:Porto_flip ;
	skos:prefLabel "Porto flip"@en .

<http://vocabulary.semantic-web.at/cocktails/d14f3ba1-9350-49a9-a9df-4d97c61f9d87> dcterms:contributor <http://localhost/user/blumauera> ;
	dcterms:created "2015-05-02T17:21:28Z"^^xsd:dateTime ;
	dcterms:creator <http://localhost/user/blumauera> ;
	dcterms:modified "2015-05-07T06:49:01Z"^^xsd:dateTime ;
	<http://schema.semantic-web.at/ppt/inScheme> <http://vocabulary.semantic-web.at/cocktails/591cf89a-57af-49b8-9042-3fc77408c93e> ;
	<http://schema.semantic-web.at/ppt/inSubtree> <http://vocabulary.semantic-web.at/cocktails/403d1249-f37f-4f43-bebf-8dde9677d886> ;
	<http://vocabulary.semantic-web.at/cocktail-ontology/is-part-of> <http://vocabulary.semantic-web.at/cocktails/c3b197cc-8583-4e2f-8e45-3a7fed1309c1> ;
	a <http://vocabulary.semantic-web.at/cocktail-ontology/Alcoholic-Beverages> , <http://vocabulary.semantic-web.at/cocktail-ontology/Beverages> , <http://vocabulary.semantic-web.at/cocktail-ontology/Ingredients> , skos:Concept ;
	skos:altLabel "Irish whisky"@en ;
	skos:broader <http://vocabulary.semantic-web.at/cocktails/c4339109-ae35-4be9-a7e8-b5dfd206e960> ;
	skos:definition "Irish whiskey (Irish: Fuisce or uisce beatha) is whiskey made in Ireland. Key regulations defining Irish whiskey and its production are established by the Irish Whiskey Act of 1980, and are relatively simple (for example, in contrast with those for Scotch and Bourbon whiskey)."@en ;
	skos:exactMatch dbpedia:Irish_whiskey ;
	skos:prefLabel "Irish whiskey"@en .

<http://vocabulary.semantic-web.at/cocktails/d40e2215-bc1b-4bae-8cf8-d10b1ad36d44> dcterms:contributor <http://localhost/user/blumauera> ;
	dcterms:created "2015-05-01T14:40:12Z"^^xsd:dateTime ;
	dcterms:creator <http://localhost/user/blumauera> ;
	dcterms:modified "2015-05-01T14:40:42Z"^^xsd:dateTime ;
	<http://schema.semantic-web.at/ppt/inScheme> <http://vocabulary.semantic-web.at/cocktails/591cf89a-57af-49b8-9042-3fc77408c93e> ;
	<http://schema.semantic-web.at/ppt/inSubtree> <http://vocabulary.semantic-web.at/cocktails/403d1249-f37f-4f43-bebf-8dde9677d886> ;
	a <http://vocabulary.semantic-web.at/cocktail-ontology/Alcoholic-Beverages> , <http://vocabulary.semantic-web.at/cocktail-ontology/Beverages> , <http://vocabulary.semantic-web.at/cocktail-ontology/Ingredients> , skos:Concept ;
	skos:altLabel "Aromatic bitters"@en , "Bitter tonic"@en , "Herbal Bitters"@en ;
	skos:broader <http://vocabulary.semantic-web.at/cocktails/2944baef-5338-421b-a5f5-0e51f75244c2> ;
	skos:definition "A bitters is an alcoholic beverage flavored with herbal essences and has a bitter or bittersweet flavor. Numerous brands of bitters were formerly marketed as patent medicines, but are now considered to be digestifs rather than medicines. They commonly have an alcoholic strength of 45% ABV and are used as digestifs and as flavoring in cocktails."@en ;
	skos:exactMatch dbpedia:Bitters ;
	skos:narrower <http://vocabulary.semantic-web.at/cocktails/1d8d3cdc-91a7-421d-ad66-4814f475eddc> , <http://vocabulary.semantic-web.at/cocktails/5c291fe9-6fdb-4939-930d-dacbc67171a5> , <http://vocabulary.semantic-web.at/cocktails/7c831f82-c54d-4d31-ab40-97e1d6226cf2> , <http://vocabulary.semantic-web.at/cocktails/809f470a-4be7-47e8-9356-cb71009c31c2> , <http://vocabulary.semantic-web.at/cocktails/fbfae34b-60d5-47e6-83dc-31507a8d4f78> ;
	skos:prefLabel "Bitters"@en .

<http://vocabulary.semantic-web.at/cocktails/d5286375-41b3-468b-9602-8fcf698e3e83> dcterms:contributor <http://localhost/user/muecksteinm> ;
	dcterms:created "2015-05-02T07:24:42Z"^^xsd:dateTime ;
	dcterms:creator <http://localhost/user/blumauera> ;
	dcterms:modified "2015-09-07T11:34:07Z"^^xsd:dateTime ;
	<http://schema.semantic-web.at/ppt/inScheme> <http://vocabulary.semantic-web.at/cocktails/591cf89a-57af-49b8-9042-3fc77408c93e> ;
	<http://schema.semantic-web.at/ppt/propagateType> <http://vocabulary.semantic-web.at/cocktail-ontology/Alcoholic-Beverages> ;
	a <http://vocabulary.semantic-web.at/cocktail-ontology/Alcoholic-Beverages> , <http://vocabulary.semantic-web.at/cocktail-ontology/Beverages> , <http://vocabulary.semantic-web.at/cocktail-ontology/Ingredients> , skos:Concept ;
	skos:altLabel "Cooking Wine"@en , "Fine wine"@en , "Food wine"@en , "Grape wine"@en , "Kha'y"@en , "Red Wine"@en , "SARAP"@en , "Sacre Bleu Wine"@en , "Vin Rouge"@en , "Vinous"@en , "Wine storage temperature"@en , "Wines"@en , "ŞARAP"@en ;
	skos:broader <http://vocabulary.semantic-web.at/cocktails/f3000285-36b0-4ffe-af90-740c2dd8fff5> ;
	skos:definition "Wine is an alcoholic beverage made from fermented grapes or other fruits. The natural chemical balance of grapes lets them ferment without the addition of sugars, acids, enzymes, water, or other nutrients. Yeast consumes the sugars in the grapes and converts them into alcohol. Different varieties of grapes and strains of yeasts produce different types of wine."@en ;
	skos:exactMatch dbpedia:Wine ;
	skos:narrower <http://vocabulary.semantic-web.at/cocktails/70c69ab8-78ab-41b8-a93c-314cdeda1da4> , <http://vocabulary.semantic-web.at/cocktails/71399fc3-e67c-4b55-88a7-64c6b96128bc> , <http://vocabulary.semantic-web.at/cocktails/df4ff163-a7c8-4c40-b556-f9390fd97972> ;
	skos:prefLabel "Wine"@en ;
	skos:topConceptOf <http://vocabulary.semantic-web.at/cocktails/591cf89a-57af-49b8-9042-3fc77408c93e> .

<http://vocabulary.semantic-web.at/cocktails/d530df52-cc54-4be3-8409-85734e5ec67f> dcterms:contributor <http://localhost/user/blumauera> ;
	dcterms:created "2015-05-01T14:20:48Z"^^xsd:dateTime ;
	dcterms:creator <http://localhost/user/blumauera> ;
	dcterms:modified "2015-11-20T19:25:58Z"^^xsd:dateTime ;
	<http://schema.semantic-web.at/ppt/inScheme> <http://vocabulary.semantic-web.at/cocktails/591cf89a-57af-49b8-9042-3fc77408c93e> ;
	<http://schema.semantic-web.at/ppt/inSubtree> <http://vocabulary.semantic-web.at/cocktails/403d1249-f37f-4f43-bebf-8dde9677d886> ;
	<http://vocabulary.semantic-web.at/cocktail-ontology/is-part-of> <http://vocabulary.semantic-web.at/cocktails/22f838ea-3c2b-4b63-99d1-fdb6280b5705> , <http://vocabulary.semantic-web.at/cocktails/236b36df-93ca-4408-836c-133ace53798a> , <http://vocabulary.semantic-web.at/cocktails/36671f9c-904a-4629-937a-519d094ecefc> , <http://vocabulary.semantic-web.at/cocktails/a47e8f08-057a-45f2-8398-9be51ed351fc> , <http://vocabulary.semantic-web.at/cocktails/b970d408-39ca-49b0-98fc-838f96c94608> , <http://vocabulary.semantic-web.at/cocktails/ce8f4591-ccd4-4d90-a761-244115d64061> , <http://vocabulary.semantic-web.at/cocktails/e039633b-03c1-47bd-a705-a104a4323e45> ;
	a <http://vocabulary.semantic-web.at/cocktail-ontology/Alcoholic-Beverages> , <http://vocabulary.semantic-web.at/cocktail-ontology/Beverages> , <http://vocabulary.semantic-web.at/cocktail-ontology/Ingredients> , skos:Concept ;
	skos:altLabel "Orange liqueur"@en , "Triplesec"@en , "Tripple sec"@en ;
	skos:broader <http://vocabulary.semantic-web.at/cocktails/82026d8e-0fa5-4317-8827-410133db3bbd> ;
	skos:definition "Triple sec, originally Curaçao triple sec, is a variety of Curaçao liqueur, an orange-flavoured liqueur made from the dried peels of bitter and sweet orange. Triple sec may be consumed neat as a digestif or on the rocks, but nowadays is mostly used in making cocktails such as the Margarita, White Lady, Long Island Iced Tea, and Cosmopolitan."@en ;
	skos:exactMatch dbpedia:Triple_sec ;
	skos:prefLabel "Triple sec"@en .

<http://vocabulary.semantic-web.at/cocktails/d6c5f29f-bef7-41c5-9d39-535d83e9f750> dcterms:contributor <http://localhost/user/blumauera> ;
	dcterms:created "2015-05-02T18:43:25Z"^^xsd:dateTime ;
	dcterms:creator <http://localhost/user/blumauera> ;
	dcterms:modified "2015-07-29T16:14:27Z"^^xsd:dateTime ;
	<http://schema.semantic-web.at/ppt/inScheme> <http://vocabulary.semantic-web.at/cocktails/f09732a9-a0e6-494a-8ce9-299ef036aaaf> ;
	a <http://vocabulary.semantic-web.at/cocktail-ontology/Drinkware> , skos:Concept ;
	skos:altLabel "Coffee mug"@en , "Coffee mugs"@en , "Mugs"@en , "Puzzle mug"@en , "Shaving mug"@en , "Shaving scuttle"@en , "Thermochromic mug"@en , "Toby (mug)"@en , "Travel mug"@en ;
	skos:definition "A mug is a sturdily built type of cup often used for drinking hot beverages, such as coffee, tea, or hot chocolate. Mugs often have handles and hold a larger amount of fluid than other types of cup. Usually a mug holds approximately 12 fluid ounces (350 mL) of liquid; double a tea cup. A mug is a less formal style of drink container and is not usually used in formal place settings, where a teacup or coffee cup is preferred. Shaving mugs can be used to assist in wet shaving."@en ;
	skos:exactMatch dbpedia:Mug ;
	skos:narrower <http://vocabulary.semantic-web.at/cocktails/0381bd47-ad07-428a-b5c4-ee2608f2ebd3> , <http://vocabulary.semantic-web.at/cocktails/347f5539-1dae-44fc-9e7b-a2cbe9e2e157> ;
	skos:prefLabel "Mug"@en ;
	skos:topConceptOf <http://vocabulary.semantic-web.at/cocktails/f09732a9-a0e6-494a-8ce9-299ef036aaaf> .

<http://vocabulary.semantic-web.at/cocktails/d9f071c0-8c44-43d1-9e4f-eef5709f5d98> dcterms:contributor <http://localhost/user/blumauera> ;
	dcterms:created "2015-05-02T19:30:37Z"^^xsd:dateTime ;
	dcterms:creator <http://localhost/user/blumauera> ;
	dcterms:modified "2015-05-05T07:49:33Z"^^xsd:dateTime ;
	<http://schema.semantic-web.at/ppt/inScheme> <http://vocabulary.semantic-web.at/cocktails/591cf89a-57af-49b8-9042-3fc77408c93e> ;
	<http://schema.semantic-web.at/ppt/inSubtree> <http://vocabulary.semantic-web.at/cocktails/403d1249-f37f-4f43-bebf-8dde9677d886> ;
	<http://vocabulary.semantic-web.at/cocktail-ontology/is-part-of> <http://vocabulary.semantic-web.at/cocktails/43b786b6-a1f1-4b7f-a5d9-be43d386ffb4> ;
	a <http://vocabulary.semantic-web.at/cocktail-ontology/Alcoholic-Beverages> , <http://vocabulary.semantic-web.at/cocktail-ontology/Beverages> , <http://vocabulary.semantic-web.at/cocktail-ontology/Ingredients> , skos:Concept ;
	skos:altLabel "Peruvian pisco"@en , "Pisco in Peru"@en ;
	skos:broader <http://vocabulary.semantic-web.at/cocktails/8f09ee6f-d5b9-4b8a-aa17-b0665fae4e83> ;
	skos:definition "Pisco is a colorless or yellowish-to-amber colored grape brandy produced in winemaking regions of Peru and Chile. Pisco was developed by Spanish settlers in the 16th century as an alternative to orujo, a pomace brandy that was being imported from Spain."@en ;
	skos:exactMatch dbpedia:Pisco ;
	skos:prefLabel "Pisco"@en .

<http://vocabulary.semantic-web.at/cocktails/de17b6c7-513a-4fe2-a8ee-4fdc6069ae27> dcterms:contributor <http://localhost/user/blumauera> ;
	dcterms:created "2015-05-01T14:26:37Z"^^xsd:dateTime ;
	dcterms:creator <http://localhost/user/blumauera> ;
	dcterms:modified "2015-05-01T15:02:04Z"^^xsd:dateTime ;
	<http://schema.semantic-web.at/ppt/inScheme> <http://vocabulary.semantic-web.at/cocktails/591cf89a-57af-49b8-9042-3fc77408c93e> ;
	<http://schema.semantic-web.at/ppt/inSubtree> <http://vocabulary.semantic-web.at/cocktails/e86c1671-4a67-494b-ae5d-bcb750865acc> ;
	a <http://vocabulary.semantic-web.at/cocktail-ontology/Beverages> , <http://vocabulary.semantic-web.at/cocktail-ontology/Ingredients> , <http://vocabulary.semantic-web.at/cocktail-ontology/Non-alcoholic-Beverages> , skos:Concept ;
	skos:broader <http://vocabulary.semantic-web.at/cocktails/e86c1671-4a67-494b-ae5d-bcb750865acc> ;
	skos:narrower <http://vocabulary.semantic-web.at/cocktails/61b2054a-4bb6-4dc2-8125-d69977973bed> , <http://vocabulary.semantic-web.at/cocktails/98f20476-57d7-46d3-b76d-6aac18b57788> ;
	skos:prefLabel "From egg"@en .

<http://vocabulary.semantic-web.at/cocktails/df4ff163-a7c8-4c40-b556-f9390fd97972> dcterms:contributor <http://localhost/user/blumauera> ;
	dcterms:created "2015-05-02T17:27:52Z"^^xsd:dateTime ;
	dcterms:creator <http://localhost/user/blumauera> ;
	dcterms:modified "2016-08-24T11:53:15Z"^^xsd:dateTime ;
	<http://schema.semantic-web.at/ppt/inScheme> <http://vocabulary.semantic-web.at/cocktails/591cf89a-57af-49b8-9042-3fc77408c93e> ;
	<http://schema.semantic-web.at/ppt/inSubtree> <http://vocabulary.semantic-web.at/cocktails/d5286375-41b3-468b-9602-8fcf698e3e83> ;
	<http://vocabulary.semantic-web.at/cocktail-ontology/is-part-of> <http://vocabulary.semantic-web.at/cocktails/ea946e07-e812-4492-a0ed-124d73bfbba7> ;
	a <http://vocabulary.semantic-web.at/cocktail-ontology/Alcoholic-Beverages> , <http://vocabulary.semantic-web.at/cocktail-ontology/Beverages> , <http://vocabulary.semantic-web.at/cocktail-ontology/Ingredients> , skos:Concept ;
	skos:altLabel "White wines"@en ;
	skos:broader <http://vocabulary.semantic-web.at/cocktails/d5286375-41b3-468b-9602-8fcf698e3e83> ;
	skos:definition "White wine is a wine whose color can be straw-yellow, yellow-green, and yellow-gold coloured. White wine's color can be derived from an assortment of grape varieties. White wines are made from the grape juice and grape skin or from just the juice (not the skin) of select red grapes (as in some Champagnes). White wines are often consumed with lighter meals, or as an apéritif."@en ;
	skos:exactMatch dbpedia:Category:White_wines , dbpedia:White_wine ;
	skos:prefLabel "White wine"@en .

<http://vocabulary.semantic-web.at/cocktails/dff0a7f4-ded0-48d5-bd31-881b70fbe36a> dcterms:contributor <http://localhost/user/blumauera> ;
	dcterms:created "2015-05-01T07:36:07Z"^^xsd:dateTime ;
	dcterms:creator <http://localhost/user/blumauera> ;
	dcterms:modified "2015-05-07T07:12:26Z"^^xsd:dateTime ;
	<http://schema.semantic-web.at/ppt/inScheme> <http://vocabulary.semantic-web.at/cocktails/8d052dfc-44bf-4985-8ce3-4564570a161b> ;
	<http://vocabulary.semantic-web.at/cocktail-ontology/consists-of> <http://vocabulary.semantic-web.at/cocktails/22df810d-e509-4da8-979c-0758e94de3e6> , <http://vocabulary.semantic-web.at/cocktails/2ce50273-13b2-4ba1-9ff2-8cfbd835c1f2> , <http://vocabulary.semantic-web.at/cocktails/45234a8f-9357-49d2-931b-638c48e3772e> , <http://vocabulary.semantic-web.at/cocktails/7738a6e2-84c2-4ae3-b605-8bb6420e6e28> ;
	<http://vocabulary.semantic-web.at/cocktail-ontology/iba> <http://www.iba-world.com/index.php?option=com_content&id=235&Itemid=532> ;
	<http://vocabulary.semantic-web.at/cocktail-ontology/image> <http://upload.wikimedia.org/wikipedia/commons/thumb/a/a2/Sex_On_The_Beach.jpg/440px-Sex_On_The_Beach.jpg> ;
	<http://vocabulary.semantic-web.at/cocktail-ontology/preparation> "Build all ingredients in a highball glass filled with ice. Garnish with orange slice."@en ;
	<http://vocabulary.semantic-web.at/cocktail-ontology/served> "On the rocks; poured over ice"@en ;
	<http://vocabulary.semantic-web.at/cocktail-ontology/uses> <http://vocabulary.semantic-web.at/cocktails/a54d2096-6214-4006-beaf-afcc77824710> ;
	<http://vocabulary.semantic-web.at/cocktail-ontology/uses_2> <http://vocabulary.semantic-web.at/cocktails/99171f20-c59f-40c4-998a-a9c8f1909168> ;
	a <http://vocabulary.semantic-web.at/cocktail-ontology/Cocktail> , skos:Concept ;
	skos:altLabel "Sex on the Beach (cocktail)"@en , "Sex on the Beach cocktail"@en ;
	skos:broader <http://vocabulary.semantic-web.at/cocktails/b9bf3799-a4e4-47f7-9aea-7697cc998a34> ;
	skos:definition "Sex on the Beach is a cocktail that has many variations."@en ;
	skos:exactMatch dbpedia:Sex_on_the_Beach ;
	skos:prefLabel "Sex on the Beach"@en .

<http://vocabulary.semantic-web.at/cocktails/e039633b-03c1-47bd-a705-a104a4323e45> dcterms:contributor <http://localhost/user/blumauera> ;
	dcterms:created "2015-05-01T15:17:34Z"^^xsd:dateTime ;
	dcterms:creator <http://localhost/user/blumauera> ;
	dcterms:modified "2015-05-07T06:47:54Z"^^xsd:dateTime ;
	<http://schema.semantic-web.at/ppt/inScheme> <http://vocabulary.semantic-web.at/cocktails/8d052dfc-44bf-4985-8ce3-4564570a161b> ;
	<http://vocabulary.semantic-web.at/cocktail-ontology/consists-of> <http://vocabulary.semantic-web.at/cocktails/9c2ce399-c6ae-4f4d-bf37-7fd8ffe2a19d> , <http://vocabulary.semantic-web.at/cocktails/d530df52-cc54-4be3-8409-85734e5ec67f> , <http://vocabulary.semantic-web.at/cocktails/fd76c5ab-be62-4c4b-a2c6-7fa9bc359f47> ;
	<http://vocabulary.semantic-web.at/cocktail-ontology/iba> <http://www.iba-world.com/index.php?option=com_content&id=209&Itemid=532> ;
	<http://vocabulary.semantic-web.at/cocktail-ontology/image> <http://upload.wikimedia.org/wikipedia/commons/thumb/9/94/Sidecar-cocktail.jpg/440px-Sidecar-cocktail.jpg> ;
	<http://vocabulary.semantic-web.at/cocktail-ontology/preparation> "Pour all ingredients into cocktail shaker filled with ice. Shake well and strain into cocktail glass."@en ;
	<http://vocabulary.semantic-web.at/cocktail-ontology/served> "Straight up (without ice)"@en ;
	<http://vocabulary.semantic-web.at/cocktail-ontology/uses> <http://vocabulary.semantic-web.at/cocktails/19dee0d8-fd30-469f-9ecd-91c902ff717c> ;
	a <http://vocabulary.semantic-web.at/cocktail-ontology/Cocktail> , skos:Concept ;
	skos:altLabel "Sidecar (drink)"@en , "Sidecar cocktail"@en ;
	skos:broader <http://vocabulary.semantic-web.at/cocktails/7516b400-963a-4151-8fdc-f6b23bad1dd5> , <http://vocabulary.semantic-web.at/cocktails/caae2ea0-7e60-400b-a2bb-14ef79720668> ;
	skos:definition "The Sidecar is a classic cocktail traditionally made with cognac, orange liqueur, and lemon juice. In its ingredients, the drink is perhaps most closely related to the older Brandy Daisy, which differs both in presentation and in proportions of its components."@en ;
	skos:exactMatch <http://dbpedia.org/resource/Sidecar_(cocktail)> ;
	skos:prefLabel "Sidecar"@en ;
	skos:related <http://vocabulary.semantic-web.at/cocktails/22f838ea-3c2b-4b63-99d1-fdb6280b5705> .

<http://vocabulary.semantic-web.at/cocktails/e2d63a1c-56e7-47d2-b01b-8cf88cac3d8b> dcterms:contributor <http://localhost/user/blumauera> ;
	dcterms:created "2015-05-01T08:10:23Z"^^xsd:dateTime ;
	dcterms:creator <http://localhost/user/blumauera> ;
	dcterms:modified "2015-05-07T06:51:44Z"^^xsd:dateTime ;
	<http://schema.semantic-web.at/ppt/inScheme> <http://vocabulary.semantic-web.at/cocktails/eff672ac-6601-42c6-a3e9-0adda3b45df8> ;
	<http://schema.semantic-web.at/ppt/inSubtree> <http://vocabulary.semantic-web.at/cocktails/469959a3-10dc-4539-80ff-08bf9ff2de1c> ;
	<http://vocabulary.semantic-web.at/cocktail-ontology/is-part-of> <http://vocabulary.semantic-web.at/cocktails/a5db05ca-eda3-41ef-a8ab-ba77b3e4baba> ;
	<http://vocabulary.semantic-web.at/cocktail-ontology/is-used-by_2> <http://vocabulary.semantic-web.at/cocktails/2d85fb1b-96cb-4c48-8df5-707032f34e71> ;
	a <http://vocabulary.semantic-web.at/cocktail-ontology/Garnish> , <http://vocabulary.semantic-web.at/cocktail-ontology/Ingredients> , skos:Concept ;
	skos:altLabel "Common salt"@en , "Dietary salt"@en , "Edible salt"@en , "Health effects of salt"@en , "Kitchen salt"@en , "Nac1"@en , "Normal salt"@en , "Refined salt"@en , "Refining salt"@en , "Salt (compound)"@en , "Salt (food)"@en , "Salt crystal"@en , "Salt crystals"@en , "Salt production"@en , "Salt refining"@en , "Saltmaking"@en , "Sodium salt"@en , "Table Salt"@en , "Table salt"@en ;
	skos:broader <http://vocabulary.semantic-web.at/cocktails/469959a3-10dc-4539-80ff-08bf9ff2de1c> ;
	skos:definition "Salt, also known as table salt or rock salt, is a crystalline mineral that is composed primarily of sodium chloride, a chemical compound belonging to the larger class of ionic salts. It is absolutely essential for animal life, but can be harmful to animals and plants in excess. Salt is one of the oldest, most ubiquitous food seasonings and salting is an important method of food preservation. The taste of salt (saltiness) is one of the basic human tastes."@en ;
	skos:exactMatch dbpedia:Salt ;
	skos:narrower <http://vocabulary.semantic-web.at/cocktails/6f6c504d-2272-4561-b46b-35bbccad8355> ;
	skos:prefLabel "Salt"@en .

<http://vocabulary.semantic-web.at/cocktails/e406119b-7637-43f9-9a62-5a8ea500ebc4> dcterms:contributor <http://localhost/user/blumauera> ;
	dcterms:created "2015-05-01T15:21:03Z"^^xsd:dateTime ;
	dcterms:creator <http://localhost/user/blumauera> ;
	dcterms:modified "2015-05-07T06:27:23Z"^^xsd:dateTime ;
	<http://schema.semantic-web.at/ppt/inScheme> <http://vocabulary.semantic-web.at/cocktails/591cf89a-57af-49b8-9042-3fc77408c93e> ;
	<http://schema.semantic-web.at/ppt/inSubtree> <http://vocabulary.semantic-web.at/cocktails/403d1249-f37f-4f43-bebf-8dde9677d886> ;
	<http://vocabulary.semantic-web.at/cocktail-ontology/is-part-of> <http://vocabulary.semantic-web.at/cocktails/099726a2-ec4b-4b0f-b4e4-e6f25cdfd685> , <http://vocabulary.semantic-web.at/cocktails/117bd4d2-6da3-4d69-8c79-bc1d873b5010> ;
	a <http://vocabulary.semantic-web.at/cocktail-ontology/Alcoholic-Beverages> , <http://vocabulary.semantic-web.at/cocktail-ontology/Beverages> , <http://vocabulary.semantic-web.at/cocktail-ontology/Ingredients> , skos:Concept ;
	skos:altLabel "Creme de Menthe"@en , "Creme de menthe"@en , "Creme de minthe"@en ;
	skos:broader <http://vocabulary.semantic-web.at/cocktails/47635419-edef-4b78-8da1-e58a96d96f61> , <http://vocabulary.semantic-web.at/cocktails/917d78d0-0938-4fe0-80c4-cfd2eb16e6a4> ;
	skos:definition "Crème de menthe (French for mint cream) is a sweet, mint-flavored alcoholic beverage. Its flavor is primarily derived from Corsican mint. It is available commercially in a colorless (called \"white\") and a green version (which obtains its color from the mint leaves or from the addition of coloring, if extract and not the leaves are used to make the liqueur). Both varieties have similar flavors and are interchangeable in recipes, except where the color is important."@en ;
	skos:exactMatch dbpedia:Cr%C3%A8me_de_menthe ;
	skos:prefLabel "Crème de menthe"@en .

<http://vocabulary.semantic-web.at/cocktails/e576e848-0f11-4f7a-b6b3-1ff820b02023> dcterms:contributor <http://localhost/user/blumauera> ;
	dcterms:created "2015-05-02T17:26:39Z"^^xsd:dateTime ;
	dcterms:creator <http://localhost/user/blumauera> ;
	dcterms:modified "2015-05-07T07:23:27Z"^^xsd:dateTime ;
	<http://schema.semantic-web.at/ppt/inScheme> <http://vocabulary.semantic-web.at/cocktails/f09732a9-a0e6-494a-8ce9-299ef036aaaf> ;
	<http://vocabulary.semantic-web.at/cocktail-ontology/image_2> <http://upload.wikimedia.org/wikipedia/commons/thumb/7/7e/Wineglass.svg/26px-Wineglass.svg.png> ;
	<http://vocabulary.semantic-web.at/cocktail-ontology/is-used-by> <http://vocabulary.semantic-web.at/cocktails/ea946e07-e812-4492-a0ed-124d73bfbba7> ;
	a <http://vocabulary.semantic-web.at/cocktail-ontology/Drinkware> , skos:Concept ;
	skos:altLabel "Airtwist"@en , "Boccalino"@en , "Copita"@en , "Sherry glass"@en , "Wine cup"@en , "Wine glasses"@en , "Wineglass"@en , "🍷"@en ;
	skos:broader <http://vocabulary.semantic-web.at/cocktails/2ea18d11-7415-4282-9608-7a3f497a0928> ;
	skos:definition "A wine glass is a type of glass stemware that is used to drink and taste wine. It is generally composed of three parts: the bowl, stem, and foot. Selection of a particular wine glass for a wine style is important, as the glass shape can influence its perception."@en ;
	skos:exactMatch dbpedia:Wine_glass ;
	skos:prefLabel "Wine glass"@en .

<http://vocabulary.semantic-web.at/cocktails/e5f9e219-d894-491c-a009-20336f5b8e7f> dcterms:contributor <http://localhost/user/blumauera> ;
	dcterms:created "2015-05-02T19:14:57Z"^^xsd:dateTime ;
	dcterms:creator <http://localhost/user/blumauera> ;
	dcterms:modified "2015-05-02T19:14:57Z"^^xsd:dateTime ;
	<http://schema.semantic-web.at/ppt/inScheme> <http://vocabulary.semantic-web.at/cocktails/591cf89a-57af-49b8-9042-3fc77408c93e> ;
	<http://schema.semantic-web.at/ppt/inSubtree> <http://vocabulary.semantic-web.at/cocktails/403d1249-f37f-4f43-bebf-8dde9677d886> ;
	a <http://vocabulary.semantic-web.at/cocktail-ontology/Alcoholic-Beverages> , <http://vocabulary.semantic-web.at/cocktail-ontology/Beverages> , <http://vocabulary.semantic-web.at/cocktail-ontology/Ingredients> , skos:Concept ;
	skos:altLabel "Irish Cream Liqueur"@en , "Irish creme"@en ;
	skos:broader <http://vocabulary.semantic-web.at/cocktails/a62bc4d7-b07a-4e32-9254-9facbeb8831d> ;
	skos:definition "Irish cream is a cream liqueur based on Irish whiskey, cream, and other ingredients such as coffee, which can be served on its own or used in mixed drinks or as part of a shot or a whole shot. Irish cream is very popular in the United Kingdom, Canada, and the United States. Irish cream typically has between 15 to 20% alcohol by volume (ABV). Some notable brands of Irish cream are Baileys, Carolans and Saint Brendan's."@en ;
	skos:exactMatch dbpedia:Irish_cream ;
	skos:narrower <http://vocabulary.semantic-web.at/cocktails/2e20010b-3ddb-48b9-b275-682e5c357730> ;
	skos:prefLabel "Irish cream"@en .

<http://vocabulary.semantic-web.at/cocktails/e67b1621-7be7-471d-ac8d-a368d8c68115> dcterms:contributor <http://localhost/user/blumauera> ;
	dcterms:created "2015-05-02T08:10:07Z"^^xsd:dateTime ;
	dcterms:creator <http://localhost/user/blumauera> ;
	dcterms:modified "2015-05-03T17:27:51Z"^^xsd:dateTime ;
	<http://schema.semantic-web.at/ppt/inScheme> <http://vocabulary.semantic-web.at/cocktails/591cf89a-57af-49b8-9042-3fc77408c93e> ;
	<http://schema.semantic-web.at/ppt/inSubtree> <http://vocabulary.semantic-web.at/cocktails/403d1249-f37f-4f43-bebf-8dde9677d886> ;
	<http://vocabulary.semantic-web.at/cocktail-ontology/is-part-of> <http://vocabulary.semantic-web.at/cocktails/bca7bc6d-6709-48b8-ae52-fe194c212398> ;
	a <http://vocabulary.semantic-web.at/cocktail-ontology/Alcoholic-Beverages> , <http://vocabulary.semantic-web.at/cocktail-ontology/Beverages> , <http://vocabulary.semantic-web.at/cocktail-ontology/Ingredients> , skos:Concept ;
	skos:altLabel "Brazil Cachaca"@en , "Brazil Cachaça"@en , "Cachaca"@en , "Cachaca Brazil"@en , "Cachaça Brazil"@en , "Cagaca"@en , "Caninha"@en , "Cashasa"@en , "Caxa"@en , "Caxaca"@en , "Java (cachaca)"@en , "Java (cachaça)"@en ;
	skos:broader <http://vocabulary.semantic-web.at/cocktails/f5cd2a2b-2153-4b7e-ae79-678b939765ca> ;
	skos:definition "Cachaça is a liquor made from fermented sugarcane juice. It is the most popular distilled alcoholic beverage in Brazil. It is also known as aguardente, pinga, caninha and by many other names. Cachaça is mostly produced in Brazil, where, according to 2007 figures, 1.5 billion litres (390 million gallons) are consumed annually, compared with 15 million litres (4.0 million gallons) outside the country. It is typically between 38% and 48% alcohol by volume."@en ;
	skos:exactMatch dbpedia:Cacha%C3%A7a ;
	skos:prefLabel "Cachaça"@en .

<http://vocabulary.semantic-web.at/cocktails/e76e4e97-260a-4eef-af34-111938241931> dcterms:contributor <http://localhost/user/blumauera> ;
	dcterms:created "2015-05-05T13:04:14Z"^^xsd:dateTime ;
	dcterms:creator <http://localhost/user/blumauera> ;
	dcterms:modified "2015-05-05T13:05:43Z"^^xsd:dateTime ;
	<http://schema.semantic-web.at/ppt/inScheme> <http://vocabulary.semantic-web.at/cocktails/eff672ac-6601-42c6-a3e9-0adda3b45df8> ;
	<http://schema.semantic-web.at/ppt/inSubtree> <http://vocabulary.semantic-web.at/cocktails/469959a3-10dc-4539-80ff-08bf9ff2de1c> ;
	<http://vocabulary.semantic-web.at/cocktail-ontology/is-used-by_2> <http://vocabulary.semantic-web.at/cocktails/a5db05ca-eda3-41ef-a8ab-ba77b3e4baba> ;
	a <http://vocabulary.semantic-web.at/cocktail-ontology/Garnish> , <http://vocabulary.semantic-web.at/cocktail-ontology/Ingredients> , skos:Concept ;
	skos:altLabel "Chile (capsicum)"@en , "Chile pepper"@en , "Chile peppers"@en , "Chili (capsicum)"@en , "Chili peppers"@en , "Chilies"@en , "Chilli (pepper)"@en , "Chilli pepper"@en , "Chilli peppers"@en , "Chillies"@en , "Dahon ng sili"@en , "Gochoo"@en , "Green chile"@en , "Green chili"@en , "Green chilies"@en , "Green chillies"@en , "Hot pepper"@en , "Hot peppers"@en , "Red Chili"@en , "Red Chillies"@en , "Red chile"@en , "Red chili"@en , "Red chillies"@en ;
	skos:broader <http://vocabulary.semantic-web.at/cocktails/469959a3-10dc-4539-80ff-08bf9ff2de1c> ;
	skos:definition "The chili pepper is the fruit of plants from the genus Capsicum, members of the nightshade family, Solanaceae. The term in British English and in Australia, New Zealand, India, Malaysia and other Asian countries is just chilli without \"pepper\". Chili peppers originated in the Americas. After the Columbian Exchange, many cultivars of chili pepper spread across the world, used in both food and medicine. India is the world's largest producer, consumer and exporter of chili peppers."@en ;
	skos:exactMatch dbpedia:Chili_pepper ;
	skos:prefLabel "Chili pepper"@en .

<http://vocabulary.semantic-web.at/cocktails/e86c1671-4a67-494b-ae5d-bcb750865acc> dcterms:contributor <http://localhost/user/blumauera> ;
	dcterms:created "2015-05-01T07:56:48Z"^^xsd:dateTime ;
	dcterms:creator <http://localhost/user/blumauera> ;
	dcterms:modified "2015-07-02T14:45:21Z"^^xsd:dateTime ;
	<http://schema.semantic-web.at/ppt/inScheme> <http://vocabulary.semantic-web.at/cocktails/591cf89a-57af-49b8-9042-3fc77408c93e> ;
	<http://schema.semantic-web.at/ppt/propagateType> <http://vocabulary.semantic-web.at/cocktail-ontology/Non-alcoholic-Beverages> ;
	a <http://vocabulary.semantic-web.at/cocktail-ontology/Beverages> , <http://vocabulary.semantic-web.at/cocktail-ontology/Ingredients> , <http://vocabulary.semantic-web.at/cocktail-ontology/Non-alcoholic-Beverages> , skos:Concept ;
	skos:altLabel "Classification chart of non alcoholic beverages"@en , "Freddie Bartholomew (cocktail)"@en , "Kiddie cocktail"@en , "Kiddie cocktails"@en , "List of non-alcoholic cocktails"@en , "List of non-alcoholic punches"@en , "Mock champagne"@en , "Mock tail"@en , "Mocktail"@en , "Mocktails"@en , "Non alcoholic mixed drink"@en , "Non alcoholic mixed drinks"@en , "Non-alcoholic beverages"@en , "Non-alcoholic mixed drink"@en , "Non-alcoholic mixed drinks"@en , "Nonalcoholic beverage"@en , "Nonalcoholic beverages"@en , "Virgin cocktail"@en , "Virgin cocktails"@en ;
	skos:definition "A non-alcoholic beverage (also known as a virgin drink) is defined in the U.S. as a beverage that contains less than 0.5% alcohol by volume. Non-alcoholic versions of some alcoholic beverages, such as non-alcoholic beer (\"near beer\") and cocktails (\"mocktails\"), are widely available where alcoholic beverages are sold. Sodas, juices, and sparkling cider contain no alcohol, but non-alcoholic beer and non-alcoholic wine undergo an alcohol-removal process that may leave a small amount of alcohol."@en ;
	skos:exactMatch dbpedia:Non-alcoholic_beverage ;
	skos:narrower <http://vocabulary.semantic-web.at/cocktails/204c40af-075d-4bf6-a54e-33a60c54ac35> , <http://vocabulary.semantic-web.at/cocktails/26ca4892-5265-4ce6-875c-ef92348ff7a4> , <http://vocabulary.semantic-web.at/cocktails/4f4bed20-5317-45f6-a070-f28267b6e961> , <http://vocabulary.semantic-web.at/cocktails/6c0607a9-410d-4b65-87a1-b189a8e36352> , <http://vocabulary.semantic-web.at/cocktails/a2b8e0e7-0dd0-40e2-a9a4-6178c7728cd0> , <http://vocabulary.semantic-web.at/cocktails/b6ce7a37-ceda-4e8c-86a0-fe7bc5fd0908> , <http://vocabulary.semantic-web.at/cocktails/de17b6c7-513a-4fe2-a8ee-4fdc6069ae27> ;
	skos:prefLabel "Non-alcoholic beverage"@en ;
	skos:topConceptOf <http://vocabulary.semantic-web.at/cocktails/591cf89a-57af-49b8-9042-3fc77408c93e> .

<http://vocabulary.semantic-web.at/cocktails/e90dfeeb-19f6-4c8f-8b2e-a230850fb35b> dcterms:contributor <http://localhost/user/blumauera> ;
	dcterms:created "2015-05-01T08:13:26Z"^^xsd:dateTime ;
	dcterms:creator <http://localhost/user/blumauera> ;
	dcterms:modified "2016-08-04T14:08:48Z"^^xsd:dateTime ;
	<http://schema.semantic-web.at/ppt/inScheme> <http://vocabulary.semantic-web.at/cocktails/f09732a9-a0e6-494a-8ce9-299ef036aaaf> ;
	<http://vocabulary.semantic-web.at/cocktail-ontology/image_2> <http://upload.wikimedia.org/wikipedia/commons/thumb/6/64/Margarita_Glass_Silhouette.svg/32px-Margarita_Glass_Silhouette.svg.png> ;
	<http://vocabulary.semantic-web.at/cocktail-ontology/is-used-by> <http://vocabulary.semantic-web.at/cocktails/2d85fb1b-96cb-4c48-8df5-707032f34e71> ;
	a <http://vocabulary.semantic-web.at/cocktail-ontology/Drinkware> , skos:Concept ;
	skos:altLabel "MargaGlass"@en ;
	skos:broader <http://vocabulary.semantic-web.at/cocktails/2ea18d11-7415-4282-9608-7a3f497a0928> ;
	skos:prefLabel "Margarita glass"@en .

<http://vocabulary.semantic-web.at/cocktails/e98ac9a3-64f3-4cc5-8d0d-cf8684b0e7d1> dcterms:contributor <http://localhost/user/blumauera> ;
	dcterms:created "2015-05-01T14:08:35Z"^^xsd:dateTime ;
	dcterms:creator <http://localhost/user/blumauera> ;
	dcterms:modified "2015-11-20T19:25:58Z"^^xsd:dateTime ;
	<http://schema.semantic-web.at/ppt/inScheme> <http://vocabulary.semantic-web.at/cocktails/591cf89a-57af-49b8-9042-3fc77408c93e> ;
	<http://schema.semantic-web.at/ppt/inSubtree> <http://vocabulary.semantic-web.at/cocktails/403d1249-f37f-4f43-bebf-8dde9677d886> ;
	<http://vocabulary.semantic-web.at/cocktail-ontology/image_3> <http://preview.poolparty.biz/sparqlingCocktails/resources/images/rum.png> ;
	<http://vocabulary.semantic-web.at/cocktail-ontology/is-part-of> <http://vocabulary.semantic-web.at/cocktails/4d15a643-f7c7-4ee5-8f56-4ebd2bcf74b5> ;
	a <http://vocabulary.semantic-web.at/cocktail-ontology/Alcoholic-Beverages> , <http://vocabulary.semantic-web.at/cocktail-ontology/Beverages> , <http://vocabulary.semantic-web.at/cocktail-ontology/Ingredients> , skos:Concept ;
	skos:altLabel "Cane spirit"@en , "Caña blanca"@en , "Coconut rum"@en , "Cuban rum"@en , "Gold rum"@en , "Gunpowder Rum"@en , "Hard rum"@en , "Jamaica Spirit"@en , "Jamaica Spirits"@en , "Rum (beverage)"@en , "Spiced Rum"@en , "Spiced rum"@en ;
	skos:broader <http://vocabulary.semantic-web.at/cocktails/403d1249-f37f-4f43-bebf-8dde9677d886> , <http://vocabulary.semantic-web.at/cocktails/f3000285-36b0-4ffe-af90-740c2dd8fff5> ;
	skos:definition "Rum is a distilled alcoholic beverage made from sugarcane byproducts such as molasses, or directly from sugarcane juice, by a process of fermentation and distillation. The distillate, a clear liquid, is then usually aged in oak barrels. Rum can be referred to in Spanish by descriptors such as ron viejo (\"old rum\") and ron añejo (\"aged rum\"). The majority of the world's rum production occurs in the Caribbean and Latin America."@en ;
	skos:exactMatch dbpedia:Rum ;
	skos:narrower <http://vocabulary.semantic-web.at/cocktails/59ccd2fc-1807-45eb-8621-8d3e898e6d37> , <http://vocabulary.semantic-web.at/cocktails/f5cd2a2b-2153-4b7e-ae79-678b939765ca> ;
	skos:prefLabel "Rum"@en .

<http://vocabulary.semantic-web.at/cocktails/ea946e07-e812-4492-a0ed-124d73bfbba7> dcterms:contributor <http://localhost/user/superadmin> ;
	dcterms:created "2015-05-02T17:26:56Z"^^xsd:dateTime ;
	dcterms:creator <http://localhost/user/blumauera> ;
	dcterms:modified "2016-08-26T12:43:05Z"^^xsd:dateTime ;
	<http://schema.semantic-web.at/ppt/inScheme> <http://vocabulary.semantic-web.at/cocktails/8d052dfc-44bf-4985-8ce3-4564570a161b> ;
	<http://vocabulary.semantic-web.at/cocktail-ontology/consists-of> <http://vocabulary.semantic-web.at/cocktails/687a5d86-1f4e-4a6b-b5ca-3b5d74aeafcc> , <http://vocabulary.semantic-web.at/cocktails/df4ff163-a7c8-4c40-b556-f9390fd97972> ;
	<http://vocabulary.semantic-web.at/cocktail-ontology/iba> <http://www.iba-world.com/index.php?option=com_content&id=225&Itemid=532> ;
	<http://vocabulary.semantic-web.at/cocktail-ontology/image> <http://upload.wikimedia.org/wikipedia/commons/thumb/c/c3/Kir_cocktail.jpg/440px-Kir_cocktail.jpg> ;
	<http://vocabulary.semantic-web.at/cocktail-ontology/preparation> "Pour Créme de Cassis into glass, top up with white wine. For Kir Royal: Use champagne instead of white wine."@en ;
	<http://vocabulary.semantic-web.at/cocktail-ontology/uses> <http://vocabulary.semantic-web.at/cocktails/0381bd47-ad07-428a-b5c4-ee2608f2ebd3> , <http://vocabulary.semantic-web.at/cocktails/e576e848-0f11-4f7a-b6b3-1ff820b02023> ;
	a <http://vocabulary.semantic-web.at/cocktail-ontology/Cocktail> , skos:Concept ;
	skos:altLabel "Blanc-cassis"@en , "Kir Breton"@en , "Kir Royale"@en ;
	skos:broader <http://vocabulary.semantic-web.at/cocktails/204cd4e7-58d7-4417-837a-7f9cc41663c8> , <http://vocabulary.semantic-web.at/cocktails/b523727e-7f49-4e1b-9c09-55002ee3a81e> , <http://vocabulary.semantic-web.at/cocktails/b9bf3799-a4e4-47f7-9aea-7697cc998a34> ;
	skos:definition "Kir is a popular French cocktail made with a measure of crème de cassis (blackcurrant liqueur) topped up with white wine. In France it is usually drunk as an apéritif before a meal or snack. Originally the wine used was Bourgogne Aligoté, a lesser white wine of Burgundy. Nowadays, various white wines are used throughout France, according to the region and the whim of the barkeeper. Many prefer a white Chardonnay-based Burgundy, such as Chablis."@en ;
	skos:exactMatch <http://dbpedia.org/resource/Kir_(cocktail)> ;
	skos:prefLabel "Kir"@en .

<http://vocabulary.semantic-web.at/cocktails/ec2452b9-849d-4750-8190-bc696f2271fa> dcterms:created "2015-11-18T14:46:25Z"^^xsd:dateTime ;
	dcterms:creator <http://localhost/user/blumauera> ;
	<http://schema.semantic-web.at/ppt/inScheme> <http://vocabulary.semantic-web.at/cocktails/591cf89a-57af-49b8-9042-3fc77408c93e> ;
	<http://schema.semantic-web.at/ppt/inSubtree> <http://vocabulary.semantic-web.at/cocktails/403d1249-f37f-4f43-bebf-8dde9677d886> ;
	a <http://vocabulary.semantic-web.at/cocktail-ontology/Alcoholic-Beverages> , <http://vocabulary.semantic-web.at/cocktail-ontology/Beverages> , <http://vocabulary.semantic-web.at/cocktail-ontology/Ingredients> , skos:Concept ;
	skos:broader <http://vocabulary.semantic-web.at/cocktails/2944baef-5338-421b-a5f5-0e51f75244c2> ;
	skos:narrower <http://vocabulary.semantic-web.at/cocktails/4e27dba8-ce80-4246-ad19-14f72e628959> ;
	skos:prefLabel "Cinnamon-flavored liquer"@en .

<http://vocabulary.semantic-web.at/cocktails/eddf4894-1683-44e9-9ee3-7920d3729d71> dcterms:contributor <http://localhost/user/blumauera> ;
	dcterms:created "2015-05-02T17:18:51Z"^^xsd:dateTime ;
	dcterms:creator <http://localhost/user/blumauera> ;
	dcterms:modified "2015-05-07T06:46:39Z"^^xsd:dateTime ;
	<http://schema.semantic-web.at/ppt/inScheme> <http://vocabulary.semantic-web.at/cocktails/8d052dfc-44bf-4985-8ce3-4564570a161b> ;
	<http://vocabulary.semantic-web.at/cocktail-ontology/consists-of> <http://vocabulary.semantic-web.at/cocktails/5c291fe9-6fdb-4939-930d-dacbc67171a5> , <http://vocabulary.semantic-web.at/cocktails/89ac12aa-d4f9-46d0-b127-fd8f4c21fbcc> , <http://vocabulary.semantic-web.at/cocktails/8f09ee6f-d5b9-4b8a-aa17-b0665fae4e83> ;
	<http://vocabulary.semantic-web.at/cocktail-ontology/iba> <http://www.iba-world.com/index.php?option=com_content&id=223&Itemid=532> ;
	<http://vocabulary.semantic-web.at/cocktail-ontology/image> <http://upload.wikimedia.org/wikipedia/commons/thumb/d/d9/Horse%27s_Neck_cocktail.jpg/440px-Horse%27s_Neck_cocktail.jpg> ;
	<http://vocabulary.semantic-web.at/cocktail-ontology/preparation> "Pour brandy and ginger ale directly into hi-ball glass with ice cubes. Stir gently. Garnish with rind of one lemon spiral. If required, add dashes of Angostura bitters."@en ;
	<http://vocabulary.semantic-web.at/cocktail-ontology/served> "On the rocks; poured over ice"@en ;
	<http://vocabulary.semantic-web.at/cocktail-ontology/uses> <http://vocabulary.semantic-web.at/cocktails/a54d2096-6214-4006-beaf-afcc77824710> ;
	<http://vocabulary.semantic-web.at/cocktail-ontology/uses_2> <http://vocabulary.semantic-web.at/cocktails/33df103a-03ac-4177-b620-7953fe094236> ;
	a <http://vocabulary.semantic-web.at/cocktail-ontology/Cocktail> , skos:Concept ;
	skos:broader <http://vocabulary.semantic-web.at/cocktails/b9bf3799-a4e4-47f7-9aea-7697cc998a34> ;
	skos:prefLabel "Horse's Neck"@en .

<http://vocabulary.semantic-web.at/cocktails/ee61817b-0d10-4862-b44b-740c990e676e> dcterms:contributor <http://localhost/user/blumauera> ;
	dcterms:created "2015-05-05T07:33:19Z"^^xsd:dateTime ;
	dcterms:creator <http://localhost/user/blumauera> ;
	dcterms:modified "2015-05-05T07:33:51Z"^^xsd:dateTime ;
	<http://schema.semantic-web.at/ppt/inScheme> <http://vocabulary.semantic-web.at/cocktails/591cf89a-57af-49b8-9042-3fc77408c93e> ;
	<http://schema.semantic-web.at/ppt/inSubtree> <http://vocabulary.semantic-web.at/cocktails/403d1249-f37f-4f43-bebf-8dde9677d886> ;
	<http://vocabulary.semantic-web.at/cocktail-ontology/is-part-of> <http://vocabulary.semantic-web.at/cocktails/680c7429-30a7-4044-b32f-e28c99dcb9f4> ;
	a <http://vocabulary.semantic-web.at/cocktail-ontology/Alcoholic-Beverages> , <http://vocabulary.semantic-web.at/cocktail-ontology/Beverages> , <http://vocabulary.semantic-web.at/cocktail-ontology/Ingredients> , skos:Concept ;
	skos:altLabel "Chambord Black Raspberry Liqueur"@en , "Chambord Liqueur"@en , "Chambord Liqueur Royale de France"@en , "Chambord liqueur royale de france"@en ;
	skos:broader <http://vocabulary.semantic-web.at/cocktails/0f6d360f-af24-4d66-8f70-760c927ed0a7> ;
	skos:definition "Chambord Black Raspberry Liqueur is modelled after a raspberry liqueur produced in the Loire Valley of France during the late 17th century. The liqueur was said to have been introduced to Louis XIV during one of his visits to the Château de Chambord. It was common during that time for liqueurs and cognac to be consumed with elegant meals. As of October 2011, the Chambord product brand is owned and produced by the Brown-Forman Corporation."@en ;
	skos:exactMatch <http://dbpedia.org/resource/Chambord_(liqueur)> ;
	skos:prefLabel "Chambord"@en .

<http://vocabulary.semantic-web.at/cocktails/ef0fb33b-cf31-4acb-aeb8-cff4ab5411d2> dcterms:contributor <http://localhost/user/blumauera> ;
	dcterms:created "2015-05-01T15:00:54Z"^^xsd:dateTime ;
	dcterms:creator <http://localhost/user/blumauera> ;
	dcterms:modified "2015-05-04T11:21:36Z"^^xsd:dateTime ;
	<http://schema.semantic-web.at/ppt/inScheme> <http://vocabulary.semantic-web.at/cocktails/591cf89a-57af-49b8-9042-3fc77408c93e> ;
	<http://schema.semantic-web.at/ppt/inSubtree> <http://vocabulary.semantic-web.at/cocktails/403d1249-f37f-4f43-bebf-8dde9677d886> ;
	<http://vocabulary.semantic-web.at/cocktail-ontology/is-part-of> <http://vocabulary.semantic-web.at/cocktails/cfa8539e-ede2-42ec-b563-d084ddb33280> ;
	a <http://vocabulary.semantic-web.at/cocktail-ontology/Alcoholic-Beverages> , <http://vocabulary.semantic-web.at/cocktail-ontology/Beverages> , <http://vocabulary.semantic-web.at/cocktail-ontology/Ingredients> , skos:Concept ;
	skos:altLabel "Baixo Corgo"@en , "Cima Corgo"@en , "Colheita"@en , "Colheitas"@en , "Crusted port"@en , "Douro Superior"@en , "IVDP"@en , "Instituto do Vinho do Porto"@en , "Instituto dos Vinhos do Douro e Porto"@en , "Instituto dos Vinhos do Douro e do Porto"@en , "Oporto (wine)"@en , "Pink port"@en , "Port (alcohol)"@en , "Port (wine)"@en , "Port DOC"@en , "Port wines"@en , "Port-style"@en , "Port-style wines"@en , "Port-wine"@en , "Porto Wine"@en , "Porto e Douro"@en , "Porto wine"@en , "Portonic"@en , "Ports (wine)"@en , "Portwine"@en , "Quinta port"@en , "Ruby port"@en , "Tawny (wine)"@en , "Tawny port"@en , "Vinho do Porto"@en , "White Port"@en , "Wine port"@en ;
	skos:broader <http://vocabulary.semantic-web.at/cocktails/84bf281b-95ab-4e18-a6fa-2d5156387167> ;
	skos:definition "Port wine (Porto, and often simply port) is a Portuguese fortified wine produced exclusively in the Douro Valley in the northern provinces of Portugal. It is typically a sweet, red wine, often served as a dessert wine though it also comes in dry, semi-dry, and white varieties. Fortified wines in the style of port are also produced outside Portugal, most notably in Australia, South Africa, Canada, India, Argentina, and the United States."@en ;
	skos:exactMatch dbpedia:Port_wine ;
	skos:prefLabel "Port wine"@en .

<http://vocabulary.semantic-web.at/cocktails/eff672ac-6601-42c6-a3e9-0adda3b45df8> dcterms:contributor <http://localhost/user/blumauera> ;
	dcterms:created "2015-05-01T08:08:29Z"^^xsd:dateTime ;
	dcterms:creator <http://localhost/user/blumauera> ;
	dcterms:modified "2015-05-04T11:27:10Z"^^xsd:dateTime ;
	dcterms:publisher <http://localhost/user/Semantic-Web-Company> ;
	dcterms:title "Garnish and other ingredients"@en ;
	<http://schema.semantic-web.at/ppt/appliedType> <http://vocabulary.semantic-web.at/cocktail-ontology/Garnish> ;
	a skos:ConceptScheme ;
	rdfs:label "Garnish"@en ;
	skos:hasTopConcept <http://vocabulary.semantic-web.at/cocktails/469959a3-10dc-4539-80ff-08bf9ff2de1c> , <http://vocabulary.semantic-web.at/cocktails/4f20d6bb-710d-4870-bde4-b6e835d7d13f> .

<http://vocabulary.semantic-web.at/cocktails/f01f6a10-01a5-4810-860f-d3a52fd36b1b> dcterms:contributor <http://localhost/user/blumauera> ;
	dcterms:created "2015-05-02T08:16:07Z"^^xsd:dateTime ;
	dcterms:creator <http://localhost/user/blumauera> ;
	dcterms:modified "2016-08-26T07:15:00Z"^^xsd:dateTime ;
	<http://schema.semantic-web.at/ppt/inScheme> <http://vocabulary.semantic-web.at/cocktails/8d052dfc-44bf-4985-8ce3-4564570a161b> ;
	<http://vocabulary.semantic-web.at/cocktail-ontology/consists-of> <http://vocabulary.semantic-web.at/cocktails/0f11bcdf-a69e-451f-b824-48b1743c5916> , <http://vocabulary.semantic-web.at/cocktails/88f5de3d-3de4-4a2f-9523-50bc7bb06600> , <http://vocabulary.semantic-web.at/cocktails/f5cd2a2b-2153-4b7e-ae79-678b939765ca> ;
	<http://vocabulary.semantic-web.at/cocktail-ontology/iba> <http://www.iba-world.com/index.php?option=com_content&id=218&Itemid=532> ;
	<http://vocabulary.semantic-web.at/cocktail-ontology/image> <http://upload.wikimedia.org/wikipedia/commons/thumb/e/e5/Cuba_Libre.jpg/400px-Cuba_Libre.jpg> ;
	<http://vocabulary.semantic-web.at/cocktail-ontology/preparation> "Build all ingredients in a highball glass filled with ice. Garnish with lime wedge."@en ;
	<http://vocabulary.semantic-web.at/cocktail-ontology/served> "On the rocks; poured over ice"@en ;
	<http://vocabulary.semantic-web.at/cocktail-ontology/uses> <http://vocabulary.semantic-web.at/cocktails/a54d2096-6214-4006-beaf-afcc77824710> ;
	<http://vocabulary.semantic-web.at/cocktail-ontology/uses_2> <http://vocabulary.semantic-web.at/cocktails/021c85c0-a60a-4414-8fd8-bd3383b794f1> ;
	a <http://vocabulary.semantic-web.at/cocktail-ontology/Cocktail> , skos:Concept ;
	skos:altLabel "Coke and rum"@en , "Cubalibre"@en , "Cubata"@en , "Roman Coke"@en , "Ron y coca"@en , "Rum & Coke"@en , "Rum and coke"@en , "Virgin Cuba Libre"@en ;
	skos:broader <http://vocabulary.semantic-web.at/cocktails/b9bf3799-a4e4-47f7-9aea-7697cc998a34> ;
	skos:definition "The Cuba Libre is a highball made of cola, lime, and dark or light rum. This highball is often referred to as a Rum and Coke in the United States, Canada, the UK, Ireland, Australia and New Zealand where the lime juice may or may not be included."@en , "This article is about the cocktail. For other uses, see Cuba libre (disambiguation). \"Rum and coke\" redirects here. For the Dub Pistols album, see Rum & Coke. Cuba Libre IBA Official Cocktail {{#invoke:InfoboxImage|InfoboxImage|image=CubaLibre3. jpg|size=|sizedefault=frameless|alt=}} A Cuba Libre served in a short tumbler. Type Mixed drink Primary alcohol by volume Rum Served On the rocks; poured over ice Standard garnish limepineapple wedge Standard drinkware 24 oz."@en ;
	skos:exactMatch dbpedia:Cuba_Libre ;
	skos:prefLabel "Cuba Libre"@en .

<http://vocabulary.semantic-web.at/cocktails/f09732a9-a0e6-494a-8ce9-299ef036aaaf> dcterms:contributor <http://localhost/user/blumauera> ;
	dcterms:created "2015-05-01T07:52:12Z"^^xsd:dateTime ;
	dcterms:creator <http://localhost/user/Andreas-Blumauer> ;
	dcterms:modified "2015-05-02T21:03:14Z"^^xsd:dateTime ;
	dcterms:publisher <http://localhost/user/Semantic-Web-Company> ;
	dcterms:title "Glassware"@en ;
	<http://schema.semantic-web.at/ppt/appliedType> <http://vocabulary.semantic-web.at/cocktail-ontology/Drinkware> ;
	a skos:ConceptScheme ;
	rdfs:label "Glassware"@en ;
	skos:hasTopConcept <http://vocabulary.semantic-web.at/cocktails/2e839563-8037-4e59-8dbf-27736605d687> , <http://vocabulary.semantic-web.at/cocktails/2ea18d11-7415-4282-9608-7a3f497a0928> , <http://vocabulary.semantic-web.at/cocktails/d6c5f29f-bef7-41c5-9d39-535d83e9f750> .

<http://vocabulary.semantic-web.at/cocktails/f0bfda32-3c42-457f-b6a3-bbf2a9e77b06> dcterms:contributor <http://localhost/user/blumauera> ;
	dcterms:created "2015-05-01T15:12:47Z"^^xsd:dateTime ;
	dcterms:creator <http://localhost/user/blumauera> ;
	dcterms:modified "2015-05-06T12:54:41Z"^^xsd:dateTime ;
	<http://schema.semantic-web.at/ppt/inScheme> <http://vocabulary.semantic-web.at/cocktails/591cf89a-57af-49b8-9042-3fc77408c93e> ;
	<http://schema.semantic-web.at/ppt/inSubtree> <http://vocabulary.semantic-web.at/cocktails/403d1249-f37f-4f43-bebf-8dde9677d886> ;
	<http://vocabulary.semantic-web.at/cocktail-ontology/is-part-of> <http://vocabulary.semantic-web.at/cocktails/45788a96-1fde-486b-80fc-31ad243bba31> , <http://vocabulary.semantic-web.at/cocktails/be3653af-d585-43f7-b8ce-ad75b1bd7aad> ;
	a <http://vocabulary.semantic-web.at/cocktail-ontology/Alcoholic-Beverages> , <http://vocabulary.semantic-web.at/cocktail-ontology/Beverages> , <http://vocabulary.semantic-web.at/cocktail-ontology/Ingredients> , skos:Concept ;
	skos:altLabel "Blended Scotch"@en , "Blended scotch"@en , "Scotch Whiskey"@en , "Scotch malt whisky"@en , "Scotch whiskey"@en , "Scotch whisky industry"@en , "Scotland’s whisky industry"@en , "Scottish Malt Whisky"@en , "Scottish blended whisky"@en , "Scottish whiskey"@en , "Scottish whisky"@en , "Whiskey in Scotland"@en , "Whisky in Scotland"@en ;
	skos:broader <http://vocabulary.semantic-web.at/cocktails/c4339109-ae35-4be9-a7e8-b5dfd206e960> ;
	skos:definition "Scotch whisky (often referred to simply as \"Scotch\") is malt whisky or grain whisky made in Scotland. All Scotch whisky was originally made from malt barley. Commercial distilleries began introducing whisky made from wheat and rye in the late eighteenth century."@en ;
	skos:exactMatch dbpedia:Scotch_whisky ;
	skos:narrower <http://vocabulary.semantic-web.at/cocktails/f6118c6b-90db-49ca-b0f2-2c7fbfc5fbb9> ;
	skos:prefLabel "Scotch whisky"@en .

<http://vocabulary.semantic-web.at/cocktails/f159e33f-fed0-4382-93b9-acfa28f23937> dcterms:contributor <http://localhost/user/blumauera> ;
	dcterms:created "2015-05-05T13:03:17Z"^^xsd:dateTime ;
	dcterms:creator <http://localhost/user/blumauera> ;
	dcterms:modified "2015-11-12T12:39:23Z"^^xsd:dateTime ;
	<http://schema.semantic-web.at/ppt/inScheme> <http://vocabulary.semantic-web.at/cocktails/eff672ac-6601-42c6-a3e9-0adda3b45df8> ;
	<http://schema.semantic-web.at/ppt/inSubtree> <http://vocabulary.semantic-web.at/cocktails/469959a3-10dc-4539-80ff-08bf9ff2de1c> ;
	<http://vocabulary.semantic-web.at/cocktail-ontology/is-part-of> <http://vocabulary.semantic-web.at/cocktails/a5db05ca-eda3-41ef-a8ab-ba77b3e4baba> ;
	a <http://vocabulary.semantic-web.at/cocktail-ontology/Garnish> , <http://vocabulary.semantic-web.at/cocktail-ontology/Ingredients> , skos:Concept ;
	skos:altLabel "Allium cepa"@en , "Bulb onion"@en , "Bulb onions"@en , "Dry onion"@en , "Onion fruit"@en , "Onion set"@en , "Onion skins"@en , "Onions"@en , "Pyaz"@en , "Spanish onion"@en ;
	skos:broader <http://vocabulary.semantic-web.at/cocktails/469959a3-10dc-4539-80ff-08bf9ff2de1c> ;
	skos:definition "The onion (Allium cepa), also known as the bulb onion or common onion, is used as a vegetable and is the most widely cultivated species of the genus Allium. This genus also contains several other species variously referred to as onions and cultivated for food, such as the Japanese bunching onion (A. fistulosum), Egyptian onion (A. ×proliferum), and Canada onion (A. canadense). The name \"wild onion\" is applied to a number of Allium species but A."@en ;
	skos:exactMatch dbpedia:Onion ;
	skos:prefLabel "Onion"@en .

<http://vocabulary.semantic-web.at/cocktails/f3000285-36b0-4ffe-af90-740c2dd8fff5> dcterms:contributor <http://localhost/user/turdeant> ;
	dcterms:created "2015-08-07T15:06:09Z"^^xsd:dateTime ;
	dcterms:creator <http://localhost/user/blumauera> ;
	dcterms:modified "2016-05-12T14:57:00Z"^^xsd:dateTime ;
	<http://schema.semantic-web.at/ppt/appliedType> <http://vocabulary.semantic-web.at/cocktail-ontology/Alcoholic-Beverages> ;
	<http://schema.semantic-web.at/ppt/inScheme> <http://vocabulary.semantic-web.at/cocktails/591cf89a-57af-49b8-9042-3fc77408c93e> ;
	a <http://vocabulary.semantic-web.at/cocktail-ontology/Alcoholic-Beverages> , <http://vocabulary.semantic-web.at/cocktail-ontology/Beverages> , <http://vocabulary.semantic-web.at/cocktail-ontology/Ingredients> , skos:Concept ;
	skos:altLabel "Adult beverage"@en , "Alchoholic beverage"@en , "Alcohalic beverages"@en , "Alcohol (drink)"@en , "Alcohol Consumption"@en , "Alcohol beverage"@en , "Alcohol consumption"@en , "Alcohol expectancies"@en , "Alcohol expectations"@en , "Alcoholic beverages"@en , "Alcoholic drink"@en , "Alcoholic drinks"@en , "Beverage alcohol"@en , "Boozing"@en , "Drinker (alcohol)"@en , "Drinker's"@en , "Drinkies"@en , "Drinky"@en , "Effects of alcohol on the human body"@en , "Fermanted beverage"@en , "Fermented beverage"@en , "Fermented drink"@en , "Hard drink"@en , "Hard drinks"@en , "Liquid lunch"@en , "Zundis"@en ;
	skos:definition "An alcoholic beverage is a drink containing ethyl alcohol which is commonly referred to as ethanol. Alcoholic beverages are divided into three general classes for taxation and regulation of production: beers, wines, and spirits (or distilled beverage). They are legally consumed in most countries with over 100 countries having laws regulating their production, sale, and consumption."@en ;
	skos:exactMatch dbpedia:Alcoholic_beverage ;
	skos:narrower <http://vocabulary.semantic-web.at/cocktails/22df810d-e509-4da8-979c-0758e94de3e6> , <http://vocabulary.semantic-web.at/cocktails/27c48d24-bb0b-46a3-9b0c-4b09e38a4b07> , <http://vocabulary.semantic-web.at/cocktails/2944baef-5338-421b-a5f5-0e51f75244c2> , <http://vocabulary.semantic-web.at/cocktails/5d96c50c-ee48-4c40-bb4c-4b9a42d11de6> , <http://vocabulary.semantic-web.at/cocktails/7dede323-e986-4417-b723-c9c7a7fe82ba> , <http://vocabulary.semantic-web.at/cocktails/84bf281b-95ab-4e18-a6fa-2d5156387167> , <http://vocabulary.semantic-web.at/cocktails/8f09ee6f-d5b9-4b8a-aa17-b0665fae4e83> , <http://vocabulary.semantic-web.at/cocktails/c4339109-ae35-4be9-a7e8-b5dfd206e960> , <http://vocabulary.semantic-web.at/cocktails/d5286375-41b3-468b-9602-8fcf698e3e83> , <http://vocabulary.semantic-web.at/cocktails/e98ac9a3-64f3-4cc5-8d0d-cf8684b0e7d1> ;
	skos:prefLabel "Alcoholic beverage"@en ;
	skos:topConceptOf <http://vocabulary.semantic-web.at/cocktails/591cf89a-57af-49b8-9042-3fc77408c93e> .

<http://vocabulary.semantic-web.at/cocktails/f4da82d8-eaf5-451f-824c-05564bc48816> dcterms:contributor <http://localhost/user/blumauera> ;
	dcterms:created "2015-05-02T19:09:07Z"^^xsd:dateTime ;
	dcterms:creator <http://localhost/user/blumauera> ;
	dcterms:modified "2015-05-05T07:08:20Z"^^xsd:dateTime ;
	<http://schema.semantic-web.at/ppt/inScheme> <http://vocabulary.semantic-web.at/cocktails/591cf89a-57af-49b8-9042-3fc77408c93e> ;
	<http://schema.semantic-web.at/ppt/inSubtree> <http://vocabulary.semantic-web.at/cocktails/403d1249-f37f-4f43-bebf-8dde9677d886> ;
	<http://vocabulary.semantic-web.at/cocktail-ontology/is-part-of> <http://vocabulary.semantic-web.at/cocktails/563bf7e0-0f40-41b6-a749-c4e94760204d> ;
	a <http://vocabulary.semantic-web.at/cocktail-ontology/Alcoholic-Beverages> , <http://vocabulary.semantic-web.at/cocktail-ontology/Beverages> , <http://vocabulary.semantic-web.at/cocktail-ontology/Ingredients> , skos:Concept ;
	skos:broader <http://vocabulary.semantic-web.at/cocktails/47635419-edef-4b78-8da1-e58a96d96f61> ;
	skos:prefLabel "Crème de mûre"@en .

<http://vocabulary.semantic-web.at/cocktails/f5cd2a2b-2153-4b7e-ae79-678b939765ca> dcterms:contributor <http://localhost/user/blumauera> ;
	dcterms:created "2015-05-01T14:18:41Z"^^xsd:dateTime ;
	dcterms:creator <http://localhost/user/blumauera> ;
	dcterms:modified "2015-07-02T14:55:25Z"^^xsd:dateTime ;
	<http://schema.semantic-web.at/ppt/inScheme> <http://vocabulary.semantic-web.at/cocktails/591cf89a-57af-49b8-9042-3fc77408c93e> ;
	<http://schema.semantic-web.at/ppt/inSubtree> <http://vocabulary.semantic-web.at/cocktails/403d1249-f37f-4f43-bebf-8dde9677d886> ;
	<http://vocabulary.semantic-web.at/cocktail-ontology/is-part-of> <http://vocabulary.semantic-web.at/cocktails/22f838ea-3c2b-4b63-99d1-fdb6280b5705> , <http://vocabulary.semantic-web.at/cocktails/4792b0b8-0046-47ca-8c2a-f3ad58922182> , <http://vocabulary.semantic-web.at/cocktails/785b30fd-1eb4-445b-8247-7e1e57b35b0f> , <http://vocabulary.semantic-web.at/cocktails/926b14fe-1b83-4f46-bbf9-f946be1889aa> , <http://vocabulary.semantic-web.at/cocktails/b970d408-39ca-49b0-98fc-838f96c94608> , <http://vocabulary.semantic-web.at/cocktails/bab016bd-2fd5-4809-bfe7-3225d25f116d> , <http://vocabulary.semantic-web.at/cocktails/bee1e709-b317-4f46-b06f-a22367baefdf> , <http://vocabulary.semantic-web.at/cocktails/ce8f4591-ccd4-4d90-a761-244115d64061> , <http://vocabulary.semantic-web.at/cocktails/f01f6a10-01a5-4810-860f-d3a52fd36b1b> ;
	a <http://vocabulary.semantic-web.at/cocktail-ontology/Alcoholic-Beverages> , <http://vocabulary.semantic-web.at/cocktail-ontology/Beverages> , <http://vocabulary.semantic-web.at/cocktail-ontology/Ingredients> , skos:Concept ;
	skos:altLabel "Light rum"@en ;
	skos:broader <http://vocabulary.semantic-web.at/cocktails/e98ac9a3-64f3-4cc5-8d0d-cf8684b0e7d1> ;
	skos:narrower <http://vocabulary.semantic-web.at/cocktails/c3a50c60-ccb3-4ab4-8f9f-722acdae8d50> , <http://vocabulary.semantic-web.at/cocktails/e67b1621-7be7-471d-ac8d-a368d8c68115> ;
	skos:prefLabel "White rum"@en .

<http://vocabulary.semantic-web.at/cocktails/f6118c6b-90db-49ca-b0f2-2c7fbfc5fbb9> dcterms:created "2015-05-14T14:11:18Z"^^xsd:dateTime ;
	dcterms:creator <http://localhost/user/blumauera> ;
	<http://schema.semantic-web.at/ppt/inScheme> <http://vocabulary.semantic-web.at/cocktails/591cf89a-57af-49b8-9042-3fc77408c93e> ;
	<http://schema.semantic-web.at/ppt/inSubtree> <http://vocabulary.semantic-web.at/cocktails/403d1249-f37f-4f43-bebf-8dde9677d886> ;
	a <http://vocabulary.semantic-web.at/cocktail-ontology/Alcoholic-Beverages> , <http://vocabulary.semantic-web.at/cocktail-ontology/Beverages> , <http://vocabulary.semantic-web.at/cocktail-ontology/Ingredients> , skos:Concept ;
	skos:broader <http://vocabulary.semantic-web.at/cocktails/f0bfda32-3c42-457f-b6a3-bbf2a9e77b06> ;
	skos:prefLabel "single malt"@en .

<http://vocabulary.semantic-web.at/cocktails/f632b16d-1490-4587-a637-fb393d7b1e7f> dcterms:contributor <http://localhost/user/blumauera> ;
	dcterms:created "2015-05-01T14:37:20Z"^^xsd:dateTime ;
	dcterms:creator <http://localhost/user/blumauera> ;
	dcterms:modified "2015-05-06T12:22:34Z"^^xsd:dateTime ;
	<http://schema.semantic-web.at/ppt/inScheme> <http://vocabulary.semantic-web.at/cocktails/8d052dfc-44bf-4985-8ce3-4564570a161b> ;
	<http://vocabulary.semantic-web.at/cocktail-ontology/consists-of> <http://vocabulary.semantic-web.at/cocktails/4f03a6ef-9631-4b6d-a005-7fbbdcb9b342> , <http://vocabulary.semantic-web.at/cocktails/5c291fe9-6fdb-4939-930d-dacbc67171a5> , <http://vocabulary.semantic-web.at/cocktails/8dee4eba-b6c6-4d16-b8f2-8d6cc0d9436c> ;
	<http://vocabulary.semantic-web.at/cocktail-ontology/iba> <http://www.iba-world.com/index.php?option=com_content&id=198&Itemid=532> ;
	<http://vocabulary.semantic-web.at/cocktail-ontology/image> <http://upload.wikimedia.org/wikipedia/commons/thumb/5/5a/Manhattan_cocktail.jpg/400px-Manhattan_cocktail.jpg> ;
	<http://vocabulary.semantic-web.at/cocktail-ontology/preparation> "Stirred over ice, strained into a chilled glass, garnished, and served straight up."@en ;
	<http://vocabulary.semantic-web.at/cocktail-ontology/served> "Straight up; without ice"@en ;
	<http://vocabulary.semantic-web.at/cocktail-ontology/uses> <http://vocabulary.semantic-web.at/cocktails/19dee0d8-fd30-469f-9ecd-91c902ff717c> ;
	<http://vocabulary.semantic-web.at/cocktail-ontology/uses_2> <http://vocabulary.semantic-web.at/cocktails/8a5e1790-d3c0-432e-bb85-709692b14f03> ;
	a <http://vocabulary.semantic-web.at/cocktail-ontology/Cocktail> , skos:Concept ;
	skos:altLabel "Fanciulli cocktail"@en , "Latin Manhattan"@en , "Manhattan (beverage)"@en , "Manhattan (drink)"@en , "Manhattan cocktail"@en ;
	skos:broader <http://vocabulary.semantic-web.at/cocktails/caae2ea0-7e60-400b-a2bb-14ef79720668> ;
	skos:definition "A Manhattan is a cocktail made with whiskey, sweet vermouth, and bitters. Commonly used whiskeys include rye (the traditional choice), Canadian whisky (simply called Rye in Canada), bourbon, blended whiskey and Tennessee whiskey. The cocktail is often stirred with ice and strained into a cocktail glass, where it is garnished with a Maraschino cherry with a stem. A Manhattan is also frequently served on the rocks in an Old Fashioned glass (lowball glass)."@en ;
	skos:exactMatch <http://dbpedia.org/resource/Manhattan_(cocktail)> ;
	skos:prefLabel "Manhattan"@en .

<http://vocabulary.semantic-web.at/cocktails/f9d7d22d-5d57-434a-b9e1-b9c8cde324e9> dcterms:contributor <http://localhost/user/blumauera> ;
	dcterms:created "2015-05-01T14:55:33Z"^^xsd:dateTime ;
	dcterms:creator <http://localhost/user/blumauera> ;
	dcterms:modified "2016-04-06T11:49:35Z"^^xsd:dateTime ;
	<http://schema.semantic-web.at/ppt/inScheme> <http://vocabulary.semantic-web.at/cocktails/eff672ac-6601-42c6-a3e9-0adda3b45df8> ;
	<http://schema.semantic-web.at/ppt/inSubtree> <http://vocabulary.semantic-web.at/cocktails/4f20d6bb-710d-4870-bde4-b6e835d7d13f> ;
	<http://vocabulary.semantic-web.at/cocktail-ontology/is-used-by_2> <http://vocabulary.semantic-web.at/cocktails/43111fc3-3b59-420c-a588-024cd2d33896> , <http://vocabulary.semantic-web.at/cocktails/4792b0b8-0046-47ca-8c2a-f3ad58922182> , <http://vocabulary.semantic-web.at/cocktails/9c287d15-c699-4f56-bd65-bf8cc75a2cca> ;
	a <http://vocabulary.semantic-web.at/cocktail-ontology/Garnish> , <http://vocabulary.semantic-web.at/cocktail-ontology/Ingredients> , skos:Concept ;
	skos:altLabel "A. sativus"@en , "Abacaxi"@en , "Anana"@en , "Ananas comosus"@en , "Ananas sativus"@en , "Bromelworts"@en , "Pine apples"@en , "Pine-Apple"@en , "Pine-apples"@en , "Pineapple plant"@en , "Pineapple tree"@en , "Pineapples"@en , "🍍"@en ;
	skos:broader <http://vocabulary.semantic-web.at/cocktails/4f20d6bb-710d-4870-bde4-b6e835d7d13f> ;
	skos:definition "The Pineapple (Ananas comosus), named for its resemblance to the pine cone, is a tropical plant with edible multiple fruit consisting of coalesced berries, and the most economically significant plant in the Bromeliaceae family. Pineapples may be cultivated from a crown cutting of the fruit, possibly flowering in 20–24 months and fruiting in the following six months. Pineapple does not ripen significantly post-harvest."@en ;
	skos:exactMatch dbpedia:Pineapple ;
	skos:prefLabel "Pineapple"@en .

<http://vocabulary.semantic-web.at/cocktails/fb278b46-3c67-48b0-b9eb-7ea037294f5f> dcterms:contributor <http://localhost/user/blumauera> ;
	dcterms:created "2015-05-04T10:13:43Z"^^xsd:dateTime ;
	dcterms:creator <http://localhost/user/blumauera> ;
	dcterms:modified "2016-04-04T09:11:48Z"^^xsd:dateTime ;
	<http://schema.semantic-web.at/ppt/inScheme> <http://vocabulary.semantic-web.at/cocktails/8d052dfc-44bf-4985-8ce3-4564570a161b> ;
	<http://vocabulary.semantic-web.at/cocktail-ontology/consists-of> <http://vocabulary.semantic-web.at/cocktails/3c94f5fc-4664-4177-a880-88643c0be9c1> , <http://vocabulary.semantic-web.at/cocktails/3e2d26b8-928b-462d-99ee-59eac11b241f> , <http://vocabulary.semantic-web.at/cocktails/4f03a6ef-9631-4b6d-a005-7fbbdcb9b342> , <http://vocabulary.semantic-web.at/cocktails/5c291fe9-6fdb-4939-930d-dacbc67171a5> , <http://vocabulary.semantic-web.at/cocktails/84c72e0e-7830-46ef-ac35-44cad56d27ec> ;
	<http://vocabulary.semantic-web.at/cocktail-ontology/iba> <http://www.iba-world.com/index.php?option=com_content&id=202&Itemid=532> ;
	<http://vocabulary.semantic-web.at/cocktail-ontology/image> <http://upload.wikimedia.org/wikipedia/commons/thumb/0/0a/Trago_old_fashioned.jpg/440px-Trago_old_fashioned.jpg> ;
	<http://vocabulary.semantic-web.at/cocktail-ontology/preparation> "Place sugar cube in old-fashioned glass and saturate with bitters, add a dash of plain water. Muddle until dissolve.  Fill the glass with ice cubes and add whisky.  Garnish with orange slice and a cocktail cherry."@en ;
	<http://vocabulary.semantic-web.at/cocktail-ontology/served> "On the rocks; poured over ice"@en ;
	<http://vocabulary.semantic-web.at/cocktail-ontology/uses> <http://vocabulary.semantic-web.at/cocktails/2dce3576-2603-41f9-8dce-ab21f639c2a7> ;
	<http://vocabulary.semantic-web.at/cocktail-ontology/uses_2> <http://vocabulary.semantic-web.at/cocktails/62fbc16f-3f84-4cc7-8c6f-5afebfc1510a> , <http://vocabulary.semantic-web.at/cocktails/99171f20-c59f-40c4-998a-a9c8f1909168> ;
	a <http://vocabulary.semantic-web.at/cocktail-ontology/Cocktail> , skos:Concept ;
	skos:altLabel "Old Fashioned (cocktail)"@en , "Old fashioned cocktail"@en , "Old-Fashioned"@en ;
	skos:broader <http://vocabulary.semantic-web.at/cocktails/caae2ea0-7e60-400b-a2bb-14ef79720668> ;
	skos:definition "The Old Fashioned is an IBA Official Cocktail made by muddling dissolved sugar with bitters then adding alcohol, such as whiskey or brandy, and a twist of citrus rind. It is traditionally served in a short, round, 8–12 US fl oz (&#160) tumbler-like glass, which is called an Old Fashioned glass, named after the drink. The Old Fashioned is one of six basic drinks listed in David A. Embury's The Fine Art of Mixing Drinks."@en ;
	skos:exactMatch dbpedia:Old_Fashioned ;
	skos:prefLabel "Old Fashioned"@en .

<http://vocabulary.semantic-web.at/cocktails/fbfae34b-60d5-47e6-83dc-31507a8d4f78> dcterms:contributor <http://localhost/user/blumauera> ;
	dcterms:created "2015-05-01T15:14:50Z"^^xsd:dateTime ;
	dcterms:creator <http://localhost/user/blumauera> ;
	dcterms:modified "2015-05-04T11:37:39Z"^^xsd:dateTime ;
	<http://schema.semantic-web.at/ppt/inScheme> <http://vocabulary.semantic-web.at/cocktails/591cf89a-57af-49b8-9042-3fc77408c93e> ;
	<http://schema.semantic-web.at/ppt/inSubtree> <http://vocabulary.semantic-web.at/cocktails/403d1249-f37f-4f43-bebf-8dde9677d886> ;
	<http://vocabulary.semantic-web.at/cocktail-ontology/is-part-of> <http://vocabulary.semantic-web.at/cocktails/1576f08f-5936-4071-b85e-d4e85f31c303> ;
	a <http://vocabulary.semantic-web.at/cocktail-ontology/Alcoholic-Beverages> , <http://vocabulary.semantic-web.at/cocktail-ontology/Beverages> , <http://vocabulary.semantic-web.at/cocktail-ontology/Ingredients> , skos:Concept ;
	skos:broader <http://vocabulary.semantic-web.at/cocktails/d40e2215-bc1b-4bae-8cf8-d10b1ad36d44> ;
	skos:prefLabel "Peychaud's Bitters"@en .

<http://vocabulary.semantic-web.at/cocktails/fd76c5ab-be62-4c4b-a2c6-7fa9bc359f47> dcterms:contributor <http://localhost/user/blumauera> ;
	dcterms:created "2015-05-01T08:24:54Z"^^xsd:dateTime ;
	dcterms:creator <http://localhost/user/blumauera> ;
	dcterms:modified "2015-05-06T12:47:44Z"^^xsd:dateTime ;
	<http://schema.semantic-web.at/ppt/inScheme> <http://vocabulary.semantic-web.at/cocktails/591cf89a-57af-49b8-9042-3fc77408c93e> ;
	<http://schema.semantic-web.at/ppt/inSubtree> <http://vocabulary.semantic-web.at/cocktails/403d1249-f37f-4f43-bebf-8dde9677d886> ;
	<http://vocabulary.semantic-web.at/cocktail-ontology/is-part-of> <http://vocabulary.semantic-web.at/cocktails/099726a2-ec4b-4b0f-b4e4-e6f25cdfd685> , <http://vocabulary.semantic-web.at/cocktails/1576f08f-5936-4071-b85e-d4e85f31c303> , <http://vocabulary.semantic-web.at/cocktails/21b94d69-280e-4546-be1a-fdd1d9aa5d32> , <http://vocabulary.semantic-web.at/cocktails/22f838ea-3c2b-4b63-99d1-fdb6280b5705> , <http://vocabulary.semantic-web.at/cocktails/52117ab2-dcb8-4d28-a366-ddd932e58219> , <http://vocabulary.semantic-web.at/cocktails/61a18ebf-fd92-4ef1-8ab1-bfd3c26867b9> , <http://vocabulary.semantic-web.at/cocktails/e039633b-03c1-47bd-a705-a104a4323e45> ;
	a <http://vocabulary.semantic-web.at/cocktail-ontology/Alcoholic-Beverages> , <http://vocabulary.semantic-web.at/cocktail-ontology/Beverages> , <http://vocabulary.semantic-web.at/cocktail-ontology/Ingredients> , skos:Concept ;
	skos:altLabel "Bon bois"@en , "Bons Bois"@en , "Borderies"@en , "Cognac (brandy)"@en , "Cognac (drink)"@en , "Cognac (spirit)"@en , "Cognacs"@en , "Coneyak"@en , "Congac"@en , "Congnac"@en , "Fine Champagne"@en , "Fine champagne"@en , "Very Superior Old Pale"@en , "קוניאק"@en ;
	skos:broader <http://vocabulary.semantic-web.at/cocktails/8f09ee6f-d5b9-4b8a-aa17-b0665fae4e83> ;
	skos:definition "Cognac, named after the town of Cognac in France, is a variety of brandy. It is produced in the wine-growing region surrounding the town from which it takes its name, in the French Departements of Charente and Charente-Maritime. For a distilled brandy to bear the name Cognac, an Appellation d'origine contrôlée, its production methods must meet certain legal requirements."@en ;
	skos:exactMatch dbpedia:Cognac ;
	skos:prefLabel "Cognac"@en .

<http://vocabulary.semantic-web.at/cocktails/fece03b5-ec0b-4e47-964d-cc5dc09fd7fb> dcterms:contributor <http://localhost/user/blumauera> ;
	dcterms:created "2015-05-02T07:22:10Z"^^xsd:dateTime ;
	dcterms:creator <http://localhost/user/blumauera> ;
	dcterms:modified "2015-12-11T08:53:54Z"^^xsd:dateTime ;
	<http://schema.semantic-web.at/ppt/inScheme> <http://vocabulary.semantic-web.at/cocktails/f09732a9-a0e6-494a-8ce9-299ef036aaaf> ;
	<http://vocabulary.semantic-web.at/cocktail-ontology/image_2> <http://upload.wikimedia.org/wikipedia/commons/thumb/3/37/Flutesil.svg/18px-Flutesil.svg.png> ;
	<http://vocabulary.semantic-web.at/cocktail-ontology/is-used-by> <http://vocabulary.semantic-web.at/cocktails/61a18ebf-fd92-4ef1-8ab1-bfd3c26867b9> , <http://vocabulary.semantic-web.at/cocktails/698723d7-e8b8-410e-91a8-9bdc867b3f8a> , <http://vocabulary.semantic-web.at/cocktails/a73d88e9-0c50-45d2-b364-9dec5abe206d> , <http://vocabulary.semantic-web.at/cocktails/b00a123f-a2b5-49d2-8325-a81d1d26ddc6> , <http://vocabulary.semantic-web.at/cocktails/c2249dc0-0529-4a11-ad82-5d710b5e9c31> ;
	a <http://vocabulary.semantic-web.at/cocktail-ontology/Drinkware> , skos:Concept ;
	skos:altLabel "Champagne coupe"@en , "Champagne glass"@en , "Champagne saucer"@en , "Champagne stemware"@en , "Champagne-glass"@en , "Coupe glass"@en ;
	skos:broader <http://vocabulary.semantic-web.at/cocktails/2ea18d11-7415-4282-9608-7a3f497a0928> ;
	skos:definition "Champagne stemware refers to the flute and coupe glasses used in the enjoyment of champagne, other sparkling wines, and certain beers."@en ;
	skos:exactMatch dbpedia:Champagne_stemware ;
	skos:prefLabel "Champagne flute"@en .
